<?xml version="1.0"?>
<rdf:RDF xmlns="https://w3id.org/isoiec5087/-1/v1/"
     xml:base="https://w3id.org/isoiec5087/-1/v1/"
     xmlns:cc="http://creativecommons.org/ns#"
     xmlns:dcterms="http://purl.org/dc/terms/"
     xmlns:owl="http://www.w3.org/2002/07/owl#"
     xmlns:rdf="http://www.w3.org/1999/02/22-rdf-syntax-ns#"
     xmlns:rdfs="http://www.w3.org/2000/01/rdf-schema#"
     xmlns:skos="http://www.w3.org/2004/02/skos/core#"
     xmlns:vann="http://purl.org/vocab/vann/"
     xmlns:xml="http://www.w3.org/XML/1998/namespace"
     xmlns:xsd="http://www.w3.org/2001/XMLSchema#"
     xmlns:prov="http://www.w3.org/ns/prov#"
     xmlns:org="http://www.w3.org/ns/org#"
     xmlns:time="http://www.w3.org/2006/time#">
    <owl:Ontology rdf:about="https://w3id.org/isoiec5087/-1/v1/">
    	<!-- Identity -->
    	<dcterms:title>Information technology - City data model - Part 1: Foundation level concepts</dcterms:title>
        <rdfs:seeAlso rdf:resource="https://www.iso.org/standard/80718.html"/>
        <dcterms:bibliographicCitation>ISO/IEC 5087-1:2023</dcterms:bibliographicCitation>
    	<skos:definition>This ontology specifies the foundation-level concepts of the city data model.</skos:definition>
    	<vann:preferredNamespaceUri>https://w3id.org/isoiec5087/-1/v1/</vann:preferredNamespaceUri>
    	<vann:preferredNamespacePrefix>cdm1</vann:preferredNamespacePrefix>

    		
    	<!-- Provenance -->
        <dcterms:creator>Megan Katsumi</dcterms:creator>
        <dcterms:creator>Mark Fox</dcterms:creator>
    	<dcterms:creator>Kenneth Vaughn</dcterms:creator>
        <dcterms:issued rdf:datatype="xsd:date">2023</dcterms:issued> <!-- Date of the source document, comment out if draft -->
        <owl:priorVersion rdf:datatype="xsd:date">2017-11-05</owl:priorVersion> <!-- Date of prior ontology file, if any -->
		<dcterms:created rdf:datatype="xsd:date">2026-01-13</dcterms:created> <!-- Date of creation of this ontology file -->
        <owl:versionInfo>1.3.0</owl:versionInfo>
        <owl:versionIRI rdf:resource="https://w3id.org/isoiec5087/-1/v1/r3.0"/>
        <rdfs:comment>The prior version of this ontology was divided into a distinct file 
            for each pattern contained within Part 1; this version combines all of the 
            patterns into a single file for ease of reference. Some of the prior component 
            ontology files were labelled as v1.2. This update does not make any semantic
            changes from the approved ontology, but does correct several references 
            resulting in a change greater than a patch but less than a major change. As 
            such, it is published as v1.3.0.</rdfs:comment>
        
        <!-- License -->
        <cc:license>http://creativecommons.org/licenses/by/4.0/</cc:license>
        
        <!-- Imports -->
        <owl:imports rdf:resource="http://www.w3.org/ns/prov"/>
        <owl:imports rdf:resource="http://www.w3.org/ns/org"/>
        <owl:imports rdf:resource="http://www.w3.org/2006/time"/>

    </owl:Ontology>
    

    <!-- 
    ///////////////////////////////////////////////////////////////////////////////////////
    //
    // Object Properties
    //
    ///////////////////////////////////////////////////////////////////////////////////////
     -->
    <!-- https://w3id.org/isoiec5087/-1/v1/CdmObjectProperty -->

    <owl:ObjectProperty rdf:about="https://w3id.org/isoiec5087/-1/v1/CdmObjectProperty">
        <skos:definition>Added for organizational purposes, to identify all object properties defined in the City Data Model.</skos:definition>
    </owl:ObjectProperty>


    <!-- https://w3id.org/isoiec5087/-1/v1/FoundationalCdmObjectProperty -->

    <owl:ObjectProperty rdf:about="https://w3id.org/isoiec5087/-1/v1/FoundationalCdmObjectProperty">
        <rdfs:subPropertyOf rdf:resource="https://w3id.org/isoiec5087/-1/v1/CdmObjectProperty"/>
        <skos:definition>Added for organizational purposes, to identify all foundational object properties defined in the City Data Model.</skos:definition>
    </owl:ObjectProperty>


    <!-- https://w3id.org/isoiec5087/-1/v1/achievedAt -->
<!-- Ask Grok about what the axioms mean and whether they are properly declared and in the right locations. In particular 
 conjunctiveAchievedAt is defined separately as a subtype while the others listed are not. It seems as if these axioms 
 should be declared within the subtypes not in the parent. Also, it seems strange to have two description fields in the 
 axiom. Finally, this info is not in 5087-1. Also, do we want the -->
    <owl:ObjectProperty rdf:about="https://w3id.org/isoiec5087/-1/v1/achievedAt">
        <skos:definition>Identifies the time Interval or Instant during which the State was satisfied.</skos:definition>
        <rdfs:subPropertyOf rdf:resource="https://w3id.org/isoiec5087/-1/v1/FoundationalCdmObjectProperty"/>
        <rdfs:domain rdf:resource="https://w3id.org/isoiec5087/-1/v1/State"/>
        <rdfs:range rdf:resource="time:TemporalEntity"/>
        <owl:propertyChainAxiom rdf:parseType="Collection">
            <rdf:Description>
                <owl:inverseOf rdf:resource="https://w3id.org/isoiec5087/-1/v1/effectOf"/>
            </rdf:Description>
            <rdf:Description rdf:about="https://w3id.org/isoiec5087/-1/v1/endOf"/>
        </owl:propertyChainAxiom>
        <owl:propertyChainAxiom rdf:parseType="Collection">
            <rdf:Description>
                <owl:inverseOf rdf:resource="https://w3id.org/isoiec5087/-1/v1/hasDecomp"/>
            </rdf:Description>
            <rdf:Description rdf:about="https://w3id.org/isoiec5087/-1/v1/conjunctiveAchievedAt"/>
            <rdf:Description rdf:about="http://www.w3.org/2006/time#intervalDuring"/>
        </owl:propertyChainAxiom>
        <owl:propertyChainAxiom rdf:parseType="Collection">
            <rdf:Description>
                <owl:inverseOf rdf:resource="https://w3id.org/isoiec5087/-1/v1/preconditionOf"/>
            </rdf:Description>
            <rdf:Description rdf:about="https://w3id.org/isoiec5087/-1/v1/beginOf"/>
        </owl:propertyChainAxiom>
    </owl:ObjectProperty>
    


    <!-- https://w3id.org/isoiec5087/-1/v1/beginOf -->

    <owl:ObjectProperty rdf:about="https://w3id.org/isoiec5087/-1/v1/beginOf">
        <rdfs:subPropertyOf rdf:resource="https://w3id.org/isoiec5087/-1/v1/ActivityOntologyProperty"/>
        <rdfs:domain rdf:resource="https://w3id.org/isoiec5087/-1/v1/Activity"/>
        <rdfs:range rdf:resource="time:Instant"/>
        <owl:propertyChainAxiom rdf:parseType="Collection">
            <rdf:Description rdf:about="https://w3id.org/isoiec5087/-1/v1/occursAt"/>
            <rdf:Description rdf:about="http://www.w3.org/2006/time#hasBeginning"/>
        </owl:propertyChainAxiom>
    </owl:ObjectProperty>
    


    <!-- https://w3id.org/isoiec5087/-1/v1/causedBy -->

    <owl:ObjectProperty rdf:about="https://w3id.org/isoiec5087/-1/v1/causedBy">
        <rdfs:subPropertyOf rdf:resource="https://w3id.org/isoiec5087/-1/v1/ActivityOntologyProperty"/>
        <owl:inverseOf rdf:resource="https://w3id.org/isoiec5087/-1/v1/causes"/>
    </owl:ObjectProperty>
    


    <!-- https://w3id.org/isoiec5087/-1/v1/causes -->

    <owl:ObjectProperty rdf:about="https://w3id.org/isoiec5087/-1/v1/causes">
        <rdfs:subPropertyOf rdf:resource="https://w3id.org/isoiec5087/-1/v1/ActivityOntologyProperty"/>
    </owl:ObjectProperty>
    


    <!-- https://w3id.org/isoiec5087/-1/v1/conjunctiveAchievedAt -->

    <owl:ObjectProperty rdf:about="https://w3id.org/isoiec5087/-1/v1/conjunctiveAchievedAt">
        <rdfs:subPropertyOf rdf:resource="https://w3id.org/isoiec5087/-1/v1/achievedAt"/>
        <rdfs:domain rdf:resource="https://w3id.org/isoiec5087/-1/v1/ConjunctiveState"/>
    </owl:ObjectProperty>
    


    <!-- https://w3id.org/isoiec5087/-1/v1/disjunctiveAchievedAt -->

    <owl:ObjectProperty rdf:about="https://w3id.org/isoiec5087/-1/v1/disjunctiveAchievedAt">
        <rdfs:subPropertyOf rdf:resource="https://w3id.org/isoiec5087/-1/v1/achievedAt"/>
        <rdfs:domain rdf:resource="https://w3id.org/isoiec5087/-1/v1/DisjunctiveState"/>
    </owl:ObjectProperty>
    


    <!-- https://w3id.org/isoiec5087/-1/v1/effectOf -->

    <owl:ObjectProperty rdf:about="https://w3id.org/isoiec5087/-1/v1/effectOf">
        <skos:definition>Identifies an Activity that the State was realized by.</skos:definition>
        <rdfs:subPropertyOf rdf:resource="https://w3id.org/isoiec5087/-1/v1/ActivityOntologyProperty"/>
        <owl:inverseOf rdf:resource="https://w3id.org/isoiec5087/-1/v1/hasEffect"/>
    </owl:ObjectProperty>
    


    <!-- https://w3id.org/isoiec5087/-1/v1/enabledBy -->

    <owl:ObjectProperty rdf:about="https://w3id.org/isoiec5087/-1/v1/enabledBy">
        <rdfs:subPropertyOf rdf:resource="https://w3id.org/isoiec5087/-1/v1/ActivityOntologyProperty"/>
        <owl:inverseOf rdf:resource="https://w3id.org/isoiec5087/-1/v1/enables"/>
    </owl:ObjectProperty>
    


    <!-- https://w3id.org/isoiec5087/-1/v1/enables -->

    <owl:ObjectProperty rdf:about="https://w3id.org/isoiec5087/-1/v1/enables">
        <rdfs:subPropertyOf rdf:resource="https://w3id.org/isoiec5087/-1/v1/ActivityOntologyProperty"/>
    </owl:ObjectProperty>
    


    <!-- https://w3id.org/isoiec5087/-1/v1/endOf -->

    <owl:ObjectProperty rdf:about="https://w3id.org/isoiec5087/-1/v1/endOf">
        <rdfs:subPropertyOf rdf:resource="https://w3id.org/isoiec5087/-1/v1/ActivityOntologyProperty"/>
        <rdfs:domain rdf:resource="https://w3id.org/isoiec5087/-1/v1/Activity"/>
        <rdfs:range rdf:resource="time:Instant"/>
        <owl:propertyChainAxiom rdf:parseType="Collection">
            <rdf:Description rdf:about="https://w3id.org/isoiec5087/-1/v1/occursAt"/>
            <rdf:Description rdf:about="http://www.w3.org/2006/time#hasEnd"/>
        </owl:propertyChainAxiom>
    </owl:ObjectProperty>
    


    <!-- https://w3id.org/isoiec5087/-1/v1/hasDecomp -->

    <owl:ObjectProperty rdf:about="https://w3id.org/isoiec5087/-1/v1/hasDecomp">
        <rdfs:subPropertyOf rdf:resource="https://w3id.org/isoiec5087/-1/v1/hasSubstate"/>
        <rdfs:domain rdf:resource="https://w3id.org/isoiec5087/-1/v1/State"/>
        <rdfs:range rdf:resource="https://w3id.org/isoiec5087/-1/v1/State"/>
    </owl:ObjectProperty>
    


    <!-- https://w3id.org/isoiec5087/-1/v1/hasEffect -->

    <owl:ObjectProperty rdf:about="https://w3id.org/isoiec5087/-1/v1/hasEffect">
        <rdfs:subPropertyOf rdf:resource="https://w3id.org/isoiec5087/-1/v1/causedBy"/>
        <rdfs:domain rdf:resource="https://w3id.org/isoiec5087/-1/v1/Activity"/>
        <rdfs:range rdf:resource="https://w3id.org/isoiec5087/-1/v1/State"/>
    </owl:ObjectProperty>
    


    <!-- https://w3id.org/isoiec5087/-1/v1/hasPrecondition -->

    <owl:ObjectProperty rdf:about="https://w3id.org/isoiec5087/-1/v1/hasPrecondition">
        <rdfs:subPropertyOf rdf:resource="https://w3id.org/isoiec5087/-1/v1/enabledBy"/>
        <owl:inverseOf rdf:resource="https://w3id.org/isoiec5087/-1/v1/preconditionOf"/>
        <rdfs:domain rdf:resource="https://w3id.org/isoiec5087/-1/v1/Activity"/>
        <rdfs:range rdf:resource="https://w3id.org/isoiec5087/-1/v1/State"/>
    </owl:ObjectProperty>
    


    <!-- https://w3id.org/isoiec5087/-1/v1/hasStatus -->

    <owl:ObjectProperty rdf:about="https://w3id.org/isoiec5087/-1/v1/hasStatus">
        <rdfs:subPropertyOf rdf:resource="https://w3id.org/isoiec5087/-1/v1/ActivityOntologyProperty"/>
    </owl:ObjectProperty>
    


    <!-- https://w3id.org/isoiec5087/-1/v1/hasSubactivity -->

    <owl:ObjectProperty rdf:about="https://w3id.org/isoiec5087/-1/v1/hasSubactivity">
        <rdfs:subPropertyOf rdf:resource="https://w3id.org/isoiec5087/-1/v1/ActivityOntologyProperty"/>
    </owl:ObjectProperty>
    


    <!-- https://w3id.org/isoiec5087/-1/v1/hasSubstate -->

    <owl:ObjectProperty rdf:about="https://w3id.org/isoiec5087/-1/v1/hasSubstate">
        <rdfs:subPropertyOf rdf:resource="https://w3id.org/isoiec5087/-1/v1/ActivityOntologyProperty"/>
        <rdf:type rdf:resource="owl:TransitiveProperty"/>
    </owl:ObjectProperty>
    


    <!-- https://w3id.org/isoiec5087/-1/v1/occursAfter -->

    <owl:ObjectProperty rdf:about="https://w3id.org/isoiec5087/-1/v1/occursAfter">
        <rdfs:subPropertyOf rdf:resource="https://w3id.org/isoiec5087/-1/v1/ActivityOntologyProperty"/>
        <owl:inverseOf rdf:resource="https://w3id.org/isoiec5087/-1/v1/occursBefore"/>
    </owl:ObjectProperty>
    


    <!-- https://w3id.org/isoiec5087/-1/v1/occursAt -->

    <owl:ObjectProperty rdf:about="https://w3id.org/isoiec5087/-1/v1/occursAt">
        <rdfs:subPropertyOf rdf:resource="https://w3id.org/isoiec5087/-1/v1/ActivityOntologyProperty"/>
        <rdfs:range rdf:resource="time:TemporalEntity"/>
    </owl:ObjectProperty>
    


    <!-- https://w3id.org/isoiec5087/-1/v1/occursBefore -->

    <owl:ObjectProperty rdf:about="https://w3id.org/isoiec5087/-1/v1/occursBefore">
        <rdfs:subPropertyOf rdf:resource="https://w3id.org/isoiec5087/-1/v1/ActivityOntologyProperty"/>
        <rdf:type rdf:resource="owl:TransitiveProperty"/>
        <rdfs:domain rdf:resource="https://w3id.org/isoiec5087/-1/v1/Activity"/>
        <rdfs:range rdf:resource="https://w3id.org/isoiec5087/-1/v1/Activity"/>
        <rdfs:comment>An activity occursBefore another if its endOf instant is before the beginOf instant of the other activity; the occursBefore relation is transitive. We cannot define this semantics in OWL, though it could be captured in future work by an extension with rules.</rdfs:comment>
    </owl:ObjectProperty>
    


    <!-- https://w3id.org/isoiec5087/-1/v1/occursDirectlyAfter -->

    <owl:ObjectProperty rdf:about="https://w3id.org/isoiec5087/-1/v1/occursDirectlyAfter">
        <rdfs:subPropertyOf rdf:resource="https://w3id.org/isoiec5087/-1/v1/occursAfter"/>
        <owl:inverseOf rdf:resource="https://w3id.org/isoiec5087/-1/v1/occursDirectlyBefore"/>
    </owl:ObjectProperty>
    


    <!-- https://w3id.org/isoiec5087/-1/v1/occursDirectlyBefore -->

    <owl:ObjectProperty rdf:about="https://w3id.org/isoiec5087/-1/v1/occursDirectlyBefore">
        <rdfs:subPropertyOf rdf:resource="https://w3id.org/isoiec5087/-1/v1/occursBefore"/>
        <rdfs:domain rdf:resource="https://w3id.org/isoiec5087/-1/v1/Activity"/>
        <rdfs:range rdf:resource="https://w3id.org/isoiec5087/-1/v1/Activity"/>
        <rdfs:comment>An activity occursDirectlyBefore another if it occursAt an interval that meets the interval of the other activity. We cannot define this semantics in OWL, though it could be captured by an extension with rules.</rdfs:comment>
    </owl:ObjectProperty>
    


    <!-- https://w3id.org/isoiec5087/-1/v1/preconditionOf -->

    <owl:ObjectProperty rdf:about="https://w3id.org/isoiec5087/-1/v1/preconditionOf">
        <skos:definition></skos:definition>
        <rdfs:subPropertyOf rdf:resource="https://w3id.org/isoiec5087/-1/v1/ActivityOntologyProperty"/>
    </owl:ObjectProperty>
    


    <!-- https://w3id.org/isoiec5087/-1/v1/satisfiedBy -->

    <owl:ObjectProperty rdf:about="https://w3id.org/isoiec5087/-1/v1/satisfiedBy">
        <rdfs:subPropertyOf rdf:resource="https://w3id.org/isoiec5087/-1/v1/ActivityOntologyProperty"/>
    </owl:ObjectProperty>
    


    <!-- https://w3id.org/isoiec5087/-1/v1/scheduledFor -->

    <owl:ObjectProperty rdf:about="https://w3id.org/isoiec5087/-1/v1/scheduledFor">
        <skos:definition>Identifies a time Interval during which the State is scheduled to be realized.</skos:definition>
        <rdfs:subPropertyOf rdf:resource="https://w3id.org/isoiec5087/-1/v1/ActivityOntologyProperty"/>
    </owl:ObjectProperty>
    


    <!-- https://w3id.org/isoiec5087/-1/v1/terminalAchievedAt -->

    <owl:ObjectProperty rdf:about="https://w3id.org/isoiec5087/-1/v1/terminalAchievedAt">
        <rdfs:subPropertyOf rdf:resource="https://w3id.org/isoiec5087/-1/v1/achievedAt"/>
        <rdfs:domain rdf:resource="https://w3id.org/isoiec5087/-1/v1/TerminalState"/>
    </owl:ObjectProperty>
    


    <!-- 
    ///////////////////////////////////////////////////////////////////////////////////////
    //
    // Classes
    //
    ///////////////////////////////////////////////////////////////////////////////////////
     -->

    <!-- https://w3id.org/isoiec5087/-1/v1/Activity -->

    <owl:Class rdf:about="https://w3id.org/isoiec5087/-1/v1/Activity">
        <rdfs:subClassOf rdf:resource="https://w3id.org/isoiec5087/-1/v1/ActivityOntologyThing"/>
        <rdfs:subClassOf>
            <owl:Restriction>
                <owl:onProperty rdf:resource="https://w3id.org/isoiec5087/-1/v1/occursAt"/>
                <owl:someValuesFrom rdf:resource="time:Interval"/>
            </owl:Restriction>
        </rdfs:subClassOf>
        <rdfs:subClassOf>
            <owl:Restriction>
                <owl:onProperty rdf:resource="https://w3id.org/isoiec5087/-1/v1/associatedLocation"/>
                <owl:allValuesFrom rdf:resource="https://w3id.org/isoiec5087/-1/v1/Location"/>
            </owl:Restriction>
        </rdfs:subClassOf>
        <rdfs:subClassOf>
            <owl:Restriction>
                <owl:onProperty rdf:resource="https://w3id.org/isoiec5087/-1/v1/causes"/>
                <owl:allValuesFrom rdf:resource="https://w3id.org/isoiec5087/-1/v1/State"/>
            </owl:Restriction>
        </rdfs:subClassOf>
        <rdfs:subClassOf>
            <owl:Restriction>
                <owl:onProperty rdf:resource="https://w3id.org/isoiec5087/-1/v1/enabledBy"/>
                <owl:allValuesFrom rdf:resource="https://w3id.org/isoiec5087/-1/v1/State"/>
            </owl:Restriction>
        </rdfs:subClassOf>
        <rdfs:subClassOf>
            <owl:Restriction>
                <owl:onProperty rdf:resource="https://w3id.org/isoiec5087/-1/v1/hasEffect"/>
                <owl:allValuesFrom rdf:resource="https://w3id.org/isoiec5087/-1/v1/State"/>
            </owl:Restriction>
        </rdfs:subClassOf>
        <rdfs:subClassOf>
            <owl:Restriction>
                <owl:onProperty rdf:resource="https://w3id.org/isoiec5087/-1/v1/hasPrecondition"/>
                <owl:allValuesFrom rdf:resource="https://w3id.org/isoiec5087/-1/v1/State"/>
            </owl:Restriction>
        </rdfs:subClassOf>
        <rdfs:subClassOf>
            <owl:Restriction>
                <owl:onProperty rdf:resource="https://w3id.org/isoiec5087/-1/v1/hasSubactivity"/>
                <owl:allValuesFrom rdf:resource="https://w3id.org/isoiec5087/-1/v1/Activity"/>
            </owl:Restriction>
        </rdfs:subClassOf>
        <rdfs:subClassOf>
            <owl:Restriction>
                <owl:onProperty rdf:resource="https://w3id.org/isoiec5087/-1/v1/occursBefore"/>
                <owl:allValuesFrom rdf:resource="https://w3id.org/isoiec5087/-1/v1/Activity"/>
            </owl:Restriction>
        </rdfs:subClassOf>
        <rdfs:subClassOf>
            <owl:Restriction>
                <owl:onProperty rdf:resource="https://w3id.org/isoiec5087/-1/v1/occursDirectlyBefore"/>
                <owl:allValuesFrom rdf:resource="https://w3id.org/isoiec5087/-1/v1/Activity"/>
            </owl:Restriction>
        </rdfs:subClassOf>
        <rdfs:subClassOf>
            <owl:Restriction>
                <owl:onProperty rdf:resource="https://w3id.org/isoiec5087/-1/v1/hasStatus"/>
                <owl:qualifiedCardinality rdf:datatype="xsd:nonNegativeInteger">1</owl:qualifiedCardinality>
                <owl:onClass rdf:resource="https://w3id.org/isoiec5087/-1/v1/ActivityStatus"/>
            </owl:Restriction>
        </rdfs:subClassOf>
        <skos:definition>An Activity describes something that occurs in the domain.
An Activity may be further defined by (decomposed into) Subactivities.
An Activity may have precondition and/or effect State.
An Activity may be enabled by or cause some State. An enabling of causing state is a generalization of a precondition/effect; an Activity is enabled by or causes some State if it has a subactivity with a precondition or effect (respectively) of that State. 
In other words, the state may not be required directly before, or cause directly after the activity, but by some more specialized sub-activity.
An Activity occurs at some point in time and space.
An Activity takes place during some interval, and so has some duration.
An Activity may have some Manifestations that participate in it.</skos:definition>
    </owl:Class>
    


    <!-- https://w3id.org/isoiec5087/-1/v1/ActivityOntologyThing -->

    <owl:Class rdf:about="https://w3id.org/isoiec5087/-1/v1/ActivityOntologyThing">
        <skos:definition>Added for organizational purposes, to identify all classes defined in the Activity ontology.</skos:definition>
    </owl:Class>
    


    <!-- https://w3id.org/isoiec5087/-1/v1/ActivityStatus -->

    <owl:Class rdf:about="https://w3id.org/isoiec5087/-1/v1/ActivityStatus">
        <rdfs:subClassOf rdf:resource="https://w3id.org/isoiec5087/-1/v1/ActivityOntologyThing"/>
    </owl:Class>
    


    <!-- https://w3id.org/isoiec5087/-1/v1/ConjunctiveState -->

    <owl:Class rdf:about="https://w3id.org/isoiec5087/-1/v1/ConjunctiveState">
        <rdfs:subClassOf rdf:resource="https://w3id.org/isoiec5087/-1/v1/NonTerminalState"/>
        <owl:disjointWith rdf:resource="https://w3id.org/isoiec5087/-1/v1/DisjunctiveState"/>
        <skos:definition>Naturally, a conjunctive state type is defined by the conjunction of its child state types, whereas a disjunctive state type is defined by the disjunction of its child states.</skos:definition>
    </owl:Class>
    


    <!-- https://w3id.org/isoiec5087/-1/v1/DisjunctiveState -->

    <owl:Class rdf:about="https://w3id.org/isoiec5087/-1/v1/DisjunctiveState">
        <rdfs:subClassOf rdf:resource="https://w3id.org/isoiec5087/-1/v1/NonTerminalState"/>
        <skos:definition>Naturally, a conjunctive state type is defined by the conjunction of its child state types, whereas a disjunctive state type is defined by the disjunction of its child states.</skos:definition>
    </owl:Class>
    


    <!-- https://w3id.org/isoiec5087/-1/v1/ManifestationState -->

    <owl:Class rdf:about="https://w3id.org/isoiec5087/-1/v1/ManifestationState">
        <rdfs:subClassOf rdf:resource="https://w3id.org/isoiec5087/-1/v1/TerminalState"/>
        <rdfs:subClassOf>
            <owl:Restriction>
                <owl:onProperty rdf:resource="https://w3id.org/isoiec5087/-1/v1/satisfiedBy"/>
                <owl:allValuesFrom rdf:resource="https://w3id.org/isoiec5087/-1/v1/Manifestation"/>
            </owl:Restriction>
        </rdfs:subClassOf>
    </owl:Class>
    


    <!-- https://w3id.org/isoiec5087/-1/v1/NonTerminalState -->

    <owl:Class rdf:about="https://w3id.org/isoiec5087/-1/v1/NonTerminalState">
        <rdfs:subClassOf rdf:resource="https://w3id.org/isoiec5087/-1/v1/State"/>
        <rdfs:subClassOf>
            <owl:Class>
                <owl:intersectionOf rdf:parseType="Collection">
                    <owl:Restriction>
                        <owl:onProperty rdf:resource="https://w3id.org/isoiec5087/-1/v1/hasDecomp"/>
                        <owl:allValuesFrom rdf:resource="https://w3id.org/isoiec5087/-1/v1/State"/>
                    </owl:Restriction>
                    <owl:Restriction>
                        <owl:onProperty rdf:resource="https://w3id.org/isoiec5087/-1/v1/hasDecomp"/>
                        <owl:minQualifiedCardinality rdf:datatype="xsd:nonNegativeInteger">2</owl:minQualifiedCardinality>
                        <owl:onClass rdf:resource="https://w3id.org/isoiec5087/-1/v1/State"/>
                    </owl:Restriction>
                </owl:intersectionOf>
            </owl:Class>
        </rdfs:subClassOf>
        <rdfs:subClassOf>
            <owl:Restriction>
                <owl:onProperty rdf:resource="https://w3id.org/isoiec5087/-1/v1/hasSubstate"/>
                <owl:allValuesFrom rdf:resource="https://w3id.org/isoiec5087/-1/v1/State"/>
            </owl:Restriction>
        </rdfs:subClassOf>
        <owl:disjointWith rdf:resource="https://w3id.org/isoiec5087/-1/v1/TerminalState"/>
        <skos:definition>A non-terminal state type has substates. It may be conjunctive or disjunctive. 
A state type cannot be both conjunctive and disjunctive.
	ConjunctiveStateType disjointWith DisjunctiveStateType
Conjunctive and disjunctive state types, which do have substates, are achieved at some time if their decomposition of state types is achieved.
Note that in this representation, decomp_of is not a transitive relation, it only refers to the direct children of a non-terminal state type. A more general relation that is transitive is the substate relation.
decomp_of(x,y) -&gt; substate(x,y)</skos:definition>
    </owl:Class>
    


    <!-- https://w3id.org/isoiec5087/-1/v1/State -->

    <owl:Class rdf:about="https://w3id.org/isoiec5087/-1/v1/State">
        <rdfs:subClassOf rdf:resource="https://w3id.org/isoiec5087/-1/v1/ActivityOntologyThing"/>
        <rdfs:subClassOf>
            <owl:Restriction>
                <owl:onProperty rdf:resource="https://w3id.org/isoiec5087/-1/v1/causedBy"/>
                <owl:allValuesFrom rdf:resource="https://w3id.org/isoiec5087/-1/v1/Activity"/>
            </owl:Restriction>
        </rdfs:subClassOf>
        <rdfs:subClassOf>
            <owl:Restriction>
                <owl:onProperty rdf:resource="https://w3id.org/isoiec5087/-1/v1/effectOf"/>
                <owl:allValuesFrom rdf:resource="https://w3id.org/isoiec5087/-1/v1/Activity"/>
            </owl:Restriction>
        </rdfs:subClassOf>
        <rdfs:subClassOf>
            <owl:Restriction>
                <owl:onProperty rdf:resource="https://w3id.org/isoiec5087/-1/v1/enables"/>
                <owl:allValuesFrom rdf:resource="https://w3id.org/isoiec5087/-1/v1/Activity"/>
            </owl:Restriction>
        </rdfs:subClassOf>
        <rdfs:subClassOf>
            <owl:Restriction>
                <owl:onProperty rdf:resource="https://w3id.org/isoiec5087/-1/v1/preconditionOf"/>
                <owl:allValuesFrom rdf:resource="https://w3id.org/isoiec5087/-1/v1/Activity"/>
            </owl:Restriction>
        </rdfs:subClassOf>
        <rdfs:subClassOf>
            <owl:Restriction>
                <owl:onProperty rdf:resource="https://w3id.org/isoiec5087/-1/v1/hasStatus"/>
                <owl:qualifiedCardinality rdf:datatype="xsd:nonNegativeInteger">1</owl:qualifiedCardinality>
                <owl:onClass rdf:resource="https://w3id.org/isoiec5087/-1/v1/StateStatus"/>
            </owl:Restriction>
        </rdfs:subClassOf>
        <skos:definition>A state refers to a class of manifestations. It may be a precondition or effect of some Activity, or more generally it may enabled or be caused by some Activity. If a state is complex, it may refer to some combination of classes of manifestations.
A note on complex states:
Say that a shopping activity, Activity-Shop, requires both the VehicleW30LGas state, but also some state wherein the mall is open, OpenMall. Each state would first be defined separately. Then, we can simply state:
precondition(VehicleW30LGas,Activity-Shop) AND  precondition(OpenMall,Activity-Shop)
were the preconditions required disjunctively, we could state:
precondition(VehicleW30LGas,Activity-Shop) OR precondition(OpenMall,Activity-Shop)
However, in large and complex domains, there will be cases in which the above approach is undesirable. In particular, due to the complexity of the description that results as the state being described becomes more detailed. In many cases it will be more natural and convenient to be able to refer to a single, aggregate state. We therefore extend the representation of States to capture aggregation, as approached in the concept of state trees introduced by TOVE as a construct for the activity cluster.

A State may be either non-terminal or terminal. A terminal state has no child states, and therefore refers directly to a class of manifestations, whereas a non-terminal state has child states, which may define some classes of manifestations, or further define some other complex states.
	NonTerminalState(x) v TerminalState(x) = State(x)
A state  cannot be both non-terminal and terminal.
	TerminalState disjointWith NonTerminalState</skos:definition>
    </owl:Class>
    


    <!-- https://w3id.org/isoiec5087/-1/v1/StateStatus -->

    <owl:Class rdf:about="https://w3id.org/isoiec5087/-1/v1/StateStatus">
        <rdfs:subClassOf rdf:resource="https://w3id.org/isoiec5087/-1/v1/ActivityOntologyThing"/>
    </owl:Class>
    


    <!-- https://w3id.org/isoiec5087/-1/v1/TerminalState -->

    <owl:Class rdf:about="https://w3id.org/isoiec5087/-1/v1/TerminalState">
        <rdfs:subClassOf rdf:resource="https://w3id.org/isoiec5087/-1/v1/State"/>
        <rdfs:subClassOf>
            <owl:Restriction>
                <owl:onProperty rdf:resource="https://w3id.org/isoiec5087/-1/v1/hasDecomp"/>
                <owl:qualifiedCardinality rdf:datatype="xsd:nonNegativeInteger">0</owl:qualifiedCardinality>
                <owl:onClass rdf:resource="https://w3id.org/isoiec5087/-1/v1/State"/>
            </owl:Restriction>
        </rdfs:subClassOf>
        <skos:definition>A terminal state type has no substates (cannot be decomposed). It corresponds to a particular class of manifestations. A terminal state is achieved at some time if and only if there exists a manifestation within its defined classification, that exists at that time.

hasResource: links to the resource participating in the state
hasQuantity: specifies the quantity of resource participating in the state</skos:definition>
    </owl:Class>
    


    <!-- https://w3id.org/isoiec5087/-1/v1/AgentOntologyObjectProperty -->

    <owl:ObjectProperty rdf:about="https://w3id.org/isoiec5087/-1/v1/AgentOntologyObjectProperty"/>
    


    <!-- https://w3id.org/isoiec5087/-1/v1/performedBy -->

    <owl:ObjectProperty rdf:about="https://w3id.org/isoiec5087/-1/v1/performedBy">
        <rdfs:subPropertyOf rdf:resource="https://w3id.org/isoiec5087/-1/v1/AgentOntologyObjectProperty"/>
        <owl:inverseOf rdf:resource="https://w3id.org/isoiec5087/-1/v1/performs"/>
    </owl:ObjectProperty>
    


    <!-- https://w3id.org/isoiec5087/-1/v1/performs -->

    <owl:ObjectProperty rdf:about="https://w3id.org/isoiec5087/-1/v1/performs">
        <rdfs:subPropertyOf rdf:resource="https://w3id.org/isoiec5087/-1/v1/AgentOntologyObjectProperty"/>
        <rdf:type rdf:resource="owl:ReflexiveProperty"/>
    </owl:ObjectProperty>
    


    <!-- 
    ///////////////////////////////////////////////////////////////////////////////////////
    //
    // Data properties
    //
    ///////////////////////////////////////////////////////////////////////////////////////
     -->

    


    <!-- https://w3id.org/isoiec5087/-1/v1/AgentOntologyDataProperty -->

    <owl:DatatypeProperty rdf:about="https://w3id.org/isoiec5087/-1/v1/AgentOntologyDataProperty"/>
    


    <!-- 
    ///////////////////////////////////////////////////////////////////////////////////////
    //
    // Classes
    //
    ///////////////////////////////////////////////////////////////////////////////////////
     -->

    <!-- https://w3id.org/isoiec5087/-1/v1/Agent -->

    <owl:Class rdf:about="https://w3id.org/isoiec5087/-1/v1/Agent">
        <rdfs:subClassOf rdf:resource="https://w3id.org/isoiec5087/-1/v1/AgentOntologyThing"/>
        <rdfs:subClassOf rdf:resource="http://xmlns.com/foaf/0.1/Agent"/>
        <rdfs:subClassOf>
            <owl:Restriction>
                <owl:onProperty rdf:resource="https://w3id.org/isoiec5087/-1/v1/performs"/>
                <owl:allValuesFrom rdf:resource="https://w3id.org/isoiec5087/-1/v1/Activity"/>
            </owl:Restriction>
        </rdfs:subClassOf>
        <rdfs:subClassOf>
            <owl:Restriction>
                <owl:onProperty rdf:resource="https://w3id.org/isoiec5087/-1/v1/resourceOf"/>
                <owl:allValuesFrom rdf:resource="https://w3id.org/isoiec5087/-1/v1/Activity"/>
            </owl:Restriction>
        </rdfs:subClassOf>
        <rdfs:subClassOf>
            <owl:Restriction>
                <owl:onProperty rdf:resource="https://w3id.org/isoiec5087/-1/v1/hasName"/>
                <owl:qualifiedCardinality rdf:datatype="xsd:nonNegativeInteger">1</owl:qualifiedCardinality>
                <owl:onDataRange rdf:resource="xsd:string"/>
            </owl:Restriction>
        </rdfs:subClassOf>
        <rdfs:comment>An Agent may be a Person or Organization. This is captured in the Person and Ontology patterns.  An Agent can also perform an Activity. 
We do not include Software or Mechanical Device (at this time). An Agent can be a member of an organization and hold zero or more posts in an organization.</rdfs:comment>
    </owl:Class>
    


    <!-- https://w3id.org/isoiec5087/-1/v1/AgentOntologyThing -->

    <owl:Class rdf:about="https://w3id.org/isoiec5087/-1/v1/AgentOntologyThing"/>
    <!-- 
    ///////////////////////////////////////////////////////////////////////////////////////
    //
    // Object Properties
    //
    ///////////////////////////////////////////////////////////////////////////////////////
     -->


    <!-- https://w3id.org/isoiec5087/-1/v1/AgreementOntologyObjectProperty -->

    <owl:ObjectProperty rdf:about="https://w3id.org/isoiec5087/-1/v1/AgreementOntologyObjectProperty"/>
    


    <!-- https://w3id.org/isoiec5087/-1/v1/agentInvolvedIn -->

    <owl:ObjectProperty rdf:about="https://w3id.org/isoiec5087/-1/v1/agentInvolvedIn">
        <rdfs:subPropertyOf rdf:resource="https://w3id.org/isoiec5087/-1/v1/AgreementOntologyObjectProperty"/>
        <owl:inverseOf rdf:resource="https://w3id.org/isoiec5087/-1/v1/involvesAgent"/>
    </owl:ObjectProperty>
    


    <!-- https://w3id.org/isoiec5087/-1/v1/commitsToActivity -->

    <owl:ObjectProperty rdf:about="https://w3id.org/isoiec5087/-1/v1/commitsToActivity">
        <rdfs:subPropertyOf rdf:resource="https://w3id.org/isoiec5087/-1/v1/AgreementOntologyObjectProperty"/>
    </owl:ObjectProperty>
    


    <!-- https://w3id.org/isoiec5087/-1/v1/establishedOn -->

    <owl:ObjectProperty rdf:about="https://w3id.org/isoiec5087/-1/v1/establishedOn">
        <rdfs:subPropertyOf rdf:resource="https://w3id.org/isoiec5087/-1/v1/AgreementOntologyObjectProperty"/>
    </owl:ObjectProperty>
    


    <!-- https://w3id.org/isoiec5087/-1/v1/hasClaim -->

    <owl:ObjectProperty rdf:about="https://w3id.org/isoiec5087/-1/v1/hasClaim">
        <rdfs:subPropertyOf rdf:resource="https://w3id.org/isoiec5087/-1/v1/agentInvolvedIn"/>
    </owl:ObjectProperty>
    


    <!-- https://w3id.org/isoiec5087/-1/v1/hasDuty -->

    <owl:ObjectProperty rdf:about="https://w3id.org/isoiec5087/-1/v1/hasDuty">
        <rdfs:subPropertyOf rdf:resource="https://w3id.org/isoiec5087/-1/v1/agentInvolvedIn"/>
    </owl:ObjectProperty>
    


    <!-- https://w3id.org/isoiec5087/-1/v1/hasNoClaim -->

    <owl:ObjectProperty rdf:about="https://w3id.org/isoiec5087/-1/v1/hasNoClaim">
        <rdfs:subPropertyOf rdf:resource="https://w3id.org/isoiec5087/-1/v1/agentInvolvedIn"/>
    </owl:ObjectProperty>
    


    <!-- https://w3id.org/isoiec5087/-1/v1/hasPrivilege -->

    <owl:ObjectProperty rdf:about="https://w3id.org/isoiec5087/-1/v1/hasPrivilege">
        <rdfs:subPropertyOf rdf:resource="https://w3id.org/isoiec5087/-1/v1/agentInvolvedIn"/>
    </owl:ObjectProperty>
    


    <!-- https://w3id.org/isoiec5087/-1/v1/hasSubAgreement -->

    <owl:ObjectProperty rdf:about="https://w3id.org/isoiec5087/-1/v1/hasSubAgreement">
        <rdfs:subPropertyOf rdf:resource="https://w3id.org/isoiec5087/-1/v1/AgreementOntologyObjectProperty"/>
    </owl:ObjectProperty>
    


    <!-- https://w3id.org/isoiec5087/-1/v1/involvesAgent -->

    <owl:ObjectProperty rdf:about="https://w3id.org/isoiec5087/-1/v1/involvesAgent">
        <rdfs:subPropertyOf rdf:resource="https://w3id.org/isoiec5087/-1/v1/AgreementOntologyObjectProperty"/>
    </owl:ObjectProperty>
    


    <!-- https://w3id.org/isoiec5087/-1/v1/validFor -->

    <owl:ObjectProperty rdf:about="https://w3id.org/isoiec5087/-1/v1/validFor">
        <rdfs:subPropertyOf rdf:resource="https://w3id.org/isoiec5087/-1/v1/AgreementOntologyObjectProperty"/>
    </owl:ObjectProperty>
    


    <!-- https://w3id.org/isoiec5087/-1/v1/validIn -->

    <owl:ObjectProperty rdf:about="https://w3id.org/isoiec5087/-1/v1/validIn">
        <rdfs:subPropertyOf rdf:resource="https://w3id.org/isoiec5087/-1/v1/AgreementOntologyObjectProperty"/>
    </owl:ObjectProperty>
    


    <!-- 
    ///////////////////////////////////////////////////////////////////////////////////////
    //
    // Data properties
    //
    ///////////////////////////////////////////////////////////////////////////////////////
     -->

    


    <!-- https://w3id.org/isoiec5087/-1/v1/AgreementOntologyDataProperty -->

    <owl:DatatypeProperty rdf:about="https://w3id.org/isoiec5087/-1/v1/AgreementOntologyDataProperty"/>
    


    <!-- 
    ///////////////////////////////////////////////////////////////////////////////////////
    //
    // Classes
    //
    ///////////////////////////////////////////////////////////////////////////////////////
     -->

    


    <!-- https://w3id.org/isoiec5087/-1/v1/Agent -->

    <owl:Class rdf:about="https://w3id.org/isoiec5087/-1/v1/Agent">
        <rdfs:subClassOf rdf:resource="https://w3id.org/isoiec5087/-1/v1/Agent"/>
        <rdfs:subClassOf rdf:resource="https://w3id.org/isoiec5087/-1/v1/AgreementOntologyThing"/>
        <rdfs:subClassOf>
            <owl:Restriction>
                <owl:onProperty rdf:resource="https://w3id.org/isoiec5087/-1/v1/hasClaim"/>
                <owl:allValuesFrom rdf:resource="https://w3id.org/isoiec5087/-1/v1/AtomicAgreement"/>
            </owl:Restriction>
        </rdfs:subClassOf>
        <rdfs:subClassOf>
            <owl:Restriction>
                <owl:onProperty rdf:resource="https://w3id.org/isoiec5087/-1/v1/hasDuty"/>
                <owl:allValuesFrom rdf:resource="https://w3id.org/isoiec5087/-1/v1/AtomicAgreement"/>
            </owl:Restriction>
        </rdfs:subClassOf>
        <rdfs:subClassOf>
            <owl:Restriction>
                <owl:onProperty rdf:resource="https://w3id.org/isoiec5087/-1/v1/hasNoClaim"/>
                <owl:allValuesFrom rdf:resource="https://w3id.org/isoiec5087/-1/v1/AtomicAgreement"/>
            </owl:Restriction>
        </rdfs:subClassOf>
        <rdfs:subClassOf>
            <owl:Restriction>
                <owl:onProperty rdf:resource="https://w3id.org/isoiec5087/-1/v1/hasPrivilege"/>
                <owl:allValuesFrom rdf:resource="https://w3id.org/isoiec5087/-1/v1/AtomicAgreement"/>
            </owl:Restriction>
        </rdfs:subClassOf>
    </owl:Class>
    


    <!-- https://w3id.org/isoiec5087/-1/v1/Agreement -->

    <owl:Class rdf:about="https://w3id.org/isoiec5087/-1/v1/Agreement">
        <rdfs:subClassOf rdf:resource="https://w3id.org/isoiec5087/-1/v1/AgreementOntologyThing"/>
        <rdfs:subClassOf>
            <owl:Restriction>
                <owl:onProperty rdf:resource="https://w3id.org/isoiec5087/-1/v1/establishedOn"/>
                <owl:allValuesFrom rdf:resource="time:Instant"/>
            </owl:Restriction>
        </rdfs:subClassOf>
        <rdfs:subClassOf>
            <owl:Restriction>
                <owl:onProperty rdf:resource="https://w3id.org/isoiec5087/-1/v1/validFor"/>
                <owl:allValuesFrom rdf:resource="time:Interval"/>
            </owl:Restriction>
        </rdfs:subClassOf>
        <rdfs:subClassOf>
            <owl:Restriction>
                <owl:onProperty rdf:resource="https://w3id.org/isoiec5087/-1/v1/validIn"/>
                <owl:allValuesFrom rdf:resource="http://ontology.eil.utoronto.ca/5087/1/SpatialLoc/Location"/>
            </owl:Restriction>
        </rdfs:subClassOf>
        <rdfs:subClassOf>
            <owl:Restriction>
                <owl:onProperty rdf:resource="https://w3id.org/isoiec5087/-1/v1/involvesAgent"/>
                <owl:minQualifiedCardinality rdf:datatype="xsd:nonNegativeInteger">2</owl:minQualifiedCardinality>
                <owl:onClass rdf:resource="https://w3id.org/isoiec5087/-1/v1/Agent"/>
            </owl:Restriction>
        </rdfs:subClassOf>
        <rdfs:comment xml:lang="en">The class Agreement has the following properties:
•	involvesAgent: identifies the agents that are party to the agreement.
•	validIn: identifies the location where the agreement is valid.
•	establishedOn: specifies the instant of time that agreement was created.
•	validFor: specifies the time interval during which the agreement is in force.</rdfs:comment>
    </owl:Class>
    


    <!-- https://w3id.org/isoiec5087/-1/v1/AgreementOntologyThing -->

    <owl:Class rdf:about="https://w3id.org/isoiec5087/-1/v1/AgreementOntologyThing"/>
    


    <!-- https://w3id.org/isoiec5087/-1/v1/AtomicAgreement -->

    <owl:Class rdf:about="https://w3id.org/isoiec5087/-1/v1/AtomicAgreement">
        <rdfs:subClassOf rdf:resource="https://w3id.org/isoiec5087/-1/v1/Agreement"/>
        <rdfs:subClassOf>
            <owl:Restriction>
                <owl:onProperty rdf:resource="https://w3id.org/isoiec5087/-1/v1/commitsToActivity"/>
                <owl:someValuesFrom rdf:resource="https://w3id.org/isoiec5087/-1/v1/Activity"/>
            </owl:Restriction>
        </rdfs:subClassOf>
        <rdfs:subClassOf>
            <owl:Restriction>
                <owl:onProperty>
                    <rdf:Description>
                        <owl:inverseOf rdf:resource="https://w3id.org/isoiec5087/-1/v1/hasClaim"/>
                    </rdf:Description>
                </owl:onProperty>
                <owl:allValuesFrom rdf:resource="https://w3id.org/isoiec5087/-1/v1/Agent"/>
            </owl:Restriction>
        </rdfs:subClassOf>
        <rdfs:subClassOf>
            <owl:Restriction>
                <owl:onProperty>
                    <rdf:Description>
                        <owl:inverseOf rdf:resource="https://w3id.org/isoiec5087/-1/v1/hasDuty"/>
                    </rdf:Description>
                </owl:onProperty>
                <owl:allValuesFrom rdf:resource="https://w3id.org/isoiec5087/-1/v1/Agent"/>
            </owl:Restriction>
        </rdfs:subClassOf>
        <rdfs:subClassOf>
            <owl:Restriction>
                <owl:onProperty>
                    <rdf:Description>
                        <owl:inverseOf rdf:resource="https://w3id.org/isoiec5087/-1/v1/hasNoClaim"/>
                    </rdf:Description>
                </owl:onProperty>
                <owl:allValuesFrom rdf:resource="https://w3id.org/isoiec5087/-1/v1/Agent"/>
            </owl:Restriction>
        </rdfs:subClassOf>
        <rdfs:subClassOf>
            <owl:Restriction>
                <owl:onProperty>
                    <rdf:Description>
                        <owl:inverseOf rdf:resource="https://w3id.org/isoiec5087/-1/v1/hasPrivilege"/>
                    </rdf:Description>
                </owl:onProperty>
                <owl:allValuesFrom rdf:resource="https://w3id.org/isoiec5087/-1/v1/Agent"/>
            </owl:Restriction>
        </rdfs:subClassOf>
        <rdfs:subClassOf>
            <owl:Restriction>
                <owl:onProperty rdf:resource="https://w3id.org/isoiec5087/-1/v1/hasSubAgreement"/>
                <owl:qualifiedCardinality rdf:datatype="xsd:nonNegativeInteger">0</owl:qualifiedCardinality>
                <owl:onClass rdf:resource="https://w3id.org/isoiec5087/-1/v1/Agreement"/>
            </owl:Restriction>
        </rdfs:subClassOf>
        <owl:disjointWith rdf:resource="https://w3id.org/isoiec5087/-1/v1/ComplexAgreement"/>
        <rdfs:comment xml:lang="en">AtomicAgreement is a subclass of Agreement and specifies the “essence” of an agreement.  In particular it identifies how agents participating in the agreement are involved:
•	forActivity: identifies the activity that the atomic agreement is for.
•	inverse hasClaim: links the agreement to any agent that has a claim.
•	inverse hasNoClaim: links the agreement to any agent that does not have a claim.
•	inverse hasDuty: links the agreement to any agent that has a duty to perform the activity.
•	inverse hasPrivilege: links the agreement to any agent that has the privilege to perform the activity.</rdfs:comment>
        <rdfs:label xml:lang="en">Atomic Agreement</rdfs:label>
    </owl:Class>
    


    <!-- https://w3id.org/isoiec5087/-1/v1/ComplexAgreement -->

    <owl:Class rdf:about="https://w3id.org/isoiec5087/-1/v1/ComplexAgreement">
        <rdfs:subClassOf rdf:resource="https://w3id.org/isoiec5087/-1/v1/Agreement"/>
        <rdfs:subClassOf>
            <owl:Restriction>
                <owl:onProperty rdf:resource="https://w3id.org/isoiec5087/-1/v1/hasSubAgreement"/>
                <owl:minQualifiedCardinality rdf:datatype="xsd:nonNegativeInteger">2</owl:minQualifiedCardinality>
                <owl:onClass rdf:resource="https://w3id.org/isoiec5087/-1/v1/Agreement"/>
            </owl:Restriction>
        </rdfs:subClassOf>
        <rdfs:comment xml:lang="en">ComplexAgreement is a subclass of Agreement and has one additional property:
•	hasSubAgreement: identifies two or more agreements that comprise the agreement.</rdfs:comment>
        <rdfs:label xml:lang="en">Complex Agreement</rdfs:label>
    </owl:Class>
    


    <!-- https://w3id.org/isoiec5087/-1/v1/ConjunctiveAgreement -->

    <owl:Class rdf:about="https://w3id.org/isoiec5087/-1/v1/ConjunctiveAgreement">
        <rdfs:subClassOf rdf:resource="https://w3id.org/isoiec5087/-1/v1/ComplexAgreement"/>
        <owl:disjointWith rdf:resource="https://w3id.org/isoiec5087/-1/v1/DisjunctiveAgreement"/>
    </owl:Class>
    


    <!-- https://w3id.org/isoiec5087/-1/v1/DisjunctiveAgreement -->

    <owl:Class rdf:about="https://w3id.org/isoiec5087/-1/v1/DisjunctiveAgreement">
        <rdfs:subClassOf rdf:resource="https://w3id.org/isoiec5087/-1/v1/ComplexAgreement"/>
    </owl:Class>

        <!-- 
    ///////////////////////////////////////////////////////////////////////////////////////
    //
    // Object Properties
    //
    ///////////////////////////////////////////////////////////////////////////////////////
     -->

    <!-- https://w3id.org/citydata/test/ChangeOntologyProperty -->

    <owl:ObjectProperty rdf:about="https://w3id.org/citydata/test/ChangeOntologyProperty">
        <rdfs:comment>Added for organizational purposes to group properties defined in the Change Ontology.</rdfs:comment>
    </owl:ObjectProperty>
    


    <!-- https://w3id.org/citydata/test/existsAt -->

    <owl:ObjectProperty rdf:about="https://w3id.org/citydata/test/existsAt">
        <rdfs:subPropertyOf rdf:resource="https://w3id.org/citydata/test/ChangeOntologyProperty"/>
        <rdf:type rdf:resource="owl:FunctionalProperty"/>
        <rdfs:domain rdf:resource="https://w3id.org/citydata/test/Manifestation"/>
        <rdfs:range rdf:resource="time:TemporalEntity"/>
        <skos:definition>Objects (e.g. perdurants and their manifestations) exist at some time interval or time point.</skos:definition>
    </owl:ObjectProperty>
    


    <!-- https://w3id.org/citydata/test/hasFirstManifestation -->

    <owl:ObjectProperty rdf:about="https://w3id.org/citydata/test/hasFirstManifestation">
        <rdfs:subPropertyOf rdf:resource="https://w3id.org/citydata/test/ChangeOntologyProperty"/>
        <rdf:type rdf:resource="owl:FunctionalProperty"/>
    </owl:ObjectProperty>
    


    <!-- https://w3id.org/citydata/test/hasLatestManifestation -->

    <owl:ObjectProperty rdf:about="https://w3id.org/citydata/test/hasLatestManifestation">
        <rdfs:subPropertyOf rdf:resource="https://w3id.org/citydata/test/ChangeOntologyProperty"/>
        <rdf:type rdf:resource="owl:FunctionalProperty"/>
        <rdfs:domain rdf:resource="https://w3id.org/citydata/test/FirstManifestation"/>
        <rdfs:range rdf:resource="https://w3id.org/citydata/test/Manifestation"/>
    </owl:ObjectProperty>
    


    <!-- https://w3id.org/citydata/test/hasManifestation -->

    <owl:ObjectProperty rdf:about="https://w3id.org/citydata/test/hasManifestation">
        <rdfs:subPropertyOf rdf:resource="https://w3id.org/citydata/test/ChangeOntologyProperty"/>
        <rdfs:range rdf:resource="https://w3id.org/citydata/test/Manifestation"/>
    </owl:ObjectProperty>
    


    <!-- https://w3id.org/citydata/test/hasNextManifestation -->

    <owl:ObjectProperty rdf:about="https://w3id.org/citydata/test/hasNextManifestation">
        <rdfs:subPropertyOf rdf:resource="https://w3id.org/citydata/test/ChangeOntologyProperty"/>
        <owl:inverseOf rdf:resource="https://w3id.org/citydata/test/hasPreviousManifestation"/>
        <rdf:type rdf:resource="owl:FunctionalProperty"/>
        <rdf:type rdf:resource="owl:InverseFunctionalProperty"/>
        <rdfs:domain rdf:resource="https://w3id.org/citydata/test/Manifestation"/>
        <rdfs:range rdf:resource="https://w3id.org/citydata/test/Manifestation"/>
    </owl:ObjectProperty>
    


    <!-- https://w3id.org/citydata/test/hasPreviousManifestation -->

    <owl:ObjectProperty rdf:about="https://w3id.org/citydata/test/hasPreviousManifestation">
        <rdfs:subPropertyOf rdf:resource="https://w3id.org/citydata/test/ChangeOntologyProperty"/>
        <rdf:type rdf:resource="owl:FunctionalProperty"/>
    </owl:ObjectProperty>
    


    <!-- https://w3id.org/citydata/test/precedesManifestation -->

    <owl:ObjectProperty rdf:about="https://w3id.org/citydata/test/precedesManifestation">
        <rdfs:subPropertyOf rdf:resource="https://w3id.org/citydata/test/ChangeOntologyProperty"/>
        <rdf:type rdf:resource="owl:FunctionalProperty"/>
        <rdfs:domain rdf:resource="https://w3id.org/citydata/test/FirstManifestation"/>
        <rdfs:range>
            <owl:Class>
                <owl:intersectionOf rdf:parseType="Collection">
                    <rdf:Description rdf:about="https://w3id.org/citydata/test/Manifestation"/>
                    <owl:Class>
                        <owl:complementOf rdf:resource="https://w3id.org/citydata/test/FirstManifestation"/>
                    </owl:Class>
                </owl:intersectionOf>
            </owl:Class>
        </rdfs:range>
        <rdfs:comment>The relationship between the FirstManifestation and all subsequent Manifestations.</rdfs:comment>
    </owl:ObjectProperty>
    


    <!-- 
    ///////////////////////////////////////////////////////////////////////////////////////
    //
    // Classes
    //
    ///////////////////////////////////////////////////////////////////////////////////////
     -->


    <!-- https://w3id.org/citydata/test/ChangeOntologyThing -->

    <owl:Class rdf:about="https://w3id.org/citydata/test/ChangeOntologyThing">
        <rdfs:comment>Added for organizational purposes to group the classes defined in the Change Ontology.</rdfs:comment>
    </owl:Class>
    


    <!-- https://w3id.org/citydata/test/FirstManifestation -->

    <owl:Class rdf:about="https://w3id.org/citydata/test/FirstManifestation">
        <rdfs:subClassOf rdf:resource="https://w3id.org/citydata/test/Manifestation"/>
        <rdfs:subClassOf>
            <owl:Restriction>
                <owl:onProperty rdf:resource="https://w3id.org/citydata/test/precedesManifestation"/>
                <owl:allValuesFrom>
                    <owl:Class>
                        <owl:intersectionOf rdf:parseType="Collection">
                            <rdf:Description rdf:about="https://w3id.org/citydata/test/Manifestation"/>
                            <owl:Class>
                                <owl:complementOf rdf:resource="https://w3id.org/citydata/test/FirstManifestation"/>
                            </owl:Class>
                        </owl:intersectionOf>
                    </owl:Class>
                </owl:allValuesFrom>
            </owl:Restriction>
        </rdfs:subClassOf>
        <rdfs:subClassOf>
            <owl:Restriction>
                <owl:onProperty rdf:resource="https://w3id.org/citydata/test/hasLatestManifestation"/>
                <owl:qualifiedCardinality rdf:datatype="xsd:nonNegativeInteger">1</owl:qualifiedCardinality>
                <owl:onClass rdf:resource="https://w3id.org/citydata/test/Manifestation"/>
            </owl:Restriction>
        </rdfs:subClassOf>
        <rdfs:comment>A FirstManifestation represents the first instance in a series of Manifestations corresponding to a particular object.

•	precedesManifestation: identifies all subsequent Manifestations that follow a particular First Manifestation.</rdfs:comment>
    </owl:Class>
    


    <!-- https://w3id.org/citydata/test/Manifestation -->

    <owl:Class rdf:about="https://w3id.org/citydata/test/Manifestation">
        <rdfs:subClassOf rdf:resource="https://w3id.org/citydata/test/ChangeOntologyThing"/>
        <rdfs:subClassOf>
            <owl:Restriction>
                <owl:onProperty rdf:resource="https://w3id.org/citydata/test/existsAt"/>
                <owl:qualifiedCardinality rdf:datatype="xsd:nonNegativeInteger">1</owl:qualifiedCardinality>
                <owl:onClass rdf:resource="time:TemporalEntity"/>
            </owl:Restriction>
        </rdfs:subClassOf>
        <rdfs:subClassOf>
            <owl:Restriction>
                <owl:onProperty rdf:resource="https://w3id.org/citydata/test/hasFirstManifestation"/>
                <owl:qualifiedCardinality rdf:datatype="xsd:nonNegativeInteger">1</owl:qualifiedCardinality>
                <owl:onClass rdf:resource="https://w3id.org/citydata/test/Manifestation"/>
            </owl:Restriction>
        </rdfs:subClassOf>
        <rdfs:subClassOf>
            <owl:Restriction>
                <owl:onProperty rdf:resource="https://w3id.org/citydata/test/hasNextManifestation"/>
                <owl:maxQualifiedCardinality rdf:datatype="xsd:nonNegativeInteger">1</owl:maxQualifiedCardinality>
                <owl:onClass rdf:resource="https://w3id.org/citydata/test/Manifestation"/>
            </owl:Restriction>
        </rdfs:subClassOf>
        <rdfs:subClassOf>
            <owl:Restriction>
                <owl:onProperty rdf:resource="https://w3id.org/citydata/test/hasPreviousManifestation"/>
                <owl:maxQualifiedCardinality rdf:datatype="xsd:nonNegativeInteger">1</owl:maxQualifiedCardinality>
                <owl:onClass rdf:resource="https://w3id.org/citydata/test/Manifestation"/>
            </owl:Restriction>
        </rdfs:subClassOf>
        <rdfs:comment xml:lang="en">Manifestations may be interpreted as “snapshots” of an object at some point in time. This enables the representation of changing attributes of an object, without losing information about its past values/relationships. The properties of the class must then be identified as properties that are (and aren't) subject to change, in order to distinguish between the static and dynamic aspects of a particular entity.

•	existsAt: identifies the TemporalEntity that reflects the Instant of Interval in time during which the snapshot of the object holds (is valid). 
•	hasNextManifestation: identifies the immediate successive Manifestation (i.e. the subsequent snapshot of the object).
•	hasPreviousManifestation: identifies the immediate previous Manifestation (i.e., the prior snapshot of the object).
•	precedesManifestation: identifies all subsequent Manifestations that follow a particular First Manifestation. In other words, the First Manifestation is related to each and every subsequent manifestation via the precedesManifestation.
•	hasFirstManifestation: identifies the First Manifestation that is related to a particular Manifestation (i.e., for some snapshot of an object, it identifies the first such snapshot of the object).
•	hastLastManifestation: identifies the most recent Manifestation that is related to a particular Manifestation (i.e., for some snapshot of an object, it identifies the most recent snapshot of the object).</rdfs:comment>
    </owl:Class>

        

 
    <!-- 
    ///////////////////////////////////////////////////////////////////////////////////////
    //
    // Object Properties
    //
    ///////////////////////////////////////////////////////////////////////////////////////
     -->

    


    <!-- https://w3id.org/isoiec5087/-1/v1/cityUnitsProperty -->

    <owl:ObjectProperty rdf:about="https://w3id.org/isoiec5087/-1/v1/cityUnitsProperty"/>
    


    <!-- https://w3id.org/isoiec5087/-1/v1/aggregateOf -->

    <owl:ObjectProperty rdf:about="https://w3id.org/isoiec5087/-1/v1/aggregateOf">
        <rdfs:subPropertyOf rdf:resource="https://w3id.org/isoiec5087/-1/v1/cityUnitsProperty"/>
        <rdfs:domain rdf:resource="https://w3id.org/isoiec21972/v1/Quantity"/>
    </owl:ObjectProperty>
    


    <!-- https://w3id.org/isoiec5087/-1/v1/aggregateOver -->

    <owl:ObjectProperty rdf:about="https://w3id.org/isoiec5087/-1/v1/aggregateOver">
        <rdfs:subPropertyOf rdf:resource="https://w3id.org/isoiec5087/-1/v1/cityUnitsProperty"/>
        <rdfs:domain rdf:resource="https://w3id.org/isoiec21972/v1/Quantity"/>
    </owl:ObjectProperty>
    


    <!-- https://w3id.org/isoiec5087/-1/v1/derived_unit -->

    <owl:ObjectProperty rdf:about="https://w3id.org/isoiec5087/-1/v1/derived_unit">
        <rdfs:subPropertyOf rdf:resource="https://w3id.org/isoiec5087/-1/v1/cityUnitsProperty"/>
    </owl:ObjectProperty>
    


    <!-- https://w3id.org/isoiec5087/-1/v1/hasAggregateFunction -->

    <owl:ObjectProperty rdf:about="https://w3id.org/isoiec5087/-1/v1/hasAggregateFunction">
        <rdfs:subPropertyOf rdf:resource="https://w3id.org/isoiec5087/-1/v1/cityUnitsProperty"/>
        <rdfs:domain rdf:resource="https://w3id.org/isoiec21972/v1/Quantity"/>
        <rdfs:range rdf:resource="https://w3id.org/isoiec5087/-1/v1/Function"/>
    </owl:ObjectProperty>
    


    <!-- https://w3id.org/isoiec21972/v1/base_unit -->

    <owl:ObjectProperty rdf:about="https://w3id.org/isoiec21972/v1/base_unit">
        <rdfs:subPropertyOf rdf:resource="https://w3id.org/isoiec5087/-1/v1/cityUnitsProperty"/>
        <rdfs:domain rdf:resource="https://w3id.org/isoiec21972/v1/System_of_units"/>
        <rdfs:range rdf:resource="https://w3id.org/isoiec21972/v1/Unit_of_measure"/>
    </owl:ObjectProperty>
    


    <!-- https://w3id.org/isoiec21972/v1/cardinality_of -->

    <owl:ObjectProperty rdf:about="https://w3id.org/isoiec21972/v1/cardinality_of">
        <rdfs:subPropertyOf rdf:resource="https://w3id.org/isoiec5087/-1/v1/cityUnitsProperty"/>
    </owl:ObjectProperty>
    


    <!-- https://w3id.org/isoiec21972/v1/defined_by -->

    <owl:ObjectProperty rdf:about="https://w3id.org/isoiec21972/v1/defined_by">
        <rdfs:subPropertyOf rdf:resource="https://w3id.org/isoiec5087/-1/v1/cityUnitsProperty"/>
    </owl:ObjectProperty>
    


    <!-- https://w3id.org/isoiec21972/v1/denominator -->

    <owl:ObjectProperty rdf:about="https://w3id.org/isoiec21972/v1/denominator">
        <rdfs:subPropertyOf rdf:resource="https://w3id.org/isoiec5087/-1/v1/cityUnitsProperty"/>
        <rdfs:domain rdf:resource="https://w3id.org/isoiec21972/v1/Unit_of_measureDivision"/>
        <rdfs:range rdf:resource="https://w3id.org/isoiec21972/v1/Unit_of_measure"/>
        <rdfs:label>has denominator</rdfs:label>
    </owl:ObjectProperty>
    


    <!-- https://w3id.org/isoiec21972/v1/for_time_interval -->

    <owl:ObjectProperty rdf:about="https://w3id.org/isoiec21972/v1/for_time_interval">
        <rdfs:subPropertyOf rdf:resource="https://w3id.org/isoiec5087/-1/v1/cityUnitsProperty"/>
    </owl:ObjectProperty>
    


    <!-- https://w3id.org/isoiec21972/v1/numerator -->

    <owl:ObjectProperty rdf:about="https://w3id.org/isoiec21972/v1/numerator">
        <rdfs:subPropertyOf rdf:resource="https://w3id.org/isoiec5087/-1/v1/cityUnitsProperty"/>
        <rdfs:domain rdf:resource="https://w3id.org/isoiec21972/v1/Unit_of_measureDivision"/>
        <rdfs:range rdf:resource="https://w3id.org/isoiec21972/v1/Unit_of_measure"/>
        <rdfs:label>has numerator</rdfs:label>
    </owl:ObjectProperty>
    


    <!-- https://w3id.org/isoiec21972/v1/unit_of_measure -->

    <owl:ObjectProperty rdf:about="https://w3id.org/isoiec21972/v1/unit_of_measure">
        <rdfs:subPropertyOf rdf:resource="https://w3id.org/isoiec5087/-1/v1/cityUnitsProperty"/>
        <rdfs:label>has unit</rdfs:label>
    </owl:ObjectProperty>
    


    <!-- https://w3id.org/isoiec21972/v1/value -->

    <owl:ObjectProperty rdf:about="https://w3id.org/isoiec21972/v1/value">
        <rdfs:subPropertyOf rdf:resource="https://w3id.org/isoiec5087/-1/v1/cityUnitsProperty"/>
        <rdfs:domain rdf:resource="https://w3id.org/isoiec21972/v1/Quantity"/>
        <rdfs:label>has value</rdfs:label>
    </owl:ObjectProperty>
    


    <!-- 
    ///////////////////////////////////////////////////////////////////////////////////////
    //
    // Data properties
    //
    ///////////////////////////////////////////////////////////////////////////////////////
     -->

    


    <!-- https://w3id.org/isoiec5087/-1/v1/cityUnitsDataProperty -->

    <owl:DatatypeProperty rdf:about="https://w3id.org/isoiec5087/-1/v1/cityUnitsDataProperty">
        <skos:definition>Data property introduced for organization purposes, to identify data properties defined in the Units of Measure Ontology.</skos:definition>
    </owl:DatatypeProperty>
    


    <!-- https://w3id.org/isoiec5087/-1/v1/hasRelativeYear -->

    <owl:DatatypeProperty rdf:about="https://w3id.org/isoiec5087/-1/v1/hasRelativeYear">
        <rdfs:subPropertyOf rdf:resource="https://w3id.org/isoiec5087/-1/v1/cityUnitsDataProperty"/>
    </owl:DatatypeProperty>
    


    <!-- https://w3id.org/isoiec21972/v1/exponent -->

    <owl:DatatypeProperty rdf:about="https://w3id.org/isoiec21972/v1/exponent">
        <rdfs:subPropertyOf rdf:resource="https://w3id.org/isoiec5087/-1/v1/cityUnitsDataProperty"/>
    </owl:DatatypeProperty>
    


    <!-- https://w3id.org/isoiec21972/v1/factor -->

    <owl:DatatypeProperty rdf:about="https://w3id.org/isoiec21972/v1/factor">
        <rdfs:subPropertyOf rdf:resource="https://w3id.org/isoiec5087/-1/v1/cityUnitsDataProperty"/>
    </owl:DatatypeProperty>
    


    <!-- https://w3id.org/isoiec21972/v1/numerical_value -->

    <owl:DatatypeProperty rdf:about="https://w3id.org/isoiec21972/v1/numerical_value">
        <rdfs:subPropertyOf rdf:resource="https://w3id.org/isoiec5087/-1/v1/cityUnitsDataProperty"/>
        <rdf:type rdf:resource="owl:FunctionalProperty"/>
        <rdfs:label>has numerical value</rdfs:label>
    </owl:DatatypeProperty>
    


    <!-- 
    ///////////////////////////////////////////////////////////////////////////////////////
    //
    // Classes
    //
    ///////////////////////////////////////////////////////////////////////////////////////
     -->

    


    <!-- https://w3id.org/isoiec5087/-1/v1/Acceleration -->

    <owl:Class rdf:about="https://w3id.org/isoiec5087/-1/v1/Acceleration">
        <rdfs:subClassOf rdf:resource="https://w3id.org/isoiec21972/v1/Quantity"/>
        <rdfs:subClassOf>
            <owl:Restriction>
                <owl:onProperty rdf:resource="https://w3id.org/isoiec21972/v1/value"/>
                <owl:allValuesFrom>
                    <owl:Restriction>
                        <owl:onProperty rdf:resource="https://w3id.org/isoiec21972/v1/unit_of_measure"/>
                        <owl:allValuesFrom rdf:resource="https://w3id.org/isoiec5087/-1/v1/AccelerationUnit"/>
                    </owl:Restriction>
                </owl:allValuesFrom>
            </owl:Restriction>
        </rdfs:subClassOf>
        <rdfs:label>acceleration</rdfs:label>
    </owl:Class>
    


    <!-- https://w3id.org/isoiec5087/-1/v1/AccelerationUnit -->

    <owl:Class rdf:about="https://w3id.org/isoiec5087/-1/v1/AccelerationUnit">
        <rdfs:subClassOf rdf:resource="https://w3id.org/isoiec21972/v1/Unit_of_measure"/>
        <rdfs:label>acceleration unit</rdfs:label>
    </owl:Class>
    


    <!-- https://w3id.org/isoiec5087/-1/v1/AmountOfMoney -->

    <owl:Class rdf:about="https://w3id.org/isoiec5087/-1/v1/AmountOfMoney">
        <rdfs:subClassOf rdf:resource="https://w3id.org/isoiec21972/v1/Quantity"/>
        <rdfs:subClassOf>
            <owl:Restriction>
                <owl:onProperty rdf:resource="https://w3id.org/isoiec21972/v1/value"/>
                <owl:allValuesFrom>
                    <owl:Restriction>
                        <owl:onProperty rdf:resource="https://w3id.org/isoiec21972/v1/unit_of_measure"/>
                        <owl:allValuesFrom rdf:resource="https://w3id.org/isoiec21972/v1/Monetary_unit"/>
                    </owl:Restriction>
                </owl:allValuesFrom>
            </owl:Restriction>
        </rdfs:subClassOf>
        <rdfs:label>amount of money</rdfs:label>
    </owl:Class>
    


    <!-- https://w3id.org/isoiec5087/-1/v1/Area -->

    <owl:Class rdf:about="https://w3id.org/isoiec5087/-1/v1/Area">
        <rdfs:subClassOf rdf:resource="https://w3id.org/isoiec21972/v1/Quantity"/>
        <rdfs:subClassOf>
            <owl:Restriction>
                <owl:onProperty rdf:resource="https://w3id.org/isoiec21972/v1/value"/>
                <owl:allValuesFrom>
                    <owl:Restriction>
                        <owl:onProperty rdf:resource="https://w3id.org/isoiec21972/v1/unit_of_measure"/>
                        <owl:allValuesFrom rdf:resource="https://w3id.org/isoiec5087/-1/v1/AreaUnit"/>
                    </owl:Restriction>
                </owl:allValuesFrom>
            </owl:Restriction>
        </rdfs:subClassOf>
        <rdfs:comment>Area expresses the two-dimensional size of a defined part of a surface, typically a region bounded by a closed curve. It is a derived quantity in the International System of Units. Area is length squared.</rdfs:comment>
        <rdfs:label>area</rdfs:label>
    </owl:Class>
    


    <!-- https://w3id.org/isoiec5087/-1/v1/AreaUnit -->

    <owl:Class rdf:about="https://w3id.org/isoiec5087/-1/v1/AreaUnit">
        <rdfs:subClassOf rdf:resource="https://w3id.org/isoiec21972/v1/Unit_of_measure"/>
        <rdfs:label>area unit</rdfs:label>
    </owl:Class>
    


    <!-- https://w3id.org/isoiec5087/-1/v1/Capacity -->

    <owl:Class rdf:about="https://w3id.org/isoiec5087/-1/v1/Capacity">
        <rdfs:subClassOf rdf:resource="https://w3id.org/isoiec5087/-1/v1/CityUnitsThing"/>
        <rdfs:subClassOf>
            <owl:Restriction>
                <owl:onProperty rdf:resource="https://w3id.org/isoiec21972/v1/defined_by"/>
                <owl:minCardinality rdf:datatype="xsd:nonNegativeInteger">1</owl:minCardinality>
            </owl:Restriction>
        </rdfs:subClassOf>
    </owl:Class>
    


    <!-- https://w3id.org/isoiec5087/-1/v1/CapacityRate -->

    <owl:Class rdf:about="https://w3id.org/isoiec5087/-1/v1/CapacityRate">
        <rdfs:subClassOf rdf:resource="https://w3id.org/isoiec21972/v1/Quantity"/>
        <rdfs:subClassOf>
            <owl:Restriction>
                <owl:onProperty rdf:resource="https://w3id.org/isoiec21972/v1/value"/>
                <owl:allValuesFrom>
                    <owl:Restriction>
                        <owl:onProperty rdf:resource="https://w3id.org/isoiec21972/v1/unit_of_measure"/>
                        <owl:allValuesFrom rdf:resource="https://w3id.org/isoiec5087/-1/v1/CardinalityUnitPerTime"/>
                    </owl:Restriction>
                </owl:allValuesFrom>
            </owl:Restriction>
        </rdfs:subClassOf>
        <rdfs:subClassOf>
            <owl:Restriction>
                <owl:onProperty rdf:resource="https://w3id.org/isoiec21972/v1/cardinality_of"/>
                <owl:qualifiedCardinality rdf:datatype="xsd:nonNegativeInteger">1</owl:qualifiedCardinality>
                <owl:onClass rdf:resource="https://w3id.org/isoiec5087/-1/v1/Capacity"/>
            </owl:Restriction>
        </rdfs:subClassOf>
    </owl:Class>
    


    <!-- https://w3id.org/isoiec5087/-1/v1/CapacitySize -->

    <owl:Class rdf:about="https://w3id.org/isoiec5087/-1/v1/CapacitySize">
        <rdfs:subClassOf rdf:resource="https://w3id.org/isoiec21972/v1/Quantity"/>
        <rdfs:subClassOf>
            <owl:Restriction>
                <owl:onProperty rdf:resource="https://w3id.org/isoiec21972/v1/value"/>
                <owl:allValuesFrom>
                    <owl:Restriction>
                        <owl:onProperty rdf:resource="https://w3id.org/isoiec21972/v1/unit_of_measure"/>
                        <owl:allValuesFrom rdf:resource="https://w3id.org/isoiec21972/v1/Cardinality_unit"/>
                    </owl:Restriction>
                </owl:allValuesFrom>
            </owl:Restriction>
        </rdfs:subClassOf>
        <rdfs:subClassOf>
            <owl:Restriction>
                <owl:onProperty rdf:resource="https://w3id.org/isoiec21972/v1/cardinality_of"/>
                <owl:qualifiedCardinality rdf:datatype="xsd:nonNegativeInteger">1</owl:qualifiedCardinality>
                <owl:onClass rdf:resource="https://w3id.org/isoiec5087/-1/v1/Capacity"/>
            </owl:Restriction>
        </rdfs:subClassOf>
    </owl:Class>
    


    <!-- https://w3id.org/isoiec5087/-1/v1/CardinalityMeasure -->

    <owl:Class rdf:about="https://w3id.org/isoiec5087/-1/v1/CardinalityMeasure">
        <rdfs:subClassOf rdf:resource="https://w3id.org/isoiec21972/v1/Measure"/>
        <rdfs:subClassOf>
            <owl:Restriction>
                <owl:onProperty rdf:resource="https://w3id.org/isoiec21972/v1/unit_of_measure"/>
                <owl:allValuesFrom rdf:resource="https://w3id.org/isoiec21972/v1/Cardinality_unit"/>
            </owl:Restriction>
        </rdfs:subClassOf>
    </owl:Class>
    


    <!-- https://w3id.org/isoiec5087/-1/v1/CardinalityUnitPerTime -->

    <owl:Class rdf:about="https://w3id.org/isoiec5087/-1/v1/CardinalityUnitPerTime">
        <rdfs:subClassOf rdf:resource="https://w3id.org/isoiec21972/v1/Unit_of_measureDivision"/>
        <rdfs:subClassOf>
            <owl:Restriction>
                <owl:onProperty rdf:resource="https://w3id.org/isoiec21972/v1/denominator"/>
                <owl:allValuesFrom rdf:resource="https://w3id.org/isoiec5087/-1/v1/TimeUnit"/>
            </owl:Restriction>
        </rdfs:subClassOf>
        <rdfs:subClassOf>
            <owl:Restriction>
                <owl:onProperty rdf:resource="https://w3id.org/isoiec21972/v1/numerator"/>
                <owl:allValuesFrom rdf:resource="https://w3id.org/isoiec21972/v1/Cardinality_unit"/>
            </owl:Restriction>
        </rdfs:subClassOf>
    </owl:Class>
    


    <!-- https://w3id.org/isoiec5087/-1/v1/CityUnitsThing -->

    <owl:Class rdf:about="https://w3id.org/isoiec5087/-1/v1/CityUnitsThing"/>
    


    <!-- https://w3id.org/isoiec5087/-1/v1/Duration -->

    <owl:Class rdf:about="https://w3id.org/isoiec5087/-1/v1/Duration">
        <rdfs:subClassOf rdf:resource="https://w3id.org/isoiec21972/v1/Quantity"/>
        <rdfs:subClassOf rdf:resource="time:TemporalDuration"/>
        <rdfs:subClassOf>
            <owl:Restriction>
                <owl:onProperty rdf:resource="https://w3id.org/isoiec21972/v1/value"/>
                <owl:allValuesFrom>
                    <owl:Restriction>
                        <owl:onProperty rdf:resource="https://w3id.org/isoiec21972/v1/unit_of_measure"/>
                        <owl:allValuesFrom rdf:resource="https://w3id.org/isoiec5087/-1/v1/TimeUnit"/>
                    </owl:Restriction>
                </owl:allValuesFrom>
            </owl:Restriction>
        </rdfs:subClassOf>
        <rdfs:label>duration</rdfs:label>
    </owl:Class>
    


    <!-- https://w3id.org/isoiec5087/-1/v1/Function -->

    <owl:Class rdf:about="https://w3id.org/isoiec5087/-1/v1/Function">
        <rdfs:subClassOf rdf:resource="https://w3id.org/isoiec5087/-1/v1/CityUnitsThing"/>
        <rdfs:label>function</rdfs:label>
    </owl:Class>
    


    <!-- https://w3id.org/isoiec5087/-1/v1/Geo_Position_unit -->

    <owl:Class rdf:about="https://w3id.org/isoiec5087/-1/v1/Geo_Position_unit">
        <rdfs:subClassOf rdf:resource="https://w3id.org/isoiec21972/v1/Unit_of_measure"/>
        <rdfs:comment>Reference systems to indicate geographic position.</rdfs:comment>
    </owl:Class>
    


    <!-- https://w3id.org/isoiec5087/-1/v1/Length -->

    <owl:Class rdf:about="https://w3id.org/isoiec5087/-1/v1/Length">
        <rdfs:subClassOf rdf:resource="https://w3id.org/isoiec21972/v1/Quantity"/>
        <rdfs:subClassOf>
            <owl:Restriction>
                <owl:onProperty rdf:resource="https://w3id.org/isoiec21972/v1/value"/>
                <owl:allValuesFrom>
                    <owl:Class>
                        <owl:intersectionOf rdf:parseType="Collection">
                            <rdf:Description rdf:about="https://w3id.org/isoiec21972/v1/Measure"/>
                            <owl:Restriction>
                                <owl:onProperty rdf:resource="https://w3id.org/isoiec21972/v1/unit_of_measure"/>
                                <owl:allValuesFrom rdf:resource="https://w3id.org/isoiec5087/-1/v1/LengthUnit"/>
                            </owl:Restriction>
                        </owl:intersectionOf>
                    </owl:Class>
                </owl:allValuesFrom>
            </owl:Restriction>
        </rdfs:subClassOf>
        <rdfs:comment>Length is the amount of space between two geographical points along a curve. It is a base quantity in the International System of Units and other systems of units. Length is speed times time. The metre, a base unit of length in the International System of Units, is defined in terms of speed of light during a certain time interval.</rdfs:comment>
        <rdfs:label>length</rdfs:label>
    </owl:Class>
    


    <!-- https://w3id.org/isoiec5087/-1/v1/LengthUnit -->

    <owl:Class rdf:about="https://w3id.org/isoiec5087/-1/v1/LengthUnit">
        <rdfs:subClassOf rdf:resource="https://w3id.org/isoiec21972/v1/Unit_of_measure"/>
        <rdfs:label>length unit</rdfs:label>
    </owl:Class>
    


    <!-- https://w3id.org/isoiec5087/-1/v1/Mass -->

    <owl:Class rdf:about="https://w3id.org/isoiec5087/-1/v1/Mass">
        <rdfs:subClassOf rdf:resource="https://w3id.org/isoiec21972/v1/Quantity"/>
        <rdfs:subClassOf>
            <owl:Restriction>
                <owl:onProperty rdf:resource="https://w3id.org/isoiec21972/v1/value"/>
                <owl:allValuesFrom>
                    <owl:Restriction>
                        <owl:onProperty rdf:resource="https://w3id.org/isoiec21972/v1/unit_of_measure"/>
                        <owl:allValuesFrom rdf:resource="https://w3id.org/isoiec5087/-1/v1/MassUnit"/>
                    </owl:Restriction>
                </owl:allValuesFrom>
            </owl:Restriction>
        </rdfs:subClassOf>
        <rdfs:comment>Mass is the amount of matter of a phenomenon. It is a base quantity in the International System of Units. Mass is force divided by acceleration.</rdfs:comment>
        <rdfs:label>mass</rdfs:label>
    </owl:Class>
    


    <!-- https://w3id.org/isoiec5087/-1/v1/MassUnit -->

    <owl:Class rdf:about="https://w3id.org/isoiec5087/-1/v1/MassUnit">
        <rdfs:subClassOf rdf:resource="https://w3id.org/isoiec21972/v1/Unit_of_measure"/>
        <rdfs:label>mass unit</rdfs:label>
    </owl:Class>
    


    <!-- https://w3id.org/isoiec5087/-1/v1/MonetaryValue -->

    <owl:Class rdf:about="https://w3id.org/isoiec5087/-1/v1/MonetaryValue">
        <rdfs:subClassOf rdf:resource="https://w3id.org/isoiec21972/v1/Measure"/>
        <rdfs:subClassOf>
            <owl:Restriction>
                <owl:onProperty rdf:resource="https://w3id.org/isoiec21972/v1/unit_of_measure"/>
                <owl:allValuesFrom rdf:resource="https://w3id.org/isoiec21972/v1/Monetary_unit"/>
            </owl:Restriction>
        </rdfs:subClassOf>
        <rdfs:subClassOf>
            <owl:Restriction>
                <owl:onProperty rdf:resource="https://w3id.org/isoiec5087/-1/v1/hasRelativeYear"/>
                <owl:qualifiedCardinality rdf:datatype="xsd:nonNegativeInteger">1</owl:qualifiedCardinality>
                <owl:onDataRange rdf:resource="xsd:gYear"/>
            </owl:Restriction>
        </rdfs:subClassOf>
        <rdfs:comment>A Monetary Value has a numerical value that is relative to a particular date (year).
A Monetary Value is measured with some currency.</rdfs:comment>
    </owl:Class>
    


    <!-- https://w3id.org/isoiec5087/-1/v1/Ratio -->

    <owl:Class rdf:about="https://w3id.org/isoiec5087/-1/v1/Ratio">
        <rdfs:subClassOf rdf:resource="https://w3id.org/isoiec21972/v1/Quantity"/>
        <rdfs:label>ratio</rdfs:label>
    </owl:Class>
    


    <!-- https://w3id.org/isoiec5087/-1/v1/Speed -->

    <owl:Class rdf:about="https://w3id.org/isoiec5087/-1/v1/Speed">
        <rdfs:subClassOf rdf:resource="https://w3id.org/isoiec21972/v1/Quantity"/>
        <rdfs:subClassOf>
            <owl:Restriction>
                <owl:onProperty rdf:resource="https://w3id.org/isoiec21972/v1/value"/>
                <owl:allValuesFrom>
                    <owl:Restriction>
                        <owl:onProperty rdf:resource="https://w3id.org/isoiec21972/v1/unit_of_measure"/>
                        <owl:allValuesFrom rdf:resource="https://w3id.org/isoiec5087/-1/v1/SpeedUnit"/>
                    </owl:Restriction>
                </owl:allValuesFrom>
            </owl:Restriction>
        </rdfs:subClassOf>
        <rdfs:comment>Speed is the time rate of motion measured by the distance moved over in unit time.</rdfs:comment>
        <rdfs:label>speed</rdfs:label>
    </owl:Class>
    


    <!-- https://w3id.org/isoiec5087/-1/v1/SpeedUnit -->

    <owl:Class rdf:about="https://w3id.org/isoiec5087/-1/v1/SpeedUnit">
        <rdfs:subClassOf rdf:resource="https://w3id.org/isoiec21972/v1/Unit_of_measure"/>
        <rdfs:label>speed unit</rdfs:label>
    </owl:Class>
    


    <!-- https://w3id.org/isoiec5087/-1/v1/TimeUnit -->

    <owl:Class rdf:about="https://w3id.org/isoiec5087/-1/v1/TimeUnit">
        <rdfs:subClassOf rdf:resource="https://w3id.org/isoiec21972/v1/Unit_of_measure"/>
        <rdfs:label>time unit</rdfs:label>
    </owl:Class>
    


    <!-- https://w3id.org/isoiec5087/-1/v1/ValueOfMoney -->

    <owl:Class rdf:about="https://w3id.org/isoiec5087/-1/v1/ValueOfMoney">
        <rdfs:subClassOf rdf:resource="https://w3id.org/isoiec5087/-1/v1/AmountOfMoney"/>
        <rdfs:subClassOf>
            <owl:Restriction>
                <owl:onProperty rdf:resource="https://w3id.org/isoiec21972/v1/value"/>
                <owl:allValuesFrom rdf:resource="https://w3id.org/isoiec5087/-1/v1/MonetaryValue"/>
            </owl:Restriction>
        </rdfs:subClassOf>
        <rdfs:comment>An amount of money that is defined relative to a particular year.</rdfs:comment>
    </owl:Class>
    


    <!-- https://w3id.org/isoiec5087/-1/v1/Volume -->

    <owl:Class rdf:about="https://w3id.org/isoiec5087/-1/v1/Volume">
        <rdfs:subClassOf rdf:resource="https://w3id.org/isoiec21972/v1/Quantity"/>
        <rdfs:subClassOf>
            <owl:Restriction>
                <owl:onProperty rdf:resource="https://w3id.org/isoiec21972/v1/value"/>
                <owl:allValuesFrom>
                    <owl:Restriction>
                        <owl:onProperty rdf:resource="https://w3id.org/isoiec21972/v1/unit_of_measure"/>
                        <owl:allValuesFrom rdf:resource="https://w3id.org/isoiec5087/-1/v1/VolumeUnit"/>
                    </owl:Restriction>
                </owl:allValuesFrom>
            </owl:Restriction>
        </rdfs:subClassOf>
        <rdfs:comment>Volume is a measure of how much three-dimensional space any phenomenon occupies. It is a derived quantity in the International System of Units. Volume is length to the power 3.</rdfs:comment>
        <rdfs:label>volume</rdfs:label>
    </owl:Class>
    


    <!-- https://w3id.org/isoiec5087/-1/v1/VolumeUnit -->

    <owl:Class rdf:about="https://w3id.org/isoiec5087/-1/v1/VolumeUnit">
        <rdfs:subClassOf rdf:resource="https://w3id.org/isoiec21972/v1/Unit_of_measure"/>
        <rdfs:label>volume unit</rdfs:label>
    </owl:Class>
    


    <!-- https://w3id.org/isoiec21972/v1/Cardinality_unit -->

    <owl:Class rdf:about="https://w3id.org/isoiec21972/v1/Cardinality_unit">
        <rdfs:subClassOf rdf:resource="https://w3id.org/isoiec21972/v1/Unit_of_measure"/>
        <rdfs:comment>Just as the meter is the unit of measure for length, a gci:Cardinality_unit is the unit of measure for the size of a set. The gci:Cardinality_unit is a ratio scale: gci:Cardinality_scale, which is a subclass of om:Ratio_scale and is has a zero element (namely zero).</rdfs:comment>
        <rdfs:comment>Reused from GCI Foundation Ontology</rdfs:comment>
        <rdfs:label>Cardinality Unit</rdfs:label>
    </owl:Class>
    


    <!-- https://w3id.org/isoiec21972/v1/Distinct_count -->

    <rdf:Description rdf:about="https://w3id.org/isoiec21972/v1/Distinct_count">
        <owl:equivalentClass rdf:resource="https://w3id.org/isoiec21972/v1/Population_size"/>
    </rdf:Description>
    


    <!-- https://w3id.org/isoiec21972/v1/Measure -->

    <owl:Class rdf:about="https://w3id.org/isoiec21972/v1/Measure">
        <rdfs:subClassOf rdf:resource="https://w3id.org/isoiec5087/-1/v1/CityUnitsThing"/>
        <rdfs:subClassOf>
            <owl:Restriction>
                <owl:onProperty rdf:resource="https://w3id.org/isoiec21972/v1/unit_of_measure"/>
                <owl:allValuesFrom rdf:resource="https://w3id.org/isoiec21972/v1/Unit_of_measure"/>
            </owl:Restriction>
        </rdfs:subClassOf>
        <rdfs:label>measure</rdfs:label>
    </owl:Class>
    


    <!-- https://w3id.org/isoiec21972/v1/Measurement_scale -->

    <owl:Class rdf:about="https://w3id.org/isoiec21972/v1/Measurement_scale">
        <rdfs:subClassOf rdf:resource="https://w3id.org/isoiec5087/-1/v1/CityUnitsThing"/>
        <rdfs:label>scale</rdfs:label>
    </owl:Class>
    


    <!-- https://w3id.org/isoiec21972/v1/Monetary_unit -->

    <owl:Class rdf:about="https://w3id.org/isoiec21972/v1/Monetary_unit">
        <rdfs:subClassOf rdf:resource="https://w3id.org/isoiec21972/v1/Unit_of_measure"/>
        <rdfs:label>amount of money unit</rdfs:label>
    </owl:Class>
    


    <!-- https://w3id.org/isoiec21972/v1/Population -->

    <owl:Class rdf:about="https://w3id.org/isoiec21972/v1/Population">
        <rdfs:subClassOf rdf:resource="https://w3id.org/isoiec5087/-1/v1/CityUnitsThing"/>
        <rdfs:subClassOf>
            <owl:Restriction>
                <owl:onProperty rdf:resource="https://w3id.org/isoiec21972/v1/defined_by"/>
                <owl:minCardinality rdf:datatype="xsd:nonNegativeInteger">1</owl:minCardinality>
            </owl:Restriction>
        </rdfs:subClassOf>
        <rdfs:subClassOf>
            <owl:Restriction>
                <owl:onProperty rdf:resource="https://w3id.org/isoiec21972/v1/for_time_interval"/>
                <owl:qualifiedCardinality rdf:datatype="xsd:nonNegativeInteger">1</owl:qualifiedCardinality>
                <owl:onClass rdf:resource="time:DateTimeDescription"/>
            </owl:Restriction>
        </rdfs:subClassOf>
        <rdfs:comment>The govstat Population is specialized for indicator use to include what defines a member of the population, the location of the population, and the time the population was measured.</rdfs:comment>
    </owl:Class>
    


    <!-- https://w3id.org/isoiec21972/v1/Population_measure -->

    <owl:Class rdf:about="https://w3id.org/isoiec21972/v1/Population_measure">
        <rdfs:subClassOf rdf:resource="https://w3id.org/isoiec5087/-1/v1/CardinalityMeasure"/>
        <rdfs:subClassOf>
            <owl:Restriction>
                <owl:onProperty rdf:resource="https://w3id.org/isoiec21972/v1/unit_of_measure"/>
                <owl:allValuesFrom rdf:resource="https://w3id.org/isoiec21972/v1/Cardinality_unit"/>
            </owl:Restriction>
        </rdfs:subClassOf>
        <rdfs:comment>Reused from GCI Foundation ontology</rdfs:comment>
        <rdfs:label>Population Measure</rdfs:label>
        <rdfs:label>gci:Cardinality_unit is the unit of measure for the size of a set. The gci:Cardinality_unit is a ratio scale: gci:Cardinality_scale, which is a subclass of om:Ratio_scale and is has a zero element (namely zero).</rdfs:label>
    </owl:Class>
    


    <!-- https://w3id.org/isoiec21972/v1/Population_size -->

    <owl:Class rdf:about="https://w3id.org/isoiec21972/v1/Population_size">
        <rdfs:subClassOf rdf:resource="https://w3id.org/isoiec21972/v1/Quantity"/>
        <rdfs:subClassOf>
            <owl:Restriction>
                <owl:onProperty rdf:resource="https://w3id.org/isoiec21972/v1/value"/>
                <owl:allValuesFrom rdf:resource="https://w3id.org/isoiec21972/v1/Population_measure"/>
            </owl:Restriction>
        </rdfs:subClassOf>
        <rdfs:subClassOf>
            <owl:Restriction>
                <owl:onProperty rdf:resource="https://w3id.org/isoiec21972/v1/cardinality_of"/>
                <owl:qualifiedCardinality rdf:datatype="xsd:nonNegativeInteger">1</owl:qualifiedCardinality>
                <owl:onClass rdf:resource="https://w3id.org/isoiec21972/v1/Population"/>
            </owl:Restriction>
        </rdfs:subClassOf>
        <rdfs:comment>Reused from GCI Foundation ontology: http://ontology.eil.utoronto.ca/GCI/Foundation/GCI-Foundation-v2.owl</rdfs:comment>
        <rdfs:comment>gci:Population_size is a subclass of om:Quantity.  Its om:unit_of_measure is the gci:population_cardinality_unit. It is also a subclass of gs:Cardinality which provides the cardinality_of property that links to a gs:Population.</rdfs:comment>
        <rdfs:label>Population Size</rdfs:label>
    </owl:Class>
    


    <!-- https://w3id.org/isoiec21972/v1/Quantity -->

    <owl:Class rdf:about="https://w3id.org/isoiec21972/v1/Quantity">
        <rdfs:subClassOf rdf:resource="https://w3id.org/isoiec5087/-1/v1/CityUnitsThing"/>
        <rdfs:subClassOf>
            <owl:Restriction>
                <owl:onProperty rdf:resource="https://w3id.org/isoiec21972/v1/value"/>
                <owl:allValuesFrom rdf:resource="https://w3id.org/isoiec21972/v1/Measure"/>
            </owl:Restriction>
        </rdfs:subClassOf>
        <rdfs:label>quantity</rdfs:label>
    </owl:Class>
    


    <!-- https://w3id.org/isoiec21972/v1/System_of_units -->

    <owl:Class rdf:about="https://w3id.org/isoiec21972/v1/System_of_units">
        <rdfs:subClassOf rdf:resource="https://w3id.org/isoiec5087/-1/v1/CityUnitsThing"/>
        <rdfs:comment>In order to achieve a coherent, interdependent set of units of measure in the wide variety of units that exist, units are organised in systems of units. A system of units is based on a set of units chosen by convention to be the system’s base units, units that are considered to be mutually independent (i.e., can’t be expressed in terms of each other).</rdfs:comment>
        <rdfs:label>system of units</rdfs:label>
    </owl:Class>
    


    <!-- https://w3id.org/isoiec21972/v1/Unit_of_measure -->

    <owl:Class rdf:about="https://w3id.org/isoiec21972/v1/Unit_of_measure">
        <rdfs:subClassOf rdf:resource="https://w3id.org/isoiec5087/-1/v1/CityUnitsThing"/>
        <rdfs:label>unit</rdfs:label>
    </owl:Class>
    


    <!-- https://w3id.org/isoiec21972/v1/Unit_of_measureDivision -->

    <owl:Class rdf:about="https://w3id.org/isoiec21972/v1/Unit_of_measureDivision">
        <rdfs:subClassOf rdf:resource="https://w3id.org/isoiec21972/v1/Unit_of_measure"/>
        <rdfs:label>unit division</rdfs:label>
    </owl:Class>
    


    <!-- 
    ///////////////////////////////////////////////////////////////////////////////////////
    //
    // Individuals
    //
    ///////////////////////////////////////////////////////////////////////////////////////
     -->

    


    <!-- https://w3id.org/isoiec5087/-1/v1/NAD83 -->

    <owl:NamedIndividual rdf:about="https://w3id.org/isoiec5087/-1/v1/NAD83">
        <rdf:type rdf:resource="https://w3id.org/isoiec5087/-1/v1/Geo_Position_unit"/>
        <rdfs:comment>North American Datum of 1983. A geodetic reference system.</rdfs:comment>
    </owl:NamedIndividual>
    


    <!-- https://w3id.org/isoiec5087/-1/v1/WGS84 -->

    <owl:NamedIndividual rdf:about="https://w3id.org/isoiec5087/-1/v1/WGS84">
        <rdf:type rdf:resource="https://w3id.org/isoiec5087/-1/v1/Geo_Position_unit"/>
        <rdfs:comment>World Geodetic System of 1984. The reference system used by GPS.</rdfs:comment>
    </owl:NamedIndividual>
    


    <!-- https://w3id.org/isoiec5087/-1/v1/average -->

    <owl:NamedIndividual rdf:about="https://w3id.org/isoiec5087/-1/v1/average">
        <rdf:type rdf:resource="https://w3id.org/isoiec5087/-1/v1/Function"/>
    </owl:NamedIndividual>

    <!-- 
    ///////////////////////////////////////////////////////////////////////////////////////
    //
    // Object Properties
    //
    ///////////////////////////////////////////////////////////////////////////////////////
     -->

    <!-- https://w3id.org/isoiec5087/-1/v1/genericObjectProperty -->

    <owl:ObjectProperty rdf:about="https://w3id.org/isoiec5087/-1/v1/genericObjectProperty"/>
    

    <!-- 
    ///////////////////////////////////////////////////////////////////////////////////////
    //
    // Data properties
    //
    ///////////////////////////////////////////////////////////////////////////////////////
     -->

    <!-- https://w3id.org/isoiec5087/-1/v1/genericDataProperty -->

    <owl:DatatypeProperty rdf:about="https://w3id.org/isoiec5087/-1/v1/genericDataProperty"/>
    


    <!-- https://w3id.org/isoiec5087/-1/v1/hasDescription -->

    <owl:DatatypeProperty rdf:about="https://w3id.org/isoiec5087/-1/v1/hasDescription">
        <rdfs:subPropertyOf rdf:resource="https://w3id.org/isoiec5087/-1/v1/genericDataProperty"/>
    </owl:DatatypeProperty>
    


    <!-- https://w3id.org/isoiec5087/-1/v1/hasIdentifier -->

    <owl:DatatypeProperty rdf:about="https://w3id.org/isoiec5087/-1/v1/hasIdentifier">
        <rdfs:subPropertyOf rdf:resource="https://w3id.org/isoiec5087/-1/v1/genericDataProperty"/>
    </owl:DatatypeProperty>
    


    <!-- https://w3id.org/isoiec5087/-1/v1/hasName -->

    <owl:DatatypeProperty rdf:about="https://w3id.org/isoiec5087/-1/v1/hasName">
        <rdfs:subPropertyOf rdf:resource="https://w3id.org/isoiec5087/-1/v1/genericDataProperty"/>
    </owl:DatatypeProperty>
    


    

    <!-- 
    ///////////////////////////////////////////////////////////////////////////////////////
    //
    // Object Properties
    //
    ///////////////////////////////////////////////////////////////////////////////////////
     -->

    


    <!-- https://w3id.org/isoiec5087/-1/v1/MereologyOntologyProperty -->

    <owl:ObjectProperty rdf:about="https://w3id.org/isoiec5087/-1/v1/MereologyOntologyProperty">
        <skos:definition>Created for organizational purposes, to identify properties defined in the Mereology ontology.</skos:definition>
    </owl:ObjectProperty>
    


    <!-- https://w3id.org/isoiec5087/-1/v1/componentOf -->

    <owl:ObjectProperty rdf:about="https://w3id.org/isoiec5087/-1/v1/componentOf">
        <rdfs:subPropertyOf rdf:resource="https://w3id.org/isoiec5087/-1/v1/properPartOf"/>
        <owl:inverseOf rdf:resource="https://w3id.org/isoiec5087/-1/v1/hasComponent"/>
        <skos:definition>Something may be a Component of some other thing
More specifically, something may be a immediate component of something; in other words, if x is an immediate component of y, then there does not exist any other object that is a component of y and has x as a component.
Component-of is transitive. Immediate component-of is not transitive.
Immediate component-of is a subproperty of component-of.</skos:definition>
    </owl:ObjectProperty>
    


    <!-- https://w3id.org/isoiec5087/-1/v1/hasComponent -->

    <owl:ObjectProperty rdf:about="https://w3id.org/isoiec5087/-1/v1/hasComponent">
        <rdfs:subPropertyOf rdf:resource="https://w3id.org/isoiec5087/-1/v1/hasProperPart"/>
    </owl:ObjectProperty>
    


    <!-- https://w3id.org/isoiec5087/-1/v1/hasProperPart -->

    <owl:ObjectProperty rdf:about="https://w3id.org/isoiec5087/-1/v1/hasProperPart">
        <rdfs:subPropertyOf rdf:resource="https://w3id.org/isoiec5087/-1/v1/MereologyOntologyProperty"/>
        <owl:inverseOf rdf:resource="https://w3id.org/isoiec5087/-1/v1/properPartOf"/>
    </owl:ObjectProperty>
    


    <!-- https://w3id.org/isoiec5087/-1/v1/immediateComponentOf -->

    <owl:ObjectProperty rdf:about="https://w3id.org/isoiec5087/-1/v1/immediateComponentOf">
        <rdfs:subPropertyOf rdf:resource="https://w3id.org/isoiec5087/-1/v1/componentOf"/>
    </owl:ObjectProperty>
    


    <!-- https://w3id.org/isoiec5087/-1/v1/properPartOf -->

    <owl:ObjectProperty rdf:about="https://w3id.org/isoiec5087/-1/v1/properPartOf">
        <rdfs:subPropertyOf rdf:resource="https://w3id.org/isoiec5087/-1/v1/MereologyOntologyProperty"/>
        <skos:definition>Something may be a Proper Part of some other thing.
An object cannot be a proper part of itself. Thus, any object must have more than one proper part.
Proper Parthood is transitive.
Proper parthood is dense and so there exist no immediate proper parts; in other words, given some object, whatever proper part, x, we choose, there exists some slightly larger proper part of the object that also has x as a proper part.</skos:definition>
    </owl:ObjectProperty>

    <!-- 
    ///////////////////////////////////////////////////////////////////////////////////////
    //
    // Object Properties
    //
    ///////////////////////////////////////////////////////////////////////////////////////
     -->


    <!-- https://w3id.org/isoiec5087/-1/v1/OrganizationStructureOntologyObjectProperty -->

    <owl:ObjectProperty rdf:about="https://w3id.org/isoiec5087/-1/v1/OrganizationStructureOntologyObjectProperty"/>
    


    <!-- http://www.w3.org/ns/org#basedAt -->

    <rdf:Description rdf:about="http://www.w3.org/ns/org#basedAt">
        <rdfs:subPropertyOf rdf:resource="https://w3id.org/isoiec5087/-1/v1/OrganizationStructureOntologyObjectProperty"/>
    </rdf:Description>
    


    <!-- http://www.w3.org/ns/org#changedBy -->

    <rdf:Description rdf:about="http://www.w3.org/ns/org#changedBy">
        <rdfs:subPropertyOf rdf:resource="https://w3id.org/isoiec5087/-1/v1/OrganizationStructureOntologyObjectProperty"/>
    </rdf:Description>
    


    <!-- http://www.w3.org/ns/org#classification -->

    <rdf:Description rdf:about="http://www.w3.org/ns/org#classification">
        <rdfs:subPropertyOf rdf:resource="https://w3id.org/isoiec5087/-1/v1/OrganizationStructureOntologyObjectProperty"/>
    </rdf:Description>
    


    <!-- http://www.w3.org/ns/org#hasMember -->

    <rdf:Description rdf:about="http://www.w3.org/ns/org#hasMember">
        <rdfs:subPropertyOf rdf:resource="https://w3id.org/isoiec5087/-1/v1/OrganizationStructureOntologyObjectProperty"/>
    </rdf:Description>
    


    <!-- http://www.w3.org/ns/org#hasMembership -->

    <rdf:Description rdf:about="http://www.w3.org/ns/org#hasMembership">
        <rdfs:subPropertyOf rdf:resource="https://w3id.org/isoiec5087/-1/v1/OrganizationStructureOntologyObjectProperty"/>
    </rdf:Description>
    


    <!-- http://www.w3.org/ns/org#hasPost -->

    <rdf:Description rdf:about="http://www.w3.org/ns/org#hasPost">
        <rdfs:subPropertyOf rdf:resource="https://w3id.org/isoiec5087/-1/v1/OrganizationStructureOntologyObjectProperty"/>
    </rdf:Description>
    


    <!-- http://www.w3.org/ns/org#hasSite -->

    <rdf:Description rdf:about="http://www.w3.org/ns/org#hasSite">
        <rdfs:subPropertyOf rdf:resource="https://w3id.org/isoiec5087/-1/v1/OrganizationStructureOntologyObjectProperty"/>
    </rdf:Description>
    


    <!-- http://www.w3.org/ns/org#hasSubOrganization -->

    <rdf:Description rdf:about="http://www.w3.org/ns/org#hasSubOrganization">
        <rdfs:subPropertyOf rdf:resource="https://w3id.org/isoiec5087/-1/v1/OrganizationStructureOntologyObjectProperty"/>
    </rdf:Description>
    


    <!-- http://www.w3.org/ns/org#heldBy -->

    <rdf:Description rdf:about="http://www.w3.org/ns/org#heldBy">
        <rdfs:subPropertyOf rdf:resource="https://w3id.org/isoiec5087/-1/v1/OrganizationStructureOntologyObjectProperty"/>
    </rdf:Description>
    


    <!-- http://www.w3.org/ns/org#holds -->

    <rdf:Description rdf:about="http://www.w3.org/ns/org#holds">
        <rdfs:subPropertyOf rdf:resource="https://w3id.org/isoiec5087/-1/v1/OrganizationStructureOntologyObjectProperty"/>
    </rdf:Description>
    


    <!-- http://www.w3.org/ns/org#linkedTo -->

    <rdf:Description rdf:about="http://www.w3.org/ns/org#linkedTo">
        <rdfs:subPropertyOf rdf:resource="https://w3id.org/isoiec5087/-1/v1/OrganizationStructureOntologyObjectProperty"/>
    </rdf:Description>
    


    <!-- http://www.w3.org/ns/org#member -->

    <rdf:Description rdf:about="http://www.w3.org/ns/org#member">
        <rdfs:subPropertyOf rdf:resource="https://w3id.org/isoiec5087/-1/v1/OrganizationStructureOntologyObjectProperty"/>
    </rdf:Description>
    


    <!-- http://www.w3.org/ns/org#memberDuring -->

    <rdf:Description rdf:about="http://www.w3.org/ns/org#memberDuring">
        <rdfs:subPropertyOf rdf:resource="https://w3id.org/isoiec5087/-1/v1/OrganizationStructureOntologyObjectProperty"/>
    </rdf:Description>
    


    <!-- http://www.w3.org/ns/org#memberOf -->

    <rdf:Description rdf:about="http://www.w3.org/ns/org#memberOf">
        <rdfs:subPropertyOf rdf:resource="https://w3id.org/isoiec5087/-1/v1/OrganizationStructureOntologyObjectProperty"/>
    </rdf:Description>
    


    <!-- http://www.w3.org/ns/org#organization -->

    <rdf:Description rdf:about="http://www.w3.org/ns/org#organization">
        <rdfs:subPropertyOf rdf:resource="https://w3id.org/isoiec5087/-1/v1/OrganizationStructureOntologyObjectProperty"/>
    </rdf:Description>
    


    <!-- http://www.w3.org/ns/org#postIn -->

    <rdf:Description rdf:about="http://www.w3.org/ns/org#postIn">
        <rdfs:subPropertyOf rdf:resource="https://w3id.org/isoiec5087/-1/v1/OrganizationStructureOntologyObjectProperty"/>
    </rdf:Description>
    


    <!-- http://www.w3.org/ns/org#remuneration -->

    <rdf:Description rdf:about="http://www.w3.org/ns/org#remuneration">
        <rdfs:subPropertyOf rdf:resource="https://w3id.org/isoiec5087/-1/v1/OrganizationStructureOntologyObjectProperty"/>
    </rdf:Description>
    


    <!-- http://www.w3.org/ns/org#reportsTo -->

    <rdf:Description rdf:about="http://www.w3.org/ns/org#reportsTo">
        <rdfs:subPropertyOf rdf:resource="https://w3id.org/isoiec5087/-1/v1/OrganizationStructureOntologyObjectProperty"/>
    </rdf:Description>
    


    <!-- http://www.w3.org/ns/org#resultingOrganization -->

    <rdf:Description rdf:about="http://www.w3.org/ns/org#resultingOrganization">
        <rdfs:subPropertyOf rdf:resource="https://w3id.org/isoiec5087/-1/v1/OrganizationStructureOntologyObjectProperty"/>
    </rdf:Description>
    


    <!-- http://www.w3.org/ns/org#role -->

    <rdf:Description rdf:about="http://www.w3.org/ns/org#role">
        <rdfs:subPropertyOf rdf:resource="https://w3id.org/isoiec5087/-1/v1/OrganizationStructureOntologyObjectProperty"/>
    </rdf:Description>
    


    <!-- http://www.w3.org/ns/org#siteAddress -->

    <rdf:Description rdf:about="http://www.w3.org/ns/org#siteAddress">
        <rdfs:subPropertyOf rdf:resource="https://w3id.org/isoiec5087/-1/v1/OrganizationStructureOntologyObjectProperty"/>
    </rdf:Description>
    


    <!-- http://www.w3.org/ns/org#siteOf -->

    <rdf:Description rdf:about="http://www.w3.org/ns/org#siteOf">
        <rdfs:subPropertyOf rdf:resource="https://w3id.org/isoiec5087/-1/v1/OrganizationStructureOntologyObjectProperty"/>
    </rdf:Description>
    


    <!-- http://www.w3.org/ns/org#transitiveSubOrganizationOf -->

    <rdf:Description rdf:about="http://www.w3.org/ns/org#transitiveSubOrganizationOf">
        <rdfs:subPropertyOf rdf:resource="https://w3id.org/isoiec5087/-1/v1/OrganizationStructureOntologyObjectProperty"/>
    </rdf:Description>
    


    <!-- 
    ///////////////////////////////////////////////////////////////////////////////////////
    //
    // Data properties
    //
    ///////////////////////////////////////////////////////////////////////////////////////
     -->

    


    <!-- https://w3id.org/isoiec5087/-1/v1/OrganizationStructureOntologyDataProperty -->

    <owl:DatatypeProperty rdf:about="https://w3id.org/isoiec5087/-1/v1/OrganizationStructureOntologyDataProperty"/>
    


    <!-- http://www.w3.org/ns/org#location -->

    <rdf:Description rdf:about="http://www.w3.org/ns/org#location">
        <rdfs:subPropertyOf rdf:resource="https://w3id.org/isoiec5087/-1/v1/OrganizationStructureOntologyDataProperty"/>
    </rdf:Description>
    


    <!-- 
    ///////////////////////////////////////////////////////////////////////////////////////
    //
    // Classes
    //
    ///////////////////////////////////////////////////////////////////////////////////////
     -->

    


    <!-- https://w3id.org/isoiec5087/-1/v1/Organization -->

    <owl:Class rdf:about="https://w3id.org/isoiec5087/-1/v1/Organization">
        <rdfs:subClassOf rdf:resource="https://w3id.org/isoiec5087/-1/v1/Agent"/>
        <rdfs:subClassOf rdf:resource="https://w3id.org/isoiec5087/-1/v1/OrganizationStructureOntologyThing"/>
        <rdfs:subClassOf rdf:resource="org:Organization"/>
        <rdfs:comment>●	Organization: “represents a collection of people organized together into a community or other social, commercial or political structure. The group has some common purpose or reason for existence which goes beyond the set of people belonging to it. An organization may itself be able to act as an agent.” Properties included are:
○	hasName: a string name of the Organization
○	org:hasMember: identifies the agents that are members of the Organization.
○	org:hasSubOrganization: identifies the sub-Organizations within the Organization.
○	org:hasUnit: indicates an OrganizationUnit which is part of the Organization.
○	org:hasPost: identifies the Posts that exist in the Organization.
○	hasAsset: identifies the assets possessed by the Organization</rdfs:comment>
    </owl:Class>
    


    <!-- https://w3id.org/isoiec5087/-1/v1/OrganizationStructureOntologyThing -->

    <owl:Class rdf:about="https://w3id.org/isoiec5087/-1/v1/OrganizationStructureOntologyThing"/>
    

    <!-- 
    ///////////////////////////////////////////////////////////////////////////////////////
    //
    // Object Properties
    //
    ///////////////////////////////////////////////////////////////////////////////////////
     -->

    


    <!-- https://w3id.org/isoiec5087/-1/v1/provOntologyObjectProperty -->

    <owl:ObjectProperty rdf:about="https://w3id.org/isoiec5087/-1/v1/provOntologyObjectProperty"/>
    


    <!-- http://www.w3.org/ns/prov#alternateOf -->

    <rdf:Description rdf:about="http://www.w3.org/ns/prov#alternateOf">
        <rdfs:subPropertyOf rdf:resource="https://w3id.org/isoiec5087/-1/v1/provOntologyObjectProperty"/>
    </rdf:Description>
    


    <!-- http://www.w3.org/ns/prov#atLocation -->

    <rdf:Description rdf:about="http://www.w3.org/ns/prov#atLocation">
        <rdfs:subPropertyOf rdf:resource="https://w3id.org/isoiec5087/-1/v1/provOntologyObjectProperty"/>
    </rdf:Description>
    


    <!-- http://www.w3.org/ns/prov#hadActivity -->

    <rdf:Description rdf:about="http://www.w3.org/ns/prov#hadActivity">
        <rdfs:subPropertyOf rdf:resource="https://w3id.org/isoiec5087/-1/v1/provOntologyObjectProperty"/>
    </rdf:Description>
    


    <!-- http://www.w3.org/ns/prov#hadGeneration -->

    <rdf:Description rdf:about="http://www.w3.org/ns/prov#hadGeneration">
        <rdfs:subPropertyOf rdf:resource="https://w3id.org/isoiec5087/-1/v1/provOntologyObjectProperty"/>
    </rdf:Description>
    


    <!-- http://www.w3.org/ns/prov#hadPlan -->

    <rdf:Description rdf:about="http://www.w3.org/ns/prov#hadPlan">
        <rdfs:subPropertyOf rdf:resource="https://w3id.org/isoiec5087/-1/v1/provOntologyObjectProperty"/>
    </rdf:Description>
    


    <!-- http://www.w3.org/ns/prov#hadRole -->

    <rdf:Description rdf:about="http://www.w3.org/ns/prov#hadRole">
        <rdfs:subPropertyOf rdf:resource="https://w3id.org/isoiec5087/-1/v1/provOntologyObjectProperty"/>
    </rdf:Description>
    


    <!-- http://www.w3.org/ns/prov#hadUsage -->

    <rdf:Description rdf:about="http://www.w3.org/ns/prov#hadUsage">
        <rdfs:subPropertyOf rdf:resource="https://w3id.org/isoiec5087/-1/v1/provOntologyObjectProperty"/>
    </rdf:Description>
    


    <!-- http://www.w3.org/ns/prov#influenced -->

    <rdf:Description rdf:about="http://www.w3.org/ns/prov#influenced">
        <rdfs:subPropertyOf rdf:resource="https://w3id.org/isoiec5087/-1/v1/provOntologyObjectProperty"/>
    </rdf:Description>
    


    <!-- http://www.w3.org/ns/prov#influencer -->

    <rdf:Description rdf:about="http://www.w3.org/ns/prov#influencer">
        <rdfs:subPropertyOf rdf:resource="https://w3id.org/isoiec5087/-1/v1/provOntologyObjectProperty"/>
    </rdf:Description>
    


    <!-- http://www.w3.org/ns/prov#qualifiedInfluence -->

    <rdf:Description rdf:about="http://www.w3.org/ns/prov#qualifiedInfluence">
        <rdfs:subPropertyOf rdf:resource="https://w3id.org/isoiec5087/-1/v1/provOntologyObjectProperty"/>
    </rdf:Description>
    


    <!-- http://www.w3.org/ns/prov#wasInfluencedBy -->

    <rdf:Description rdf:about="http://www.w3.org/ns/prov#wasInfluencedBy">
        <rdfs:subPropertyOf rdf:resource="https://w3id.org/isoiec5087/-1/v1/provOntologyObjectProperty"/>
    </rdf:Description>
    


    <!-- 
    ///////////////////////////////////////////////////////////////////////////////////////
    //
    // Data properties
    //
    ///////////////////////////////////////////////////////////////////////////////////////
     -->

    


    <!-- https://w3id.org/isoiec5087/-1/v1/provOntologyDataProperty -->

    <owl:DatatypeProperty rdf:about="https://w3id.org/isoiec5087/-1/v1/provOntologyDataProperty"/>
    


    <!-- http://www.w3.org/ns/prov#atTime -->

    <rdf:Description rdf:about="http://www.w3.org/ns/prov#atTime">
        <rdfs:subPropertyOf rdf:resource="https://w3id.org/isoiec5087/-1/v1/provOntologyDataProperty"/>
    </rdf:Description>
    


    <!-- http://www.w3.org/ns/prov#endedAtTime -->

    <rdf:Description rdf:about="http://www.w3.org/ns/prov#endedAtTime">
        <rdfs:subPropertyOf rdf:resource="https://w3id.org/isoiec5087/-1/v1/provOntologyDataProperty"/>
    </rdf:Description>
    


    <!-- http://www.w3.org/ns/prov#generatedAtTime -->

    <rdf:Description rdf:about="http://www.w3.org/ns/prov#generatedAtTime">
        <rdfs:subPropertyOf rdf:resource="https://w3id.org/isoiec5087/-1/v1/provOntologyDataProperty"/>
    </rdf:Description>
    


    <!-- http://www.w3.org/ns/prov#invalidatedAtTime -->

    <rdf:Description rdf:about="http://www.w3.org/ns/prov#invalidatedAtTime">
        <rdfs:subPropertyOf rdf:resource="https://w3id.org/isoiec5087/-1/v1/provOntologyDataProperty"/>
    </rdf:Description>
    


    <!-- http://www.w3.org/ns/prov#startedAtTime -->

    <rdf:Description rdf:about="http://www.w3.org/ns/prov#startedAtTime">
        <rdfs:subPropertyOf rdf:resource="https://w3id.org/isoiec5087/-1/v1/provOntologyDataProperty"/>
    </rdf:Description>
    


    <!-- http://www.w3.org/ns/prov#value -->

    <rdf:Description rdf:about="http://www.w3.org/ns/prov#value">
        <rdfs:subPropertyOf rdf:resource="https://w3id.org/isoiec5087/-1/v1/provOntologyDataProperty"/>
    </rdf:Description>
    


    <!-- 
    ///////////////////////////////////////////////////////////////////////////////////////
    //
    // Classes
    //
    ///////////////////////////////////////////////////////////////////////////////////////
     -->

    


    <!-- https://w3id.org/isoiec5087/-1/v1/Activity -->

    <owl:Class rdf:about="https://w3id.org/isoiec5087/-1/v1/Activity">
        <rdfs:subClassOf rdf:resource="https://w3id.org/isoiec5087/-1/v1/Activity"/>
        <rdfs:subClassOf rdf:resource="http://www.w3.org/ns/prov#Activity"/>
    </owl:Class>
    


    <!-- https://w3id.org/isoiec5087/-1/v1/Agent -->

    <owl:Class rdf:about="https://w3id.org/isoiec5087/-1/v1/Agent">
        <rdfs:subClassOf rdf:resource="https://w3id.org/isoiec5087/-1/v1/Agent"/>
        <rdfs:subClassOf rdf:resource="http://www.w3.org/ns/prov#Agent"/>
    </owl:Class>
    


    <!-- https://w3id.org/isoiec5087/-1/v1/ProvOntologyThing -->

    <owl:Class rdf:about="https://w3id.org/isoiec5087/-1/v1/ProvOntologyThing"/>
    


    <!-- http://www.w3.org/ns/prov#Activity -->

    <rdf:Description rdf:about="http://www.w3.org/ns/prov#Activity">
        <rdfs:subClassOf rdf:resource="https://w3id.org/isoiec5087/-1/v1/ProvOntologyThing"/>
    </rdf:Description>
    


    <!-- http://www.w3.org/ns/prov#Agent -->

    <owl:Class rdf:about="http://www.w3.org/ns/prov#Agent">
        <rdfs:subClassOf rdf:resource="https://w3id.org/isoiec5087/-1/v1/ProvOntologyThing"/>
    </owl:Class>
    


    <!-- http://www.w3.org/ns/prov#Entity -->

    <rdf:Description rdf:about="http://www.w3.org/ns/prov#Entity">
        <rdfs:subClassOf rdf:resource="https://w3id.org/isoiec5087/-1/v1/ProvOntologyThing"/>
    </rdf:Description>
    


    <!-- http://www.w3.org/ns/prov#Influence -->

    <owl:Class rdf:about="http://www.w3.org/ns/prov#Influence">
        <rdfs:subClassOf rdf:resource="https://w3id.org/isoiec5087/-1/v1/ProvOntologyThing"/>
    </owl:Class>
    


    <!-- http://www.w3.org/ns/prov#InstantaneousEvent -->

    <owl:Class rdf:about="http://www.w3.org/ns/prov#InstantaneousEvent">
        <rdfs:subClassOf rdf:resource="https://w3id.org/isoiec5087/-1/v1/ProvOntologyThing"/>
    </owl:Class>
    


    <!-- http://www.w3.org/ns/prov#Location -->

    <owl:Class rdf:about="http://www.w3.org/ns/prov#Location">
        <rdfs:subClassOf rdf:resource="https://w3id.org/isoiec5087/-1/v1/ProvOntologyThing"/>
    </owl:Class>
    


    <!-- http://www.w3.org/ns/prov#Role -->

    <owl:Class rdf:about="http://www.w3.org/ns/prov#Role">
        <rdfs:subClassOf rdf:resource="https://w3id.org/isoiec5087/-1/v1/ProvOntologyThing"/>
    </owl:Class>

    <!-- https://w3id.org/isoiec5087/-1/v1/AnnotationProperty -->

    <owl:AnnotationProperty rdf:about="https://w3id.org/isoiec5087/-1/v1/AnnotationProperty"/>
    


    <!-- https://w3id.org/isoiec5087/-1/v1/Literal -->

    <owl:AnnotationProperty rdf:about="https://w3id.org/isoiec5087/-1/v1/Literal"/>
    


    <!-- 
    ///////////////////////////////////////////////////////////////////////////////////////
    //
    // Datatypes
    //
    ///////////////////////////////////////////////////////////////////////////////////////
     -->

    


    <!-- http://www.w3.org/2001/XMLSchema#time -->

    <rdfs:Datatype rdf:about="http://www.w3.org/2001/XMLSchema#time"/>
    


    <!-- 
    ///////////////////////////////////////////////////////////////////////////////////////
    //
    // Object Properties
    //
    ///////////////////////////////////////////////////////////////////////////////////////
     -->

    


    <!-- http://www.w3.org/2006/time#after -->

    <rdf:Description rdf:about="http://www.w3.org/2006/time#after">
        <rdfs:subPropertyOf rdf:resource="https://w3id.org/isoiec5087/-1/v1/timeOntologyProperty"/>
    </rdf:Description>
    


    <!-- http://www.w3.org/2006/time#before -->

    <rdf:Description rdf:about="http://www.w3.org/2006/time#before">
        <rdfs:subPropertyOf rdf:resource="https://w3id.org/isoiec5087/-1/v1/timeOntologyProperty"/>
    </rdf:Description>
    


    <!-- http://www.w3.org/2006/time#dayOfWeek -->

    <rdf:Description rdf:about="http://www.w3.org/2006/time#dayOfWeek">
        <rdfs:subPropertyOf rdf:resource="https://w3id.org/isoiec5087/-1/v1/timeOntologyProperty"/>
    </rdf:Description>
    


    <!-- http://www.w3.org/2006/time#hasDateTimeDescription -->

    <rdf:Description rdf:about="http://www.w3.org/2006/time#hasDateTimeDescription">
        <rdfs:subPropertyOf rdf:resource="https://w3id.org/isoiec5087/-1/v1/timeOntologyProperty"/>
    </rdf:Description>
    


    <!-- http://www.w3.org/2006/time#hasTRS -->

    <rdf:Description rdf:about="http://www.w3.org/2006/time#hasTRS">
        <rdfs:subPropertyOf rdf:resource="https://w3id.org/isoiec5087/-1/v1/timeOntologyProperty"/>
    </rdf:Description>
    


    <!-- http://www.w3.org/2006/time#hasTemporalDuration -->

    <rdf:Description rdf:about="http://www.w3.org/2006/time#hasTemporalDuration">
        <rdfs:subPropertyOf rdf:resource="https://w3id.org/isoiec5087/-1/v1/timeOntologyProperty"/>
    </rdf:Description>
    


    <!-- http://www.w3.org/2006/time#hasTime -->

    <rdf:Description rdf:about="http://www.w3.org/2006/time#hasTime">
        <rdfs:subPropertyOf rdf:resource="https://w3id.org/isoiec5087/-1/v1/timeOntologyProperty"/>
    </rdf:Description>
    


    <!-- http://www.w3.org/2006/time#inTemporalPosition -->

    <rdf:Description rdf:about="http://www.w3.org/2006/time#inTemporalPosition">
        <rdfs:subPropertyOf rdf:resource="https://w3id.org/isoiec5087/-1/v1/timeOntologyProperty"/>
    </rdf:Description>
    


    <!-- http://www.w3.org/2006/time#inside -->

    <rdf:Description rdf:about="http://www.w3.org/2006/time#inside">
        <rdfs:subPropertyOf rdf:resource="https://w3id.org/isoiec5087/-1/v1/timeOntologyProperty"/>
    </rdf:Description>
    


    <!-- http://www.w3.org/2006/time#intervalContains -->

    <rdf:Description rdf:about="http://www.w3.org/2006/time#intervalContains">
        <rdfs:subPropertyOf rdf:resource="https://w3id.org/isoiec5087/-1/v1/timeOntologyProperty"/>
    </rdf:Description>
    


    <!-- http://www.w3.org/2006/time#intervalDisjoint -->

    <rdf:Description rdf:about="http://www.w3.org/2006/time#intervalDisjoint">
        <rdfs:subPropertyOf rdf:resource="https://w3id.org/isoiec5087/-1/v1/timeOntologyProperty"/>
    </rdf:Description>
    


    <!-- http://www.w3.org/2006/time#intervalEquals -->

    <rdf:Description rdf:about="http://www.w3.org/2006/time#intervalEquals">
        <rdfs:subPropertyOf rdf:resource="https://w3id.org/isoiec5087/-1/v1/timeOntologyProperty"/>
    </rdf:Description>
    


    <!-- http://www.w3.org/2006/time#intervalFinishedBy -->

    <rdf:Description rdf:about="http://www.w3.org/2006/time#intervalFinishedBy">
        <rdfs:subPropertyOf rdf:resource="https://w3id.org/isoiec5087/-1/v1/timeOntologyProperty"/>
    </rdf:Description>
    


    <!-- http://www.w3.org/2006/time#intervalIn -->

    <rdf:Description rdf:about="http://www.w3.org/2006/time#intervalIn">
        <rdfs:subPropertyOf rdf:resource="https://w3id.org/isoiec5087/-1/v1/timeOntologyProperty"/>
    </rdf:Description>
    


    <!-- http://www.w3.org/2006/time#intervalMeets -->

    <rdf:Description rdf:about="http://www.w3.org/2006/time#intervalMeets">
        <rdfs:subPropertyOf rdf:resource="https://w3id.org/isoiec5087/-1/v1/timeOntologyProperty"/>
    </rdf:Description>
    


    <!-- http://www.w3.org/2006/time#intervalMetBy -->

    <rdf:Description rdf:about="http://www.w3.org/2006/time#intervalMetBy">
        <rdfs:subPropertyOf rdf:resource="https://w3id.org/isoiec5087/-1/v1/timeOntologyProperty"/>
    </rdf:Description>
    


    <!-- http://www.w3.org/2006/time#intervalOverlappedBy -->

    <rdf:Description rdf:about="http://www.w3.org/2006/time#intervalOverlappedBy">
        <rdfs:subPropertyOf rdf:resource="https://w3id.org/isoiec5087/-1/v1/timeOntologyProperty"/>
    </rdf:Description>
    


    <!-- http://www.w3.org/2006/time#intervalOverlaps -->

    <rdf:Description rdf:about="http://www.w3.org/2006/time#intervalOverlaps">
        <rdfs:subPropertyOf rdf:resource="https://w3id.org/isoiec5087/-1/v1/timeOntologyProperty"/>
    </rdf:Description>
    


    <!-- http://www.w3.org/2006/time#intervalStartedBy -->

    <rdf:Description rdf:about="http://www.w3.org/2006/time#intervalStartedBy">
        <rdfs:subPropertyOf rdf:resource="https://w3id.org/isoiec5087/-1/v1/timeOntologyProperty"/>
    </rdf:Description>
    


    <!-- http://www.w3.org/2006/time#monthOfYear -->

    <rdf:Description rdf:about="http://www.w3.org/2006/time#monthOfYear">
        <rdfs:subPropertyOf rdf:resource="https://w3id.org/isoiec5087/-1/v1/timeOntologyProperty"/>
    </rdf:Description>
    


    <!-- http://www.w3.org/2006/time#timeZone -->

    <rdf:Description rdf:about="http://www.w3.org/2006/time#timeZone">
        <rdfs:subPropertyOf rdf:resource="https://w3id.org/isoiec5087/-1/v1/timeOntologyProperty"/>
    </rdf:Description>
    


    <!-- http://www.w3.org/2006/time#unitType -->

    <rdf:Description rdf:about="http://www.w3.org/2006/time#unitType">
        <rdfs:subPropertyOf rdf:resource="https://w3id.org/isoiec5087/-1/v1/timeOntologyProperty"/>
    </rdf:Description>
    


    <!-- https://w3id.org/isoiec5087/-1/v1/beginsRecurringState -->

    <owl:ObjectProperty rdf:about="https://w3id.org/isoiec5087/-1/v1/beginsRecurringState">
        <rdfs:subPropertyOf rdf:resource="https://w3id.org/isoiec5087/-1/v1/recurringEventProperty"/>
    </owl:ObjectProperty>
    


    <!-- https://w3id.org/isoiec5087/-1/v1/beginsRecurringTime -->

    <owl:ObjectProperty rdf:about="https://w3id.org/isoiec5087/-1/v1/beginsRecurringTime">
        <rdfs:subPropertyOf rdf:resource="https://w3id.org/isoiec5087/-1/v1/recurringEventProperty"/>
    </owl:ObjectProperty>
    


    <!-- https://w3id.org/isoiec5087/-1/v1/endDayOfWeek -->

    <owl:ObjectProperty rdf:about="https://w3id.org/isoiec5087/-1/v1/endDayOfWeek">
        <rdfs:subPropertyOf rdf:resource="https://w3id.org/isoiec5087/-1/v1/recurringEventProperty"/>
    </owl:ObjectProperty>
    


    <!-- https://w3id.org/isoiec5087/-1/v1/endMonth -->

    <owl:ObjectProperty rdf:about="https://w3id.org/isoiec5087/-1/v1/endMonth">
        <rdfs:subPropertyOf rdf:resource="https://w3id.org/isoiec5087/-1/v1/recurringEventProperty"/>
    </owl:ObjectProperty>
    


    <!-- https://w3id.org/isoiec5087/-1/v1/endsRecurringState -->

    <owl:ObjectProperty rdf:about="https://w3id.org/isoiec5087/-1/v1/endsRecurringState">
        <rdfs:subPropertyOf rdf:resource="https://w3id.org/isoiec5087/-1/v1/recurringEventProperty"/>
    </owl:ObjectProperty>
    


    <!-- https://w3id.org/isoiec5087/-1/v1/endsRecurringTime -->

    <owl:ObjectProperty rdf:about="https://w3id.org/isoiec5087/-1/v1/endsRecurringTime">
        <rdfs:subPropertyOf rdf:resource="https://w3id.org/isoiec5087/-1/v1/recurringEventProperty"/>
    </owl:ObjectProperty>
    


    <!-- https://w3id.org/isoiec5087/-1/v1/hasDayOfWeek -->

    <owl:ObjectProperty rdf:about="https://w3id.org/isoiec5087/-1/v1/hasDayOfWeek">
        <rdfs:subPropertyOf rdf:resource="https://w3id.org/isoiec5087/-1/v1/recurringEventProperty"/>
    </owl:ObjectProperty>
    


    <!-- https://w3id.org/isoiec5087/-1/v1/hasMonth -->

    <owl:ObjectProperty rdf:about="https://w3id.org/isoiec5087/-1/v1/hasMonth">
        <rdfs:subPropertyOf rdf:resource="https://w3id.org/isoiec5087/-1/v1/recurringEventProperty"/>
    </owl:ObjectProperty>
    


    <!-- https://w3id.org/isoiec5087/-1/v1/hasOccurrence -->

    <owl:ObjectProperty rdf:about="https://w3id.org/isoiec5087/-1/v1/hasOccurrence">
        <rdfs:subPropertyOf rdf:resource="https://w3id.org/isoiec5087/-1/v1/recurringEventProperty"/>
    </owl:ObjectProperty>
    


    <!-- https://w3id.org/isoiec5087/-1/v1/hasSubRecurringEvent -->

    <owl:ObjectProperty rdf:about="https://w3id.org/isoiec5087/-1/v1/hasSubRecurringEvent">
        <rdfs:subPropertyOf rdf:resource="https://w3id.org/isoiec5087/-1/v1/recurringEventProperty"/>
    </owl:ObjectProperty>
    


    <!-- https://w3id.org/isoiec5087/-1/v1/onDateTimeDescription -->

    <owl:ObjectProperty rdf:about="https://w3id.org/isoiec5087/-1/v1/onDateTimeDescription">
        <rdfs:subPropertyOf rdf:resource="https://w3id.org/isoiec5087/-1/v1/recurringEventProperty"/>
    </owl:ObjectProperty>
    


    <!-- https://w3id.org/isoiec5087/-1/v1/recurringEventProperty -->

    <owl:ObjectProperty rdf:about="https://w3id.org/isoiec5087/-1/v1/recurringEventProperty">
        <rdfs:comment>Property added for organizational purposes only; to group all object properties defined in the recurring event ontology.</rdfs:comment>
    </owl:ObjectProperty>
    


    <!-- https://w3id.org/isoiec5087/-1/v1/recursAddition -->

    <owl:ObjectProperty rdf:about="https://w3id.org/isoiec5087/-1/v1/recursAddition">
        <rdfs:subPropertyOf rdf:resource="https://w3id.org/isoiec5087/-1/v1/recurringEventProperty"/>
    </owl:ObjectProperty>
    


    <!-- https://w3id.org/isoiec5087/-1/v1/recursExcept -->

    <owl:ObjectProperty rdf:about="https://w3id.org/isoiec5087/-1/v1/recursExcept">
        <rdfs:subPropertyOf rdf:resource="https://w3id.org/isoiec5087/-1/v1/recurringEventProperty"/>
    </owl:ObjectProperty>
    


    <!-- https://w3id.org/isoiec5087/-1/v1/timeOntologyProperty -->

    <owl:ObjectProperty rdf:about="https://w3id.org/isoiec5087/-1/v1/timeOntologyProperty">
        <rdfs:comment>Property added for organizational purposes only; to group all object properties defined in the time ontology.</rdfs:comment>
    </owl:ObjectProperty>
    


    <!-- https://w3id.org/isoiec5087/-1/v1/associatedLocation -->

    <owl:ObjectProperty rdf:about="https://w3id.org/isoiec5087/-1/v1/associatedLocation"/>
    


    <!-- 
    ///////////////////////////////////////////////////////////////////////////////////////
    //
    // Data properties
    //
    ///////////////////////////////////////////////////////////////////////////////////////
     -->

    


    <!-- http://www.w3.org/2006/time#day -->

    <rdf:Description rdf:about="http://www.w3.org/2006/time#day">
        <rdfs:subPropertyOf rdf:resource="https://w3id.org/isoiec5087/-1/v1/timeOntologyDataProperty"/>
    </rdf:Description>
    


    <!-- http://www.w3.org/2006/time#dayOfYear -->

    <rdf:Description rdf:about="http://www.w3.org/2006/time#dayOfYear">
        <rdfs:subPropertyOf rdf:resource="https://w3id.org/isoiec5087/-1/v1/timeOntologyDataProperty"/>
    </rdf:Description>
    


    <!-- http://www.w3.org/2006/time#days -->

    <rdf:Description rdf:about="http://www.w3.org/2006/time#days">
        <rdfs:subPropertyOf rdf:resource="https://w3id.org/isoiec5087/-1/v1/timeOntologyDataProperty"/>
    </rdf:Description>
    


    <!-- http://www.w3.org/2006/time#hasXSDDuration -->

    <rdf:Description rdf:about="http://www.w3.org/2006/time#hasXSDDuration">
        <rdfs:subPropertyOf rdf:resource="https://w3id.org/isoiec5087/-1/v1/timeOntologyDataProperty"/>
    </rdf:Description>
    


    <!-- http://www.w3.org/2006/time#hour -->

    <rdf:Description rdf:about="http://www.w3.org/2006/time#hour">
        <rdfs:subPropertyOf rdf:resource="https://w3id.org/isoiec5087/-1/v1/timeOntologyDataProperty"/>
    </rdf:Description>
    


    <!-- http://www.w3.org/2006/time#hours -->

    <rdf:Description rdf:about="http://www.w3.org/2006/time#hours">
        <rdfs:subPropertyOf rdf:resource="https://w3id.org/isoiec5087/-1/v1/timeOntologyDataProperty"/>
    </rdf:Description>
    


    <!-- http://www.w3.org/2006/time#inXSDDate -->

    <rdf:Description rdf:about="http://www.w3.org/2006/time#inXSDDate">
        <rdfs:subPropertyOf rdf:resource="https://w3id.org/isoiec5087/-1/v1/timeOntologyDataProperty"/>
    </rdf:Description>
    


    <!-- http://www.w3.org/2006/time#inXSDDateTime -->

    <rdf:Description rdf:about="http://www.w3.org/2006/time#inXSDDateTime">
        <rdfs:subPropertyOf rdf:resource="https://w3id.org/isoiec5087/-1/v1/timeOntologyDataProperty"/>
    </rdf:Description>
    


    <!-- http://www.w3.org/2006/time#inXSDDateTimeStamp -->

    <rdf:Description rdf:about="http://www.w3.org/2006/time#inXSDDateTimeStamp">
        <rdfs:subPropertyOf rdf:resource="https://w3id.org/isoiec5087/-1/v1/timeOntologyDataProperty"/>
    </rdf:Description>
    


    <!-- http://www.w3.org/2006/time#inXSDgYear -->

    <rdf:Description rdf:about="http://www.w3.org/2006/time#inXSDgYear">
        <rdfs:subPropertyOf rdf:resource="https://w3id.org/isoiec5087/-1/v1/timeOntologyDataProperty"/>
    </rdf:Description>
    


    <!-- http://www.w3.org/2006/time#inXSDgYearMonth -->

    <rdf:Description rdf:about="http://www.w3.org/2006/time#inXSDgYearMonth">
        <rdfs:subPropertyOf rdf:resource="https://w3id.org/isoiec5087/-1/v1/timeOntologyDataProperty"/>
    </rdf:Description>
    


    <!-- http://www.w3.org/2006/time#minute -->

    <rdf:Description rdf:about="http://www.w3.org/2006/time#minute">
        <rdfs:subPropertyOf rdf:resource="https://w3id.org/isoiec5087/-1/v1/timeOntologyDataProperty"/>
    </rdf:Description>
    


    <!-- http://www.w3.org/2006/time#minutes -->

    <rdf:Description rdf:about="http://www.w3.org/2006/time#minutes">
        <rdfs:subPropertyOf rdf:resource="https://w3id.org/isoiec5087/-1/v1/timeOntologyDataProperty"/>
    </rdf:Description>
    


    <!-- http://www.w3.org/2006/time#month -->

    <rdf:Description rdf:about="http://www.w3.org/2006/time#month">
        <rdfs:subPropertyOf rdf:resource="https://w3id.org/isoiec5087/-1/v1/timeOntologyDataProperty"/>
    </rdf:Description>
    


    <!-- http://www.w3.org/2006/time#months -->

    <rdf:Description rdf:about="http://www.w3.org/2006/time#months">
        <rdfs:subPropertyOf rdf:resource="https://w3id.org/isoiec5087/-1/v1/timeOntologyDataProperty"/>
    </rdf:Description>
    


    <!-- http://www.w3.org/2006/time#nominalPosition -->

    <rdf:Description rdf:about="http://www.w3.org/2006/time#nominalPosition">
        <rdfs:subPropertyOf rdf:resource="https://w3id.org/isoiec5087/-1/v1/timeOntologyDataProperty"/>
    </rdf:Description>
    


    <!-- http://www.w3.org/2006/time#numericDuration -->

    <rdf:Description rdf:about="http://www.w3.org/2006/time#numericDuration">
        <rdfs:subPropertyOf rdf:resource="https://w3id.org/isoiec5087/-1/v1/timeOntologyDataProperty"/>
    </rdf:Description>
    


    <!-- http://www.w3.org/2006/time#numericPosition -->

    <rdf:Description rdf:about="http://www.w3.org/2006/time#numericPosition">
        <rdfs:subPropertyOf rdf:resource="https://w3id.org/isoiec5087/-1/v1/timeOntologyDataProperty"/>
    </rdf:Description>
    


    <!-- http://www.w3.org/2006/time#second -->

    <rdf:Description rdf:about="http://www.w3.org/2006/time#second">
        <rdfs:subPropertyOf rdf:resource="https://w3id.org/isoiec5087/-1/v1/timeOntologyDataProperty"/>
    </rdf:Description>
    


    <!-- http://www.w3.org/2006/time#seconds -->

    <rdf:Description rdf:about="http://www.w3.org/2006/time#seconds">
        <rdfs:subPropertyOf rdf:resource="https://w3id.org/isoiec5087/-1/v1/timeOntologyDataProperty"/>
    </rdf:Description>
    


    <!-- http://www.w3.org/2006/time#week -->

    <rdf:Description rdf:about="http://www.w3.org/2006/time#week">
        <rdfs:subPropertyOf rdf:resource="https://w3id.org/isoiec5087/-1/v1/timeOntologyDataProperty"/>
    </rdf:Description>
    


    <!-- http://www.w3.org/2006/time#weeks -->

    <rdf:Description rdf:about="http://www.w3.org/2006/time#weeks">
        <rdfs:subPropertyOf rdf:resource="https://w3id.org/isoiec5087/-1/v1/timeOntologyDataProperty"/>
    </rdf:Description>
    


    <!-- http://www.w3.org/2006/time#xsdDateTime -->

    <rdf:Description rdf:about="http://www.w3.org/2006/time#xsdDateTime">
        <rdfs:subPropertyOf rdf:resource="https://w3id.org/isoiec5087/-1/v1/timeOntologyDataProperty"/>
    </rdf:Description>
    


    <!-- http://www.w3.org/2006/time#year -->

    <rdf:Description rdf:about="http://www.w3.org/2006/time#year">
        <rdfs:subPropertyOf rdf:resource="https://w3id.org/isoiec5087/-1/v1/timeOntologyDataProperty"/>
    </rdf:Description>
    


    <!-- http://www.w3.org/2006/time#years -->

    <rdf:Description rdf:about="http://www.w3.org/2006/time#years">
        <rdfs:subPropertyOf rdf:resource="https://w3id.org/isoiec5087/-1/v1/timeOntologyDataProperty"/>
    </rdf:Description>
    


    <!-- https://w3id.org/isoiec5087/-1/v1/endTime -->

    <owl:DatatypeProperty rdf:about="https://w3id.org/isoiec5087/-1/v1/endTime">
        <rdfs:subPropertyOf rdf:resource="https://w3id.org/isoiec5087/-1/v1/recurringEventDataProperty"/>
    </owl:DatatypeProperty>
    


    <!-- https://w3id.org/isoiec5087/-1/v1/recurringEventDataProperty -->

    <owl:DatatypeProperty rdf:about="https://w3id.org/isoiec5087/-1/v1/recurringEventDataProperty"/>
    


    <!-- https://w3id.org/isoiec5087/-1/v1/startTime -->

    <owl:DatatypeProperty rdf:about="https://w3id.org/isoiec5087/-1/v1/startTime">
        <rdfs:subPropertyOf rdf:resource="https://w3id.org/isoiec5087/-1/v1/recurringEventDataProperty"/>
        <rdfs:range rdf:resource="xsd:time"/>
    </owl:DatatypeProperty>
    


    <!-- https://w3id.org/isoiec5087/-1/v1/timeOntologyDataProperty -->

    <owl:DatatypeProperty rdf:about="https://w3id.org/isoiec5087/-1/v1/timeOntologyDataProperty">
        <rdfs:comment>Data property added for organizational purposes only; to group all data properties defined in the time ontology.</rdfs:comment>
    </owl:DatatypeProperty>
    


    <!-- 
    ///////////////////////////////////////////////////////////////////////////////////////
    //
    // Classes
    //
    ///////////////////////////////////////////////////////////////////////////////////////
     -->

    


    <!-- https://w3id.org/isoiec5087/-1/v1/Activity -->

    <owl:Class rdf:about="https://w3id.org/isoiec5087/-1/v1/Activity"/>
    


    <!-- https://w3id.org/isoiec5087/-1/v1/State -->

    <owl:Class rdf:about="https://w3id.org/isoiec5087/-1/v1/State"/>
    


    <!-- https://w3id.org/isoiec5087/-1/v1/DailyRecurringEvent -->

    <owl:Class rdf:about="https://w3id.org/isoiec5087/-1/v1/DailyRecurringEvent">
        <rdfs:subClassOf rdf:resource="https://w3id.org/isoiec5087/-1/v1/RecurringEvent"/>
        <rdfs:subClassOf>
            <owl:Restriction>
                <owl:onProperty rdf:resource="https://w3id.org/isoiec5087/-1/v1/startTime"/>
                <owl:maxQualifiedCardinality rdf:datatype="xsd:nonNegativeInteger">1</owl:maxQualifiedCardinality>
                <owl:onDataRange rdf:resource="xsd:time"/>
            </owl:Restriction>
        </rdfs:subClassOf>
        <rdfs:comment>A DailyRecurringEvent may occur at the same time, or different times every day. Therefore, it has at most one associated time – the start time. No associated time indicates that there is no commitment to a recurring start time for the event. A DailyEvent does not necessarily have the same endtime or duration, therefore these are not specified.</rdfs:comment>
    </owl:Class>
    


    <!-- https://w3id.org/isoiec5087/-1/v1/ExceptionDay -->

    <owl:Class rdf:about="https://w3id.org/isoiec5087/-1/v1/ExceptionDay">
        <rdfs:subClassOf rdf:resource="https://w3id.org/isoiec5087/-1/v1/RecurringEventThing"/>
        <rdfs:subClassOf>
            <owl:Restriction>
                <owl:onProperty rdf:resource="https://w3id.org/isoiec5087/-1/v1/onDateTimeDescription"/>
                <owl:someValuesFrom rdf:resource="time:GeneralDateTimeDescription"/>
            </owl:Restriction>
        </rdfs:subClassOf>
        <rdfs:subClassOf>
            <owl:Restriction>
                <owl:onProperty rdf:resource="https://w3id.org/isoiec5087/-1/v1/hasName"/>
                <owl:someValuesFrom rdf:resource="xsd:string"/>
            </owl:Restriction>
        </rdfs:subClassOf>
    </owl:Class>
    


    <!-- https://w3id.org/isoiec5087/-1/v1/MonthlyRecurringEvent -->

    <owl:Class rdf:about="https://w3id.org/isoiec5087/-1/v1/MonthlyRecurringEvent">
        <rdfs:subClassOf rdf:resource="https://w3id.org/isoiec5087/-1/v1/RecurringEvent"/>
        <rdfs:subClassOf>
            <owl:Restriction>
                <owl:onProperty rdf:resource="https://w3id.org/isoiec5087/-1/v1/onDateTimeDescription"/>
                <owl:qualifiedCardinality rdf:datatype="xsd:nonNegativeInteger">1</owl:qualifiedCardinality>
                <owl:onClass rdf:resource="time:GeneralDateTimeDescription"/>
            </owl:Restriction>
        </rdfs:subClassOf>
        <rdfs:comment>A MonthlyRecurringEvent recurs regularly on the same day of each month, as specified by the dayOfMonth data property. Note that there is often ambiguity regarding the semantics of a monthly recurring event: in this formalization, a MonthlyRecurringEvent is any event that recurs regularly on the same day of each month; other interpretations sometimes consider events that recur on the same day of week, or first or last day, in which case the day of month will vary.</rdfs:comment>
    </owl:Class>
    


    <!-- https://w3id.org/isoiec5087/-1/v1/RecurringEvent -->

    <owl:Class rdf:about="https://w3id.org/isoiec5087/-1/v1/RecurringEvent">
        <rdfs:subClassOf rdf:resource="https://w3id.org/isoiec5087/-1/v1/RecurringEventThing"/>
        <rdfs:subClassOf>
            <owl:Restriction>
                <owl:onProperty rdf:resource="https://w3id.org/isoiec5087/-1/v1/beginsRecurringState"/>
                <owl:allValuesFrom rdf:resource="https://w3id.org/isoiec5087/-1/v1/State"/>
            </owl:Restriction>
        </rdfs:subClassOf>
        <rdfs:subClassOf>
            <owl:Restriction>
                <owl:onProperty rdf:resource="https://w3id.org/isoiec5087/-1/v1/beginsRecurringTime"/>
                <owl:allValuesFrom rdf:resource="time:TemporalEntity"/>
            </owl:Restriction>
        </rdfs:subClassOf>
        <rdfs:subClassOf>
            <owl:Restriction>
                <owl:onProperty rdf:resource="https://w3id.org/isoiec5087/-1/v1/endsRecurringState"/>
                <owl:allValuesFrom rdf:resource="https://w3id.org/isoiec5087/-1/v1/State"/>
            </owl:Restriction>
        </rdfs:subClassOf>
        <rdfs:subClassOf>
            <owl:Restriction>
                <owl:onProperty rdf:resource="https://w3id.org/isoiec5087/-1/v1/endsRecurringTime"/>
                <owl:allValuesFrom rdf:resource="time:TemporalEntity"/>
            </owl:Restriction>
        </rdfs:subClassOf>
        <rdfs:subClassOf>
            <owl:Restriction>
                <owl:onProperty rdf:resource="https://w3id.org/isoiec5087/-1/v1/hasDayOfWeek"/>
                <owl:allValuesFrom rdf:resource="time:DayOfWeek"/>
            </owl:Restriction>
        </rdfs:subClassOf>
        <rdfs:subClassOf>
            <owl:Restriction>
                <owl:onProperty rdf:resource="https://w3id.org/isoiec5087/-1/v1/hasOccurrence"/>
                <owl:allValuesFrom rdf:resource="https://w3id.org/isoiec5087/-1/v1/Activity"/>
            </owl:Restriction>
        </rdfs:subClassOf>
        <rdfs:subClassOf>
            <owl:Restriction>
                <owl:onProperty rdf:resource="https://w3id.org/isoiec5087/-1/v1/hasSubRecurringEvent"/>
                <owl:allValuesFrom rdf:resource="https://w3id.org/isoiec5087/-1/v1/RecurringEvent"/>
            </owl:Restriction>
        </rdfs:subClassOf>
        <rdfs:subClassOf>
            <owl:Restriction>
                <owl:onProperty rdf:resource="https://w3id.org/isoiec5087/-1/v1/onDateTimeDescription"/>
                <owl:allValuesFrom rdf:resource="time:GeneralDateTimeDescription"/>
            </owl:Restriction>
        </rdfs:subClassOf>
        <rdfs:subClassOf>
            <owl:Restriction>
                <owl:onProperty rdf:resource="https://w3id.org/isoiec5087/-1/v1/recursAddition"/>
                <owl:allValuesFrom>
                    <owl:Class>
                        <owl:unionOf rdf:parseType="Collection">
                            <rdf:Description rdf:about="http://www.w3.org/2006/time#DayOfWeek"/>
                            <rdf:Description rdf:about="http://www.w3.org/2006/time#TemporalEntity"/>
                        </owl:unionOf>
                    </owl:Class>
                </owl:allValuesFrom>
            </owl:Restriction>
        </rdfs:subClassOf>
        <rdfs:subClassOf>
            <owl:Restriction>
                <owl:onProperty rdf:resource="https://w3id.org/isoiec5087/-1/v1/recursExcept"/>
                <owl:allValuesFrom>
                    <owl:Class>
                        <owl:unionOf rdf:parseType="Collection">
                            <rdf:Description rdf:about="http://www.w3.org/2006/time#DayOfWeek"/>
                            <rdf:Description rdf:about="http://www.w3.org/2006/time#TemporalEntity"/>
                        </owl:unionOf>
                    </owl:Class>
                </owl:allValuesFrom>
            </owl:Restriction>
        </rdfs:subClassOf>
        <rdfs:subClassOf>
            <owl:Restriction>
                <owl:onProperty rdf:resource="https://w3id.org/isoiec5087/-1/v1/associatedLocation"/>
                <owl:allValuesFrom rdf:resource="https://w3id.org/isoiec5087/-1/v1/Location"/>
            </owl:Restriction>
        </rdfs:subClassOf>
        <rdfs:subClassOf>
            <owl:Restriction>
                <owl:onProperty rdf:resource="https://w3id.org/isoiec5087/-1/v1/endTime"/>
                <owl:allValuesFrom rdf:resource="xsd:time"/>
            </owl:Restriction>
        </rdfs:subClassOf>
        <rdfs:subClassOf>
            <owl:Restriction>
                <owl:onProperty rdf:resource="https://w3id.org/isoiec5087/-1/v1/startTime"/>
                <owl:allValuesFrom rdf:resource="xsd:time"/>
            </owl:Restriction>
        </rdfs:subClassOf>
        <rdfs:comment>Based on the data model defined in: http://www.vertabelo.com/blog/technical-articles/again-and-again-managing-recurring-events-in-a-data-model but is integrated into the general city ontology.</rdfs:comment>
        <rdfs:comment xml:lang="en">Recurring events are defined based on the regular interval at which they occur; this is captures using some combination of the hasTime, dayOfWeek, hasMonth, and dayOfMonth properties.  Using these properties, ontology defines the following specizliations of the RecurringEvent class. Other subclasses may be defined similarly, as required.

A RecurringEvent is defined to have the following properties:
•	hasActivity: identifies the Activities that take place at the time and location.
•	associatedLocation: identifies the locations (Features) where the event occurs.
•	hasSubRecurringEvent: identifies the sub recurring events that comprise the recurring event. As with an Activity, a RecurringEvent may be decomposed/decomposed into simpler/more complex RecurringEvents to support varying levels of granularity.
•	startTime: specifies the start time of the event’s activity using xsd:time format.
•	endTime: specifies the end time of the event’s activity using xsd:time format.
•	schema:dayOfWeek: specifies the day of the week that a weekly recurring event occurs.
•	hasMonth: specifies the month for which a yearly recurring event occurs.
•	dayOfMonth: specifies the day of the month that a monthly recurring event occurs.
•	beginsRecurringTime: defines a time to initiate the recurring event.
•	endsRecurringTime: defines a time to terminate the recurring event.
•	beginsRecurringState: defines a state that must be true in order to initiate the recurring event.
•	endsRecurringState: defines a state that must be true in order terminate the recurring event.
•	recursExcept: defines the exceptions for the recurring event, i.e., conditions when the event does not occur.  Can specify a time, day of the week, or specific dates.
•	recursAddition: defines condition when the recurrent event should be added. Can specify a time, day of the week, or specific dates.</rdfs:comment>
    </owl:Class>
    


    <!-- https://w3id.org/isoiec5087/-1/v1/RecurringEventThing -->

    <owl:Class rdf:about="https://w3id.org/isoiec5087/-1/v1/RecurringEventThing">
        <rdfs:comment>Class added for organizational purposes only; to group all classes defined in the recurring-event ontology.</rdfs:comment>
    </owl:Class>
    


    <!-- https://w3id.org/isoiec5087/-1/v1/WeeklyRecurringEvent -->

    <owl:Class rdf:about="https://w3id.org/isoiec5087/-1/v1/WeeklyRecurringEvent">
        <rdfs:subClassOf rdf:resource="https://w3id.org/isoiec5087/-1/v1/RecurringEvent"/>
        <rdfs:subClassOf>
            <owl:Restriction>
                <owl:onProperty rdf:resource="https://w3id.org/isoiec5087/-1/v1/hasDayOfWeek"/>
                <owl:qualifiedCardinality rdf:datatype="xsd:nonNegativeInteger">1</owl:qualifiedCardinality>
                <owl:onClass rdf:resource="time:DayOfWeek"/>
            </owl:Restriction>
        </rdfs:subClassOf>
        <rdfs:comment>A WeeklyRecurringEvent recurs on the regularly on the same day of the week, as specified by the schema:dayOfWeek property.</rdfs:comment>
    </owl:Class>
    


    <!-- https://w3id.org/isoiec5087/-1/v1/YearlyRecurringEvent -->

    <owl:Class rdf:about="https://w3id.org/isoiec5087/-1/v1/YearlyRecurringEvent">
        <rdfs:subClassOf rdf:resource="https://w3id.org/isoiec5087/-1/v1/RecurringEvent"/>
        <rdfs:subClassOf>
            <owl:Restriction>
                <owl:onProperty rdf:resource="https://w3id.org/isoiec5087/-1/v1/onDateTimeDescription"/>
                <owl:qualifiedCardinality rdf:datatype="xsd:nonNegativeInteger">1</owl:qualifiedCardinality>
                <owl:onClass rdf:resource="time:GeneralDateTimeDescription"/>
            </owl:Restriction>
        </rdfs:subClassOf>
        <rdfs:comment>A YearlyRecurringEvent recurs regularly on the same day of the same month, as specified by the hasMonth and dayOfMonth properties. As with MonthlyRecurringEvent, there may be ambiguity regarding the semantics of a yearly recurring event, however this formalization captures only the notion of an event that recurs on the same day of the same month (e.g. a birthday).</rdfs:comment>
    </owl:Class>
    


    <!-- https://w3id.org/isoiec5087/-1/v1/Location -->

    <owl:Class rdf:about="https://w3id.org/isoiec5087/-1/v1/Location"/>
    


    <!-- 
    ///////////////////////////////////////////////////////////////////////////////////////
    //
    // Individuals
    //
    ///////////////////////////////////////////////////////////////////////////////////////
     -->

    


    <!-- http://schema.org/Friday -->

    <owl:NamedIndividual rdf:about="http://schema.org/Friday"/>
    


    <!-- http://schema.org/Monday -->

    <owl:NamedIndividual rdf:about="http://schema.org/Monday"/>
    


    <!-- http://schema.org/PublicHoliday -->

    <owl:NamedIndividual rdf:about="http://schema.org/PublicHoliday"/>
    


    <!-- http://schema.org/Saturday -->

    <owl:NamedIndividual rdf:about="http://schema.org/Saturday"/>
    


    <!-- http://schema.org/Sunday -->

    <owl:NamedIndividual rdf:about="http://schema.org/Sunday"/>
    


    <!-- http://schema.org/Thursday -->

    <owl:NamedIndividual rdf:about="http://schema.org/Thursday"/>
    


    <!-- http://schema.org/Tuesday -->

    <owl:NamedIndividual rdf:about="http://schema.org/Tuesday"/>
    


    <!-- http://schema.org/Wednesday -->

    <owl:NamedIndividual rdf:about="http://schema.org/Wednesday"/>
    


    <!-- https://w3id.org/isoiec5087/-1/v1/April -->

    <owl:NamedIndividual rdf:about="https://w3id.org/isoiec5087/-1/v1/April"/>
    


    <!-- https://w3id.org/isoiec5087/-1/v1/August -->

    <owl:NamedIndividual rdf:about="https://w3id.org/isoiec5087/-1/v1/August"/>
    


    <!-- https://w3id.org/isoiec5087/-1/v1/December -->

    <owl:NamedIndividual rdf:about="https://w3id.org/isoiec5087/-1/v1/December"/>
    


    <!-- https://w3id.org/isoiec5087/-1/v1/February -->

    <owl:NamedIndividual rdf:about="https://w3id.org/isoiec5087/-1/v1/February"/>
    


    <!-- https://w3id.org/isoiec5087/-1/v1/January -->

    <owl:NamedIndividual rdf:about="https://w3id.org/isoiec5087/-1/v1/January"/>
    


    <!-- https://w3id.org/isoiec5087/-1/v1/July -->

    <owl:NamedIndividual rdf:about="https://w3id.org/isoiec5087/-1/v1/July"/>
    


    <!-- https://w3id.org/isoiec5087/-1/v1/June -->

    <owl:NamedIndividual rdf:about="https://w3id.org/isoiec5087/-1/v1/June"/>
    


    <!-- https://w3id.org/isoiec5087/-1/v1/March -->

    <owl:NamedIndividual rdf:about="https://w3id.org/isoiec5087/-1/v1/March"/>
    


    <!-- https://w3id.org/isoiec5087/-1/v1/May -->

    <owl:NamedIndividual rdf:about="https://w3id.org/isoiec5087/-1/v1/May"/>
    


    <!-- https://w3id.org/isoiec5087/-1/v1/November -->

    <owl:NamedIndividual rdf:about="https://w3id.org/isoiec5087/-1/v1/November"/>
    


    <!-- https://w3id.org/isoiec5087/-1/v1/October -->

    <owl:NamedIndividual rdf:about="https://w3id.org/isoiec5087/-1/v1/October"/>
    


    <!-- https://w3id.org/isoiec5087/-1/v1/September -->

    <owl:NamedIndividual rdf:about="https://w3id.org/isoiec5087/-1/v1/September"/>
    <rdf:Description>
        <AnnotationProperty></AnnotationProperty>
        <Literal>City of Toronto Integrated Subject and Service Ontology: Recurring Event Sub-Ontology</Literal>
    </rdf:Description>
    <rdf:Description>
        <AnnotationProperty></AnnotationProperty>
        <Literal>Mark S. Fox
http://eil.utoronto.ca</Literal>
    </rdf:Description>
    <rdf:Description>
        <owl:cardinality rdf:datatype="xsd:nonNegativeInteger">1</owl:cardinality>
    </rdf:Description>
    <rdf:Description>
        <owl:cardinality rdf:datatype="xsd:nonNegativeInteger">0</owl:cardinality>
    </rdf:Description>
    <rdf:Description>
        <owl:cardinality rdf:datatype="xsd:nonNegativeInteger">1</owl:cardinality>
    </rdf:Description>
    <rdf:Description>
        <owl:cardinality rdf:datatype="xsd:nonNegativeInteger">1</owl:cardinality>
    </rdf:Description>
    <rdf:Description>
        <owl:cardinality rdf:datatype="xsd:nonNegativeInteger">0</owl:cardinality>
    </rdf:Description>
    <rdf:Description>
        <owl:cardinality rdf:datatype="xsd:nonNegativeInteger">0</owl:cardinality>
    </rdf:Description>



    <!-- 
    ///////////////////////////////////////////////////////////////////////////////////////
    //
    // Annotation properties
    //
    ///////////////////////////////////////////////////////////////////////////////////////
     -->

    

    <!-- 
    ///////////////////////////////////////////////////////////////////////////////////////
    //
    // Object Properties
    //
    ///////////////////////////////////////////////////////////////////////////////////////
     -->

    


    <!-- https://w3id.org/isoiec5087/-1/v1/ResourceOntologyProperty -->

    <owl:ObjectProperty rdf:about="https://w3id.org/isoiec5087/-1/v1/ResourceOntologyProperty">
        <skos:definition>Added for organizational purposes, to identify all properties defined in the Resource ontology.</skos:definition>
    </owl:ObjectProperty>
    


    <!-- https://w3id.org/isoiec5087/-1/v1/capacityInUse -->

    <owl:ObjectProperty rdf:about="https://w3id.org/isoiec5087/-1/v1/capacityInUse">
        <rdfs:subPropertyOf rdf:resource="https://w3id.org/isoiec5087/-1/v1/ResourceOntologyProperty"/>
        <rdf:type rdf:resource="owl:FunctionalProperty"/>
    </owl:ObjectProperty>
    


    <!-- https://w3id.org/isoiec5087/-1/v1/consumedBy -->

    <owl:ObjectProperty rdf:about="https://w3id.org/isoiec5087/-1/v1/consumedBy">
        <rdfs:subPropertyOf rdf:resource="https://w3id.org/isoiec5087/-1/v1/preconditionOf"/>
        <rdfs:subPropertyOf rdf:resource="https://w3id.org/isoiec5087/-1/v1/ResourceOntologyProperty"/>
    </owl:ObjectProperty>
    


    <!-- https://w3id.org/isoiec5087/-1/v1/forResource -->

    <owl:ObjectProperty rdf:about="https://w3id.org/isoiec5087/-1/v1/forResource">
        <rdfs:subPropertyOf rdf:resource="https://w3id.org/isoiec5087/-1/v1/ResourceOntologyProperty"/>
    </owl:ObjectProperty>
    


    <!-- https://w3id.org/isoiec5087/-1/v1/forState -->

    <owl:ObjectProperty rdf:about="https://w3id.org/isoiec5087/-1/v1/forState">
        <rdfs:subPropertyOf rdf:resource="https://w3id.org/isoiec5087/-1/v1/ResourceOntologyProperty"/>
    </owl:ObjectProperty>
    


    <!-- https://w3id.org/isoiec5087/-1/v1/hasAllocation -->

    <owl:ObjectProperty rdf:about="https://w3id.org/isoiec5087/-1/v1/hasAllocation">
        <rdfs:subPropertyOf rdf:resource="https://w3id.org/isoiec5087/-1/v1/ResourceOntologyProperty"/>
    </owl:ObjectProperty>
    


    <!-- https://w3id.org/isoiec5087/-1/v1/hasAsset -->

    <owl:ObjectProperty rdf:about="https://w3id.org/isoiec5087/-1/v1/hasAsset">
        <rdfs:subPropertyOf rdf:resource="https://w3id.org/isoiec5087/-1/v1/ResourceOntologyProperty"/>
    </owl:ObjectProperty>
    


    <!-- https://w3id.org/isoiec5087/-1/v1/hasAvailableCapacity -->

    <owl:ObjectProperty rdf:about="https://w3id.org/isoiec5087/-1/v1/hasAvailableCapacity">
        <rdfs:subPropertyOf rdf:resource="https://w3id.org/isoiec5087/-1/v1/ResourceOntologyProperty"/>
    </owl:ObjectProperty>
    


    <!-- https://w3id.org/isoiec5087/-1/v1/hasCapacity -->

    <owl:ObjectProperty rdf:about="https://w3id.org/isoiec5087/-1/v1/hasCapacity">
        <rdfs:subPropertyOf rdf:resource="https://w3id.org/isoiec5087/-1/v1/ResourceOntologyProperty"/>
        <rdf:type rdf:resource="owl:FunctionalProperty"/>
    </owl:ObjectProperty>
    


    <!-- https://w3id.org/isoiec5087/-1/v1/hasOwner -->

    <owl:ObjectProperty rdf:about="https://w3id.org/isoiec5087/-1/v1/hasOwner">
        <rdfs:subPropertyOf rdf:resource="https://w3id.org/isoiec5087/-1/v1/ResourceOntologyProperty"/>
        <owl:inverseOf rdf:resource="https://w3id.org/isoiec5087/-1/v1/ownedBy"/>
        <rdfs:domain rdf:resource="https://w3id.org/isoiec5087/-1/v1/Resource"/>
        <rdfs:comment>A Resource may have some owner. The owner of a resource is subject to change over time.</rdfs:comment>
    </owl:ObjectProperty>
    


    <!-- https://w3id.org/isoiec5087/-1/v1/hasQuantity -->

    <owl:ObjectProperty rdf:about="https://w3id.org/isoiec5087/-1/v1/hasQuantity">
        <rdfs:subPropertyOf rdf:resource="https://w3id.org/isoiec5087/-1/v1/ResourceOntologyProperty"/>
    </owl:ObjectProperty>
    


    <!-- https://w3id.org/isoiec5087/-1/v1/hasResource -->

    <owl:ObjectProperty rdf:about="https://w3id.org/isoiec5087/-1/v1/hasResource">
        <rdfs:subPropertyOf rdf:resource="https://w3id.org/isoiec5087/-1/v1/ResourceOntologyProperty"/>
        <owl:inverseOf rdf:resource="https://w3id.org/isoiec5087/-1/v1/resourceOf"/>
    </owl:ObjectProperty>
    


    <!-- https://w3id.org/isoiec5087/-1/v1/ownedBy -->

    <owl:ObjectProperty rdf:about="https://w3id.org/isoiec5087/-1/v1/ownedBy">
        <rdfs:subPropertyOf rdf:resource="https://w3id.org/isoiec5087/-1/v1/ResourceOntologyProperty"/>
    </owl:ObjectProperty>
    


    <!-- https://w3id.org/isoiec5087/-1/v1/participatesIn -->

    <owl:ObjectProperty rdf:about="https://w3id.org/isoiec5087/-1/v1/participatesIn">
        <rdfs:subPropertyOf rdf:resource="https://w3id.org/isoiec5087/-1/v1/ResourceOntologyProperty"/>
    </owl:ObjectProperty>
    


    <!-- https://w3id.org/isoiec5087/-1/v1/resourceOf -->

    <owl:ObjectProperty rdf:about="https://w3id.org/isoiec5087/-1/v1/resourceOf">
        <rdfs:subPropertyOf rdf:resource="https://w3id.org/isoiec5087/-1/v1/ResourceOntologyProperty"/>
    </owl:ObjectProperty>
    


    <!-- https://w3id.org/isoiec5087/-1/v1/usedBy -->

    <owl:ObjectProperty rdf:about="https://w3id.org/isoiec5087/-1/v1/usedBy">
        <rdfs:subPropertyOf rdf:resource="https://w3id.org/isoiec5087/-1/v1/preconditionOf"/>
        <rdfs:subPropertyOf rdf:resource="https://w3id.org/isoiec5087/-1/v1/ResourceOntologyProperty"/>
    </owl:ObjectProperty>
    


    <!-- 
    ///////////////////////////////////////////////////////////////////////////////////////
    //
    // Classes
    //
    ///////////////////////////////////////////////////////////////////////////////////////
     -->

    


    <!-- https://w3id.org/isoiec21972/v1/Quantity -->

    <owl:Class rdf:about="https://w3id.org/isoiec21972/v1/Quantity"/>
    


    <!-- https://w3id.org/isoiec5087/-1/v1/ConsumeState -->

    <owl:Class rdf:about="https://w3id.org/isoiec5087/-1/v1/ConsumeState">
        <rdfs:subClassOf rdf:resource="https://w3id.org/isoiec5087/-1/v1/TerminalResourceState"/>
    </owl:Class>
    


    <!-- https://w3id.org/isoiec5087/-1/v1/DivisibleResource -->

    <owl:Class rdf:about="https://w3id.org/isoiec5087/-1/v1/DivisibleResource">
        <rdfs:subClassOf rdf:resource="https://w3id.org/isoiec5087/-1/v1/Resource"/>
        <owl:disjointWith rdf:resource="https://w3id.org/isoiec5087/-1/v1/NonDivisibleResource"/>
    </owl:Class>
    


    <!-- https://w3id.org/isoiec5087/-1/v1/NonDivisibleResource -->

    <owl:Class rdf:about="https://w3id.org/isoiec5087/-1/v1/NonDivisibleResource">
        <rdfs:subClassOf rdf:resource="https://w3id.org/isoiec5087/-1/v1/Resource"/>
    </owl:Class>
    


    <!-- https://w3id.org/isoiec5087/-1/v1/PlannedAllocation -->

    <owl:Class rdf:about="https://w3id.org/isoiec5087/-1/v1/PlannedAllocation">
        <rdfs:subClassOf rdf:resource="https://w3id.org/isoiec5087/-1/v1/Manifestation"/>
        <rdfs:subClassOf rdf:resource="https://w3id.org/isoiec5087/-1/v1/ResourceOntologyThing"/>
        <rdfs:subClassOf>
            <owl:Restriction>
                <owl:onProperty rdf:resource="time:hasTime"/>
                <owl:qualifiedCardinality rdf:datatype="xsd:nonNegativeInteger">1</owl:qualifiedCardinality>
                <owl:onClass rdf:resource="time:TemporalEntity"/>
            </owl:Restriction>
        </rdfs:subClassOf>
        <rdfs:subClassOf>
            <owl:Restriction>
                <owl:onProperty rdf:resource="https://w3id.org/isoiec5087/-1/v1/forResource"/>
                <owl:qualifiedCardinality rdf:datatype="xsd:nonNegativeInteger">1</owl:qualifiedCardinality>
                <owl:onClass rdf:resource="https://w3id.org/isoiec5087/-1/v1/Resource"/>
            </owl:Restriction>
        </rdfs:subClassOf>
        <rdfs:subClassOf>
            <owl:Restriction>
                <owl:onProperty rdf:resource="https://w3id.org/isoiec5087/-1/v1/forState"/>
                <owl:qualifiedCardinality rdf:datatype="xsd:nonNegativeInteger">1</owl:qualifiedCardinality>
                <owl:onClass rdf:resource="https://w3id.org/isoiec5087/-1/v1/State"/>
            </owl:Restriction>
        </rdfs:subClassOf>
        <rdfs:subClassOf>
            <owl:Restriction>
                <owl:onProperty rdf:resource="https://w3id.org/isoiec5087/-1/v1/hasQuantity"/>
                <owl:qualifiedCardinality rdf:datatype="xsd:nonNegativeInteger">1</owl:qualifiedCardinality>
                <owl:onClass rdf:resource="https://w3id.org/isoiec21972/v1/Quantity"/>
            </owl:Restriction>
        </rdfs:subClassOf>
        <rdfs:comment xml:lang="en">Specifies the planned allocation of a resource to an activity via a state.
forResource: specifies the resource that is being allocated
forState: specifies the state that the resource is allocated to
hasTime: specifies the DateTimeInterval that the resource is allocated to the state
hasQuantity: the amount of the resource that is allocated.

Note that Allocation is a Manifestation as the allocation may change over time.</rdfs:comment>
    </owl:Class>
    


    <!-- https://w3id.org/isoiec5087/-1/v1/ProduceState -->

    <owl:Class rdf:about="https://w3id.org/isoiec5087/-1/v1/ProduceState">
        <rdfs:subClassOf rdf:resource="https://w3id.org/isoiec5087/-1/v1/TerminalResourceState"/>
    </owl:Class>
    


    <!-- https://w3id.org/isoiec5087/-1/v1/ReleaseState -->

    <owl:Class rdf:about="https://w3id.org/isoiec5087/-1/v1/ReleaseState">
        <rdfs:subClassOf rdf:resource="https://w3id.org/isoiec5087/-1/v1/TerminalResourceState"/>
    </owl:Class>
    


    <!-- https://w3id.org/isoiec5087/-1/v1/Resource -->

    <owl:Class rdf:about="https://w3id.org/isoiec5087/-1/v1/Resource">
        <rdfs:subClassOf rdf:resource="https://w3id.org/isoiec5087/-1/v1/ResourceOntologyThing"/>
        <rdfs:subClassOf>
            <owl:Restriction>
                <owl:onProperty rdf:resource="https://w3id.org/isoiec5087/-1/v1/hasLocation"/>
                <owl:allValuesFrom rdf:resource="https://w3id.org/isoiec5087/-1/v1/Location"/>
            </owl:Restriction>
        </rdfs:subClassOf>
        <rdfs:subClassOf>
            <owl:Restriction>
                <owl:onProperty rdf:resource="https://w3id.org/isoiec5087/-1/v1/hasAllocation"/>
                <owl:allValuesFrom rdf:resource="https://w3id.org/isoiec5087/-1/v1/PlannedAllocation"/>
            </owl:Restriction>
        </rdfs:subClassOf>
        <rdfs:subClassOf>
            <owl:Restriction>
                <owl:onProperty rdf:resource="https://w3id.org/isoiec5087/-1/v1/participatesIn"/>
                <owl:minQualifiedCardinality rdf:datatype="xsd:nonNegativeInteger">1</owl:minQualifiedCardinality>
                <owl:onClass rdf:resource="https://w3id.org/isoiec5087/-1/v1/Activity"/>
            </owl:Restriction>
        </rdfs:subClassOf>
        <rdfs:subClassOf>
            <owl:Restriction>
                <owl:onProperty rdf:resource="https://w3id.org/isoiec5087/-1/v1/capacityInUse"/>
                <owl:qualifiedCardinality rdf:datatype="xsd:nonNegativeInteger">1</owl:qualifiedCardinality>
                <owl:onClass rdf:resource="https://w3id.org/isoiec21972/v1/Quantity"/>
            </owl:Restriction>
        </rdfs:subClassOf>
        <rdfs:subClassOf>
            <owl:Restriction>
                <owl:onProperty rdf:resource="https://w3id.org/isoiec5087/-1/v1/hasAvailableCapacity"/>
                <owl:qualifiedCardinality rdf:datatype="xsd:nonNegativeInteger">1</owl:qualifiedCardinality>
                <owl:onClass rdf:resource="https://w3id.org/isoiec21972/v1/Quantity"/>
            </owl:Restriction>
        </rdfs:subClassOf>
        <rdfs:subClassOf>
            <owl:Restriction>
                <owl:onProperty rdf:resource="https://w3id.org/isoiec5087/-1/v1/hasCapacity"/>
                <owl:qualifiedCardinality rdf:datatype="xsd:nonNegativeInteger">1</owl:qualifiedCardinality>
                <owl:onClass rdf:resource="https://w3id.org/isoiec21972/v1/Quantity"/>
            </owl:Restriction>
        </rdfs:subClassOf>
        <owl:disjointUnionOf rdf:parseType="Collection">
            <rdf:Description rdf:about="https://w3id.org/isoiec5087/-1/v1/DivisibleResource"/>
            <rdf:Description rdf:about="https://w3id.org/isoiec5087/-1/v1/NonDivisibleResource"/>
        </owl:disjointUnionOf>
        <skos:definition>A Resource is a generic representation of some Thing that can be &quot;used&quot; in an Activity.
A Resource may have some Location, amount or availability, according to the definition of the Manifestation or TimeVaryingEntity.
A Resource must be classified as some Resource Type.
A Resource may participate in some Activity Occurrence. In other words, it links to the Activity that the Resource is being used/consumed/produced/released at the time of the manifestation.
A specific Resource may be used in or consumed in some activity occurrence.

A Resource may have some associated location. This property captures an approximate location that may or may not differ from its actual location. For example, a landmark may be associated with a particular point (single set of coordinates), whereas the landmark itself in fact has a location that extends beyond this single point. It may even be the case that the associated location is distinct from (ie. not contained in) the actual location.</skos:definition>
    </owl:Class>
    


    <!-- https://w3id.org/isoiec5087/-1/v1/ResourceOntologyThing -->

    <owl:Class rdf:about="https://w3id.org/isoiec5087/-1/v1/ResourceOntologyThing">
        <skos:definition>Added for organizational purposes, to identify all classes defined in the Resource ontology.</skos:definition>
    </owl:Class>
    


    <!-- https://w3id.org/isoiec5087/-1/v1/TerminalResourceState -->

    <owl:Class rdf:about="https://w3id.org/isoiec5087/-1/v1/TerminalResourceState">
        <rdfs:subClassOf rdf:resource="https://w3id.org/isoiec5087/-1/v1/TerminalState"/>
        <rdfs:subClassOf rdf:resource="https://w3id.org/isoiec5087/-1/v1/ResourceOntologyThing"/>
        <rdfs:subClassOf>
            <owl:Restriction>
                <owl:onProperty rdf:resource="https://w3id.org/isoiec5087/-1/v1/hasAllocation"/>
                <owl:allValuesFrom rdf:resource="https://w3id.org/isoiec5087/-1/v1/PlannedAllocation"/>
            </owl:Restriction>
        </rdfs:subClassOf>
        <rdfs:subClassOf>
            <owl:Restriction>
                <owl:onProperty rdf:resource="https://w3id.org/isoiec5087/-1/v1/hasQuantity"/>
                <owl:allValuesFrom rdf:resource="https://w3id.org/isoiec21972/v1/Quantity"/>
            </owl:Restriction>
        </rdfs:subClassOf>
        <rdfs:subClassOf>
            <owl:Restriction>
                <owl:onProperty rdf:resource="https://w3id.org/isoiec5087/-1/v1/hasResource"/>
                <owl:allValuesFrom rdf:resource="https://w3id.org/isoiec5087/-1/v1/Resource"/>
            </owl:Restriction>
        </rdfs:subClassOf>
    </owl:Class>
    


    <!-- https://w3id.org/isoiec5087/-1/v1/UseState -->

    <owl:Class rdf:about="https://w3id.org/isoiec5087/-1/v1/UseState">
        <rdfs:subClassOf rdf:resource="https://w3id.org/isoiec5087/-1/v1/TerminalResourceState"/>
    </owl:Class>
    <rdf:Description>
        <owl:minQualifiedCardinality rdf:datatype="xsd:nonNegativeInteger">1</owl:minQualifiedCardinality>
    </rdf:Description>
    <rdf:Description>
        <owl:qualifiedCardinality rdf:datatype="xsd:nonNegativeInteger">1</owl:qualifiedCardinality>
    </rdf:Description>
    


    <!-- 
    ///////////////////////////////////////////////////////////////////////////////////////
    //
    // Annotations
    //
    ///////////////////////////////////////////////////////////////////////////////////////
     -->

    <rdf:Description rdf:about="http://www.w3.org/2003/01/geo/wgs84_pos#">
        <dcterms:date>$Date: 2009/04/20 15:00:30 $</dcterms:date>
        <skos:definition>A vocabulary for representing latitude, longitude and 
 altitude information in the WGS84 geodetic reference datum. 
 Version $Id: wgs84_pos.rdf,v 1.22 2009/04/20 15:00:30 timbl Exp $. See http://www.w3.org/2003/01/geo/ for more details.</skos:definition>
        <dcterms:title>WGS84 Geo Positioning: an RDF vocabulary</dcterms:title>
        <rdfs:comment>
Recent changes to this namespace:
$Log: wgs84_pos.rdf,v $
Revision 1.22  2009/04/20 15:00:30  timbl
Remove the time bits which have been deal with elsewhere eg in iCal.

Revision 1.21  2009/04/20 12:52:47  timbl
try again

Revision 1.20  2009/04/20 12:42:11  timbl
Add Event (edited ages ago and never checked in), and location (following discussion http://chatlogs.planetrdf.com/swig/2009-04-20#T12-36-09)

Revision 1.19  2009/04/20 12:36:31  timbl
Add Event (edited ages ago and never checked in), and location (following discussion http://chatlogs.planetrdf.com/swig/2009-04-20#T12-36-09)

Revision 1.18  2006/02/01 22:01:04  danbri
Clarified that lat and long are decimal degrees, and that alt is decimal metres about local reference ellipsoid

Revision 1.17  2004/02/06 17:38:12  danbri
Fixed a bad commit screwup

Revision 1.15  2003/04/19 11:24:08  danbri
Fixed the typo even more.

Revision 1.14  2003/04/19 11:16:56  danbri
fixed a typo

Revision 1.13  2003/02/19 22:27:27  connolly
relaxed domain constraints on lat/long/alt from Point to SpatialThing

Revision 1.12  2003/01/12 01:41:41  danbri
Trying local copy of XSLT doc.

Revision 1.11  2003/01/12 01:20:18  danbri
added a link to morten&apos;s xslt rdfs viewer.

Revision 1.10  2003/01/11 18:56:49  danbri
Removed datatype range from lat and long properties, since they would
have required each occurance of the property to mention the datatype.

Revision 1.9  2003/01/11 11:41:31  danbri
Another typo; repaired rdfs:Property to rdf:Property x4

Revision 1.8  2003/01/11 11:05:02  danbri
Added an rdfs:range for each lat/long/alt property,
http://www.w3.org/2001/XMLSchema#float

Revision 1.7  2003/01/10 20:25:16  danbri
Longer rdfs:comment for Point, trying to be Earth-centric and neutral about
coordinate system(s) at the same time. Feedback welcomed.

Revision 1.6  2003/01/10 20:18:30  danbri
Added CVS log comments into the RDF/XML as an rdfs:comment property of the
vocabulary. Note that this is not common practice (but seems both harmless
and potentially useful).


revision 1.5
date: 2003/01/10 20:14:31;  author: danbri;  state: Exp;  lines: +16 -5
Updated schema:
Added a dc:date, added url for more info. Changed the rdfs:label of the
namespace from gp to geo. Added a class Point, set as the rdfs:domain of
each property. Added XML comment on the lat_long property suggesting that
we might not need it (based on #rdfig commentary from implementors).

revision 1.4
date: 2003/01/10 20:01:07;  author: danbri;  state: Exp;  lines: +6 -5
Fixed typo; several rdfs:about attributes are now rdf:about. Thanks to MortenF in
#rdfig for catching this error.

revision 1.3
date: 2003/01/10 11:59:03;  author: danbri;  state: Exp;  lines: +4 -3
fixed buglet in vocab, added more wgs links

revision 1.2
date: 2003/01/10 11:01:11;  author: danbri;  state: Exp;  lines: +4 -4
Removed alt from the as-a-flat-string property, and switched from
space separated to comma separated.

revision 1.1
date: 2003/01/10 10:53:23;  author: danbri;  state: Exp;
basic geo vocab

</rdfs:comment>
        <rdfs:label>geo</rdfs:label>
    </rdf:Description>
    <rdf:Description rdf:about="http://www.w3.org/2003/01/geo/wgs84_pos#lat_long">
        <rdfs:comment>A comma-separated representation of a latitude, longitude coordinate.</rdfs:comment>
        <rdfs:label>lat/long</rdfs:label>
    </rdf:Description>

        <!-- 
    ///////////////////////////////////////////////////////////////////////////////////////
    //
    // Datatypes
    //
    ///////////////////////////////////////////////////////////////////////////////////////
     -->

    


    <!-- http://franz.com/ns/allegrograph/5.0/geo/nd#_lat_la_-9.+1_+9.+1_+1.-4_+1.-1_lon_lo_-1.8+2_+1.8+2_+1.-4 -->

    <rdfs:Datatype rdf:about="http://franz.com/ns/allegrograph/5.0/geo/nd#_lat_la_-9.+1_+9.+1_+1.-4_+1.-1_lon_lo_-1.8+2_+1.8+2_+1.-4">
        <skos:prefLabel>nD Lat Lon</skos:prefLabel>
    </rdfs:Datatype>
    


    <!-- 
    ///////////////////////////////////////////////////////////////////////////////////////
    //
    // Object Properties
    //
    ///////////////////////////////////////////////////////////////////////////////////////
     -->

    


    <!-- http://www.opengis.net/ont/geosparql#ehContains -->

    <owl:ObjectProperty rdf:about="http://www.opengis.net/ont/geosparql#ehContains">
        <rdfs:subPropertyOf rdf:resource="http://standards.iso.org/iso-iec/5087/-1/ed-1/en/ontology/SpatialLoc#SpatialLocOntologyProperty"/>
    </owl:ObjectProperty>
    


    <!-- http://www.opengis.net/ont/geosparql#ehCoveredBy -->

    <owl:ObjectProperty rdf:about="http://www.opengis.net/ont/geosparql#ehCoveredBy">
        <rdfs:subPropertyOf rdf:resource="http://standards.iso.org/iso-iec/5087/-1/ed-1/en/ontology/SpatialLoc#SpatialLocOntologyProperty"/>
    </owl:ObjectProperty>
    


    <!-- http://www.opengis.net/ont/geosparql#ehCovers -->

    <owl:ObjectProperty rdf:about="http://www.opengis.net/ont/geosparql#ehCovers">
        <rdfs:subPropertyOf rdf:resource="https://w3id.org/isoiec5087/-1/v1/SpatialLocOntologyProperty"/>
    </owl:ObjectProperty>
    


    <!-- http://www.opengis.net/ont/geosparql#ehDisjoint -->

    <owl:ObjectProperty rdf:about="http://www.opengis.net/ont/geosparql#ehDisjoint">
        <rdfs:subPropertyOf rdf:resource="https://w3id.org/isoiec5087/-1/v1/SpatialLocOntologyProperty"/>
    </owl:ObjectProperty>
    


    <!-- http://www.opengis.net/ont/geosparql#ehEquals -->

    <owl:ObjectProperty rdf:about="http://www.opengis.net/ont/geosparql#ehEquals">
        <rdfs:subPropertyOf rdf:resource="https://w3id.org/isoiec5087/-1/v1/SpatialLocOntologyProperty"/>
    </owl:ObjectProperty>
    


    <!-- http://www.opengis.net/ont/geosparql#ehInside -->

    <owl:ObjectProperty rdf:about="http://www.opengis.net/ont/geosparql#ehInside">
        <rdfs:subPropertyOf rdf:resource="https://w3id.org/isoiec5087/-1/v1/SpatialLocOntologyProperty"/>
    </owl:ObjectProperty>
    


    <!-- http://www.opengis.net/ont/geosparql#ehMeet -->

    <owl:ObjectProperty rdf:about="http://www.opengis.net/ont/geosparql#ehMeet">
        <rdfs:subPropertyOf rdf:resource="https://w3id.org/isoiec5087/-1/v1/SpatialLocOntologyProperty"/>
    </owl:ObjectProperty>
    


    <!-- http://www.opengis.net/ont/geosparql#ehOverlap -->

    <owl:ObjectProperty rdf:about="http://www.opengis.net/ont/geosparql#ehOverlap">
        <rdfs:subPropertyOf rdf:resource="https://w3id.org/isoiec5087/-1/v1/SpatialLocOntologyProperty"/>
    </owl:ObjectProperty>
    


    <!-- http://www.opengis.net/ont/geosparql#hasGeometry -->

    <owl:ObjectProperty rdf:about="http://www.opengis.net/ont/geosparql#hasGeometry">
        <rdfs:subPropertyOf rdf:resource="https://w3id.org/isoiec5087/-1/v1/SpatialLocOntologyProperty"/>
    </owl:ObjectProperty>
    


    <!-- http://www.opengis.net/ont/geosparql#rcc8dc -->

    <owl:ObjectProperty rdf:about="http://www.opengis.net/ont/geosparql#rcc8dc">
        <rdfs:subPropertyOf rdf:resource="https://w3id.org/isoiec5087/-1/v1/SpatialLocOntologyProperty"/>
    </owl:ObjectProperty>
    


    <!-- http://www.opengis.net/ont/geosparql#rcc8ec -->

    <owl:ObjectProperty rdf:about="http://www.opengis.net/ont/geosparql#rcc8ec">
        <rdfs:subPropertyOf rdf:resource="https://w3id.org/isoiec5087/-1/v1/SpatialLocOntologyProperty"/>
    </owl:ObjectProperty>
    


    <!-- http://www.opengis.net/ont/geosparql#rcc8eq -->

    <owl:ObjectProperty rdf:about="http://www.opengis.net/ont/geosparql#rcc8eq">
        <rdfs:subPropertyOf rdf:resource="https://w3id.org/isoiec5087/-1/v1/SpatialLocOntologyProperty"/>
    </owl:ObjectProperty>
    


    <!-- http://www.opengis.net/ont/geosparql#rcc8ntpp -->

    <owl:ObjectProperty rdf:about="http://www.opengis.net/ont/geosparql#rcc8ntpp">
        <rdfs:subPropertyOf rdf:resource="https://w3id.org/isoiec5087/-1/v1/SpatialLocOntologyProperty"/>
    </owl:ObjectProperty>
    


    <!-- http://www.opengis.net/ont/geosparql#rcc8ntppi -->

    <owl:ObjectProperty rdf:about="http://www.opengis.net/ont/geosparql#rcc8ntppi">
        <rdfs:subPropertyOf rdf:resource="https://w3id.org/isoiec5087/-1/v1/SpatialLocOntologyProperty"/>
    </owl:ObjectProperty>
    


    <!-- http://www.opengis.net/ont/geosparql#rcc8po -->

    <owl:ObjectProperty rdf:about="http://www.opengis.net/ont/geosparql#rcc8po">
        <rdfs:subPropertyOf rdf:resource="https://w3id.org/isoiec5087/-1/v1/SpatialLocOntologyProperty"/>
    </owl:ObjectProperty>
    


    <!-- http://www.opengis.net/ont/geosparql#rcc8tpp -->

    <owl:ObjectProperty rdf:about="http://www.opengis.net/ont/geosparql#rcc8tpp">
        <rdfs:subPropertyOf rdf:resource="https://w3id.org/isoiec5087/-1/v1/SpatialLocOntologyProperty"/>
    </owl:ObjectProperty>
    


    <!-- http://www.opengis.net/ont/geosparql#rcc8tppi -->

    <owl:ObjectProperty rdf:about="http://www.opengis.net/ont/geosparql#rcc8tppi">
        <rdfs:subPropertyOf rdf:resource="https://w3id.org/isoiec5087/-1/v1/SpatialLocOntologyProperty"/>
    </owl:ObjectProperty>
    


    <!-- http://www.opengis.net/ont/geosparql#sfContains -->

    <owl:ObjectProperty rdf:about="http://www.opengis.net/ont/geosparql#sfContains">
        <rdfs:subPropertyOf rdf:resource="https://w3id.org/isoiec5087/-1/v1/SpatialLocOntologyProperty"/>
        <owl:inverseOf rdf:resource="http://www.opengis.net/ont/geosparql#sfWithin"/>
    </owl:ObjectProperty>
    


    <!-- http://www.opengis.net/ont/geosparql#sfCrosses -->

    <owl:ObjectProperty rdf:about="http://www.opengis.net/ont/geosparql#sfCrosses">
        <rdfs:subPropertyOf rdf:resource="https://w3id.org/isoiec5087/-1/v1/SpatialLocOntologyProperty"/>
    </owl:ObjectProperty>
    


    <!-- http://www.opengis.net/ont/geosparql#sfDisjoint -->

    <owl:ObjectProperty rdf:about="http://www.opengis.net/ont/geosparql#sfDisjoint">
        <rdfs:subPropertyOf rdf:resource="https://w3id.org/isoiec5087/-1/v1/SpatialLocOntologyProperty"/>
    </owl:ObjectProperty>
    


    <!-- http://www.opengis.net/ont/geosparql#sfEquals -->

    <owl:ObjectProperty rdf:about="http://www.opengis.net/ont/geosparql#sfEquals">
        <rdfs:subPropertyOf rdf:resource="https://w3id.org/isoiec5087/-1/v1/SpatialLocOntologyProperty"/>
    </owl:ObjectProperty>
    


    <!-- http://www.opengis.net/ont/geosparql#sfIntersects -->

    <owl:ObjectProperty rdf:about="http://www.opengis.net/ont/geosparql#sfIntersects">
        <rdfs:subPropertyOf rdf:resource="https://w3id.org/isoiec5087/-1/v1/SpatialLocOntologyProperty"/>
    </owl:ObjectProperty>
    


    <!-- http://www.opengis.net/ont/geosparql#sfOverlaps -->

    <owl:ObjectProperty rdf:about="http://www.opengis.net/ont/geosparql#sfOverlaps">
        <rdfs:subPropertyOf rdf:resource="https://w3id.org/isoiec5087/-1/v1/SpatialLocOntologyProperty"/>
    </owl:ObjectProperty>
    


    <!-- http://www.opengis.net/ont/geosparql#sfTouches -->

    <owl:ObjectProperty rdf:about="http://www.opengis.net/ont/geosparql#sfTouches">
        <rdfs:subPropertyOf rdf:resource="https://w3id.org/isoiec5087/-1/v1/SpatialLocOntologyProperty"/>
    </owl:ObjectProperty>
    


    <!-- http://www.opengis.net/ont/geosparql#sfWithin -->

    <owl:ObjectProperty rdf:about="http://www.opengis.net/ont/geosparql#sfWithin">
        <rdfs:subPropertyOf rdf:resource="https://w3id.org/isoiec5087/-1/v1/SpatialLocOntologyProperty"/>
    </owl:ObjectProperty>
    


    <!-- http://www.w3.org/2004/02/skos/core#hasTopConcept -->

    <owl:ObjectProperty rdf:about="http://www.w3.org/2004/02/skos/core#hasTopConcept">
        <rdfs:subPropertyOf rdf:resource="https://w3id.org/isoiec5087/-1/v1/SpatialLocOntologyProperty"/>
    </owl:ObjectProperty>
    


    <!-- http://www.w3.org/2004/02/skos/core#inScheme -->

    <owl:ObjectProperty rdf:about="http://www.w3.org/2004/02/skos/core#inScheme">
        <rdfs:subPropertyOf rdf:resource="https://w3id.org/isoiec5087/-1/v1/SpatialLocOntologyProperty"/>
    </owl:ObjectProperty>
    


    <!-- http://www.w3.org/2004/02/skos/core#member -->

    <owl:ObjectProperty rdf:about="http://www.w3.org/2004/02/skos/core#member">
        <rdfs:subPropertyOf rdf:resource="https://w3id.org/isoiec5087/-1/v1/SpatialLocOntologyProperty"/>
    </owl:ObjectProperty>
    


    <!-- http://www.w3.org/2004/02/skos/core#memberList -->

    <owl:ObjectProperty rdf:about="http://www.w3.org/2004/02/skos/core#memberList">
        <rdfs:subPropertyOf rdf:resource="https://w3id.org/isoiec5087/-1/v1/SpatialLocOntologyProperty"/>
    </owl:ObjectProperty>
    


    <!-- http://www.w3.org/2004/02/skos/core#semanticRelation -->

    <owl:ObjectProperty rdf:about="http://www.w3.org/2004/02/skos/core#semanticRelation">
        <rdfs:subPropertyOf rdf:resource="https://w3id.org/isoiec5087/-1/v1/SpatialLocOntologyProperty"/>
    </owl:ObjectProperty>
    


    <!-- https://w3id.org/isoiec5087/-1/v1/properPartOf -->

    <owl:ObjectProperty rdf:about="https://w3id.org/isoiec5087/-1/v1/properPartOf"/>
    


    <!-- https://w3id.org/isoiec5087/-1/v1/SpatialLocOntologyProperty -->

    <owl:ObjectProperty rdf:about="https://w3id.org/isoiec5087/-1/v1/SpatialLocOntologyProperty">
        <rdfs:comment>Created for organizational purposes, to identify the object properties imported by geoSPARQL.</rdfs:comment>
    </owl:ObjectProperty>
    


    <!-- https://w3id.org/isoiec5087/-1/v1/associatedLocation -->

    <owl:ObjectProperty rdf:about="https://w3id.org/isoiec5087/-1/v1/associatedLocation">
        <rdfs:subPropertyOf rdf:resource="https://w3id.org/isoiec5087/-1/v1/SpatialLocOntologyProperty"/>
        <rdfs:range rdf:resource="http://www.opengis.net/ont/geosparql#SpatialObject"/>
        <rdfs:comment>Describes an approximate location of some object (spatial or non-spatial). For example, a Building has an actual location (represented by it&apos;s footprint or 3d massing), but it may also have an associated location(s) of some specific point coordinate. Recurring events may not have an actual location, but may be associated with some location (at which their occurrences are likely to occur).</rdfs:comment>
    </owl:ObjectProperty>
    


    <!-- https://w3id.org/isoiec5087/-1/v1/hasLocation -->

    <owl:ObjectProperty rdf:about="https://w3id.org/isoiec5087/-1/v1/hasLocation">
        <rdfs:subPropertyOf rdf:resource="https://w3id.org/isoiec5087/-1/v1/SpatialLocOntologyProperty"/>
        <rdfs:comment>A property intended to relate non-spatial objects (e.g. activities) to a location(s) in space.</rdfs:comment>
    </owl:ObjectProperty>
    


    <!-- https://w3id.org/isoiec5087/-1/v1/nonTangentialProperPart -->

    <owl:ObjectProperty rdf:about="https://w3id.org/isoiec5087/-1/v1/nonTangentialProperPart">
        <rdfs:subPropertyOf rdf:resource="http://www.opengis.net/ont/geosparql#rcc8ntpp"/>
        <rdfs:subPropertyOf rdf:resource="https://w3id.org/isoiec5087/-1/v1/properPartOf"/>
    </owl:ObjectProperty>
    


    <!-- https://w3id.org/isoiec5087/-1/v1/tangentialProperPart -->

    <owl:ObjectProperty rdf:about="https://w3id.org/isoiec5087/-1/v1/tangentialProperPart">
        <rdfs:subPropertyOf rdf:resource="http://www.opengis.net/ont/geosparql#rcc8tpp"/>
        <rdfs:subPropertyOf rdf:resource="https://w3id.org/isoiec5087/-1/v1/properPartOf"/>
    </owl:ObjectProperty>
    


    <!-- 
    ///////////////////////////////////////////////////////////////////////////////////////
    //
    // Data properties
    //
    ///////////////////////////////////////////////////////////////////////////////////////
     -->

    


    <!-- http://www.opengis.net/ont/geosparql#asGML -->

    <owl:DatatypeProperty rdf:about="http://www.opengis.net/ont/geosparql#asGML">
        <rdfs:subPropertyOf rdf:resource="https://w3id.org/isoiec5087/-1/v1/SpatialLocOntologyDataProperty"/>
    </owl:DatatypeProperty>
    


    <!-- http://www.opengis.net/ont/geosparql#asWKT -->

    <owl:DatatypeProperty rdf:about="http://www.opengis.net/ont/geosparql#asWKT">
        <rdfs:subPropertyOf rdf:resource="https://w3id.org/isoiec5087/-1/v1/SpatialLocOntologyDataProperty"/>
    </owl:DatatypeProperty>
    


    <!-- http://www.opengis.net/ont/geosparql#coordinateDimension -->

    <owl:DatatypeProperty rdf:about="http://www.opengis.net/ont/geosparql#coordinateDimension">
        <rdfs:subPropertyOf rdf:resource="https://w3id.org/isoiec5087/-1/v1/SpatialLocOntologyDataProperty"/>
    </owl:DatatypeProperty>
    


    <!-- http://www.opengis.net/ont/geosparql#dimension -->

    <owl:DatatypeProperty rdf:about="http://www.opengis.net/ont/geosparql#dimension">
        <rdfs:subPropertyOf rdf:resource="https://w3id.org/isoiec5087/-1/v1/SpatialLocOntologyDataProperty"/>
    </owl:DatatypeProperty>
    


    <!-- http://www.opengis.net/ont/geosparql#hasSerialization -->

    <owl:DatatypeProperty rdf:about="http://www.opengis.net/ont/geosparql#hasSerialization">
        <rdfs:subPropertyOf rdf:resource="https://w3id.org/isoiec5087/-1/v1/hasSerialization"/>
    </owl:DatatypeProperty>
    


    <!-- http://www.opengis.net/ont/geosparql#isEmpty -->

    <owl:DatatypeProperty rdf:about="http://www.opengis.net/ont/geosparql#isEmpty">
        <rdfs:subPropertyOf rdf:resource="https://w3id.org/isoiec5087/-1/v1/SpatialLocOntologyDataProperty"/>
    </owl:DatatypeProperty>
    


    <!-- http://www.opengis.net/ont/geosparql#isSimple -->

    <owl:DatatypeProperty rdf:about="http://www.opengis.net/ont/geosparql#isSimple">
        <rdfs:subPropertyOf rdf:resource="https://w3id.org/isoiec5087/-1/v1/SpatialLocOntologyDataProperty"/>
    </owl:DatatypeProperty>
    


    <!-- http://www.opengis.net/ont/geosparql#spatialDimension -->

    <owl:DatatypeProperty rdf:about="http://www.opengis.net/ont/geosparql#spatialDimension">
        <rdfs:subPropertyOf rdf:resource="https://w3id.org/isoiec5087/-1/v1/SpatialLocOntologyDataProperty"/>
    </owl:DatatypeProperty>
    


    <!-- http://www.w3.org/2004/02/skos/core#notation -->

    <owl:DatatypeProperty rdf:about="http://www.w3.org/2004/02/skos/core#notation">
        <rdfs:subPropertyOf rdf:resource="https://w3id.org/isoiec5087/-1/v1/SpatialLocOntologyDataProperty"/>
    </owl:DatatypeProperty>
    


    <!-- https://w3id.org/isoiec5087/-1/v1/SpatialLocOntologyDataProperty -->

    <owl:DatatypeProperty rdf:about="https://w3id.org/isoiec5087/-1/v1/SpatialLocOntologyDataProperty">
        <rdfs:comment>Created for organizational purposes, to identify data properties imported from geoSPARQL.</rdfs:comment>
    </owl:DatatypeProperty>
    


    <!-- https://w3id.org/isoiec5087/-1/v1/as_nDLatLon -->

    <owl:DatatypeProperty rdf:about="https://w3id.org/isoiec5087/-1/v1/as_nDLatLon">
        <rdfs:subPropertyOf rdf:resource="https://w3id.org/isoiec5087/-1/v1/hasSerialization"/>
        <rdfs:domain rdf:resource="http://www.opengis.net/ont/sf#Geometry"/>
        <rdfs:range rdf:resource="http://franz.com/ns/allegrograph/5.0/geo/nd#_lat_la_-9.+1_+9.+1_+1.-4_+1.-1_lon_lo_-1.8+2_+1.8+2_+1.-4"/>
    </owl:DatatypeProperty>
    


    <!-- https://w3id.org/isoiec5087/-1/v1/hasSerialization -->

    <owl:DatatypeProperty rdf:about="https://w3id.org/isoiec5087/-1/v1/hasSerialization">
        <rdfs:subPropertyOf rdf:resource="https://w3id.org/isoiec5087/-1/v1/SpatialLocOntologyDataProperty"/>
    </owl:DatatypeProperty>
    


    <!-- 
    ///////////////////////////////////////////////////////////////////////////////////////
    //
    // Classes
    //
    ///////////////////////////////////////////////////////////////////////////////////////
     -->

    


    <!-- http://www.opengis.net/ont/geosparql#Geometry -->

    <owl:Class rdf:about="http://www.opengis.net/ont/geosparql#Geometry">
        <rdfs:subClassOf rdf:resource="https://w3id.org/isoiec5087/-1/v1/SpatialLocOntologyThing"/>
    </owl:Class>
    


    <!-- http://www.opengis.net/ont/geosparql#SpatialObject -->

    <owl:Class rdf:about="http://www.opengis.net/ont/geosparql#SpatialObject">
        <rdfs:subClassOf rdf:resource="https://w3id.org/isoiec5087/-1/v1/SpatialLocOntologyThing"/>
    </owl:Class>
    


    <!-- http://www.opengis.net/ont/sf#Geometry -->

    <owl:Class rdf:about="http://www.opengis.net/ont/sf#Geometry">
        <rdfs:subClassOf rdf:resource="https://w3id.org/isoiec5087/-1/v1/SpatialLocOntologyThing"/>
    </owl:Class>
    


    <!-- http://www.w3.org/1999/02/22-rdf-syntax-ns#List -->

    <owl:Class rdf:about="http://www.w3.org/1999/02/22-rdf-syntax-ns#List">
        <rdfs:subClassOf rdf:resource="https://w3id.org/isoiec5087/-1/v1/SpatialLocOntologyThing"/>
    </owl:Class>
    


    <!-- http://www.w3.org/2004/02/skos/core#Collection -->

    <owl:Class rdf:about="http://www.w3.org/2004/02/skos/core#Collection">
        <rdfs:subClassOf rdf:resource="https://w3id.org/isoiec5087/-1/v1/SpatialLocOntologyThing"/>
    </owl:Class>
    


    <!-- http://www.w3.org/2004/02/skos/core#Concept -->

    <owl:Class rdf:about="http://www.w3.org/2004/02/skos/core#Concept">
        <rdfs:subClassOf rdf:resource="https://w3id.org/isoiec5087/-1/v1/SpatialLocOntologyThing"/>
    </owl:Class>
    


    <!-- http://www.w3.org/2004/02/skos/core#ConceptScheme -->

    <owl:Class rdf:about="http://www.w3.org/2004/02/skos/core#ConceptScheme">
        <rdfs:subClassOf rdf:resource="https://w3id.org/isoiec5087/-1/v1/SpatialLocOntologyThing"/>
    </owl:Class>
    


    <!-- https://w3id.org/isoiec5087/-1/v1/Location -->

    <owl:Class rdf:about="https://w3id.org/isoiec5087/-1/v1/Location">
        <rdfs:subClassOf rdf:resource="http://www.opengis.net/ont/geosparql#Geometry"/>
    </owl:Class>
    


    <!-- https://w3id.org/isoiec5087/-1/v1/SpatialLocOntologyThing -->

    <owl:Class rdf:about="https://w3id.org/isoiec5087/-1/v1/SpatialLocOntologyThing">
        <rdfs:comment>Created for organizational purposes, to identify the classes imported from geoSPARQL.</rdfs:comment>
    </owl:Class>
    


    <!-- 
    ///////////////////////////////////////////////////////////////////////////////////////
    //
    // Datatypes
    //
    ///////////////////////////////////////////////////////////////////////////////////////
     -->

    


    <!-- http://www.w3.org/2001/XMLSchema#date -->

    <rdfs:Datatype rdf:about="http://www.w3.org/2001/XMLSchema#date"/>
    


    <!-- http://www.w3.org/2001/XMLSchema#dateTimeStamp -->

    <rdf:Description rdf:about="http://www.w3.org/2001/XMLSchema#dateTimeStamp">
        <rdfs:label xml:lang="es">sello de tiempo</rdfs:label>
    </rdf:Description>
    


    <!-- http://www.w3.org/2001/XMLSchema#duration -->

    <rdfs:Datatype rdf:about="http://www.w3.org/2001/XMLSchema#duration"/>
    


    <!-- http://www.w3.org/2001/XMLSchema#gDay -->

    <rdfs:Datatype rdf:about="http://www.w3.org/2001/XMLSchema#gDay"/>
    


    <!-- http://www.w3.org/2001/XMLSchema#gMonth -->

    <rdfs:Datatype rdf:about="http://www.w3.org/2001/XMLSchema#gMonth"/>
    


    <!-- http://www.w3.org/2001/XMLSchema#gYear -->

    <rdfs:Datatype rdf:about="http://www.w3.org/2001/XMLSchema#gYear"/>
    


    <!-- http://www.w3.org/2001/XMLSchema#gYearMonth -->

    <rdfs:Datatype rdf:about="http://www.w3.org/2001/XMLSchema#gYearMonth"/>
    


    <!-- http://www.w3.org/2006/time#generalDay -->

    <rdfs:Datatype rdf:about="http://www.w3.org/2006/time#generalDay">
        <rdfs:comment xml:lang="en">Day of month - formulated as a text string with a pattern constraint to reproduce the same lexical form as gDay, except that values up to 99 are permitted, in order to support calendars with more than 31 days in a month. 
Note that the value-space is not defined, so a generic OWL2 processor cannot compute ordering relationships of values of this type.</rdfs:comment>
        <rdfs:comment xml:lang="es">Día del mes - formulado como una cadena de texto con una restricción patrón para reproducir la misma forma léxica que gDay, excepto que se permiten valores hasta el 99, con el propósito de proporcionar soporte a calendarios con meses con más de 31 días.
            Nótese que el espacio de valores no está definido, por tanto, un procesador genérico de OWL2 no puede computar relaciones de orden de valores de este tipo.</rdfs:comment>
        <rdfs:label xml:lang="es">Día generalizado</rdfs:label>
        <rdfs:label xml:lang="en">Generalized day</rdfs:label>
        <skos:definition xml:lang="en">Day of month - formulated as a text string with a pattern constraint to reproduce the same lexical form as gDay, except that values up to 99 are permitted, in order to support calendars with more than 31 days in a month. 
Note that the value-space is not defined, so a generic OWL2 processor cannot compute ordering relationships of values of this type.</skos:definition>
        <skos:definition xml:lang="en">Day of month - generalization of xsd:gDay, formulated as a text string with a pattern constraint to reproduce the same lexical form as gDay, except that values up to 99 are permitted, in order to support calendars with more than 31 days in a month. Note that the value-space is not defined, so a generic OWL2 processor cannot compute ordering relationships of values of this type. </skos:definition>
        <skos:definition xml:lang="es">Día del mes - formulado como una cadena de texto con una restricción patrón para reproducir la misma forma léxica que gDay, excepto que se permiten valores hasta el 99, con el propósito de proporcionar soporte a calendarios con meses con más de 31 días.
            Nótese que el espacio de valores no está definido, por tanto, un procesador genérico de OWL2 no puede computar relaciones de orden de valores de este tipo.</skos:definition>
    </rdfs:Datatype>
    


    <!-- http://www.w3.org/2006/time#generalMonth -->

    <rdfs:Datatype rdf:about="http://www.w3.org/2006/time#generalMonth">
        <rdfs:comment xml:lang="es">Mes del año - formulado como una cadena de texto con una restricción patrón para reproducir la misma forma léxica que gMonth, excepto que se permiten valores hasta el 20, con el propósito de proporcionar soporte a calendarios con años con más de 12 meses.
            Nótese que el espacio de valores no está definido, por tanto, un procesador genérico de OWL2 no puede computar relaciones de orden de valores de este tipo.</rdfs:comment>
        <rdfs:comment xml:lang="en">Month of year - formulated as a text string with a pattern constraint to reproduce the same lexical form as gMonth, except that values up to 20 are permitted, in order to support calendars with more than 12 months in the year. 
Note that the value-space is not defined, so a generic OWL2 processor cannot compute ordering relationships of values of this type.</rdfs:comment>
        <rdfs:label xml:lang="en">Generalized month</rdfs:label>
        <rdfs:label xml:lang="es">Mes generalizado</rdfs:label>
        <skos:definition xml:lang="es">Mes del año - formulado como una cadena de texto con una restricción patrón para reproducir la misma forma léxica que gMonth, excepto que se permiten valores hasta el 20, con el propósito de proporcionar soporte a calendarios con años con más de 12 meses.
            Nótese que el espacio de valores no está definido, por tanto, un procesador genérico de OWL2 no puede computar relaciones de orden de valores de este tipo.</skos:definition>
        <skos:definition xml:lang="en">Month of year - formulated as a text string with a pattern constraint to reproduce the same lexical form as gMonth, except that values up to 20 are permitted, in order to support calendars with more than 12 months in the year. 
Note that the value-space is not defined, so a generic OWL2 processor cannot compute ordering relationships of values of this type.</skos:definition>
        <skos:definition xml:lang="en">Month of year - generalization of xsd:gMonth, formulated as a text string with a pattern constraint to reproduce the same lexical form as gMonth, except that values up to 20 are permitted, in order to support calendars with more than 12 months in the year. Note that the value-space is not defined, so a generic OWL2 processor cannot compute ordering relationships of values of this type.</skos:definition>
    </rdfs:Datatype>
    


    <!-- http://www.w3.org/2006/time#generalYear -->

    <rdfs:Datatype rdf:about="http://www.w3.org/2006/time#generalYear">
        <rdfs:comment xml:lang="es">Número de año - formulado como una cadena de texto con una restricción patrón para reproducir la misma forma léxica que gYear, aunque no está restringido a valores del calendario gregoriano.
            Nótese que el espacio de valores no está definido, por tanto, un procesador genérico de OWL2 no puede computar relaciones de orden de valores de este tipo.</rdfs:comment>
        <rdfs:comment xml:lang="en">Year number - formulated as a text string with a pattern constraint to reproduce the same lexical form as gYear, but not restricted to values from the Gregorian calendar. 
Note that the value-space is not defined, so a generic OWL2 processor cannot compute ordering relationships of values of this type.</rdfs:comment>
        <rdfs:label xml:lang="es">Año generalizado</rdfs:label>
        <rdfs:label xml:lang="en">Generalized year</rdfs:label>
        <skos:definition xml:lang="es">Número de año - formulado como una cadena de texto con una restricción patrón para reproducir la misma forma léxica que gYear, aunque no está restringido a valores del calendario gregoriano.
            Nótese que el espacio de valores no está definido, por tanto, un procesador genérico de OWL2 no puede computar relaciones de orden de valores de este tipo.</skos:definition>
        <skos:definition xml:lang="en">Year number - formulated as a text string with a pattern constraint to reproduce the same lexical form as gYear, but not restricted to values from the Gregorian calendar. 
Note that the value-space is not defined, so a generic OWL2 processor cannot compute ordering relationships of values of this type.</skos:definition>
    </rdfs:Datatype>
    


    <!-- 
    ///////////////////////////////////////////////////////////////////////////////////////
    //
    // Object Properties
    //
    ///////////////////////////////////////////////////////////////////////////////////////
     -->

    


    <!-- https://w3id.org/isoiec5087/-1/v1/TimeOntologyProperty -->

    <owl:ObjectProperty rdf:about="https://w3id.org/isoiec5087/-1/v1/TimeOntologyProperty">
        <skos:definition>Property added for organizational purposes, to identify properties defined in the Time Ontology.</skos:definition>
    </owl:ObjectProperty>
    


    <!-- http://www.w3.org/2006/time#after -->

    <owl:ObjectProperty rdf:about="http://www.w3.org/2006/time#after">
        <rdfs:subPropertyOf rdf:resource="https://w3id.org/isoiec5087/-1/v1/TimeOntologyProperty"/>
        <owl:inverseOf rdf:resource="time:before"/>
        <rdfs:domain rdf:resource="time:TemporalEntity"/>
        <rdfs:range rdf:resource="time:TemporalEntity"/>
        <rdfs:comment xml:lang="es">Asume una dirección en el tiempo. Si una entidad temporal T1 está después de otra entidad temporal T2, entonces el principio de T1 está después del final de T2.</rdfs:comment>
        <rdfs:comment xml:lang="en">Gives directionality to time. If a temporal entity T1 is after another temporal entity T2, then the beginning of T1 is after the end of T2.</rdfs:comment>
        <rdfs:label xml:lang="en">after</rdfs:label>
        <rdfs:label xml:lang="es">después</rdfs:label>
        <skos:definition xml:lang="es">Asume una dirección en el tiempo. Si una entidad temporal T1 está después de otra entidad temporal T2, entonces el principio de T1 está después del final de T2.</skos:definition>
        <skos:definition xml:lang="en">Gives directionality to time. If a temporal entity T1 is after another temporal entity T2, then the beginning of T1 is after the end of T2.</skos:definition>
    </owl:ObjectProperty>
    


    <!-- http://www.w3.org/2006/time#before -->

    <owl:ObjectProperty rdf:about="http://www.w3.org/2006/time#before">
        <rdfs:subPropertyOf rdf:resource="https://w3id.org/isoiec5087/-1/v1/TimeOntologyProperty"/>
        <rdfs:domain rdf:resource="time:TemporalEntity"/>
        <rdfs:range rdf:resource="time:TemporalEntity"/>
        <rdfs:comment xml:lang="es">Asume una dirección en el tiempo. Si una entidad temporal T1 está antes que otra entidad temporal T2, entonces el final de T1 está antes que el principio de T2. Así, &quot;antes&quot; se puede considerar básica para instantes y derivada para intervalos.</rdfs:comment>
        <rdfs:comment xml:lang="en">Gives directionality to time. If a temporal entity T1 is before another temporal entity T2, then the end of T1 is before the beginning of T2. Thus, &quot;before&quot; can be considered to be basic to instants and derived for intervals.</rdfs:comment>
        <rdfs:label xml:lang="es">antes</rdfs:label>
        <rdfs:label xml:lang="en">before</rdfs:label>
        <skos:definition xml:lang="es">Asume una dirección en el tiempo. Si una entidad temporal T1 está antes que otra entidad temporal T2, entonces el final de T1 está antes que el principio de T2. Así, &quot;antes&quot; se puede considerar básica para instantes y derivada para intervalos.</skos:definition>
        <skos:definition xml:lang="en">Gives directionality to time. If a temporal entity T1 is before another temporal entity T2, then the end of T1 is before the beginning of T2. Thus, &quot;before&quot; can be considered to be basic to instants and derived for intervals.</skos:definition>
    </owl:ObjectProperty>
    


    <!-- http://www.w3.org/2006/time#dayOfWeek -->

    <owl:ObjectProperty rdf:about="http://www.w3.org/2006/time#dayOfWeek">
        <rdfs:subPropertyOf rdf:resource="https://w3id.org/isoiec5087/-1/v1/TimeOntologyProperty"/>
        <rdfs:domain rdf:resource="time:GeneralDateTimeDescription"/>
        <rdfs:range rdf:resource="time:DayOfWeek"/>
        <rdfs:comment>El día de la semana, cuyo valor es un miembro de la clase &apos;día de la semana&apos;.</rdfs:comment>
        <rdfs:comment xml:lang="en">The day of week, whose value is a member of the class time:DayOfWeek</rdfs:comment>
        <rdfs:label xml:lang="en">day of week</rdfs:label>
        <rdfs:label xml:lang="es">día de la semana</rdfs:label>
        <skos:definition xml:lang="es">El día de la semana, cuyo valor es un miembro de la clase &apos;día de la semana&apos;.</skos:definition>
        <skos:definition xml:lang="en">The day of week, whose value is a member of the class time:DayOfWeek</skos:definition>
    </owl:ObjectProperty>
    


    <!-- http://www.w3.org/2006/time#hasBeginning -->

    <owl:ObjectProperty rdf:about="http://www.w3.org/2006/time#hasBeginning">
        <rdfs:subPropertyOf rdf:resource="time:hasTime"/>
        <rdfs:domain rdf:resource="time:TemporalEntity"/>
        <rdfs:range rdf:resource="time:Instant"/>
        <rdfs:comment xml:lang="en">Beginning of a temporal entity</rdfs:comment>
        <rdfs:comment xml:lang="es">Comienzo de una entidad temporal.</rdfs:comment>
        <rdfs:label xml:lang="en">has beginning</rdfs:label>
        <rdfs:label xml:lang="es">tiene principio</rdfs:label>
        <skos:definition xml:lang="en">Beginning of a temporal entity.</skos:definition>
        <skos:definition xml:lang="es">Comienzo de una entidad temporal.</skos:definition>
    </owl:ObjectProperty>
    


    <!-- http://www.w3.org/2006/time#hasDateTimeDescription -->

    <owl:ObjectProperty rdf:about="http://www.w3.org/2006/time#hasDateTimeDescription">
        <rdfs:subPropertyOf rdf:resource="https://w3id.org/isoiec5087/-1/v1/TimeOntologyProperty"/>
        <rdfs:domain rdf:resource="time:DateTimeInterval"/>
        <rdfs:range rdf:resource="time:GeneralDateTimeDescription"/>
        <rdfs:comment xml:lang="es">Valor de intervalo de fecha-hora expresado como un valor estructurado. El principio y el final del intervalo coincide con los límites del elemento más corto en la descripción.</rdfs:comment>
        <rdfs:comment xml:lang="en">Value of DateTimeInterval expressed as a structured value. The beginning and end of the interval coincide with the limits of the shortest element in the description.</rdfs:comment>
        <rdfs:label xml:lang="en">has Date-Time description</rdfs:label>
        <rdfs:label xml:lang="es">tiene descripción fecha-hora</rdfs:label>
        <skos:definition xml:lang="es">Valor de intervalo de fecha-hora expresado como un valor estructurado. El principio y el final del intervalo coincide con los límites del elemento más corto en la descripción.</skos:definition>
        <skos:definition xml:lang="en">Value of DateTimeInterval expressed as a structured value. The beginning and end of the interval coincide with the limits of the shortest element in the description.</skos:definition>
    </owl:ObjectProperty>
    


    <!-- http://www.w3.org/2006/time#hasDuration -->

    <owl:ObjectProperty rdf:about="http://www.w3.org/2006/time#hasDuration">
        <rdfs:subPropertyOf rdf:resource="time:hasTemporalDuration"/>
        <rdfs:range rdf:resource="time:Duration"/>
        <rdfs:comment xml:lang="es">Duración de una entidad temporal, expresada como un valor escalado o un valor nominal.</rdfs:comment>
        <rdfs:comment xml:lang="en">Duration of a temporal entity, expressed as a scaled value or nominal value</rdfs:comment>
        <rdfs:label xml:lang="en">has duration</rdfs:label>
        <rdfs:label xml:lang="es">tiene duración</rdfs:label>
        <skos:definition xml:lang="es">Duración de una entidad temporal, evento o actividad, o cosa, expresada como un valor escalado.</skos:definition>
        <skos:definition xml:lang="en">Duration of a temporal entity, event or activity, or thing, expressed as a scaled value</skos:definition>
    </owl:ObjectProperty>
    


    <!-- http://www.w3.org/2006/time#hasDurationDescription -->

    <owl:ObjectProperty rdf:about="http://www.w3.org/2006/time#hasDurationDescription">
        <rdfs:subPropertyOf rdf:resource="time:hasTemporalDuration"/>
        <rdfs:range rdf:resource="time:GeneralDurationDescription"/>
        <rdfs:comment xml:lang="es">Duración de una entidad temporal, expresada utilizando una descripción estructurada.</rdfs:comment>
        <rdfs:comment xml:lang="en">Duration of a temporal entity, expressed using a structured description</rdfs:comment>
        <rdfs:label xml:lang="en">has duration description</rdfs:label>
        <rdfs:label xml:lang="es">tiene descripción de duración</rdfs:label>
        <skos:definition xml:lang="es">Duración de una entidad temporal, expresada utilizando una descripción estructurada.</skos:definition>
        <skos:definition xml:lang="en">Duration of a temporal entity, expressed using a structured description</skos:definition>
    </owl:ObjectProperty>
    


    <!-- http://www.w3.org/2006/time#hasEnd -->

    <owl:ObjectProperty rdf:about="http://www.w3.org/2006/time#hasEnd">
        <rdfs:subPropertyOf rdf:resource="time:hasTime"/>
        <rdfs:domain rdf:resource="time:TemporalEntity"/>
        <rdfs:range rdf:resource="time:Instant"/>
        <rdfs:comment xml:lang="en">End of a temporal entity.</rdfs:comment>
        <rdfs:comment xml:lang="es">Final de una entidad temporal.</rdfs:comment>
        <rdfs:label xml:lang="en">has end</rdfs:label>
        <rdfs:label xml:lang="es">tiene fin</rdfs:label>
        <skos:definition xml:lang="en">End of a temporal entity.</skos:definition>
        <skos:definition xml:lang="es">Final de una entidad temporal.</skos:definition>
    </owl:ObjectProperty>
    


    <!-- http://www.w3.org/2006/time#hasTRS -->

    <owl:ObjectProperty rdf:about="http://www.w3.org/2006/time#hasTRS">
        <rdfs:subPropertyOf rdf:resource="https://w3id.org/isoiec5087/-1/v1/TimeOntologyProperty"/>
        <rdf:type rdf:resource="owl:FunctionalProperty"/>
        <rdfs:domain>
            <owl:Class>
                <owl:unionOf rdf:parseType="Collection">
                    <rdf:Description rdf:about="http://www.w3.org/2006/time#GeneralDurationDescription"/>
                    <rdf:Description rdf:about="http://www.w3.org/2006/time#TemporalPosition"/>
                </owl:unionOf>
            </owl:Class>
        </rdfs:domain>
        <rdfs:range rdf:resource="time:TRS"/>
        <rdfs:comment xml:lang="es">El sistema de referencia temporal utilizado por una posición temporal o descripción de extensión.</rdfs:comment>
        <rdfs:comment xml:lang="en">The temporal reference system used by a temporal position or extent description. </rdfs:comment>
        <rdfs:label xml:lang="en">Temporal reference system used</rdfs:label>
        <rdfs:label xml:lang="es">sistema de referencia temporal utilizado</rdfs:label>
        <skos:definition xml:lang="es">El sistema de referencia temporal utilizado por una posición temporal o descripción de extensión.</skos:definition>
        <skos:definition xml:lang="en">The temporal reference system used by a temporal position or extent description. </skos:definition>
    </owl:ObjectProperty>
    


    <!-- http://www.w3.org/2006/time#hasTemporalDuration -->

    <owl:ObjectProperty rdf:about="http://www.w3.org/2006/time#hasTemporalDuration">
        <rdfs:subPropertyOf rdf:resource="https://w3id.org/isoiec5087/-1/v1/TimeOntologyProperty"/>
        <rdfs:domain rdf:resource="time:TemporalEntity"/>
        <rdfs:range rdf:resource="time:TemporalDuration"/>
        <rdfs:comment xml:lang="es">Duración de una entidad temporal.</rdfs:comment>
        <rdfs:comment xml:lang="en">Duration of a temporal entity.</rdfs:comment>
        <rdfs:label xml:lang="en">has temporal duration</rdfs:label>
        <rdfs:label xml:lang="es">tiene duración temporal</rdfs:label>
        <skos:definition xml:lang="es">Duración de una entidad temporal.</skos:definition>
        <skos:definition xml:lang="en">Duration of a temporal entity.</skos:definition>
    </owl:ObjectProperty>
    


    <!-- http://www.w3.org/2006/time#hasTime -->

    <owl:ObjectProperty rdf:about="http://www.w3.org/2006/time#hasTime">
        <rdfs:subPropertyOf rdf:resource="https://w3id.org/isoiec5087/-1/v1/TimeOntologyProperty"/>
        <rdfs:range rdf:resource="time:TemporalEntity"/>
        <rdfs:comment xml:lang="es">Proporciona soporte a la asociación de una entidad temporal (instante o intervalo) a cualquier cosa.</rdfs:comment>
        <rdfs:comment xml:lang="en">Supports the association of a temporal entity (instant or interval) to any thing</rdfs:comment>
        <rdfs:label xml:lang="en">has time</rdfs:label>
        <rdfs:label xml:lang="es">tiene tiempo</rdfs:label>
        <skos:definition xml:lang="es">Proporciona soporte a la asociación de una entidad temporal (instante o intervalo) a cualquier cosa.</skos:definition>
        <skos:definition xml:lang="en">Supports the association of a temporal entity (instant or interval) to any thing</skos:definition>
        <skos:editorialNote xml:lang="es">Característica arriesgada -añadida en la revisión del 2017 que no ha sido todavía utilizada de forma amplia.</skos:editorialNote>
        <skos:editorialNote xml:lang="en">Feature at risk - added in 2017 revision, and not yet widely used. </skos:editorialNote>
    </owl:ObjectProperty>
    


    <!-- http://www.w3.org/2006/time#inDateTime -->

    <owl:ObjectProperty rdf:about="http://www.w3.org/2006/time#inDateTime">
        <rdfs:subPropertyOf rdf:resource="time:inTemporalPosition"/>
        <rdfs:domain rdf:resource="time:Instant"/>
        <rdfs:range rdf:resource="time:GeneralDateTimeDescription"/>
        <rdfs:comment xml:lang="es">Posición de un instante, expresada utilizando una descripción estructurada.</rdfs:comment>
        <rdfs:comment xml:lang="en">Position of an instant, expressed using a structured description</rdfs:comment>
        <rdfs:label xml:lang="es">en descripción de fecha-hora</rdfs:label>
        <rdfs:label xml:lang="en">in date-time description</rdfs:label>
        <skos:definition xml:lang="es">Posición de un instante, expresada utilizando una descripción estructurada.</skos:definition>
        <skos:definition xml:lang="en">Position of an instant, expressed using a structured description</skos:definition>
    </owl:ObjectProperty>
    


    <!-- http://www.w3.org/2006/time#inTemporalPosition -->

    <owl:ObjectProperty rdf:about="http://www.w3.org/2006/time#inTemporalPosition">
        <rdfs:subPropertyOf rdf:resource="https://w3id.org/isoiec5087/-1/v1/TimeOntologyProperty"/>
        <rdfs:domain rdf:resource="time:Instant"/>
        <rdfs:range rdf:resource="time:TemporalPosition"/>
        <rdfs:comment xml:lang="es">Posición de un instante de tiempo.</rdfs:comment>
        <rdfs:comment xml:lang="en">Position of a time instant</rdfs:comment>
        <rdfs:label xml:lang="en">Temporal position</rdfs:label>
        <rdfs:label xml:lang="es">posición temporal</rdfs:label>
        <skos:definition xml:lang="es">Posición de un instante de tiempo.</skos:definition>
        <skos:definition xml:lang="en">Position of a time instant</skos:definition>
    </owl:ObjectProperty>
    


    <!-- http://www.w3.org/2006/time#inTimePosition -->

    <owl:ObjectProperty rdf:about="http://www.w3.org/2006/time#inTimePosition">
        <rdfs:subPropertyOf rdf:resource="time:inTemporalPosition"/>
        <rdfs:domain rdf:resource="time:Instant"/>
        <rdfs:range rdf:resource="time:TimePosition"/>
        <rdfs:comment xml:lang="es">Posición de un instante, expresada como una coordenada temporal o un valor nominal.</rdfs:comment>
        <rdfs:comment xml:lang="en">Position of an instant, expressed as a temporal coordinate or nominal value</rdfs:comment>
        <rdfs:label xml:lang="en">Time position</rdfs:label>
        <rdfs:label xml:lang="es">posición de tiempo</rdfs:label>
        <skos:definition xml:lang="es">Posición de un instante, expresada como una coordenada temporal o un valor nominal.</skos:definition>
        <skos:definition xml:lang="en">Position of a time instant expressed as a TimePosition</skos:definition>
    </owl:ObjectProperty>
    


    <!-- http://www.w3.org/2006/time#inside -->

    <owl:ObjectProperty rdf:about="http://www.w3.org/2006/time#inside">
        <rdfs:subPropertyOf rdf:resource="https://w3id.org/isoiec5087/-1/v1/TimeOntologyProperty"/>
        <rdfs:domain rdf:resource="time:Interval"/>
        <rdfs:range rdf:resource="time:Instant"/>
        <rdfs:comment xml:lang="en">An instant that falls inside the interval. It is not intended to include beginnings and ends of intervals.</rdfs:comment>
        <rdfs:comment xml:lang="es">Un instante que cae dentro del intervalo. Se asume que no es ni el principio ni el final de ningún intervalo.</rdfs:comment>
        <rdfs:label xml:lang="en">has time instant inside</rdfs:label>
        <rdfs:label xml:lang="es">tiene instante de tiempo dentro</rdfs:label>
        <skos:definition xml:lang="en">An instant that falls inside the interval. It is not intended to include beginnings and ends of intervals.</skos:definition>
        <skos:definition xml:lang="es">Un instante que cae dentro del intervalo. Se asume que no es ni el principio ni el final de ningún intervalo.</skos:definition>
    </owl:ObjectProperty>
    


    <!-- http://www.w3.org/2006/time#intervalAfter -->

    <owl:ObjectProperty rdf:about="http://www.w3.org/2006/time#intervalAfter">
        <rdfs:subPropertyOf rdf:resource="time:after"/>
        <rdfs:subPropertyOf rdf:resource="time:intervalDisjoint"/>
        <owl:inverseOf rdf:resource="time:intervalBefore"/>
        <rdfs:domain rdf:resource="time:ProperInterval"/>
        <rdfs:range rdf:resource="time:ProperInterval"/>
        <rdfs:comment xml:lang="en">If a proper interval T1 is intervalAfter another proper interval T2, then the beginning of T1 is after the end of T2.</rdfs:comment>
        <rdfs:comment>Si un intervalo propio T1 es posterior a otro intervalo propio T2, entonces el principio de T1 está después que el final de T2.</rdfs:comment>
        <rdfs:label xml:lang="en">interval after</rdfs:label>
        <rdfs:label xml:lang="es">intervalo posterior</rdfs:label>
        <skos:definition xml:lang="en">If a proper interval T1 is intervalAfter another proper interval T2, then the beginning of T1 is after the end of T2.</skos:definition>
        <skos:definition xml:lang="es">Si un intervalo propio T1 es posterior a otro intervalo propio T2, entonces el principio de T1 está después que el final de T2.</skos:definition>
    </owl:ObjectProperty>
    


    <!-- http://www.w3.org/2006/time#intervalBefore -->

    <owl:ObjectProperty rdf:about="http://www.w3.org/2006/time#intervalBefore">
        <rdfs:subPropertyOf rdf:resource="time:before"/>
        <rdfs:subPropertyOf rdf:resource="time:intervalDisjoint"/>
        <rdfs:domain rdf:resource="time:ProperInterval"/>
        <rdfs:range rdf:resource="time:ProperInterval"/>
        <rdfs:comment xml:lang="en">If a proper interval T1 is intervalBefore another proper interval T2, then the end of T1 is before the beginning of T2.</rdfs:comment>
        <rdfs:comment xml:lang="es">Si un intervalo propio T1 está antes que otro intervalo propio T2, entonces el final de T1 está antes que el principio de T2.</rdfs:comment>
        <rdfs:label xml:lang="en">interval before</rdfs:label>
        <rdfs:label xml:lang="es">intervalo anterior</rdfs:label>
        <skos:definition xml:lang="en">If a proper interval T1 is intervalBefore another proper interval T2, then the end of T1 is before the beginning of T2.</skos:definition>
        <skos:definition xml:lang="es">Si un intervalo propio T1 está antes que otro intervalo propio T2, entonces el final de T1 está antes que el principio de T2.</skos:definition>
    </owl:ObjectProperty>
    


    <!-- http://www.w3.org/2006/time#intervalContains -->

    <owl:ObjectProperty rdf:about="http://www.w3.org/2006/time#intervalContains">
        <rdfs:subPropertyOf rdf:resource="https://w3id.org/isoiec5087/-1/v1/TimeOntologyProperty"/>
        <owl:inverseOf rdf:resource="time:intervalDuring"/>
        <rdfs:domain rdf:resource="time:ProperInterval"/>
        <rdfs:range rdf:resource="time:ProperInterval"/>
        <rdfs:comment xml:lang="en">If a proper interval T1 is intervalContains another proper interval T2, then the beginning of T1 is before the beginning of T2, and the end of T1 is after the end of T2.</rdfs:comment>
        <rdfs:comment xml:lang="es">Si un intervalo propio T1 contiene otro intervalo propio T2, entonces el principio de T1 está antes que el principio de T2, y el final de T1 está después del final de T2.</rdfs:comment>
        <rdfs:label xml:lang="en">interval contains</rdfs:label>
        <rdfs:label xml:lang="es">intervalo contiene</rdfs:label>
        <skos:definition xml:lang="en">If a proper interval T1 is intervalContains another proper interval T2, then the beginning of T1 is before the beginning of T2, and the end of T1 is after the end of T2.</skos:definition>
        <skos:definition xml:lang="es">Si un intervalo propio T1 contiene otro intervalo propio T2, entonces el principio de T1 está antes que el principio de T2, y el final de T1 está después del final de T2.</skos:definition>
    </owl:ObjectProperty>
    


    <!-- http://www.w3.org/2006/time#intervalDisjoint -->

    <owl:ObjectProperty rdf:about="http://www.w3.org/2006/time#intervalDisjoint">
        <rdfs:subPropertyOf rdf:resource="https://w3id.org/isoiec5087/-1/v1/TimeOntologyProperty"/>
        <rdfs:domain rdf:resource="time:ProperInterval"/>
        <rdfs:range rdf:resource="time:ProperInterval"/>
        <rdfs:comment xml:lang="en">If a proper interval T1 is intervalDisjoint another proper interval T2, then the beginning of T1 is after the end of T2, or the end of T1 is before the beginning of T2, i.e. the intervals do not overlap in any way, but their ordering relationship is not known.</rdfs:comment>
        <rdfs:comment xml:lang="es">Si un intervalo propio T1 es disjunto con otro intervalo propio T2, entonces el principio de T1 está después del final de T2, o el final de T1 está antes que el principio de T2, es decir, los intervalos no se solapan de ninguna forma, aunque su relación de orden no se conozca.</rdfs:comment>
        <rdfs:label xml:lang="en">interval disjoint</rdfs:label>
        <rdfs:label xml:lang="es">intervalo disjunto</rdfs:label>
        <skos:definition xml:lang="en">If a proper interval T1 is intervalDisjoint another proper interval T2, then the beginning of T1 is after the end of T2, or the end of T1 is before the beginning of T2, i.e. the intervals do not overlap in any way, but their ordering relationship is not known.</skos:definition>
        <skos:definition xml:lang="es">Si un intervalo propio T1 es disjunto con otro intervalo propio T2, entonces el principio de T1 está después del final de T2, o el final de T1 está antes que el principio de T2, es decir, los intervalos no se solapan de ninguna forma, aunque su relación de orden no se conozca.</skos:definition>
        <skos:note xml:lang="es">Esta relación entre intervalos no estaba incluida en las 13 relaciones básicas definidas por Allen (1984), pero está definida en T.3 como la unión de &apos;intervalo anterior&apos; con &apos;intervalo posterior&apos;. Sin embargo, esto está fuera de la expresividad de OWL2, por tanto, está implementado como una propiedad explícita, con &apos;intervalo anterior&apos; e &apos;intervalo posterior&apos; como sub-propiedades.</skos:note>
        <skos:note xml:lang="en">This interval relation is not included in the 13 basic relationships defined in Allen (1984), but is defined in (T.3) as the union of :intervalBefore v :intervalAfter . However, that is outside OWL2 expressivity, so is implemented as an explicit property, with :intervalBefore , :intervalAfter as sub-properties</skos:note>
    </owl:ObjectProperty>
    


    <!-- http://www.w3.org/2006/time#intervalDuring -->

    <owl:ObjectProperty rdf:about="http://www.w3.org/2006/time#intervalDuring">
        <rdfs:subPropertyOf rdf:resource="time:intervalIn"/>
        <rdfs:domain rdf:resource="time:ProperInterval"/>
        <rdfs:range rdf:resource="time:ProperInterval"/>
        <rdfs:comment xml:lang="en">If a proper interval T1 is intervalDuring another proper interval T2, then the beginning of T1 is after the beginning of T2, and the end of T1 is before the end of T2.</rdfs:comment>
        <rdfs:comment xml:lang="es">Si un intervalo propio T1 está durante otro intervalo propio T2, entonces del principio de T1 está después del principio de T2, y el final de T1 está antes que el final de T2.</rdfs:comment>
        <rdfs:label xml:lang="en">interval during</rdfs:label>
        <rdfs:label xml:lang="es">intervalo durante</rdfs:label>
        <skos:definition xml:lang="en">If a proper interval T1 is intervalDuring another proper interval T2, then the beginning of T1 is after the beginning of T2, and the end of T1 is before the end of T2.</skos:definition>
        <skos:definition xml:lang="es">Si un intervalo propio T1 está durante otro intervalo propio T2, entonces del principio de T1 está después del principio de T2, y el final de T1 está antes que el final de T2.</skos:definition>
    </owl:ObjectProperty>
    


    <!-- http://www.w3.org/2006/time#intervalEquals -->

    <owl:ObjectProperty rdf:about="http://www.w3.org/2006/time#intervalEquals">
        <rdfs:subPropertyOf rdf:resource="https://w3id.org/isoiec5087/-1/v1/TimeOntologyProperty"/>
        <rdfs:domain rdf:resource="time:ProperInterval"/>
        <rdfs:range rdf:resource="time:ProperInterval"/>
        <owl:propertyDisjointWith rdf:resource="time:intervalIn"/>
        <rdfs:comment xml:lang="en">If a proper interval T1 is intervalEquals another proper interval T2, then the beginning of T1 is coincident with the beginning of T2, and the end of T1 is coincident with the end of T2.</rdfs:comment>
        <rdfs:comment xml:lang="es">Si un intervalo propio T1 es igual a otro intervalo propio T2, entonces el principio de T1 coincide con el principio de T2, y el final de T1 coincide con el final de T2.</rdfs:comment>
        <rdfs:label xml:lang="en">interval equals</rdfs:label>
        <rdfs:label xml:lang="es">intervalo igual</rdfs:label>
        <skos:definition xml:lang="en">If a proper interval T1 is intervalEquals another proper interval T2, then the beginning of T1 is coincident with the beginning of T2, and the end of T1 is coincident with the end of T2.</skos:definition>
        <skos:definition xml:lang="es">Si un intervalo propio T1 es igual a otro intervalo propio T2, entonces el principio de T1 coincide con el principio de T2, y el final de T1 coincide con el final de T2.</skos:definition>
    </owl:ObjectProperty>
    


    <!-- http://www.w3.org/2006/time#intervalFinishedBy -->

    <owl:ObjectProperty rdf:about="http://www.w3.org/2006/time#intervalFinishedBy">
        <rdfs:subPropertyOf rdf:resource="https://w3id.org/isoiec5087/-1/v1/TimeOntologyProperty"/>
        <owl:inverseOf rdf:resource="time:intervalFinishes"/>
        <rdfs:domain rdf:resource="time:ProperInterval"/>
        <rdfs:range rdf:resource="time:ProperInterval"/>
        <rdfs:comment xml:lang="en">If a proper interval T1 is intervalFinishedBy another proper interval T2, then the beginning of T1 is before the beginning of T2, and the end of T1 is coincident with the end of T2.</rdfs:comment>
        <rdfs:comment xml:lang="es">Si un intervalo propio T1 está terminado por otro intervalo propio T2, entonces el principio de T1 está antes que el principio de T2, y el final de T1 coincide con el final de T2.</rdfs:comment>
        <rdfs:label xml:lang="en">interval finished by</rdfs:label>
        <rdfs:label xml:lang="es">intervalo terminado por</rdfs:label>
        <skos:definition xml:lang="en">If a proper interval T1 is intervalFinishedBy another proper interval T2, then the beginning of T1 is before the beginning of T2, and the end of T1 is coincident with the end of T2.</skos:definition>
        <skos:definition xml:lang="es">Si un intervalo propio T1 está terminado por otro intervalo propio T2, entonces el principio de T1 está antes que el principio de T2, y el final de T1 coincide con el final de T2.</skos:definition>
    </owl:ObjectProperty>
    


    <!-- http://www.w3.org/2006/time#intervalFinishes -->

    <owl:ObjectProperty rdf:about="http://www.w3.org/2006/time#intervalFinishes">
        <rdfs:subPropertyOf rdf:resource="time:intervalIn"/>
        <rdfs:domain rdf:resource="time:ProperInterval"/>
        <rdfs:range rdf:resource="time:ProperInterval"/>
        <rdfs:comment xml:lang="en">If a proper interval T1 is intervalFinishes another proper interval T2, then the beginning of T1 is after the beginning of T2, and the end of T1 is coincident with the end of T2.</rdfs:comment>
        <rdfs:comment xml:lang="es">Si un intervalo propio T1 termina otro intervalo propio T2, entonces del principio de T1 está después del principio de T2, y el final de T1 coincide con el final de T2.</rdfs:comment>
        <rdfs:label xml:lang="en">interval finishes</rdfs:label>
        <rdfs:label xml:lang="es">intervalo termina</rdfs:label>
        <skos:definition xml:lang="en">If a proper interval T1 is intervalFinishes another proper interval T2, then the beginning of T1 is after the beginning of T2, and the end of T1 is coincident with the end of T2.</skos:definition>
        <skos:definition xml:lang="es">Si un intervalo propio T1 termina otro intervalo propio T2, entonces del principio de T1 está después del principio de T2, y el final de T1 coincide con el final de T2.</skos:definition>
    </owl:ObjectProperty>
    


    <!-- http://www.w3.org/2006/time#intervalIn -->

    <owl:ObjectProperty rdf:about="http://www.w3.org/2006/time#intervalIn">
        <rdfs:subPropertyOf rdf:resource="https://w3id.org/isoiec5087/-1/v1/TimeOntologyProperty"/>
        <rdfs:domain rdf:resource="time:ProperInterval"/>
        <rdfs:range rdf:resource="time:ProperInterval"/>
        <rdfs:comment xml:lang="en">If a proper interval T1 is intervalIn another proper interval T2, then the beginning of T1 is after the beginning of T2 or is coincident with the beginning of T2, and the end of T1 is before the end of T2, or is coincident with the end of T2, except that end of T1 may not be coincident with the end of T2 if the beginning of T1 is coincident with the beginning of T2.</rdfs:comment>
        <rdfs:comment xml:lang="es">Si un intervalo propio T1 es un intervalo interior a otro intervalo propio T2, entonces el principio de T1 está después del principio de T2 o coincide con el principio de T2, y el final de T1 está antes que el final de T2, o coincide con el final de T2, excepto que el final de T1 puede no coincidir con el final de T2 si el principio de T1 coincide con el principio de T2.</rdfs:comment>
        <rdfs:label xml:lang="en">interval in</rdfs:label>
        <rdfs:label xml:lang="es">intervalo interior</rdfs:label>
        <skos:definition xml:lang="en">If a proper interval T1 is intervalIn another proper interval T2, then the beginning of T1 is after the beginning of T2 or is coincident with the beginning of T2, and the end of T1 is before the end of T2, or is coincident with the end of T2, except that end of T1 may not be coincident with the end of T2 if the beginning of T1 is coincident with the beginning of T2.</skos:definition>
        <skos:definition xml:lang="es">Si un intervalo propio T1 es un intervalo interior a otro intervalo propio T2, entonces el principio de T1 está después del principio de T2 o coincide con el principio de T2, y el final de T1 está antes que el final de T2, o coincide con el final de T2, excepto que el final de T1 puede no coincidir con el final de T2 si el principio de T1 coincide con el principio de T2.</skos:definition>
        <skos:note xml:lang="es">Esta relación entre intervalos no estaba incluida en las 13 relaciones básicas definidas por Allen (1984), pero se hace referencia a ella como &quot;una relación importante&quot; en Allen y Ferguson (1997). Es la unión disjunta de &apos;intervalo empieza&apos;, &apos;intervalo durante&apos; y con &apos;intervalo termina&apos;. Sin embargo, esto está fuera de la expresividad de OWL2, por tanto, se implementa como una propiedad explícita, con &apos;intervalo empieza&apos;, &apos;intervalo durante&apos; e &apos;intervalo termina&apos; como sub-propiedades.</skos:note>
        <skos:note xml:lang="en">This interval relation is not included in the 13 basic relationships defined in Allen (1984), but is referred to as &apos;an important relationship&apos; in Allen and Ferguson (1997). It is the disjoint union of :intervalStarts v :intervalDuring v :intervalFinishes . However, that is outside OWL2 expressivity, so is implemented as an explicit property, with :intervalStarts , :intervalDuring , :intervalFinishes as sub-properties</skos:note>
    </owl:ObjectProperty>
    


    <!-- http://www.w3.org/2006/time#intervalMeets -->

    <owl:ObjectProperty rdf:about="http://www.w3.org/2006/time#intervalMeets">
        <rdfs:subPropertyOf rdf:resource="https://w3id.org/isoiec5087/-1/v1/TimeOntologyProperty"/>
        <owl:inverseOf rdf:resource="time:intervalMetBy"/>
        <rdfs:domain rdf:resource="time:ProperInterval"/>
        <rdfs:range rdf:resource="time:ProperInterval"/>
        <rdfs:comment xml:lang="en">If a proper interval T1 is intervalMeets another proper interval T2, then the end of T1 is coincident with the beginning of T2.</rdfs:comment>
        <rdfs:comment xml:lang="es">Si un intervalo propio T1 se encuentra con otro intervalo propio T2, entonces el final de T1 coincide con el principio de T2.</rdfs:comment>
        <rdfs:label xml:lang="en">interval meets</rdfs:label>
        <rdfs:label xml:lang="es">intervalo se encuentra</rdfs:label>
        <skos:definition xml:lang="en">If a proper interval T1 is intervalMeets another proper interval T2, then the end of T1 is coincident with the beginning of T2.</skos:definition>
        <skos:definition xml:lang="es">Si un intervalo propio T1 se encuentra con otro intervalo propio T2, entonces el final de T1 coincide con el principio de T2.</skos:definition>
    </owl:ObjectProperty>
    


    <!-- http://www.w3.org/2006/time#intervalMetBy -->

    <owl:ObjectProperty rdf:about="http://www.w3.org/2006/time#intervalMetBy">
        <rdfs:subPropertyOf rdf:resource="https://w3id.org/isoiec5087/-1/v1/TimeOntologyProperty"/>
        <rdfs:domain rdf:resource="time:ProperInterval"/>
        <rdfs:range rdf:resource="time:ProperInterval"/>
        <rdfs:comment xml:lang="en">If a proper interval T1 is intervalMetBy another proper interval T2, then the beginning of T1 is coincident with the end of T2.</rdfs:comment>
        <rdfs:comment xml:lang="es">Si un intervalo propio T1 es &apos;intervalo encontrado por&apos; otro intervalo propio T2, entonces el principio de T1 coincide con el final de T2.</rdfs:comment>
        <rdfs:label xml:lang="en">interval met by</rdfs:label>
        <rdfs:label xml:lang="es">intervalo encontrado por</rdfs:label>
        <skos:definition xml:lang="en">If a proper interval T1 is intervalMetBy another proper interval T2, then the beginning of T1 is coincident with the end of T2.</skos:definition>
        <skos:definition xml:lang="es">Si un intervalo propio T1 es &apos;intervalo encontrado por&apos; otro intervalo propio T2, entonces el principio de T1 coincide con el final de T2.</skos:definition>
    </owl:ObjectProperty>
    


    <!-- http://www.w3.org/2006/time#intervalOverlappedBy -->

    <owl:ObjectProperty rdf:about="http://www.w3.org/2006/time#intervalOverlappedBy">
        <rdfs:subPropertyOf rdf:resource="https://w3id.org/isoiec5087/-1/v1/TimeOntologyProperty"/>
        <owl:inverseOf rdf:resource="time:intervalOverlaps"/>
        <rdfs:domain rdf:resource="time:ProperInterval"/>
        <rdfs:range rdf:resource="time:ProperInterval"/>
        <rdfs:comment xml:lang="en">If a proper interval T1 is intervalOverlappedBy another proper interval T2, then the beginning of T1 is after the beginning of T2, the beginning of T1 is before the end of T2, and the end of T1 is after the end of T2.</rdfs:comment>
        <rdfs:comment xml:lang="es">Si un intervalo propio T1 es &apos;intervalo solapado por&apos; otro intervalo propio T2, entonces el principio de T1 es posterior al principio de T2, y el principio de T1 es anterior al final de T2, y el final de T1 es posterior al final de T2.</rdfs:comment>
        <rdfs:label xml:lang="en">interval overlapped by</rdfs:label>
        <rdfs:label xml:lang="es">intervalo solapado por</rdfs:label>
        <skos:definition xml:lang="en">If a proper interval T1 is intervalOverlappedBy another proper interval T2, then the beginning of T1 is after the beginning of T2, the beginning of T1 is before the end of T2, and the end of T1 is after the end of T2.</skos:definition>
        <skos:definition xml:lang="es">Si un intervalo propio T1 es &apos;intervalo solapado por&apos; otro intervalo propio T2, entonces el principio de T1 es posterior al principio de T2, y el principio de T1 es anterior al final de T2, y el final de T1 es posterior al final de T2.</skos:definition>
    </owl:ObjectProperty>
    


    <!-- http://www.w3.org/2006/time#intervalOverlaps -->

    <owl:ObjectProperty rdf:about="http://www.w3.org/2006/time#intervalOverlaps">
        <rdfs:subPropertyOf rdf:resource="https://w3id.org/isoiec5087/-1/v1/TimeOntologyProperty"/>
        <rdfs:domain rdf:resource="time:ProperInterval"/>
        <rdfs:range rdf:resource="time:ProperInterval"/>
        <rdfs:comment xml:lang="es">Asume una dirección en el tiempo. Si una entidad temporal T1 está después de otra entidad temporal T2, entonces el principio de T1 está después del final de T2.</rdfs:comment>
        <rdfs:comment xml:lang="en">If a proper interval T1 is intervalOverlaps another proper interval T2, then the beginning of T1 is before the beginning of T2, the end of T1 is after the beginning of T2, and the end of T1 is before the end of T2.</rdfs:comment>
        <rdfs:comment xml:lang="es">Si un intervalo propio T1 se solapa con otro intervalo propio T2, entonces el principio de T1 es anterior al principio de T2, el final de T1 es posterior al principio de T2, y el final de T1 es anterior al final de T2.</rdfs:comment>
        <rdfs:label xml:lang="en">interval overlaps</rdfs:label>
        <rdfs:label xml:lang="es">intervalo se solapa</rdfs:label>
        <skos:definition xml:lang="en">If a proper interval T1 is intervalOverlaps another proper interval T2, then the beginning of T1 is before the beginning of T2, the end of T1 is after the beginning of T2, and the end of T1 is before the end of T2.</skos:definition>
        <skos:definition xml:lang="es">Si un intervalo propio T1 se solapa con otro intervalo propio T2, entonces el principio de T1 es anterior al principio de T2, el final de T1 es posterior al principio de T2, y el final de T1 es anterior al final de T2.</skos:definition>
    </owl:ObjectProperty>
    


    <!-- http://www.w3.org/2006/time#intervalStartedBy -->

    <owl:ObjectProperty rdf:about="http://www.w3.org/2006/time#intervalStartedBy">
        <rdfs:subPropertyOf rdf:resource="https://w3id.org/isoiec5087/-1/v1/TimeOntologyProperty"/>
        <owl:inverseOf rdf:resource="time:intervalStarts"/>
        <rdfs:domain rdf:resource="time:ProperInterval"/>
        <rdfs:range rdf:resource="time:ProperInterval"/>
        <rdfs:comment xml:lang="en">If a proper interval T1 is intervalStarted another proper interval T2, then the beginning of T1 is coincident with the beginning of T2, and the end of T1 is after the end of T2.</rdfs:comment>
        <rdfs:comment xml:lang="es">Si un intervalo propio T1 es empezado por otro intervalo propio T2, entonces el principio de T1 coincide con el principio de T2, y el final de T1 es posterior al final de T2.</rdfs:comment>
        <rdfs:label xml:lang="en">interval started by</rdfs:label>
        <skos:definition xml:lang="en">If a proper interval T1 is intervalStarted another proper interval T2, then the beginning of T1 is coincident with the beginning of T2, and the end of T1 is after the end of T2.</skos:definition>
        <skos:definition xml:lang="es">Si un intervalo propio T1 es empezado por otro intervalo propio T2, entonces el principio de T1 coincide con el principio de T2, y el final de T1 es posterior al final de T2.</skos:definition>
    </owl:ObjectProperty>
    


    <!-- http://www.w3.org/2006/time#intervalStarts -->

    <owl:ObjectProperty rdf:about="http://www.w3.org/2006/time#intervalStarts">
        <rdfs:subPropertyOf rdf:resource="time:intervalIn"/>
        <rdfs:domain rdf:resource="time:ProperInterval"/>
        <rdfs:range rdf:resource="time:ProperInterval"/>
        <rdfs:comment xml:lang="en">If a proper interval T1 is intervalStarts another proper interval T2, then the beginning of T1 is coincident with the beginning of T2, and the end of T1 is before the end of T2.</rdfs:comment>
        <rdfs:comment xml:lang="es">Si un intervalo propio T1 empieza otro intervalo propio T2, entonces del principio de T1 con el principio de T2, y el final de T1 es anterior al final de T2.</rdfs:comment>
        <rdfs:label xml:lang="en">interval starts</rdfs:label>
        <rdfs:label xml:lang="es">intervalo empieza</rdfs:label>
        <skos:definition xml:lang="en">If a proper interval T1 is intervalStarts another proper interval T2, then the beginning of T1 is coincident with the beginning of T2, and the end of T1 is before the end of T2.</skos:definition>
        <skos:definition xml:lang="es">Si un intervalo propio T1 empieza otro intervalo propio T2, entonces del principio de T1 con el final de T2, y el final de T1 es anterior al final de T2.</skos:definition>
    </owl:ObjectProperty>
    


    <!-- http://www.w3.org/2006/time#monthOfYear -->

    <owl:ObjectProperty rdf:about="http://www.w3.org/2006/time#monthOfYear">
        <rdfs:subPropertyOf rdf:resource="https://w3id.org/isoiec5087/-1/v1/TimeOntologyProperty"/>
        <rdfs:domain rdf:resource="time:GeneralDateTimeDescription"/>
        <rdfs:range rdf:resource="time:MonthOfYear"/>
        <rdfs:comment xml:lang="es">El mes del año, cuyo valor es un miembro de la clase &apos;mes del año&apos;.</rdfs:comment>
        <rdfs:comment xml:lang="en">The month of the year, whose value is a member of the class time:MonthOfYear</rdfs:comment>
        <rdfs:label xml:lang="es">mes del año</rdfs:label>
        <rdfs:label xml:lang="en">month of year</rdfs:label>
        <skos:definition xml:lang="es">El mes del año, cuyo valor es un miembro de la clase &apos;mes del año&apos;.</skos:definition>
        <skos:definition xml:lang="en">The month of the year, whose value is a member of the class time:MonthOfYear</skos:definition>
        <skos:editorialNote xml:lang="es">Característica arriesgada - añadida en la revisión de 2017, y todavía no ampliamente utilizada.</skos:editorialNote>
        <skos:editorialNote xml:lang="en">Feature at risk - added in 2017 revision, and not yet widely used. </skos:editorialNote>
    </owl:ObjectProperty>
    


    <!-- http://www.w3.org/2006/time#timeZone -->

    <owl:ObjectProperty rdf:about="http://www.w3.org/2006/time#timeZone">
        <rdfs:subPropertyOf rdf:resource="https://w3id.org/isoiec5087/-1/v1/TimeOntologyProperty"/>
        <rdfs:domain rdf:resource="time:GeneralDateTimeDescription"/>
        <rdfs:range rdf:resource="time:TimeZone"/>
        <rdfs:comment xml:lang="en">The time zone for clock elements in the temporal position</rdfs:comment>
        <rdfs:label xml:lang="es">en huso horario</rdfs:label>
        <rdfs:label xml:lang="en">in time zone</rdfs:label>
        <skos:historyNote xml:lang="es">En la versión original de OWL-Time de 2006, el rango de &apos;en huso horario&apos; se definió en un espacio de nombres diferente &quot;http://www.w3.org/2006/timezone#&quot;.
            Un axioma de alineación permite que los datos codificados de acuerdo con la versión anterior sean consistentes con la ontología actualizada.</skos:historyNote>
        <skos:historyNote>In the original 2006 version of OWL-Time, the range of time:timeZone was a TimeZone class in a separate namespace &quot;http://www.w3.org/2006/timezone#&quot;. 
An alignment axiom 
	tzont:TimeZone rdfs:subClassOf time:TimeZone . 
allows data encoded according to the previous version to be consistent with the updated ontology. </skos:historyNote>
        <skos:note>IANA maintains a database of timezones. These are well maintained and generally considered authoritative, but individual items are not available at individual URIs, so cannot be used directly in data expressed using OWL-Time.

DBPedia provides a set of resources corresponding to the IANA timezones, with a URI for each (e.g. http://dbpedia.org/resource/Australia/Eucla). The World Clock service also provides a list of time zones with the description of each available as an individual webpage with a convenient individual URI (e.g. https://www.timeanddate.com/time/zones/acwst). These or other, similar, resources might be used as a value of the time:timeZone property.</skos:note>
        <skos:note xml:lang="es">IANA mantiene una base de datos de husos horarios. Éstas están bien mantenidas y generalmente se consideran autorizadas, pero los ítems individuales no están disponibles en URIs individuales, por tanto, no se pueden utilizar directamente en datos expresados utilizando OWL-Time.
            La BDPedia proporciona un conjunto de recursos correspondientes a los husos horarios de IANA, con una URI para cada uno (por ejemplo, http://dbpedia.org/resource/Australia/Eucla). El Servicio de Reloj Mundial también proporciona una lista de husos horarios con la descripción de cada uno de los disponibles como una página Web individual con una URI adecuada individual (por ejemplo, https://www.timeanddate.com/time/zones/acwst). Éstos, y otros recursos similares, se puden usar como un valor de la propiedad &apos;huso horario&apos;.</skos:note>
    </owl:ObjectProperty>
    


    <!-- http://www.w3.org/2006/time#unitType -->

    <owl:ObjectProperty rdf:about="http://www.w3.org/2006/time#unitType">
        <rdfs:subPropertyOf rdf:resource="https://w3id.org/isoiec5087/-1/v1/TimeOntologyProperty"/>
        <rdfs:domain>
            <owl:Class>
                <owl:unionOf rdf:parseType="Collection">
                    <rdf:Description rdf:about="http://www.w3.org/2006/time#Duration"/>
                    <rdf:Description rdf:about="http://www.w3.org/2006/time#GeneralDateTimeDescription"/>
                </owl:unionOf>
            </owl:Class>
        </rdfs:domain>
        <rdfs:range rdf:resource="time:TemporalUnit"/>
        <rdfs:comment xml:lang="es">La unidad de tiempo que proporciona la precisión de un valor fecha-hora o la escala de una extensión temporal.</rdfs:comment>
        <rdfs:comment xml:lang="en">The temporal unit which provides the precision of a date-time value or scale of a temporal extent</rdfs:comment>
        <rdfs:label xml:lang="en">temporal unit type</rdfs:label>
        <rdfs:label xml:lang="es">tipo de unidad temporal</rdfs:label>
    </owl:ObjectProperty>
    


    <!-- 
    ///////////////////////////////////////////////////////////////////////////////////////
    //
    // Data properties
    //
    ///////////////////////////////////////////////////////////////////////////////////////
     -->

    


    <!-- https://w3id.org/isoiec5087/-1/v1/TimeOntologyDataProperty -->

    <owl:DatatypeProperty rdf:about="https://w3id.org/isoiec5087/-1/v1/TimeOntologyDataProperty">
        <skos:definition>Data property added for organizational purposes, to identify data properties defined in the Time Ontology.</skos:definition>
    </owl:DatatypeProperty>
    


    <!-- http://www.w3.org/2006/time#day -->

    <owl:DatatypeProperty rdf:about="http://www.w3.org/2006/time#day">
        <rdfs:subPropertyOf rdf:resource="https://w3id.org/isoiec5087/-1/v1/TimeOntologyDataProperty"/>
        <rdfs:domain rdf:resource="time:GeneralDateTimeDescription"/>
        <rdfs:comment xml:lang="en">Day position in a calendar-clock system.

The range of this property is not specified, so can be replaced by any specific representation of a calendar day from any calendar. </rdfs:comment>
        <rdfs:comment xml:lang="es">Posición de día en un sistema calendario-reloj.</rdfs:comment>
        <rdfs:label xml:lang="en">day</rdfs:label>
        <rdfs:label xml:lang="es">día</rdfs:label>
        <skos:definition xml:lang="en">Day position in a calendar-clock system.

The range of this property is not specified, so can be replaced by any specific representation of a calendar day from any calendar. </skos:definition>
        <skos:definition xml:lang="es">Posición de día en un sistema calendario-reloj.

El rango de esta propiedad no está especificado, por tanto, se puede reemplazar por una representación específica de un día de calendario de cualquier calendario.</skos:definition>
    </owl:DatatypeProperty>
    


    <!-- http://www.w3.org/2006/time#dayOfYear -->

    <owl:DatatypeProperty rdf:about="http://www.w3.org/2006/time#dayOfYear">
        <rdfs:subPropertyOf rdf:resource="https://w3id.org/isoiec5087/-1/v1/TimeOntologyDataProperty"/>
        <rdfs:domain rdf:resource="time:GeneralDateTimeDescription"/>
        <rdfs:range rdf:resource="xsd:nonNegativeInteger"/>
        <rdfs:comment xml:lang="es">El número de día en el año.</rdfs:comment>
        <rdfs:comment xml:lang="en">The number of the day within the year</rdfs:comment>
        <rdfs:label xml:lang="en">day of year</rdfs:label>
        <rdfs:label xml:lang="es">día del año</rdfs:label>
        <skos:definition xml:lang="es">El número de día en el año.</skos:definition>
        <skos:definition xml:lang="en">The number of the day within the year</skos:definition>
    </owl:DatatypeProperty>
    


    <!-- http://www.w3.org/2006/time#days -->

    <owl:DatatypeProperty rdf:about="http://www.w3.org/2006/time#days">
        <rdfs:subPropertyOf rdf:resource="https://w3id.org/isoiec5087/-1/v1/TimeOntologyDataProperty"/>
        <rdfs:domain rdf:resource="time:GeneralDurationDescription"/>
        <rdfs:range rdf:resource="xsd:decimal"/>
        <rdfs:comment xml:lang="es">Longitud de, o elemento de la longitud de, una extensión temporal expresada en días.</rdfs:comment>
        <rdfs:comment xml:lang="en">length of, or element of the length of, a temporal extent expressed in days</rdfs:comment>
        <rdfs:label xml:lang="en">days duration</rdfs:label>
        <rdfs:label xml:lang="es">duración en días</rdfs:label>
        <skos:definition xml:lang="es">Longitud de, o elemento de la longitud de, una extensión temporal expresada en días.</skos:definition>
        <skos:definition xml:lang="en">length of, or element of the length of, a temporal extent expressed in days</skos:definition>
    </owl:DatatypeProperty>
    


    <!-- http://www.w3.org/2006/time#hasXSDDuration -->

    <owl:DatatypeProperty rdf:about="http://www.w3.org/2006/time#hasXSDDuration">
        <rdfs:subPropertyOf rdf:resource="https://w3id.org/isoiec5087/-1/v1/TimeOntologyDataProperty"/>
        <rdfs:domain rdf:resource="time:TemporalEntity"/>
        <rdfs:range rdf:resource="xsd:duration"/>
        <rdfs:comment xml:lang="es">Extensión de una entidad temporal, expresada utilizando xsd:duration.</rdfs:comment>
        <rdfs:comment xml:lang="en">Extent of a temporal entity, expressed using xsd:duration</rdfs:comment>
        <rdfs:label xml:lang="en">has XSD duration</rdfs:label>
        <rdfs:label xml:lang="es">tiene duración XSD</rdfs:label>
        <skos:definition xml:lang="es">Extensión de una entidad temporal, expresada utilizando xsd:duration.</skos:definition>
        <skos:definition xml:lang="en">Extent of a temporal entity, expressed using xsd:duration</skos:definition>
        <skos:editorialNote xml:lang="es">Característica arriesgada - añadida en la revisión de 2017, y todavía no ampliamente utilizada.</skos:editorialNote>
        <skos:editorialNote xml:lang="en">Feature at risk - added in 2017 revision, and not yet widely used. </skos:editorialNote>
    </owl:DatatypeProperty>
    


    <!-- http://www.w3.org/2006/time#hour -->

    <owl:DatatypeProperty rdf:about="http://www.w3.org/2006/time#hour">
        <rdfs:subPropertyOf rdf:resource="https://w3id.org/isoiec5087/-1/v1/TimeOntologyDataProperty"/>
        <rdfs:domain rdf:resource="time:GeneralDateTimeDescription"/>
        <rdfs:range rdf:resource="xsd:nonNegativeInteger"/>
        <rdfs:comment xml:lang="en">Hour position in a calendar-clock system.</rdfs:comment>
        <rdfs:comment xml:lang="es">Posición de hora en un sistema calendario-reloj.</rdfs:comment>
        <rdfs:label xml:lang="es">hora</rdfs:label>
        <rdfs:label xml:lang="en">hour</rdfs:label>
        <skos:definition xml:lang="en">Hour position in a calendar-clock system.</skos:definition>
        <skos:definition xml:lang="es">Posición de hora en un sistema calendario-reloj.</skos:definition>
    </owl:DatatypeProperty>
    


    <!-- http://www.w3.org/2006/time#hours -->

    <owl:DatatypeProperty rdf:about="http://www.w3.org/2006/time#hours">
        <rdfs:subPropertyOf rdf:resource="https://w3id.org/isoiec5087/-1/v1/TimeOntologyDataProperty"/>
        <rdfs:domain rdf:resource="time:GeneralDurationDescription"/>
        <rdfs:range rdf:resource="xsd:decimal"/>
        <rdfs:comment xml:lang="es">Longitud de, o elemento de la longitud de, una extensión temporal expresada en horas.</rdfs:comment>
        <rdfs:comment xml:lang="en">length of, or element of the length of, a temporal extent expressed in hours</rdfs:comment>
        <rdfs:label xml:lang="es">duración en horas</rdfs:label>
        <rdfs:label xml:lang="en">hours duration</rdfs:label>
        <skos:definition xml:lang="es">Longitud de, o elemento de la longitud de, una extensión temporal expresada en horas.</skos:definition>
        <skos:definition xml:lang="en">length of, or element of the length of, a temporal extent expressed in hours</skos:definition>
    </owl:DatatypeProperty>
    


    <!-- http://www.w3.org/2006/time#inXSDDate -->

    <owl:DatatypeProperty rdf:about="http://www.w3.org/2006/time#inXSDDate">
        <rdfs:subPropertyOf rdf:resource="https://w3id.org/isoiec5087/-1/v1/TimeOntologyDataProperty"/>
        <rdfs:domain rdf:resource="time:Instant"/>
        <rdfs:range rdf:resource="xsd:date"/>
        <rdfs:comment xml:lang="es">Posición de un instante, expresado utilizando xsd:date.</rdfs:comment>
        <rdfs:comment xml:lang="en">Position of an instant, expressed using xsd:date</rdfs:comment>
        <rdfs:label xml:lang="es">en fecha XSD</rdfs:label>
        <rdfs:label xml:lang="en">in XSD date</rdfs:label>
        <skos:definition xml:lang="es">Posición de un instante, expresado utilizando xsd:date.</skos:definition>
        <skos:definition xml:lang="en">Position of an instant, expressed using xsd:date</skos:definition>
    </owl:DatatypeProperty>
    


    <!-- http://www.w3.org/2006/time#inXSDDateTime -->

    <owl:DatatypeProperty rdf:about="http://www.w3.org/2006/time#inXSDDateTime">
        <rdfs:domain rdf:resource="time:Instant"/>
        <rdfs:range rdf:resource="xsd:dateTime"/>
        <rdfs:comment xml:lang="es">Posición de un instante, expresado utilizando xsd:dateTime.</rdfs:comment>
        <rdfs:comment xml:lang="en">Position of an instant, expressed using xsd:dateTime</rdfs:comment>
        <rdfs:label xml:lang="es">en fecha-tiempo XSD</rdfs:label>
        <rdfs:label xml:lang="en">in XSD Date-Time</rdfs:label>
        <owl:deprecated rdf:datatype="xsd:boolean">true</owl:deprecated>
        <skos:definition xml:lang="es">Posición de un instante, expresado utilizando xsd:dateTime.</skos:definition>
        <skos:definition xml:lang="en">Position of an instant, expressed using xsd:dateTime</skos:definition>
        <skos:note xml:lang="es">La propiedad &apos;en fecha-hora XSD&apos; ha sido reemplazada por &apos;en fecha-sello de tiempo XSD&apos; que hace obligatorio el campo &apos;huso horario&apos;.</skos:note>
        <skos:note xml:lang="en">The property :inXSDDateTime is replaced by :inXSDDateTimeStamp which makes the time-zone field mandatory.</skos:note>
    </owl:DatatypeProperty>
    


    <!-- http://www.w3.org/2006/time#inXSDDateTimeStamp -->

    <owl:DatatypeProperty rdf:about="http://www.w3.org/2006/time#inXSDDateTimeStamp">
        <rdfs:subPropertyOf rdf:resource="https://w3id.org/isoiec5087/-1/v1/TimeOntologyDataProperty"/>
        <rdfs:domain rdf:resource="time:Instant"/>
        <rdfs:range rdf:resource="xsd:dateTimeStamp"/>
        <rdfs:comment xml:lang="es">Posición de un instante, expresado utilizando xsd:dateTimeStamp.</rdfs:comment>
        <rdfs:comment xml:lang="en">Position of an instant, expressed using xsd:dateTimeStamp</rdfs:comment>
        <rdfs:label xml:lang="es">en fecha-sello de tiempo XSD</rdfs:label>
        <rdfs:label xml:lang="en">in XSD Date-Time-Stamp</rdfs:label>
        <skos:definition xml:lang="es">Posición de un instante, expresado utilizando xsd:dateTimeStamp.</skos:definition>
        <skos:definition xml:lang="en">Position of an instant, expressed using xsd:dateTimeStamp</skos:definition>
    </owl:DatatypeProperty>
    


    <!-- http://www.w3.org/2006/time#inXSDgYear -->

    <owl:DatatypeProperty rdf:about="http://www.w3.org/2006/time#inXSDgYear">
        <rdfs:subPropertyOf rdf:resource="https://w3id.org/isoiec5087/-1/v1/TimeOntologyDataProperty"/>
        <rdfs:domain rdf:resource="time:Instant"/>
        <rdfs:range rdf:resource="xsd:gYear"/>
        <rdfs:comment xml:lang="es">Posición de un instante, expresado utilizando xsd:gYear.</rdfs:comment>
        <rdfs:comment xml:lang="en">Position of an instant, expressed using xsd:gYear</rdfs:comment>
        <rdfs:label xml:lang="es">en año gregoriano XSD</rdfs:label>
        <rdfs:label xml:lang="en">in XSD g-Year</rdfs:label>
        <skos:definition xml:lang="es">Posición de un instante, expresado utilizando xsd:gYear.</skos:definition>
        <skos:definition xml:lang="en">Position of an instant, expressed using xsd:gYear</skos:definition>
    </owl:DatatypeProperty>
    


    <!-- http://www.w3.org/2006/time#inXSDgYearMonth -->

    <owl:DatatypeProperty rdf:about="http://www.w3.org/2006/time#inXSDgYearMonth">
        <rdfs:subPropertyOf rdf:resource="https://w3id.org/isoiec5087/-1/v1/TimeOntologyDataProperty"/>
        <rdfs:domain rdf:resource="time:Instant"/>
        <rdfs:range rdf:resource="xsd:gYearMonth"/>
        <rdfs:comment xml:lang="es">Posición de un instante, expresado utilizando xsd:gYearMonth.</rdfs:comment>
        <rdfs:comment xml:lang="en">Position of an instant, expressed using xsd:gYearMonth</rdfs:comment>
        <rdfs:label xml:lang="es">en año-mes gregoriano XSD</rdfs:label>
        <rdfs:label xml:lang="en">in XSD g-YearMonth</rdfs:label>
        <skos:definition xml:lang="es">Posición de un instante, expresado utilizando xsd:gYearMonth.</skos:definition>
        <skos:definition xml:lang="en">Position of an instant, expressed using xsd:gYearMonth</skos:definition>
    </owl:DatatypeProperty>
    


    <!-- http://www.w3.org/2006/time#minute -->

    <owl:DatatypeProperty rdf:about="http://www.w3.org/2006/time#minute">
        <rdfs:subPropertyOf rdf:resource="https://w3id.org/isoiec5087/-1/v1/TimeOntologyDataProperty"/>
        <rdfs:domain rdf:resource="time:GeneralDateTimeDescription"/>
        <rdfs:range rdf:resource="xsd:nonNegativeInteger"/>
        <rdfs:comment xml:lang="en">Minute position in a calendar-clock system.</rdfs:comment>
        <rdfs:comment xml:lang="es">Posición de minuto en un sistema calendario-reloj.</rdfs:comment>
        <rdfs:label xml:lang="en">minute</rdfs:label>
        <rdfs:label xml:lang="es">minuto</rdfs:label>
        <skos:definition xml:lang="en">Minute position in a calendar-clock system.</skos:definition>
        <skos:definition xml:lang="es">Posición de minuto en un sistema calendario-reloj.</skos:definition>
    </owl:DatatypeProperty>
    


    <!-- http://www.w3.org/2006/time#minutes -->

    <owl:DatatypeProperty rdf:about="http://www.w3.org/2006/time#minutes">
        <rdfs:subPropertyOf rdf:resource="https://w3id.org/isoiec5087/-1/v1/TimeOntologyDataProperty"/>
        <rdfs:domain rdf:resource="time:GeneralDurationDescription"/>
        <rdfs:range rdf:resource="xsd:decimal"/>
        <rdfs:comment xml:lang="es">Longitud de, o elemento de la longitud de, una extensión temporal expresada en minutos.</rdfs:comment>
        <rdfs:comment xml:lang="en">length, or element of, a temporal extent expressed in minutes</rdfs:comment>
        <rdfs:label xml:lang="en">minutes</rdfs:label>
        <rdfs:label xml:lang="es">minutos</rdfs:label>
        <skos:definition xml:lang="es">Longitud de, o elemento de la longitud de, una extensión temporal expresada en minutos.</skos:definition>
        <skos:definition xml:lang="en">length, or element of, a temporal extent expressed in minutes</skos:definition>
    </owl:DatatypeProperty>
    


    <!-- http://www.w3.org/2006/time#month -->

    <owl:DatatypeProperty rdf:about="http://www.w3.org/2006/time#month">
        <rdfs:subPropertyOf rdf:resource="https://w3id.org/isoiec5087/-1/v1/TimeOntologyDataProperty"/>
        <rdfs:domain rdf:resource="time:GeneralDateTimeDescription"/>
        <rdfs:comment xml:lang="en">Month position in a calendar-clock system.

The range of this property is not specified, so can be replaced by any specific representation of a calendar month from any calendar. </rdfs:comment>
        <rdfs:comment xml:lang="es">Posición de mes en un sistema calendario-reloj.
    El rango de esta propiedad no está especificado, por tanto, se puede reemplazar por cualquier representación específica de un mes de calendario de un calendario cualquiera.</rdfs:comment>
        <rdfs:label xml:lang="es">mes</rdfs:label>
        <rdfs:label xml:lang="en">month</rdfs:label>
        <skos:definition xml:lang="en">Month position in a calendar-clock system.

The range of this property is not specified, so can be replaced by any specific representation of a calendar month from any calendar. </skos:definition>
        <skos:definition xml:lang="es">Posición de mes en un sistema calendario-reloj.
            El rango de esta propiedad no está especificado, por tanto, se puede reemplazar por cualquier representación específica de un mes de calendario de un calendario cualquiera.</skos:definition>
    </owl:DatatypeProperty>
    


    <!-- http://www.w3.org/2006/time#months -->

    <owl:DatatypeProperty rdf:about="http://www.w3.org/2006/time#months">
        <rdfs:subPropertyOf rdf:resource="https://w3id.org/isoiec5087/-1/v1/TimeOntologyDataProperty"/>
        <rdfs:domain rdf:resource="time:GeneralDurationDescription"/>
        <rdfs:range rdf:resource="xsd:decimal"/>
        <rdfs:comment xml:lang="es">Longitud de, o elemento de la longitud de, una extensión temporal expresada en meses.</rdfs:comment>
        <rdfs:comment xml:lang="en">length of, or element of the length of, a temporal extent expressed in months</rdfs:comment>
        <rdfs:label xml:lang="es">duración en meses</rdfs:label>
        <rdfs:label xml:lang="en">months duration</rdfs:label>
        <skos:definition xml:lang="es">Longitud de, o elemento de la longitud de, una extensión temporal expresada en meses.</skos:definition>
        <skos:definition xml:lang="en">length of, or element of the length of, a temporal extent expressed in months</skos:definition>
    </owl:DatatypeProperty>
    


    <!-- http://www.w3.org/2006/time#nominalPosition -->

    <owl:DatatypeProperty rdf:about="http://www.w3.org/2006/time#nominalPosition">
        <rdfs:subPropertyOf rdf:resource="https://w3id.org/isoiec5087/-1/v1/TimeOntologyDataProperty"/>
        <rdfs:domain rdf:resource="time:TimePosition"/>
        <rdfs:range rdf:resource="xsd:string"/>
        <rdfs:comment xml:lang="es">El valor (nominal) que indica posición temporal en un sistema de referencia ordinal.</rdfs:comment>
        <rdfs:comment xml:lang="en">The (nominal) value indicating temporal position in an ordinal reference system </rdfs:comment>
        <rdfs:label xml:lang="en">Name of temporal position</rdfs:label>
        <rdfs:label xml:lang="es">nombre de posición temporal</rdfs:label>
        <skos:definition xml:lang="es">El valor (nominal) que indica posición temporal en un sistema de referencia ordinal.</skos:definition>
        <skos:definition xml:lang="en">The (nominal) value indicating temporal position in an ordinal reference system </skos:definition>
    </owl:DatatypeProperty>
    


    <!-- http://www.w3.org/2006/time#numericDuration -->

    <owl:DatatypeProperty rdf:about="http://www.w3.org/2006/time#numericDuration">
        <rdfs:subPropertyOf rdf:resource="https://w3id.org/isoiec5087/-1/v1/TimeOntologyDataProperty"/>
        <rdfs:domain rdf:resource="time:Duration"/>
        <rdfs:range rdf:resource="xsd:decimal"/>
        <rdfs:comment xml:lang="es">Valor de una extensión temporal expresada como un número decimal escalado por una unidad de tiempo.</rdfs:comment>
        <rdfs:comment xml:lang="en">Value of a temporal extent expressed as a decimal number scaled by a temporal unit</rdfs:comment>
        <rdfs:label xml:lang="en">Numeric value of temporal duration</rdfs:label>
        <rdfs:label xml:lang="es">valor numérico de duración temporal</rdfs:label>
        <skos:definition xml:lang="es">Valor de una extensión temporal expresada como un número decimal escalado por una unidad de tiempo.</skos:definition>
        <skos:definition xml:lang="en">Value of a temporal extent expressed as a decimal number scaled by a temporal unit</skos:definition>
    </owl:DatatypeProperty>
    


    <!-- http://www.w3.org/2006/time#numericPosition -->

    <owl:DatatypeProperty rdf:about="http://www.w3.org/2006/time#numericPosition">
        <rdfs:subPropertyOf rdf:resource="https://w3id.org/isoiec5087/-1/v1/TimeOntologyDataProperty"/>
        <rdfs:domain rdf:resource="time:TimePosition"/>
        <rdfs:range rdf:resource="xsd:decimal"/>
        <rdfs:comment xml:lang="es">El valor (numérico) que indica posición temporal en un sistema de referencia ordinal.</rdfs:comment>
        <rdfs:comment xml:lang="en">The (numeric) value indicating position within a temporal coordinate system </rdfs:comment>
        <rdfs:label xml:lang="en">Numeric value of temporal position</rdfs:label>
        <rdfs:label xml:lang="es">valor numérico de posición temporal</rdfs:label>
        <skos:definition xml:lang="es">El valor (numérico) que indica posición temporal en un sistema de referencia ordinal.</skos:definition>
        <skos:definition xml:lang="en">The (numeric) value indicating position within a temporal coordinate system </skos:definition>
    </owl:DatatypeProperty>
    


    <!-- http://www.w3.org/2006/time#second -->

    <owl:DatatypeProperty rdf:about="http://www.w3.org/2006/time#second">
        <rdfs:subPropertyOf rdf:resource="https://w3id.org/isoiec5087/-1/v1/TimeOntologyDataProperty"/>
        <rdfs:domain rdf:resource="time:GeneralDateTimeDescription"/>
        <rdfs:range rdf:resource="xsd:decimal"/>
        <rdfs:comment xml:lang="es">Posición de segundo en un sistema calendario-reloj.</rdfs:comment>
        <rdfs:comment xml:lang="en">Second position in a calendar-clock system.</rdfs:comment>
        <rdfs:label xml:lang="en">second</rdfs:label>
        <rdfs:label xml:lang="es">segundo</rdfs:label>
    </owl:DatatypeProperty>
    


    <!-- http://www.w3.org/2006/time#seconds -->

    <owl:DatatypeProperty rdf:about="http://www.w3.org/2006/time#seconds">
        <rdfs:subPropertyOf rdf:resource="https://w3id.org/isoiec5087/-1/v1/TimeOntologyDataProperty"/>
        <rdfs:domain rdf:resource="time:GeneralDurationDescription"/>
        <rdfs:range rdf:resource="xsd:decimal"/>
        <rdfs:comment xml:lang="es">Longitud de, o elemento de la longitud de, una extensión temporal expresada en segundos.</rdfs:comment>
        <rdfs:comment xml:lang="en">length of, or element of the length of, a temporal extent expressed in seconds</rdfs:comment>
        <rdfs:label xml:lang="es">duración en segundos</rdfs:label>
        <rdfs:label xml:lang="en">seconds duration</rdfs:label>
        <rdfs:seeAlso rdf:resource="http://www.bipm.org/en/publications/si-brochure/second.html"/>
    </owl:DatatypeProperty>
    


    <!-- http://www.w3.org/2006/time#week -->

    <owl:DatatypeProperty rdf:about="http://www.w3.org/2006/time#week">
        <rdfs:subPropertyOf rdf:resource="https://w3id.org/isoiec5087/-1/v1/TimeOntologyDataProperty"/>
        <rdfs:domain rdf:resource="time:GeneralDateTimeDescription"/>
        <rdfs:range rdf:resource="xsd:nonNegativeInteger"/>
        <rdfs:comment xml:lang="es">Número de semana en el año.</rdfs:comment>
        <rdfs:comment xml:lang="en">Week number within the year.</rdfs:comment>
        <rdfs:label xml:lang="es">semana</rdfs:label>
        <rdfs:label xml:lang="en">week</rdfs:label>
        <skos:note xml:lang="en">Weeks are numbered differently depending on the calendar in use and the local language or cultural conventions (locale). ISO-8601 specifies that the first week of the year includes at least four days, and that Monday is the first day of the week. In that system, week 1 is the week that contains the first Thursday in the year.</skos:note>
        <skos:scopeNote xml:lang="es">Las semanas están numeradas de forma diferente dependiendo del calendario en uso y de las convenciones lingüísticas y culturales locales (locale en inglés). El ISO-8601 especifica que la primera semana del año incluye al menos cuatro días, y que el lunes es el primer día de la semana. En ese sistema, la semana 1 es la semana que contiene el primer jueves del año.</skos:scopeNote>
    </owl:DatatypeProperty>
    


    <!-- http://www.w3.org/2006/time#weeks -->

    <owl:DatatypeProperty rdf:about="http://www.w3.org/2006/time#weeks">
        <rdfs:subPropertyOf rdf:resource="https://w3id.org/isoiec5087/-1/v1/TimeOntologyDataProperty"/>
        <rdfs:domain rdf:resource="time:GeneralDurationDescription"/>
        <rdfs:range rdf:resource="xsd:decimal"/>
        <rdfs:comment xml:lang="es">Longitud de, o elemento de la longitud de, una extensión temporal expresada en semanas.</rdfs:comment>
        <rdfs:comment xml:lang="en">length of, or element of the length of, a temporal extent expressed in weeks</rdfs:comment>
        <rdfs:label xml:lang="es">duración en semanas</rdfs:label>
        <rdfs:label xml:lang="en">weeks duration</rdfs:label>
    </owl:DatatypeProperty>
    


    <!-- http://www.w3.org/2006/time#xsdDateTime -->

    <owl:DatatypeProperty rdf:about="http://www.w3.org/2006/time#xsdDateTime">
        <rdfs:domain rdf:resource="time:DateTimeInterval"/>
        <rdfs:range rdf:resource="xsd:dateTime"/>
        <rdfs:comment xml:lang="es">Valor de &apos;intervalo de fecha-hora&apos; expresado como un valor compacto.</rdfs:comment>
        <rdfs:comment xml:lang="en">Value of DateTimeInterval expressed as a compact value.</rdfs:comment>
        <rdfs:label xml:lang="en">has XSD date-time</rdfs:label>
        <rdfs:label xml:lang="es">tiene fecha-hora XSD</rdfs:label>
        <owl:deprecated rdf:datatype="xsd:boolean">true</owl:deprecated>
        <skos:note xml:lang="en">Using xsd:dateTime in this place means that the duration of the interval is implicit: it corresponds to the length of the smallest non-zero element of the date-time literal. However, this rule cannot be used for intervals whose duration is more than one rank smaller than the starting time - e.g. the first minute or second of a day, the first hour of a month, or the first day of a year. In these cases the desired interval cannot be distinguished from the interval corresponding to the next rank up. Because of this essential ambiguity, use of this property is not recommended and it is deprecated.</skos:note>
        <skos:note>Utilizando xsd:dateTime en este lugar significa que la duración del intervalo está implícita: se corresponde con la longitud del elemento más pequeño distinto de cero del literal fecha-hora. Sin embargo, esta regla no se puede utilizar para intervalos cuya duración es mayor que un rango más pequeño que el tiempo de comienzo - p.ej. el primer minuto o segundo del día, la primera hora del mes, o el primer día del año. En estos casos el intervalo deseado no se puede distinguir del intervalo correspondiente al próximo rango más alto. Debido a esta ambigüedad esencial, no se recomienda el uso de esta propiedad y está desaprobada.</skos:note>
    </owl:DatatypeProperty>
    


    <!-- http://www.w3.org/2006/time#year -->

    <owl:DatatypeProperty rdf:about="http://www.w3.org/2006/time#year">
        <rdfs:subPropertyOf rdf:resource="https://w3id.org/isoiec5087/-1/v1/TimeOntologyDataProperty"/>
        <rdfs:domain rdf:resource="time:GeneralDateTimeDescription"/>
        <rdfs:comment xml:lang="es">Posición de año en un sistema calendario-reloj.

l rango de esta propiedad no está especificado, por tanto, se puede reemplazar por cualquier representación específica de un año de calendario de un calendario cualquiera.</rdfs:comment>
        <rdfs:comment xml:lang="en">Year position in a calendar-clock system.

The range of this property is not specified, so can be replaced by any specific representation of a calendar year from any calendar. </rdfs:comment>
        <rdfs:label xml:lang="en">year</rdfs:label>
    </owl:DatatypeProperty>
    


    <!-- http://www.w3.org/2006/time#years -->

    <owl:DatatypeProperty rdf:about="http://www.w3.org/2006/time#years">
        <rdfs:subPropertyOf rdf:resource="https://w3id.org/isoiec5087/-1/v1/TimeOntologyDataProperty"/>
        <rdfs:domain rdf:resource="time:GeneralDurationDescription"/>
        <rdfs:range rdf:resource="xsd:decimal"/>
        <rdfs:comment xml:lang="es">Longitud de, o elemento de la longitud de, una extensión temporal expresada en años.</rdfs:comment>
        <rdfs:comment xml:lang="en">length of, or element of the length of, a temporal extent expressed in years</rdfs:comment>
        <rdfs:label xml:lang="es">duración en años</rdfs:label>
        <rdfs:label xml:lang="en">years duration</rdfs:label>
    </owl:DatatypeProperty>
    


    <!-- 
    ///////////////////////////////////////////////////////////////////////////////////////
    //
    // Classes
    //
    ///////////////////////////////////////////////////////////////////////////////////////
     -->

    


    <!-- https://w3id.org/isoiec5087/-1/v1/TimeOntologyThing -->

    <owl:Class rdf:about="https://w3id.org/isoiec5087/-1/v1/TimeOntologyThing">
        <skos:definition>Class added for organizational purposes, to identify classes defined in the Time Ontology.</skos:definition>
    </owl:Class>
    


    <!-- http://www.w3.org/2006/time#DateTimeDescription -->

    <owl:Class rdf:about="http://www.w3.org/2006/time#DateTimeDescription">
        <rdfs:subClassOf rdf:resource="time:GeneralDateTimeDescription"/>
        <rdfs:subClassOf>
            <owl:Restriction>
                <owl:onProperty rdf:resource="time:hasTRS"/>
                <owl:hasValue rdf:resource="http://www.opengis.net/def/uom/ISO-8601/0/Gregorian"/>
            </owl:Restriction>
        </rdfs:subClassOf>
        <rdfs:subClassOf>
            <owl:Restriction>
                <owl:onProperty rdf:resource="time:day"/>
                <owl:allValuesFrom rdf:resource="xsd:gDay"/>
            </owl:Restriction>
        </rdfs:subClassOf>
        <rdfs:subClassOf>
            <owl:Restriction>
                <owl:onProperty rdf:resource="time:month"/>
                <owl:allValuesFrom rdf:resource="xsd:gMonth"/>
            </owl:Restriction>
        </rdfs:subClassOf>
        <rdfs:subClassOf>
            <owl:Restriction>
                <owl:onProperty rdf:resource="time:year"/>
                <owl:allValuesFrom rdf:resource="xsd:gYear"/>
            </owl:Restriction>
        </rdfs:subClassOf>
        <rdfs:comment xml:lang="es">Descripción de fecha y tiempo estructurada con valores separados para los diferentes elementos de un sistema calendario-reloj. El sistema de referencia temporal está fijado al calendario gregoriano, y el rango de las propiedades año, mes, día restringidas a los correspondientes tipos del XML Schema xsd:gYear, xsd:gMonth y xsd:gDay respectivamente.</rdfs:comment>
        <rdfs:comment xml:lang="en">Description of date and time structured with separate values for the various elements of a calendar-clock system. The temporal reference system is fixed to Gregorian Calendar, and the range of year, month, day properties restricted to corresponding XML Schema types xsd:gYear, xsd:gMonth and xsd:gDay, respectively.</rdfs:comment>
        <rdfs:label xml:lang="en">Date-Time description</rdfs:label>
        <rdfs:label xml:lang="es">descripción de fecha-tiempo</rdfs:label>
        <skos:definition xml:lang="es">Descripción de fecha y tiempo estructurada con valores separados para los diferentes elementos de un sistema calendario-reloj. El sistema de referencia temporal está fijado al calendario gregoriano, y el rango de las propiedades año, mes, día restringidas a los correspondientes tipos del XML Schema xsd:gYear, xsd:gMonth y xsd:gDay respectivamente.</skos:definition>
        <skos:definition xml:lang="en">Description of date and time structured with separate values for the various elements of a calendar-clock system. The temporal reference system is fixed to Gregorian Calendar, and the range of year, month, day properties restricted to corresponding XML Schema types xsd:gYear, xsd:gMonth and xsd:gDay, respectively.</skos:definition>
    </owl:Class>
    


    <!-- http://www.w3.org/2006/time#DateTimeInterval -->

    <owl:Class rdf:about="http://www.w3.org/2006/time#DateTimeInterval">
        <rdfs:subClassOf rdf:resource="time:ProperInterval"/>
        <rdfs:subClassOf>
            <owl:Restriction>
                <owl:onProperty rdf:resource="time:hasDateTimeDescription"/>
                <owl:allValuesFrom rdf:resource="time:GeneralDateTimeDescription"/>
            </owl:Restriction>
        </rdfs:subClassOf>
        <rdfs:subClassOf>
            <owl:Restriction>
                <owl:onProperty rdf:resource="time:xsdDateTime"/>
                <owl:allValuesFrom rdf:resource="xsd:dateTime"/>
            </owl:Restriction>
        </rdfs:subClassOf>
        <rdfs:comment xml:lang="es">&apos;intervalo de fecha-hora&apos; es una subclase de &apos;intervalo propio&apos;, definida utilizando el multi-elemento &apos;descripción de fecha-hora&apos;.</rdfs:comment>
        <rdfs:comment xml:lang="en">DateTimeInterval is a subclass of ProperInterval, defined using the multi-element DateTimeDescription.</rdfs:comment>
        <rdfs:label xml:lang="en">Date-time interval</rdfs:label>
        <rdfs:label xml:lang="es">intervalo de fecha-hora</rdfs:label>
        <skos:definition xml:lang="es">&apos;intervalo de fecha-hora&apos; es una subclase de &apos;intervalo propio&apos;, definida utilizando el multi-elemento &apos;descripción de fecha-hora&apos;.</skos:definition>
        <skos:definition xml:lang="en">DateTimeInterval is a subclass of ProperInterval, defined using the multi-element DateTimeDescription.</skos:definition>
        <skos:note xml:lang="es">&apos;intervalo de fecha-hora&apos; se puede utilizar sólo para un intervalo cuyos límites coinciden con un elemento de fecha-hora alineados con el calendario y la zona horaria indicados. Por ejemplo, aunque ambos tienen una duración de un día, el intervalo de 24 horas que empieza en la media noche del comienzo del 8 mayo en Europa Central se puede expresar como un &apos;intervalo de fecha-hora&apos;, el intervalo de 24 horas que empieza a las 1:30pm no.</skos:note>
        <skos:note xml:lang="en">:DateTimeInterval can only be used for an interval whose limits coincide with a date-time element aligned to the calendar and timezone indicated. For example, while both have a duration of one day, the 24-hour interval beginning at midnight at the beginning of 8 May in Central Europe can be expressed as a :DateTimeInterval, but the 24-hour interval starting at 1:30pm cannot.</skos:note>
    </owl:Class>
    


    <!-- http://www.w3.org/2006/time#DayOfWeek -->

    <owl:Class rdf:about="http://www.w3.org/2006/time#DayOfWeek">
        <rdfs:subClassOf rdf:resource="https://w3id.org/isoiec5087/-1/v1/TimeOntologyThing"/>
        <rdfs:comment xml:lang="es">El día de la semana</rdfs:comment>
        <rdfs:comment xml:lang="en">The day of week</rdfs:comment>
        <rdfs:label xml:lang="en">Day of week</rdfs:label>
        <rdfs:label xml:lang="es">día de la semana</rdfs:label>
        <skos:changeNote xml:lang="en">Remove enumeration from definition, in order to allow other days to be used when required in other calendars. 
NOTE: existing days are still present as members of the class, but the class membership is now open. 

In the original OWL-Time the following constraint appeared: 
  owl:oneOf (
      time:Monday
      time:Tuesday
      time:Wednesday
      time:Thursday
      time:Friday
      time:Saturday
      time:Sunday
    ) ;</skos:changeNote>
        <skos:definition xml:lang="es">El día de la semana</skos:definition>
        <skos:definition xml:lang="en">The day of week</skos:definition>
        <skos:note xml:lang="es">La pertenencia a la clase &apos;día de la semana&apos; está abierta, para permitir longitudes de semana alternativas y diferentes nombres de días.</skos:note>
        <skos:note xml:lang="en">Membership of the class :DayOfWeek is open, to allow for alternative week lengths and different day names.</skos:note>
    </owl:Class>
    


    <!-- http://www.w3.org/2006/time#Duration -->

    <owl:Class rdf:about="http://www.w3.org/2006/time#Duration">
        <rdfs:subClassOf rdf:resource="time:TemporalDuration"/>
        <rdfs:subClassOf>
            <owl:Restriction>
                <owl:onProperty rdf:resource="time:unitType"/>
                <owl:cardinality rdf:datatype="xsd:nonNegativeInteger">1</owl:cardinality>
            </owl:Restriction>
        </rdfs:subClassOf>
        <rdfs:subClassOf>
            <owl:Restriction>
                <owl:onProperty rdf:resource="time:numericDuration"/>
                <owl:cardinality rdf:datatype="xsd:nonNegativeInteger">1</owl:cardinality>
            </owl:Restriction>
        </rdfs:subClassOf>
        <rdfs:comment xml:lang="es">Duración de una extensión temporal expresada como un número escalado por una unidad temporal.</rdfs:comment>
        <rdfs:comment xml:lang="en">Duration of a temporal extent expressed as a number scaled by a temporal unit</rdfs:comment>
        <rdfs:label xml:lang="en">Time duration</rdfs:label>
        <rdfs:label>duración de tiempo</rdfs:label>
        <skos:definition xml:lang="es">Duración de una extensión temporal expresada como un número escalado por una unidad temporal.</skos:definition>
        <skos:definition xml:lang="en">Duration of a temporal extent expressed as a number scaled by a temporal unit</skos:definition>
        <skos:note xml:lang="es">Alternativa a &apos;descripción de tiempo&apos; para proporcionar descripción soporte a una duración temporal diferente a utilizar un sistema de calendario/reloj.</skos:note>
        <skos:note xml:lang="en">Alternative to time:DurationDescription to support description of a temporal duration other than using a calendar/clock system.</skos:note>
    </owl:Class>
    


    <!-- http://www.w3.org/2006/time#DurationDescription -->

    <owl:Class rdf:about="http://www.w3.org/2006/time#DurationDescription">
        <rdfs:subClassOf rdf:resource="time:GeneralDurationDescription"/>
        <rdfs:subClassOf>
            <owl:Restriction>
                <owl:onProperty rdf:resource="time:hasTRS"/>
                <owl:hasValue rdf:resource="http://www.opengis.net/def/uom/ISO-8601/0/Gregorian"/>
            </owl:Restriction>
        </rdfs:subClassOf>
        <rdfs:subClassOf>
            <owl:Restriction>
                <owl:onProperty rdf:resource="time:days"/>
                <owl:allValuesFrom rdf:resource="xsd:decimal"/>
            </owl:Restriction>
        </rdfs:subClassOf>
        <rdfs:subClassOf>
            <owl:Restriction>
                <owl:onProperty rdf:resource="time:hours"/>
                <owl:allValuesFrom rdf:resource="xsd:decimal"/>
            </owl:Restriction>
        </rdfs:subClassOf>
        <rdfs:subClassOf>
            <owl:Restriction>
                <owl:onProperty rdf:resource="time:minutes"/>
                <owl:allValuesFrom rdf:resource="xsd:decimal"/>
            </owl:Restriction>
        </rdfs:subClassOf>
        <rdfs:subClassOf>
            <owl:Restriction>
                <owl:onProperty rdf:resource="time:months"/>
                <owl:allValuesFrom rdf:resource="xsd:decimal"/>
            </owl:Restriction>
        </rdfs:subClassOf>
        <rdfs:subClassOf>
            <owl:Restriction>
                <owl:onProperty rdf:resource="time:seconds"/>
                <owl:allValuesFrom rdf:resource="xsd:decimal"/>
            </owl:Restriction>
        </rdfs:subClassOf>
        <rdfs:subClassOf>
            <owl:Restriction>
                <owl:onProperty rdf:resource="time:weeks"/>
                <owl:allValuesFrom rdf:resource="xsd:decimal"/>
            </owl:Restriction>
        </rdfs:subClassOf>
        <rdfs:subClassOf>
            <owl:Restriction>
                <owl:onProperty rdf:resource="time:years"/>
                <owl:allValuesFrom rdf:resource="xsd:decimal"/>
            </owl:Restriction>
        </rdfs:subClassOf>
        <rdfs:comment xml:lang="es">Descripción de extensión temporal estructurada con valores separados para los distintos elementos de un sistema de horario-calendario. El sistema de referencia temporal se fija al calendario gregoriano, y el intervalo de cada una de las propiedades numéricas se restringe a xsd:decimal.</rdfs:comment>
        <rdfs:comment xml:lang="en">Description of temporal extent structured with separate values for the various elements of a calendar-clock system. The temporal reference system is fixed to Gregorian Calendar, and the range of each of the numeric properties is restricted to xsd:decimal</rdfs:comment>
        <rdfs:label xml:lang="en">Duration description</rdfs:label>
        <rdfs:label xml:lang="es">descripción de duración</rdfs:label>
        <skos:definition xml:lang="es">Descripción de extensión temporal estructurada con valores separados para los distintos elementos de un sistema de horario-calendario. El sistema de referencia temporal se fija al calendario gregoriano, y el intervalo de cada una de las propiedades numéricas se restringe a xsd:decimal.</skos:definition>
        <skos:definition xml:lang="en">Description of temporal extent structured with separate values for the various elements of a calendar-clock system. The temporal reference system is fixed to Gregorian Calendar, and the range of each of the numeric properties is restricted to xsd:decimal</skos:definition>
        <skos:note xml:lang="es">En el calendario gregoriano la longitud de los meses no es fija. Por lo tanto, un valor como &quot;2,5 meses&quot; no se puede comparar exactamente con una duración similar expresada en términos de semanas o días.</skos:note>
        <skos:note xml:lang="en">In the Gregorian calendar the length of the month is not fixed. Therefore, a value like &quot;2.5 months&quot; cannot be exactly compared with a similar duration expressed in terms of weeks or days.</skos:note>
    </owl:Class>
    


    <!-- http://www.w3.org/2006/time#GeneralDateTimeDescription -->

    <owl:Class rdf:about="http://www.w3.org/2006/time#GeneralDateTimeDescription">
        <rdfs:subClassOf rdf:resource="time:TemporalPosition"/>
        <rdfs:subClassOf>
            <owl:Restriction>
                <owl:onProperty rdf:resource="time:unitType"/>
                <owl:qualifiedCardinality rdf:datatype="xsd:nonNegativeInteger">1</owl:qualifiedCardinality>
                <owl:onClass rdf:resource="time:TemporalUnit"/>
            </owl:Restriction>
        </rdfs:subClassOf>
        <rdfs:subClassOf>
            <owl:Restriction>
                <owl:onProperty rdf:resource="time:dayOfWeek"/>
                <owl:maxQualifiedCardinality rdf:datatype="xsd:nonNegativeInteger">1</owl:maxQualifiedCardinality>
                <owl:onClass rdf:resource="time:DayOfWeek"/>
            </owl:Restriction>
        </rdfs:subClassOf>
        <rdfs:subClassOf>
            <owl:Restriction>
                <owl:onProperty rdf:resource="time:monthOfYear"/>
                <owl:maxQualifiedCardinality rdf:datatype="xsd:nonNegativeInteger">1</owl:maxQualifiedCardinality>
                <owl:onClass rdf:resource="time:MonthOfYear"/>
            </owl:Restriction>
        </rdfs:subClassOf>
        <rdfs:subClassOf>
            <owl:Restriction>
                <owl:onProperty rdf:resource="time:timeZone"/>
                <owl:maxQualifiedCardinality rdf:datatype="xsd:nonNegativeInteger">1</owl:maxQualifiedCardinality>
                <owl:onClass rdf:resource="time:TimeZone"/>
            </owl:Restriction>
        </rdfs:subClassOf>
        <rdfs:subClassOf>
            <owl:Restriction>
                <owl:onProperty rdf:resource="time:day"/>
                <owl:maxCardinality rdf:datatype="xsd:nonNegativeInteger">1</owl:maxCardinality>
            </owl:Restriction>
        </rdfs:subClassOf>
        <rdfs:subClassOf>
            <owl:Restriction>
                <owl:onProperty rdf:resource="time:dayOfYear"/>
                <owl:maxCardinality rdf:datatype="xsd:nonNegativeInteger">1</owl:maxCardinality>
            </owl:Restriction>
        </rdfs:subClassOf>
        <rdfs:subClassOf>
            <owl:Restriction>
                <owl:onProperty rdf:resource="time:hour"/>
                <owl:maxCardinality rdf:datatype="xsd:nonNegativeInteger">1</owl:maxCardinality>
            </owl:Restriction>
        </rdfs:subClassOf>
        <rdfs:subClassOf>
            <owl:Restriction>
                <owl:onProperty rdf:resource="time:minute"/>
                <owl:maxCardinality rdf:datatype="xsd:nonNegativeInteger">1</owl:maxCardinality>
            </owl:Restriction>
        </rdfs:subClassOf>
        <rdfs:subClassOf>
            <owl:Restriction>
                <owl:onProperty rdf:resource="time:month"/>
                <owl:maxCardinality rdf:datatype="xsd:nonNegativeInteger">1</owl:maxCardinality>
            </owl:Restriction>
        </rdfs:subClassOf>
        <rdfs:subClassOf>
            <owl:Restriction>
                <owl:onProperty rdf:resource="time:second"/>
                <owl:maxQualifiedCardinality rdf:datatype="xsd:nonNegativeInteger">1</owl:maxQualifiedCardinality>
                <owl:onDataRange rdf:resource="xsd:decimal"/>
            </owl:Restriction>
        </rdfs:subClassOf>
        <rdfs:subClassOf>
            <owl:Restriction>
                <owl:onProperty rdf:resource="time:week"/>
                <owl:maxQualifiedCardinality rdf:datatype="xsd:nonNegativeInteger">1</owl:maxQualifiedCardinality>
                <owl:onDataRange rdf:resource="xsd:nonNegativeInteger"/>
            </owl:Restriction>
        </rdfs:subClassOf>
        <rdfs:subClassOf>
            <owl:Restriction>
                <owl:onProperty rdf:resource="time:year"/>
                <owl:maxQualifiedCardinality rdf:datatype="xsd:nonNegativeInteger">1</owl:maxQualifiedCardinality>
                <owl:onDataRange rdf:resource="xsd:nonNegativeInteger"/>
            </owl:Restriction>
        </rdfs:subClassOf>
        <rdfs:comment xml:lang="es">Descripción de fecha y hora estructurada con valores separados para los distintos elementos de un sistema calendario-reloj.</rdfs:comment>
        <rdfs:comment xml:lang="en">Description of date and time structured with separate values for the various elements of a calendar-clock system</rdfs:comment>
        <rdfs:label xml:lang="en">Generalized date-time description</rdfs:label>
        <rdfs:label xml:lang="es">descripción de fecha-hora generalizada</rdfs:label>
        <skos:definition>Descripción de fecha y hora estructurada con valores separados para los distintos elementos de un sistema calendario-reloj.</skos:definition>
        <skos:definition xml:lang="en">Description of date and time structured with separate values for the various elements of a calendar-clock system</skos:definition>
        <skos:note xml:lang="es">Algunas combinaciones de propiedades son redundantes - por ejemplo, dentro de un &apos;año&apos; especificado si se proporciona &apos;día del año&apos; entonces &apos;día&apos; y &apos;mes&apos; se pueden computar, y viceversa. Los valores individuales deberían ser consistentes entre ellos y con el calendario, indicado a través del valor de la propiedad &apos;tiene TRS&apos;.</skos:note>
        <skos:note>Some combinations of properties are redundant - for example, within a specified :year if :dayOfYear is provided then :day and :month can be computed, and vice versa. Individual values should be consistent with each other and the calendar, indicated through the value of the :hasTRS property.</skos:note>
    </owl:Class>
    


    <!-- http://www.w3.org/2006/time#GeneralDurationDescription -->

    <owl:Class rdf:about="http://www.w3.org/2006/time#GeneralDurationDescription">
        <rdfs:subClassOf rdf:resource="time:TemporalDuration"/>
        <rdfs:subClassOf>
            <owl:Restriction>
                <owl:onProperty rdf:resource="time:hasTRS"/>
                <owl:cardinality rdf:datatype="xsd:nonNegativeInteger">1</owl:cardinality>
            </owl:Restriction>
        </rdfs:subClassOf>
        <rdfs:subClassOf>
            <owl:Restriction>
                <owl:onProperty rdf:resource="time:days"/>
                <owl:maxCardinality rdf:datatype="xsd:nonNegativeInteger">1</owl:maxCardinality>
            </owl:Restriction>
        </rdfs:subClassOf>
        <rdfs:subClassOf>
            <owl:Restriction>
                <owl:onProperty rdf:resource="time:hours"/>
                <owl:maxCardinality rdf:datatype="xsd:nonNegativeInteger">1</owl:maxCardinality>
            </owl:Restriction>
        </rdfs:subClassOf>
        <rdfs:subClassOf>
            <owl:Restriction>
                <owl:onProperty rdf:resource="time:minutes"/>
                <owl:maxCardinality rdf:datatype="xsd:nonNegativeInteger">1</owl:maxCardinality>
            </owl:Restriction>
        </rdfs:subClassOf>
        <rdfs:subClassOf>
            <owl:Restriction>
                <owl:onProperty rdf:resource="time:months"/>
                <owl:maxCardinality rdf:datatype="xsd:nonNegativeInteger">1</owl:maxCardinality>
            </owl:Restriction>
        </rdfs:subClassOf>
        <rdfs:subClassOf>
            <owl:Restriction>
                <owl:onProperty rdf:resource="time:seconds"/>
                <owl:maxCardinality rdf:datatype="xsd:nonNegativeInteger">1</owl:maxCardinality>
            </owl:Restriction>
        </rdfs:subClassOf>
        <rdfs:subClassOf>
            <owl:Restriction>
                <owl:onProperty rdf:resource="time:weeks"/>
                <owl:maxCardinality rdf:datatype="xsd:nonNegativeInteger">1</owl:maxCardinality>
            </owl:Restriction>
        </rdfs:subClassOf>
        <rdfs:subClassOf>
            <owl:Restriction>
                <owl:onProperty rdf:resource="time:years"/>
                <owl:maxCardinality rdf:datatype="xsd:nonNegativeInteger">1</owl:maxCardinality>
            </owl:Restriction>
        </rdfs:subClassOf>
        <rdfs:comment xml:lang="es">Descripción de extensión temporal estructurada con valores separados para los distintos elementos de un sistema de horario-calendario.</rdfs:comment>
        <rdfs:comment xml:lang="en">Description of temporal extent structured with separate values for the various elements of a calendar-clock system.</rdfs:comment>
        <rdfs:label xml:lang="en">Generalized duration description</rdfs:label>
        <rdfs:label xml:lang="es">descripción de duración generalizada</rdfs:label>
        <skos:definition xml:lang="es">Descripción de extensión temporal estructurada con valores separados para los distintos elementos de un sistema de horario-calendario.</skos:definition>
        <skos:definition xml:lang="en">Description of temporal extent structured with separate values for the various elements of a calendar-clock system.</skos:definition>
        <skos:note xml:lang="es">La extensión de una duración de tiempo expresada como una &apos;descripción de duración general&apos; depende del Sistema de Referencia Temporal. En algunos calendarios la longitud de la semana o del mes no es constante a lo largo del año. Por tanto, un valor como &quot;25 meses&quot; puede no ser necesariamente ser comparado con un duración similar expresada en términos de semanas o días. Cuando se consideran calendarios que no están basados en el movimiento de la Tierra, se deben tomar incluso más precauciones en la comparación de duraciones.</skos:note>
        <skos:note xml:lang="en">The extent of a time duration expressed as a GeneralDurationDescription depends on the Temporal Reference System. In some calendars the length of the week or month is not constant within the year. Therefore, a value like &quot;2.5 months&quot; may not necessarily be exactly compared with a similar duration expressed in terms of weeks or days. When non-earth-based calendars are considered even more care must be taken in comparing durations.</skos:note>
    </owl:Class>
    


    <!-- http://www.w3.org/2006/time#Instant -->

    <owl:Class rdf:about="http://www.w3.org/2006/time#Instant">
        <rdfs:subClassOf rdf:resource="time:TemporalEntity"/>
        <rdfs:subClassOf>
            <owl:Restriction>
                <owl:onProperty rdf:resource="time:inDateTime"/>
                <owl:allValuesFrom rdf:resource="time:GeneralDateTimeDescription"/>
            </owl:Restriction>
        </rdfs:subClassOf>
        <rdfs:subClassOf>
            <owl:Restriction>
                <owl:onProperty rdf:resource="time:inTemporalPosition"/>
                <owl:allValuesFrom rdf:resource="time:TemporalPosition"/>
            </owl:Restriction>
        </rdfs:subClassOf>
        <rdfs:subClassOf>
            <owl:Restriction>
                <owl:onProperty rdf:resource="time:inTimePosition"/>
                <owl:allValuesFrom rdf:resource="time:TimePosition"/>
            </owl:Restriction>
        </rdfs:subClassOf>
        <rdfs:subClassOf>
            <owl:Restriction>
                <owl:onProperty rdf:resource="time:inXSDDate"/>
                <owl:allValuesFrom rdf:resource="xsd:date"/>
            </owl:Restriction>
        </rdfs:subClassOf>
        <rdfs:subClassOf>
            <owl:Restriction>
                <owl:onProperty rdf:resource="time:inXSDDateTimeStamp"/>
                <owl:allValuesFrom rdf:resource="xsd:dateTimeStamp"/>
            </owl:Restriction>
        </rdfs:subClassOf>
        <rdfs:subClassOf>
            <owl:Restriction>
                <owl:onProperty rdf:resource="time:inXSDgYear"/>
                <owl:allValuesFrom rdf:resource="xsd:gYear"/>
            </owl:Restriction>
        </rdfs:subClassOf>
        <rdfs:subClassOf>
            <owl:Restriction>
                <owl:onProperty rdf:resource="time:inXSDgYearMonth"/>
                <owl:allValuesFrom rdf:resource="xsd:gYearMonth"/>
            </owl:Restriction>
        </rdfs:subClassOf>
        <owl:disjointWith rdf:resource="time:ProperInterval"/>
        <rdfs:comment xml:lang="en">A temporal entity with zero extent or duration</rdfs:comment>
        <rdfs:comment xml:lang="es">Una entidad temporal con una extensión o duración cero.</rdfs:comment>
        <rdfs:label xml:lang="en">Time instant</rdfs:label>
        <rdfs:label xml:lang="es">instante de tiempo.</rdfs:label>
        <skos:definition xml:lang="en">A temporal entity with zero extent or duration</skos:definition>
        <skos:definition xml:lang="es">Una entidad temporal con una extensión o duración cero.</skos:definition>
    </owl:Class>
    


    <!-- http://www.w3.org/2006/time#Interval -->

    <owl:Class rdf:about="http://www.w3.org/2006/time#Interval">
        <rdfs:subClassOf rdf:resource="time:TemporalEntity"/>
        <rdfs:subClassOf>
            <owl:Restriction>
                <owl:onProperty rdf:resource="time:inside"/>
                <owl:someValuesFrom rdf:resource="time:Instant"/>
            </owl:Restriction>
        </rdfs:subClassOf>
        <rdfs:comment xml:lang="en">A temporal entity with an extent or duration</rdfs:comment>
        <rdfs:comment xml:lang="es">Una entidad temporal con una extensión o duración.</rdfs:comment>
        <rdfs:label xml:lang="en">Time interval</rdfs:label>
        <rdfs:label xml:lang="es">intervalo de tiempo</rdfs:label>
        <skos:definition xml:lang="en">A temporal entity with an extent or duration</skos:definition>
        <skos:definition xml:lang="es">Una entidad temporal con una extensión o duración.</skos:definition>
    </owl:Class>
    


    <!-- http://www.w3.org/2006/time#January -->

    <owl:Class rdf:about="http://www.w3.org/2006/time#January">
        <rdfs:subClassOf rdf:resource="time:DateTimeDescription"/>
        <rdfs:subClassOf>
            <owl:Restriction>
                <owl:onProperty rdf:resource="time:unitType"/>
                <owl:hasValue rdf:resource="time:unitMonth"/>
            </owl:Restriction>
        </rdfs:subClassOf>
        <rdfs:subClassOf>
            <owl:Restriction>
                <owl:onProperty rdf:resource="time:month"/>
                <owl:hasValue>--01</owl:hasValue>
            </owl:Restriction>
        </rdfs:subClassOf>
        <rdfs:label>January</rdfs:label>
        <owl:deprecated rdf:datatype="xsd:boolean">true</owl:deprecated>
        <skos:historyNote>This class was present in the 2006 version of OWL-Time. It was presented as an example of how DateTimeDescription could be specialized, but does not belong in the revised ontology. </skos:historyNote>
    </owl:Class>
    


    <!-- http://www.w3.org/2006/time#MonthOfYear -->

    <owl:Class rdf:about="http://www.w3.org/2006/time#MonthOfYear">
        <rdfs:subClassOf rdf:resource="time:DateTimeDescription"/>
        <rdfs:subClassOf>
            <owl:Restriction>
                <owl:onProperty rdf:resource="time:unitType"/>
                <owl:hasValue rdf:resource="time:unitMonth"/>
            </owl:Restriction>
        </rdfs:subClassOf>
        <rdfs:subClassOf>
            <owl:Restriction>
                <owl:onProperty rdf:resource="time:day"/>
                <owl:cardinality rdf:datatype="xsd:nonNegativeInteger">0</owl:cardinality>
            </owl:Restriction>
        </rdfs:subClassOf>
        <rdfs:subClassOf>
            <owl:Restriction>
                <owl:onProperty rdf:resource="time:hour"/>
                <owl:cardinality rdf:datatype="xsd:nonNegativeInteger">0</owl:cardinality>
            </owl:Restriction>
        </rdfs:subClassOf>
        <rdfs:subClassOf>
            <owl:Restriction>
                <owl:onProperty rdf:resource="time:minute"/>
                <owl:cardinality rdf:datatype="xsd:nonNegativeInteger">0</owl:cardinality>
            </owl:Restriction>
        </rdfs:subClassOf>
        <rdfs:subClassOf>
            <owl:Restriction>
                <owl:onProperty rdf:resource="time:month"/>
                <owl:cardinality rdf:datatype="xsd:nonNegativeInteger">1</owl:cardinality>
            </owl:Restriction>
        </rdfs:subClassOf>
        <rdfs:subClassOf>
            <owl:Restriction>
                <owl:onProperty rdf:resource="time:second"/>
                <owl:cardinality rdf:datatype="xsd:nonNegativeInteger">0</owl:cardinality>
            </owl:Restriction>
        </rdfs:subClassOf>
        <rdfs:subClassOf>
            <owl:Restriction>
                <owl:onProperty rdf:resource="time:week"/>
                <owl:cardinality rdf:datatype="xsd:nonNegativeInteger">0</owl:cardinality>
            </owl:Restriction>
        </rdfs:subClassOf>
        <rdfs:subClassOf>
            <owl:Restriction>
                <owl:onProperty rdf:resource="time:year"/>
                <owl:cardinality rdf:datatype="xsd:nonNegativeInteger">0</owl:cardinality>
            </owl:Restriction>
        </rdfs:subClassOf>
        <rdfs:comment xml:lang="es">El mes del año.</rdfs:comment>
        <rdfs:comment xml:lang="en">The month of the year</rdfs:comment>
        <rdfs:label xml:lang="en">Month of year</rdfs:label>
        <rdfs:label xml:lang="es">mes del año</rdfs:label>
        <skos:definition xml:lang="es">El mes del año.</skos:definition>
        <skos:definition xml:lang="en">The month of the year</skos:definition>
        <skos:editorialNote xml:lang="es">Característica en riesgo - añadida en la revisión de 2017, y no utilizada todavía de forma amplia.</skos:editorialNote>
        <skos:editorialNote xml:lang="en">Feature at risk - added in 2017 revision, and not yet widely used. </skos:editorialNote>
        <skos:note xml:lang="es">La pertenencia a la clase &apos;mes del año&apos; está abierta, a permitir calendarios anuales alternativos y diferentes nombres de meses.</skos:note>
        <skos:note xml:lang="en">Membership of the class :MonthOfYear is open, to allow for alternative annual calendars and different month names.</skos:note>
    </owl:Class>
    


    <!-- http://www.w3.org/2006/time#ProperInterval -->

    <owl:Class rdf:about="http://www.w3.org/2006/time#ProperInterval">
        <rdfs:subClassOf rdf:resource="time:Interval"/>
        <rdfs:subClassOf>
            <owl:Restriction>
                <owl:onProperty rdf:resource="time:intervalAfter"/>
                <owl:allValuesFrom rdf:resource="time:ProperInterval"/>
            </owl:Restriction>
        </rdfs:subClassOf>
        <rdfs:subClassOf>
            <owl:Restriction>
                <owl:onProperty rdf:resource="time:intervalBefore"/>
                <owl:allValuesFrom rdf:resource="time:ProperInterval"/>
            </owl:Restriction>
        </rdfs:subClassOf>
        <rdfs:subClassOf>
            <owl:Restriction>
                <owl:onProperty rdf:resource="time:intervalContains"/>
                <owl:allValuesFrom rdf:resource="time:ProperInterval"/>
            </owl:Restriction>
        </rdfs:subClassOf>
        <rdfs:subClassOf>
            <owl:Restriction>
                <owl:onProperty rdf:resource="time:intervalDisjoint"/>
                <owl:allValuesFrom rdf:resource="time:ProperInterval"/>
            </owl:Restriction>
        </rdfs:subClassOf>
        <rdfs:subClassOf>
            <owl:Restriction>
                <owl:onProperty rdf:resource="time:intervalDuring"/>
                <owl:allValuesFrom rdf:resource="time:ProperInterval"/>
            </owl:Restriction>
        </rdfs:subClassOf>
        <rdfs:subClassOf>
            <owl:Restriction>
                <owl:onProperty rdf:resource="time:intervalEquals"/>
                <owl:allValuesFrom rdf:resource="time:ProperInterval"/>
            </owl:Restriction>
        </rdfs:subClassOf>
        <rdfs:subClassOf>
            <owl:Restriction>
                <owl:onProperty rdf:resource="time:intervalFinishedBy"/>
                <owl:allValuesFrom rdf:resource="time:ProperInterval"/>
            </owl:Restriction>
        </rdfs:subClassOf>
        <rdfs:subClassOf>
            <owl:Restriction>
                <owl:onProperty rdf:resource="time:intervalFinishes"/>
                <owl:allValuesFrom rdf:resource="time:ProperInterval"/>
            </owl:Restriction>
        </rdfs:subClassOf>
        <rdfs:subClassOf>
            <owl:Restriction>
                <owl:onProperty rdf:resource="time:intervalIn"/>
                <owl:allValuesFrom rdf:resource="time:ProperInterval"/>
            </owl:Restriction>
        </rdfs:subClassOf>
        <rdfs:subClassOf>
            <owl:Restriction>
                <owl:onProperty rdf:resource="time:intervalMeets"/>
                <owl:allValuesFrom rdf:resource="time:ProperInterval"/>
            </owl:Restriction>
        </rdfs:subClassOf>
        <rdfs:subClassOf>
            <owl:Restriction>
                <owl:onProperty rdf:resource="time:intervalMetBy"/>
                <owl:allValuesFrom rdf:resource="time:ProperInterval"/>
            </owl:Restriction>
        </rdfs:subClassOf>
        <rdfs:subClassOf>
            <owl:Restriction>
                <owl:onProperty rdf:resource="time:intervalOverlappedBy"/>
                <owl:allValuesFrom rdf:resource="time:ProperInterval"/>
            </owl:Restriction>
        </rdfs:subClassOf>
        <rdfs:subClassOf>
            <owl:Restriction>
                <owl:onProperty rdf:resource="time:intervalOverlaps"/>
                <owl:allValuesFrom rdf:resource="time:ProperInterval"/>
            </owl:Restriction>
        </rdfs:subClassOf>
        <rdfs:subClassOf>
            <owl:Restriction>
                <owl:onProperty rdf:resource="time:intervalStartedBy"/>
                <owl:allValuesFrom rdf:resource="time:ProperInterval"/>
            </owl:Restriction>
        </rdfs:subClassOf>
        <rdfs:subClassOf>
            <owl:Restriction>
                <owl:onProperty rdf:resource="time:intervalStarts"/>
                <owl:allValuesFrom rdf:resource="time:ProperInterval"/>
            </owl:Restriction>
        </rdfs:subClassOf>
        <rdfs:comment xml:lang="en">A temporal entity with non-zero extent or duration, i.e. for which the value of the beginning and end are different</rdfs:comment>
        <rdfs:comment xml:lang="es">Una entidad temporal con extensión o duración distinta de cero, es decir, para la cual los valores de principio y fin del intervalo son diferentes.</rdfs:comment>
        <rdfs:label xml:lang="en">Proper interval</rdfs:label>
        <rdfs:label xml:lang="es">intervalo propio</rdfs:label>
        <skos:definition xml:lang="en">A temporal entity with non-zero extent or duration, i.e. for which the value of the beginning and end are different</skos:definition>
        <skos:definition xml:lang="es">Una entidad temporal con extensión o duración distinta de cero, es decir, para la cual los valores de principio y fin del intervalo son diferentes.</skos:definition>
    </owl:Class>
    


    <!-- http://www.w3.org/2006/time#TRS -->

    <owl:Class rdf:about="http://www.w3.org/2006/time#TRS">
        <rdfs:subClassOf rdf:resource="https://w3id.org/isoiec5087/-1/v1/TimeOntologyThing"/>
        <rdfs:comment xml:lang="en">A temporal reference system, such as a temporal coordinate system (with an origin, direction, and scale), a calendar-clock combination, or a (possibly hierarchical) ordinal system. 

This is a stub class, representing the set of all temporal reference systems.</rdfs:comment>
        <rdfs:comment xml:lang="es">Un sistema de referencia temporal, tal como un sistema de coordenadas temporales (con un origen, una dirección y una escala), una combinación calendario-reloj, o un sistema ordinal (posiblemente jerárquico).
        Esta clase comodín representa el conjunto de todos los sistemas de referencia temporal.</rdfs:comment>
        <rdfs:label xml:lang="en">Temporal Reference System</rdfs:label>
        <rdfs:label xml:lang="es">sistema de referencia temporal</rdfs:label>
        <skos:definition xml:lang="en">A temporal reference system, such as a temporal coordinate system (with an origin, direction, and scale), a calendar-clock combination, or a (possibly hierarchical) ordinal system. 

This is a stub class, representing the set of all temporal reference systems.</skos:definition>
        <skos:definition xml:lang="es">Un sistema de referencia temporal, tal como un sistema de coordenadas temporales (con un origen, una dirección y una escala), una combinación calendario-reloj, o un sistema ordinal (posiblemente jerárquico).
    Esta clase comodín representa el conjunto de todos los sistemas de referencia temporal.</skos:definition>
        <skos:note xml:lang="en">A taxonomy of temporal reference systems is provided in ISO 19108:2002 [ISO19108], including (a) calendar + clock systems; (b) temporal coordinate systems (i.e. numeric offset from an epoch); (c) temporal ordinal reference systems (i.e. ordered sequence of named intervals, not necessarily of equal duration).</skos:note>
        <skos:note xml:lang="es">En el ISO 19108:2002 [ISO19108] se proporciona una taxonomía de sistemas de referencia temporal, incluyendo (a) sistemas de calendario + reloj; (b) sistemas de coordenadas temporales (es decir, desplazamiento numérico a partir de una época); (c) sistemas de referencia ordinales temporales (es decir, secuencia ordenada de intervalos nombrados, no necesariamente de igual duración).</skos:note>
    </owl:Class>
    


    <!-- http://www.w3.org/2006/time#TemporalDuration -->

    <owl:Class rdf:about="http://www.w3.org/2006/time#TemporalDuration">
        <rdfs:subClassOf rdf:resource="https://w3id.org/isoiec5087/-1/v1/TimeOntologyThing"/>
        <rdfs:comment xml:lang="es">Extensión de tiempo; duración de un intervalo de tiempo independiente de su posición de inicio particular.</rdfs:comment>
        <rdfs:comment xml:lang="en">Time extent; duration of a time interval separate from its particular start position</rdfs:comment>
        <rdfs:label xml:lang="en">Temporal duration</rdfs:label>
        <rdfs:label xml:lang="es">duración temporal</rdfs:label>
        <skos:definition xml:lang="es">Extensión de tiempo; duración de un intervalo de tiempo independiente de su posición de inicio particular.</skos:definition>
        <skos:definition xml:lang="en">Time extent; duration of a time interval separate from its particular start position</skos:definition>
    </owl:Class>
    


    <!-- http://www.w3.org/2006/time#TemporalEntity -->

    <owl:Class rdf:about="http://www.w3.org/2006/time#TemporalEntity">
        <owl:equivalentClass>
            <owl:Class>
                <owl:unionOf rdf:parseType="Collection">
                    <rdf:Description rdf:about="http://www.w3.org/2006/time#Instant"/>
                    <rdf:Description rdf:about="http://www.w3.org/2006/time#Interval"/>
                </owl:unionOf>
            </owl:Class>
        </owl:equivalentClass>
        <rdfs:subClassOf rdf:resource="https://w3id.org/isoiec5087/-1/v1/TimeOntologyThing"/>
        <rdfs:subClassOf>
            <owl:Restriction>
                <owl:onProperty rdf:resource="time:after"/>
                <owl:allValuesFrom rdf:resource="time:TemporalEntity"/>
            </owl:Restriction>
        </rdfs:subClassOf>
        <rdfs:subClassOf>
            <owl:Restriction>
                <owl:onProperty rdf:resource="time:before"/>
                <owl:allValuesFrom rdf:resource="time:TemporalEntity"/>
            </owl:Restriction>
        </rdfs:subClassOf>
        <rdfs:subClassOf>
            <owl:Restriction>
                <owl:onProperty rdf:resource="time:hasBeginning"/>
                <owl:allValuesFrom rdf:resource="time:Instant"/>
            </owl:Restriction>
        </rdfs:subClassOf>
        <rdfs:subClassOf>
            <owl:Restriction>
                <owl:onProperty rdf:resource="time:hasEnd"/>
                <owl:allValuesFrom rdf:resource="time:Instant"/>
            </owl:Restriction>
        </rdfs:subClassOf>
        <rdfs:subClassOf>
            <owl:Restriction>
                <owl:onProperty rdf:resource="time:hasTemporalDuration"/>
                <owl:allValuesFrom rdf:resource="time:TemporalDuration"/>
            </owl:Restriction>
        </rdfs:subClassOf>
        <rdfs:subClassOf>
            <owl:Restriction>
                <owl:onProperty rdf:resource="time:hasXSDDuration"/>
                <owl:allValuesFrom rdf:resource="xsd:duration"/>
            </owl:Restriction>
        </rdfs:subClassOf>
        <rdfs:comment xml:lang="en">A temporal interval or instant.</rdfs:comment>
        <rdfs:comment xml:lang="es">Un intervalo temporal o un instante.</rdfs:comment>
        <rdfs:label xml:lang="en">Temporal entity</rdfs:label>
        <rdfs:label xml:lang="es">entidad temporal</rdfs:label>
        <skos:definition xml:lang="en">A temporal interval or instant.</skos:definition>
        <skos:definition xml:lang="es">Un intervalo temporal o un instante.</skos:definition>
    </owl:Class>
    


    <!-- http://www.w3.org/2006/time#TemporalPosition -->

    <owl:Class rdf:about="http://www.w3.org/2006/time#TemporalPosition">
        <rdfs:subClassOf rdf:resource="https://w3id.org/isoiec5087/-1/v1/TimeOntologyThing"/>
        <rdfs:subClassOf>
            <owl:Restriction>
                <owl:onProperty rdf:resource="time:hasTRS"/>
                <owl:cardinality rdf:datatype="xsd:nonNegativeInteger">1</owl:cardinality>
            </owl:Restriction>
        </rdfs:subClassOf>
        <rdfs:comment xml:lang="en">A position on a time-line</rdfs:comment>
        <rdfs:comment xml:lang="es">Una posición sobre una línea de tiempo.</rdfs:comment>
        <rdfs:label xml:lang="en">Temporal position</rdfs:label>
        <rdfs:label xml:lang="es">posición temporal</rdfs:label>
        <skos:definition xml:lang="en">A position on a time-line</skos:definition>
        <skos:definition xml:lang="es">Una posición sobre una línea de tiempo.</skos:definition>
    </owl:Class>
    


    <!-- http://www.w3.org/2006/time#TemporalUnit -->

    <owl:Class rdf:about="http://www.w3.org/2006/time#TemporalUnit">
        <rdfs:subClassOf rdf:resource="time:TemporalDuration"/>
        <rdfs:comment xml:lang="en">A standard duration, which provides a scale factor for a time extent, or the granularity or precision for a time position.</rdfs:comment>
        <rdfs:comment xml:lang="es">Una duración estándar, que proporciona un factor de escala para una extensión de tiempo, o la granularidad o precisión para una posición de tiempo.</rdfs:comment>
        <rdfs:label xml:lang="en">Temporal unit</rdfs:label>
        <rdfs:label xml:lang="es">unidad de tiempo</rdfs:label>
        <skos:changeNote xml:lang="en">Remove enumeration from definition, in order to allow other units to be used when required in other coordinate systems. 
NOTE: existing units are still present as members of the class, but the class membership is now open. 

In the original OWL-Time the following constraint appeared: 
  owl:oneOf (
      time:unitSecond
      time:unitMinute
      time:unitHour
      time:unitDay
      time:unitWeek
      time:unitMonth
      time:unitYear
    ) ;</skos:changeNote>
        <skos:definition xml:lang="en">A standard duration, which provides a scale factor for a time extent, or the granularity or precision for a time position.</skos:definition>
        <skos:definition xml:lang="es">Una duración estándar, que proporciona un factor de escala para una extensión de tiempo, o la granularidad o precisión para una posición de tiempo.</skos:definition>
        <skos:note xml:lang="es">La pertenencia de la clase &apos;unidad de tiempo&apos; está abierta, para permitir otras unidades de tiempo utilizadas en algunas aplicaciones técnicas (por ejemplo, millones de años o el mes Baha&apos;i).</skos:note>
        <skos:note xml:lang="en">Membership of the class TemporalUnit is open, to allow for other temporal units used in some technical applications (e.g. millions of years, Baha&apos;i month).</skos:note>
    </owl:Class>
    


    <!-- http://www.w3.org/2006/time#TimePosition -->

    <owl:Class rdf:about="http://www.w3.org/2006/time#TimePosition">
        <rdfs:subClassOf rdf:resource="time:TemporalPosition"/>
        <rdfs:subClassOf>
            <owl:Class>
                <owl:unionOf rdf:parseType="Collection">
                    <owl:Restriction>
                        <owl:onProperty rdf:resource="time:nominalPosition"/>
                        <owl:cardinality rdf:datatype="xsd:nonNegativeInteger">1</owl:cardinality>
                    </owl:Restriction>
                    <owl:Restriction>
                        <owl:onProperty rdf:resource="time:numericPosition"/>
                        <owl:cardinality rdf:datatype="xsd:nonNegativeInteger">1</owl:cardinality>
                    </owl:Restriction>
                </owl:unionOf>
            </owl:Class>
        </rdfs:subClassOf>
        <rdfs:comment xml:lang="en">A temporal position described using either a (nominal) value from an ordinal reference system, or a (numeric) value in a temporal coordinate system. </rdfs:comment>
        <rdfs:comment xml:lang="es">Una posición temporal descrita utilizando bien un valor (nominal) de un sistema de referencia ordinal, o un valor (numérico) en un sistema de coordenadas temporales.</rdfs:comment>
        <rdfs:label xml:lang="en">Time position</rdfs:label>
        <rdfs:label xml:lang="es">posición de tiempo</rdfs:label>
        <skos:definition xml:lang="en">A temporal position described using either a (nominal) value from an ordinal reference system, or a (numeric) value in a temporal coordinate system. </skos:definition>
        <skos:definition xml:lang="es">Una posición temporal descrita utilizando bien un valor (nominal) de un sistema de referencia ordinal, o un valor (numérico) en un sistema de coordenadas temporales.</skos:definition>
    </owl:Class>
    


    <!-- http://www.w3.org/2006/time#TimeZone -->

    <owl:Class rdf:about="http://www.w3.org/2006/time#TimeZone">
        <rdfs:subClassOf rdf:resource="https://w3id.org/isoiec5087/-1/v1/TimeOntologyThing"/>
        <rdfs:comment xml:lang="en">A Time Zone specifies the amount by which the local time is offset from UTC. 
	A time zone is usually denoted geographically (e.g. Australian Eastern Daylight Time), with a constant value in a given region. 
The region where it applies and the offset from UTC are specified by a locally recognised governing authority.</rdfs:comment>
        <rdfs:comment xml:lang="es">Un huso horario especifica la cantidad en que la hora local está desplazada con respecto a UTC.
        Un huso horario normalmente se denota geográficamente (p.ej. el horario de verano del este de Australia), con un valor constante en una región dada.
        La región donde aplica y el desplazamiento desde UTC las especifica una autoridad gubernamental localmente reconocida.</rdfs:comment>
        <rdfs:label xml:lang="en">Time Zone</rdfs:label>
        <rdfs:label xml:lang="es">huso horario</rdfs:label>
        <skos:definition xml:lang="en">A Time Zone specifies the amount by which the local time is offset from UTC. 
	A time zone is usually denoted geographically (e.g. Australian Eastern Daylight Time), with a constant value in a given region. 
The region where it applies and the offset from UTC are specified by a locally recognised governing authority.</skos:definition>
        <skos:definition xml:lang="es">Un huso horario especifica la cantidad en que la hora local está desplazada con respecto a UTC.
    Un huso horario normalmente se denota geográficamente (p.ej. el horario de verano del este de Australia), con un valor constante en una región dada.
    La región donde aplica y el desplazamiento desde UTC las especifica una autoridad gubernamental localmente reconocida.</skos:definition>
        <skos:historyNote xml:lang="es">En la versión original de OWL-Time de 2006, se definió, en un espacio de nombres diferente &quot;http://www.w3.org/2006/timezone#&quot;, la clase &apos;huso horario&apos;, con varias propiedades específicas correspondientes a un modelo específico de huso horario.
    En la versión actual hay una clase con el mismo nombre local en el espacio de nombres de OWL-Time, eliminando la dependencia del espacio de nombres externo.
    Un axioma de alineación permite que los datos codificados de acuerdo con la versión anterior sean consistentes con la ontología actualizada.</skos:historyNote>
        <skos:historyNote>In the original 2006 version of OWL-Time, the TimeZone class, with several properties corresponding to a specific model of time-zones, was defined in a separate namespace &quot;http://www.w3.org/2006/timezone#&quot;. 

In the current version a class with same local name is put into the main OWL-Time namespace, removing the dependency on the external namespace. 

An alignment axiom 
	tzont:TimeZone rdfs:subClassOf time:TimeZone . 
allows data encoded according to the previous version to be consistent with the updated ontology. </skos:historyNote>
        <skos:note xml:lang="en">A designated timezone is associated with a geographic region. However, for a particular region the offset from UTC often varies seasonally, and the dates of the changes may vary from year to year. The timezone designation usually changes for the different seasons (e.g. Australian Eastern Standard Time vs. Australian Eastern Daylight Time). Furthermore, the offset for a timezone may change over longer timescales, though its designation might not.  

Detailed guidance about working with time zones is given in http://www.w3.org/TR/timezone/ .</skos:note>
        <skos:note xml:lang="en">An ontology for time zone descriptions was described in [owl-time-20060927] and provided as RDF in a separate namespace tzont:. However, that ontology was incomplete in scope, and the example datasets were selective. Furthermore, since the use of a class from an external ontology as the range of an ObjectProperty in OWL-Time creates a dependency, reference to the time zone class has been replaced with the &apos;stub&apos; class in the normative part of this version of OWL-Time.</skos:note>
        <skos:note xml:lang="es">Un huso horario designado está asociado con una región geográfica. Sin embargo, para una región particular el desplazamiento desde UTC a menudo varía según las estaciones, y las fechas de los cambios pueden variar de un año a otro. La designación de huso horario  normalmente cambia de una estación a otra (por ejemplo, el horario estándar frente al horario de verano ambos del este de Australia). Además, del desplazamiento para un huso horario puede cambiar sobre escalas de tiempo mayores, aunque su designación no lo haga.
    Se puede encontrar una guía detallada sobre el funcionamiento de husos horarios en http://www.w3.org/TR/timezone/.&quot;@es , &quot;En [owl-time-20060927] se describió una ontología para descripciones de husos horarios, y se proporcionó en un espacio de nombres separado tzont:. Sin embargo, dicha ontología estaba incompleta en su alcance, y el ejemplo de conjuntos de datos (datasets) era selectivo. Además, puesto que el uso de una clase de una ontología externa como el rango de una propiedad de objeto en OWL-Time crea una dependencia, la referencia a la clase huso horario se ha reemplazado por una clase que viene a ser un &quot;cajón de sastre&quot; en la en la parte normativa de esta versión de OWL-Time.</skos:note>
        <skos:scopeNote xml:lang="es">En esta implementación &apos;huso horario&apos; no tiene definidas propiedades. Se debería pensar como una superclase &quot;abstracta&quot; de todas las implementaciones de huso horario específicas.</skos:scopeNote>
        <skos:scopeNote>In this implementation TimeZone has no properties defined. It should be thought of as an &apos;abstract&apos; superclass of all specific timezone implementations.</skos:scopeNote>
    </owl:Class>
    


    <!-- http://www.w3.org/2006/time#Year -->

    <owl:Class rdf:about="http://www.w3.org/2006/time#Year">
        <rdfs:subClassOf rdf:resource="time:DurationDescription"/>
        <rdfs:subClassOf>
            <owl:Restriction>
                <owl:onProperty rdf:resource="time:days"/>
                <owl:cardinality rdf:datatype="xsd:nonNegativeInteger">0</owl:cardinality>
            </owl:Restriction>
        </rdfs:subClassOf>
        <rdfs:subClassOf>
            <owl:Restriction>
                <owl:onProperty rdf:resource="time:hours"/>
                <owl:cardinality rdf:datatype="xsd:nonNegativeInteger">0</owl:cardinality>
            </owl:Restriction>
        </rdfs:subClassOf>
        <rdfs:subClassOf>
            <owl:Restriction>
                <owl:onProperty rdf:resource="time:minutes"/>
                <owl:cardinality rdf:datatype="xsd:nonNegativeInteger">0</owl:cardinality>
            </owl:Restriction>
        </rdfs:subClassOf>
        <rdfs:subClassOf>
            <owl:Restriction>
                <owl:onProperty rdf:resource="time:months"/>
                <owl:cardinality rdf:datatype="xsd:nonNegativeInteger">0</owl:cardinality>
            </owl:Restriction>
        </rdfs:subClassOf>
        <rdfs:subClassOf>
            <owl:Restriction>
                <owl:onProperty rdf:resource="time:seconds"/>
                <owl:cardinality rdf:datatype="xsd:nonNegativeInteger">0</owl:cardinality>
            </owl:Restriction>
        </rdfs:subClassOf>
        <rdfs:subClassOf>
            <owl:Restriction>
                <owl:onProperty rdf:resource="time:weeks"/>
                <owl:cardinality rdf:datatype="xsd:nonNegativeInteger">0</owl:cardinality>
            </owl:Restriction>
        </rdfs:subClassOf>
        <rdfs:subClassOf>
            <owl:Restriction>
                <owl:onProperty rdf:resource="time:years"/>
                <owl:cardinality rdf:datatype="xsd:nonNegativeInteger">1</owl:cardinality>
            </owl:Restriction>
        </rdfs:subClassOf>
        <rdfs:comment>Year duration</rdfs:comment>
        <rdfs:label xml:lang="en">Year</rdfs:label>
        <owl:deprecated rdf:datatype="xsd:boolean">true</owl:deprecated>
        <skos:definition>Year duration</skos:definition>
        <skos:historyNote>Year was proposed in the 2006 version of OWL-Time as an example of how DurationDescription could be specialized to allow for a duration to be restricted to a number of years. 

It is deprecated in this edition of OWL-Time. </skos:historyNote>
        <skos:prefLabel xml:lang="it">Anno</skos:prefLabel>
        <skos:prefLabel xml:lang="fr">Année (calendrier)</skos:prefLabel>
        <skos:prefLabel xml:lang="pt">Ano</skos:prefLabel>
        <skos:prefLabel xml:lang="es">Año</skos:prefLabel>
        <skos:prefLabel xml:lang="nl">Jaar</skos:prefLabel>
        <skos:prefLabel xml:lang="de">Jahr</skos:prefLabel>
        <skos:prefLabel xml:lang="pl">Rok</skos:prefLabel>
        <skos:prefLabel xml:lang="en">Year</skos:prefLabel>
        <skos:prefLabel xml:lang="ru">Год</skos:prefLabel>
        <skos:prefLabel xml:lang="ar">سنة</skos:prefLabel>
        <skos:prefLabel xml:lang="ja">年</skos:prefLabel>
        <skos:prefLabel xml:lang="zh">年</skos:prefLabel>
    </owl:Class>
    


    <!-- 
    ///////////////////////////////////////////////////////////////////////////////////////
    //
    // Individuals
    //
    ///////////////////////////////////////////////////////////////////////////////////////
     -->

    


    <!-- http://www.opengis.net/def/uom/ISO-8601/0/Gregorian -->

    <owl:NamedIndividual rdf:about="http://www.opengis.net/def/uom/ISO-8601/0/Gregorian"/>
    


    <!-- http://www.w3.org/2006/time#Friday -->

    <owl:NamedIndividual rdf:about="http://www.w3.org/2006/time#Friday">
        <rdf:type rdf:resource="time:DayOfWeek"/>
        <rdfs:label xml:lang="en">Friday</rdfs:label>
        <skos:prefLabel xml:lang="de">Freitag</skos:prefLabel>
        <skos:prefLabel xml:lang="en">Friday</skos:prefLabel>
        <skos:prefLabel xml:lang="pl">Piątek</skos:prefLabel>
        <skos:prefLabel xml:lang="pt">Sexta-feira</skos:prefLabel>
        <skos:prefLabel xml:lang="fr">Vendredi</skos:prefLabel>
        <skos:prefLabel xml:lang="it">Venerdì</skos:prefLabel>
        <skos:prefLabel xml:lang="es">Viernes</skos:prefLabel>
        <skos:prefLabel xml:lang="nl">Vrijdag</skos:prefLabel>
        <skos:prefLabel xml:lang="ru">Пятница</skos:prefLabel>
        <skos:prefLabel xml:lang="ar">الجمعة</skos:prefLabel>
        <skos:prefLabel xml:lang="zh">星期五</skos:prefLabel>
        <skos:prefLabel xml:lang="ja">金曜日</skos:prefLabel>
    </owl:NamedIndividual>
    


    <!-- http://www.w3.org/2006/time#Monday -->

    <owl:NamedIndividual rdf:about="http://www.w3.org/2006/time#Monday">
        <rdf:type rdf:resource="time:DayOfWeek"/>
        <rdfs:label xml:lang="en">Monday</rdfs:label>
        <skos:prefLabel xml:lang="fr">Lundi</skos:prefLabel>
        <skos:prefLabel xml:lang="it">Lunedì</skos:prefLabel>
        <skos:prefLabel xml:lang="es">Lunes</skos:prefLabel>
        <skos:prefLabel xml:lang="nl">Maandag</skos:prefLabel>
        <skos:prefLabel xml:lang="en">Monday</skos:prefLabel>
        <skos:prefLabel xml:lang="de">Montag</skos:prefLabel>
        <skos:prefLabel xml:lang="pl">Poniedziałek</skos:prefLabel>
        <skos:prefLabel xml:lang="pt">Segunda-feira</skos:prefLabel>
        <skos:prefLabel xml:lang="ru">Понедельник</skos:prefLabel>
        <skos:prefLabel xml:lang="ar">الاثنين</skos:prefLabel>
        <skos:prefLabel xml:lang="zh">星期一</skos:prefLabel>
        <skos:prefLabel xml:lang="ja">月曜日</skos:prefLabel>
    </owl:NamedIndividual>
    


    <!-- http://www.w3.org/2006/time#Saturday -->

    <owl:NamedIndividual rdf:about="http://www.w3.org/2006/time#Saturday">
        <rdf:type rdf:resource="time:DayOfWeek"/>
        <rdfs:label xml:lang="en">Saturday</rdfs:label>
        <skos:prefLabel xml:lang="it">Sabato</skos:prefLabel>
        <skos:prefLabel xml:lang="fr">Samedi</skos:prefLabel>
        <skos:prefLabel xml:lang="de">Samstag</skos:prefLabel>
        <skos:prefLabel xml:lang="en">Saturday</skos:prefLabel>
        <skos:prefLabel xml:lang="pl">Sobota</skos:prefLabel>
        <skos:prefLabel xml:lang="es">Sábado</skos:prefLabel>
        <skos:prefLabel xml:lang="pt">Sábado</skos:prefLabel>
        <skos:prefLabel xml:lang="nl">Zaterdag</skos:prefLabel>
        <skos:prefLabel xml:lang="ru">Суббота</skos:prefLabel>
        <skos:prefLabel xml:lang="ar">السبت</skos:prefLabel>
        <skos:prefLabel xml:lang="ja">土曜日</skos:prefLabel>
        <skos:prefLabel xml:lang="zh">星期六</skos:prefLabel>
    </owl:NamedIndividual>
    


    <!-- http://www.w3.org/2006/time#Sunday -->

    <owl:NamedIndividual rdf:about="http://www.w3.org/2006/time#Sunday">
        <rdf:type rdf:resource="time:DayOfWeek"/>
        <rdfs:label xml:lang="en">Sunday</rdfs:label>
        <skos:prefLabel xml:lang="fr">Dimanche</skos:prefLabel>
        <skos:prefLabel xml:lang="it">Domenica</skos:prefLabel>
        <skos:prefLabel xml:lang="es">Domingo</skos:prefLabel>
        <skos:prefLabel xml:lang="pt">Domingo</skos:prefLabel>
        <skos:prefLabel xml:lang="pl">Niedziela</skos:prefLabel>
        <skos:prefLabel xml:lang="de">Sonntag</skos:prefLabel>
        <skos:prefLabel xml:lang="en">Sunday</skos:prefLabel>
        <skos:prefLabel xml:lang="nl">Zondag</skos:prefLabel>
        <skos:prefLabel xml:lang="ru">Воскресенье</skos:prefLabel>
        <skos:prefLabel xml:lang="ar">الأحد (يوم)</skos:prefLabel>
        <skos:prefLabel xml:lang="ja">日曜日</skos:prefLabel>
        <skos:prefLabel xml:lang="zh">星期日</skos:prefLabel>
    </owl:NamedIndividual>
    


    <!-- http://www.w3.org/2006/time#Thursday -->

    <owl:NamedIndividual rdf:about="http://www.w3.org/2006/time#Thursday">
        <rdf:type rdf:resource="time:DayOfWeek"/>
        <rdfs:label xml:lang="en">Thursday</rdfs:label>
        <skos:prefLabel xml:lang="pl">Czwartek</skos:prefLabel>
        <skos:prefLabel xml:lang="nl">Donderdag</skos:prefLabel>
        <skos:prefLabel xml:lang="de">Donnerstag</skos:prefLabel>
        <skos:prefLabel xml:lang="it">Giovedì</skos:prefLabel>
        <skos:prefLabel xml:lang="fr">Jeudi</skos:prefLabel>
        <skos:prefLabel xml:lang="es">Jueves</skos:prefLabel>
        <skos:prefLabel xml:lang="pt">Quinta-feira</skos:prefLabel>
        <skos:prefLabel xml:lang="en">Thursday</skos:prefLabel>
        <skos:prefLabel xml:lang="ru">Четверг</skos:prefLabel>
        <skos:prefLabel xml:lang="ar">الخميس</skos:prefLabel>
        <skos:prefLabel xml:lang="zh">星期四</skos:prefLabel>
        <skos:prefLabel xml:lang="ja">木曜日</skos:prefLabel>
    </owl:NamedIndividual>
    


    <!-- http://www.w3.org/2006/time#Tuesday -->

    <owl:NamedIndividual rdf:about="http://www.w3.org/2006/time#Tuesday">
        <rdf:type rdf:resource="time:DayOfWeek"/>
        <rdfs:label xml:lang="en">Tuesday</rdfs:label>
        <skos:prefLabel xml:lang="de">Dienstag</skos:prefLabel>
        <skos:prefLabel xml:lang="nl">Dinsdag</skos:prefLabel>
        <skos:prefLabel xml:lang="fr">Mardi</skos:prefLabel>
        <skos:prefLabel xml:lang="it">Martedì</skos:prefLabel>
        <skos:prefLabel xml:lang="es">Martes</skos:prefLabel>
        <skos:prefLabel xml:lang="pt">Terça-feira</skos:prefLabel>
        <skos:prefLabel xml:lang="en">Tuesday</skos:prefLabel>
        <skos:prefLabel xml:lang="pl">Wtorek</skos:prefLabel>
        <skos:prefLabel xml:lang="ru">Вторник</skos:prefLabel>
        <skos:prefLabel xml:lang="ar">الثلاثاء</skos:prefLabel>
        <skos:prefLabel xml:lang="zh">星期二</skos:prefLabel>
        <skos:prefLabel xml:lang="ja">火曜日</skos:prefLabel>
    </owl:NamedIndividual>
    


    <!-- http://www.w3.org/2006/time#Wednesday -->

    <owl:NamedIndividual rdf:about="http://www.w3.org/2006/time#Wednesday">
        <rdf:type rdf:resource="time:DayOfWeek"/>
        <rdfs:label xml:lang="en">Wednesday</rdfs:label>
        <skos:prefLabel xml:lang="it">Mercoledì</skos:prefLabel>
        <skos:prefLabel xml:lang="fr">Mercredi</skos:prefLabel>
        <skos:prefLabel xml:lang="de">Mittwoch</skos:prefLabel>
        <skos:prefLabel xml:lang="es">Miércoles</skos:prefLabel>
        <skos:prefLabel xml:lang="pt">Quarta-feira</skos:prefLabel>
        <skos:prefLabel xml:lang="en">Wednesday</skos:prefLabel>
        <skos:prefLabel xml:lang="nl">Woensdag</skos:prefLabel>
        <skos:prefLabel xml:lang="pl">Środa</skos:prefLabel>
        <skos:prefLabel xml:lang="ru">Среда</skos:prefLabel>
        <skos:prefLabel xml:lang="ar">الأربعاء</skos:prefLabel>
        <skos:prefLabel xml:lang="zh">星期三</skos:prefLabel>
        <skos:prefLabel xml:lang="ja">水曜日</skos:prefLabel>
    </owl:NamedIndividual>
    


    <!-- http://www.w3.org/2006/time#unitDay -->

    <owl:NamedIndividual rdf:about="http://www.w3.org/2006/time#unitDay">
        <rdf:type rdf:resource="time:TemporalUnit"/>
        <time:days rdf:datatype="xsd:decimal">1</time:days>
        <time:hours rdf:datatype="xsd:decimal">0</time:hours>
        <time:minutes rdf:datatype="xsd:decimal">0</time:minutes>
        <time:months rdf:datatype="xsd:decimal">0</time:months>
        <time:seconds rdf:datatype="xsd:decimal">0</time:seconds>
        <time:weeks rdf:datatype="xsd:decimal">0</time:weeks>
        <time:years rdf:datatype="xsd:decimal">0</time:years>
        <rdfs:label xml:lang="en">Day (unit of temporal duration)</rdfs:label>
        <skos:prefLabel xml:lang="de">Tag</skos:prefLabel>
        <skos:prefLabel xml:lang="nl">dag</skos:prefLabel>
        <skos:prefLabel xml:lang="en">day</skos:prefLabel>
        <skos:prefLabel xml:lang="pt">dia</skos:prefLabel>
        <skos:prefLabel xml:lang="pl">doba</skos:prefLabel>
        <skos:prefLabel xml:lang="es">día</skos:prefLabel>
        <skos:prefLabel xml:lang="it">giorno</skos:prefLabel>
        <skos:prefLabel xml:lang="fr">jour</skos:prefLabel>
        <skos:prefLabel xml:lang="ar">يوماً ما</skos:prefLabel>
        <skos:prefLabel xml:lang="jp">ある日</skos:prefLabel>
        <skos:prefLabel xml:lang="zh">一天</skos:prefLabel>
        <skos:prefLabel xml:lang="kr">언젠가</skos:prefLabel>
    </owl:NamedIndividual>
    


    <!-- http://www.w3.org/2006/time#unitHour -->

    <owl:NamedIndividual rdf:about="http://www.w3.org/2006/time#unitHour">
        <rdf:type rdf:resource="time:TemporalUnit"/>
        <time:days rdf:datatype="xsd:decimal">0</time:days>
        <time:hours rdf:datatype="xsd:decimal">1</time:hours>
        <time:minutes rdf:datatype="xsd:decimal">0</time:minutes>
        <time:months rdf:datatype="xsd:decimal">0</time:months>
        <time:seconds rdf:datatype="xsd:decimal">0</time:seconds>
        <time:weeks rdf:datatype="xsd:decimal">0</time:weeks>
        <time:years rdf:datatype="xsd:decimal">0</time:years>
        <rdfs:label xml:lang="en">Hour (unit of temporal duration)</rdfs:label>
        <skos:prefLabel xml:lang="de">Stunde</skos:prefLabel>
        <skos:prefLabel xml:lang="pl">godzina</skos:prefLabel>
        <skos:prefLabel xml:lang="fr">heure</skos:prefLabel>
        <skos:prefLabel xml:lang="es">hora</skos:prefLabel>
        <skos:prefLabel xml:lang="pt">hora</skos:prefLabel>
        <skos:prefLabel xml:lang="en">hour</skos:prefLabel>
        <skos:prefLabel xml:lang="it">ora</skos:prefLabel>
        <skos:prefLabel xml:lang="nl">uur</skos:prefLabel>
        <skos:prefLabel>один час&quot;@ru</skos:prefLabel>
        <skos:prefLabel xml:lang="ar">ساعة واحدة</skos:prefLabel>
        <skos:prefLabel xml:lang="zh">一小時</skos:prefLabel>
        <skos:prefLabel xml:lang="jp">一時間</skos:prefLabel>
        <skos:prefLabel xml:lang="kr">한 시간</skos:prefLabel>
    </owl:NamedIndividual>
    


    <!-- http://www.w3.org/2006/time#unitMinute -->

    <owl:NamedIndividual rdf:about="http://www.w3.org/2006/time#unitMinute">
        <rdf:type rdf:resource="time:TemporalUnit"/>
        <time:days rdf:datatype="xsd:decimal">0</time:days>
        <time:hours rdf:datatype="xsd:decimal">0</time:hours>
        <time:minutes rdf:datatype="xsd:decimal">1</time:minutes>
        <time:months rdf:datatype="xsd:decimal">0</time:months>
        <time:seconds rdf:datatype="xsd:decimal">0</time:seconds>
        <time:weeks rdf:datatype="xsd:decimal">0</time:weeks>
        <time:years rdf:datatype="xsd:decimal">0</time:years>
        <rdfs:label xml:lang="en">Minute (unit of temporal duration)</rdfs:label>
        <skos:prefLabel xml:lang="de">Minute</skos:prefLabel>
        <skos:prefLabel xml:lang="pl">minuta</skos:prefLabel>
        <skos:prefLabel xml:lang="en">minute</skos:prefLabel>
        <skos:prefLabel xml:lang="fr">minute</skos:prefLabel>
        <skos:prefLabel xml:lang="es">minuto</skos:prefLabel>
        <skos:prefLabel xml:lang="it">minuto</skos:prefLabel>
        <skos:prefLabel xml:lang="pt">minuto</skos:prefLabel>
        <skos:prefLabel xml:lang="nl">minuut</skos:prefLabel>
        <skos:prefLabel xml:lang="ru">одна минута</skos:prefLabel>
        <skos:prefLabel xml:lang="ar">دقيقة واحدة</skos:prefLabel>
        <skos:prefLabel xml:lang="jp">一分</skos:prefLabel>
        <skos:prefLabel xml:lang="zh">等一下</skos:prefLabel>
        <skos:prefLabel xml:lang="kr">분</skos:prefLabel>
    </owl:NamedIndividual>
    


    <!-- http://www.w3.org/2006/time#unitMonth -->

    <owl:NamedIndividual rdf:about="http://www.w3.org/2006/time#unitMonth">
        <rdf:type rdf:resource="time:TemporalUnit"/>
        <time:days rdf:datatype="xsd:decimal">0</time:days>
        <time:hours rdf:datatype="xsd:decimal">0</time:hours>
        <time:minutes rdf:datatype="xsd:decimal">0</time:minutes>
        <time:months rdf:datatype="xsd:decimal">1</time:months>
        <time:seconds rdf:datatype="xsd:decimal">0</time:seconds>
        <time:weeks rdf:datatype="xsd:decimal">0</time:weeks>
        <time:years rdf:datatype="xsd:decimal">0</time:years>
        <rdfs:label xml:lang="en">Month (unit of temporal duration)</rdfs:label>
        <skos:prefLabel xml:lang="de">Monat</skos:prefLabel>
        <skos:prefLabel xml:lang="nl">maand</skos:prefLabel>
        <skos:prefLabel xml:lang="es">mes</skos:prefLabel>
        <skos:prefLabel xml:lang="it">mese</skos:prefLabel>
        <skos:prefLabel xml:lang="pl">miesiąc</skos:prefLabel>
        <skos:prefLabel xml:lang="fr">mois</skos:prefLabel>
        <skos:prefLabel xml:lang="de">monat</skos:prefLabel>
        <skos:prefLabel xml:lang="en">month</skos:prefLabel>
        <skos:prefLabel xml:lang="ru">один месяц</skos:prefLabel>
        <skos:prefLabel xml:lang="ar">شهر واحد</skos:prefLabel>
        <skos:prefLabel xml:lang="jp">一か月</skos:prefLabel>
        <skos:prefLabel xml:lang="zh">一個月</skos:prefLabel>
        <skos:prefLabel xml:lang="kr">한달</skos:prefLabel>
    </owl:NamedIndividual>
    


    <!-- http://www.w3.org/2006/time#unitSecond -->

    <owl:NamedIndividual rdf:about="http://www.w3.org/2006/time#unitSecond">
        <rdf:type rdf:resource="time:TemporalUnit"/>
        <time:days rdf:datatype="xsd:decimal">0</time:days>
        <time:hours rdf:datatype="xsd:decimal">0</time:hours>
        <time:minutes rdf:datatype="xsd:decimal">0</time:minutes>
        <time:months rdf:datatype="xsd:decimal">0</time:months>
        <time:seconds rdf:datatype="xsd:decimal">1</time:seconds>
        <time:weeks rdf:datatype="xsd:decimal">0</time:weeks>
        <time:years rdf:datatype="xsd:decimal">0</time:years>
        <rdfs:label xml:lang="en">Second (unit of temporal duration)</rdfs:label>
        <skos:prefLabel xml:lang="de">Sekunde</skos:prefLabel>
        <skos:prefLabel xml:lang="pl">Sekundę</skos:prefLabel>
        <skos:prefLabel xml:lang="en">second</skos:prefLabel>
        <skos:prefLabel xml:lang="fr">seconde</skos:prefLabel>
        <skos:prefLabel xml:lang="nl">seconde</skos:prefLabel>
        <skos:prefLabel xml:lang="it">secondo</skos:prefLabel>
        <skos:prefLabel xml:lang="es">segundo</skos:prefLabel>
        <skos:prefLabel xml:lang="pt">segundo</skos:prefLabel>
        <skos:prefLabel xml:lang="ar">ثانية واحدة</skos:prefLabel>
        <skos:prefLabel xml:lang="jp">一秒</skos:prefLabel>
        <skos:prefLabel xml:lang="zh">一秒</skos:prefLabel>
        <skos:prefLabel xml:lang="kr">일초</skos:prefLabel>
    </owl:NamedIndividual>
    


    <!-- http://www.w3.org/2006/time#unitWeek -->

    <owl:NamedIndividual rdf:about="http://www.w3.org/2006/time#unitWeek">
        <rdf:type rdf:resource="time:TemporalUnit"/>
        <time:days rdf:datatype="xsd:decimal">0</time:days>
        <time:hours rdf:datatype="xsd:decimal">0</time:hours>
        <time:minutes rdf:datatype="xsd:decimal">0</time:minutes>
        <time:months rdf:datatype="xsd:decimal">0</time:months>
        <time:seconds rdf:datatype="xsd:decimal">0</time:seconds>
        <time:weeks rdf:datatype="xsd:decimal">1</time:weeks>
        <time:years rdf:datatype="xsd:decimal">0</time:years>
        <rdfs:label xml:lang="en">Week (unit of temporal duration)</rdfs:label>
        <skos:prefLabel xml:lang="de">Woche</skos:prefLabel>
        <skos:prefLabel xml:lang="fr">semaine</skos:prefLabel>
        <skos:prefLabel xml:lang="es">semana</skos:prefLabel>
        <skos:prefLabel xml:lang="pt">semana</skos:prefLabel>
        <skos:prefLabel xml:lang="it">settimana</skos:prefLabel>
        <skos:prefLabel xml:lang="pl">tydzień</skos:prefLabel>
        <skos:prefLabel xml:lang="en">week</skos:prefLabel>
        <skos:prefLabel xml:lang="nl">week</skos:prefLabel>
        <skos:prefLabel xml:lang="ru">одна неделя</skos:prefLabel>
        <skos:prefLabel xml:lang="ar">سبوع واحد</skos:prefLabel>
        <skos:prefLabel xml:lang="zh">一周</skos:prefLabel>
        <skos:prefLabel xml:lang="jp">一週間</skos:prefLabel>
        <skos:prefLabel xml:lang="kr">일주일</skos:prefLabel>
    </owl:NamedIndividual>
    


    <!-- http://www.w3.org/2006/time#unitYear -->

    <owl:NamedIndividual rdf:about="http://www.w3.org/2006/time#unitYear">
        <rdf:type rdf:resource="time:TemporalUnit"/>
        <time:days rdf:datatype="xsd:decimal">0</time:days>
        <time:hours rdf:datatype="xsd:decimal">0</time:hours>
        <time:minutes rdf:datatype="xsd:decimal">0</time:minutes>
        <time:months rdf:datatype="xsd:decimal">0</time:months>
        <time:seconds rdf:datatype="xsd:decimal">0</time:seconds>
        <time:weeks rdf:datatype="xsd:decimal">0</time:weeks>
        <time:years rdf:datatype="xsd:decimal">1</time:years>
        <rdfs:label xml:lang="en">Year (unit of temporal duration)</rdfs:label>
        <skos:prefLabel xml:lang="kr">1 년</skos:prefLabel>
        <skos:prefLabel xml:lang="jp">1年</skos:prefLabel>
        <skos:prefLabel xml:lang="de">Jahr</skos:prefLabel>
        <skos:prefLabel xml:lang="pl">Rok</skos:prefLabel>
        <skos:prefLabel xml:lang="fr">an</skos:prefLabel>
        <skos:prefLabel xml:lang="it">anno</skos:prefLabel>
        <skos:prefLabel xml:lang="pt">ano</skos:prefLabel>
        <skos:prefLabel xml:lang="nl">jaar</skos:prefLabel>
        <skos:prefLabel xml:lang="pl">rok</skos:prefLabel>
        <skos:prefLabel xml:lang="es">un año</skos:prefLabel>
        <skos:prefLabel xml:lang="en">year</skos:prefLabel>
        <skos:prefLabel xml:lang="ru">один год</skos:prefLabel>
        <skos:prefLabel xml:lang="ar">سنة واحدة</skos:prefLabel>
        <skos:prefLabel xml:lang="zh">一年</skos:prefLabel>
    </owl:NamedIndividual>
    <rdf:Description>
        <xsd:pattern>-?([1-9][0-9]{3,}|0[0-9]{3})(Z|(\+|-)((0[0-9]|1[0-3]):[0-5][0-9]|14:00))?</xsd:pattern>
    </rdf:Description>
    <rdf:Description>
        <xsd:pattern>---(0[1-9]|[1-9][0-9])(Z|(\+|-)((0[0-9]|1[0-3]):[0-5][0-9]|14:00))?</xsd:pattern>
    </rdf:Description>
    <rdf:Description>
        <xsd:pattern>--(0[1-9]|1[0-9]|20)(Z|(\+|-)((0[0-9]|1[0-3]):[0-5][0-9]|14:00))?</xsd:pattern>
    </rdf:Description>
    <rdf:Description>
        <xsd:pattern>-?([1-9][0-9]{3,}|0[0-9]{3})(Z|(\+|-)((0[0-9]|1[0-3]):[0-5][0-9]|14:00))?</xsd:pattern>
    </rdf:Description>
    <rdf:Description>
        <xsd:pattern>---(0[1-9]|[1-9][0-9])(Z|(\+|-)((0[0-9]|1[0-3]):[0-5][0-9]|14:00))?</xsd:pattern>
    </rdf:Description>
    <rdf:Description>
        <xsd:pattern>--(0[1-9]|1[0-9]|20)(Z|(\+|-)((0[0-9]|1[0-3]):[0-5][0-9]|14:00))?</xsd:pattern>
    </rdf:Description>
</rdf:RDF>
