<?xml version="1.0"?>
<rdf:RDF xmlns="https://w3id.org/citydata/part1/v1/"
     xml:base="https://w3id.org/citydata/part1/v1/"
     xmlns:cc="http://creativecommons.org/ns#"
     xmlns:dcterms="http://purl.org/dc/terms/"
     xmlns:owl="http://www.w3.org/2002/07/owl#"
     xmlns:rdf="http://www.w3.org/1999/02/22-rdf-syntax-ns#"
     xmlns:rdfs="http://www.w3.org/2000/01/rdf-schema#"
     xmlns:skos="http://www.w3.org/2004/02/skos/core#"
     xmlns:vann="http://purl.org/vocab/vann/"
     xmlns:xml="http://www.w3.org/XML/1998/namespace"
     xmlns:xsd="http://www.w3.org/2001/XMLSchema#"
     xmlns:time="http://www.w3.org/2006/time#">
    <owl:Ontology rdf:about="https://w3id.org/citydata/part1/v1/ActivityPattern">
    	<!-- Identity -->
    	<dcterms:title>Information technology - City data model - Part 1: Foundation level concepts - Activity Pattern</dcterms:title>
    	<skos:definition>This ontology specifies the foundation-level concepts related to the activity pattern of the city data model.</skos:definition>
    	<vann:preferredNamespaceUri>https://w3id.org/citydata/part1/v1/</vann:preferredNamespaceUri>
    	<vann:preferredNamespacePrefix>cdm1</vann:preferredNamespacePrefix>
    		
    	<!-- Provenance -->
        <dcterms:creator>Megan Katsumi</dcterms:creator>
        <dcterms:creator>Mark Fox</dcterms:creator>
    	<dcterms:creator>Kenneth Vaughn</dcterms:creator>
        <dcterms:issued rdf:datatype="http://www.w3.org/2001/XMLSchema#date">2023</dcterms:issued> <!-- Date of the source document, comment out if draft -->
        <owl:priorVersion rdf:datatype="http://www.w3.org/2001/XMLSchema#date">2017-11-05</owl:priorVersion> <!-- Date of prior ontology file, if any -->
		<dcterms:modified rdf:datatype="http://www.w3.org/2001/XMLSchema#date">2026-02-06</dcterms:modified> <!-- Date of this ontology file -->
        <owl:versionInfo>1.3.0</owl:versionInfo>
        <owl:versionIRI rdf:resource="https://w3id.org/citydata/part1/v1/r3.0"/>
        <rdfs:comment>The prior version of this ontology used a different ontology IRI. This update remains semantically consistent with the version adopted as ISO 5087-1:2023.</rdfs:comment>
        
        <!-- License -->
        <cc:license>http://creativecommons.org/licenses/by/4.0/</cc:license>
        
        <!-- Imports -->
        <owl:imports rdf:resource="http://www.w3.org/2006/time"/>
        <owl:imports rdf:resource="https://w3id.org/citydata/part1/v1/ChangePattern"/>
        <owl:imports rdf:resource="https://w3id.org/citydata/part1/v1/SpatialLocPattern"/>
    </owl:Ontology>

    <!-- 
    ///////////////////////////////////////////////////////////////////////////////////////
    //
    // Object Properties
    //
    ///////////////////////////////////////////////////////////////////////////////////////
     -->

    <!-- https://w3id.org/citydata/part1/v1/ActivityObjectProperty -->

    <owl:ObjectProperty rdf:about="https://w3id.org/citydata/part1/v1/ActivityObjectProperty">
        <rdfs:subPropertyOf rdf:resource="https://w3id.org/citydata/part1/v1/FoundationalCdmObjectProperty"/>
        <skos:definition>Added for organizational purposes, to identify all activity object properties defined in the City Data Model.</skos:definition>
    </owl:ObjectProperty>


    <!-- https://w3id.org/citydata/part1/v1/achievedAt -->
    <owl:ObjectProperty rdf:about="https://w3id.org/citydata/part1/v1/achievedAt">
        <skos:definition>Identifies the time Interval or Instant during which the State was satisfied.</skos:definition>
        <rdfs:subPropertyOf rdf:resource="https://w3id.org/citydata/part1/v1/ActivityObjectProperty"/>
        <rdfs:domain rdf:resource="https://w3id.org/citydata/part1/v1/State"/>
        <rdfs:range rdf:resource="http://www.w3.org/2006/time#TemporalEntity"/>
        <!-- Issue: Axioms not in ISO/IEC 5087-1 -->
        <owl:propertyChainAxiom rdf:parseType="Collection">
            <rdf:Description>
                <owl:inverseOf rdf:resource="https://w3id.org/citydata/part1/v1/effectOf"/>
            </rdf:Description>
            <rdf:Description rdf:about="https://w3id.org/citydata/part1/v1/endOf"/>
        </owl:propertyChainAxiom>
        <owl:propertyChainAxiom rdf:parseType="Collection">
            <rdf:Description>
                <owl:inverseOf rdf:resource="https://w3id.org/citydata/part1/v1/hasDecomp"/>
            </rdf:Description>
            <rdf:Description rdf:about="https://w3id.org/citydata/part1/v1/conjunctiveAchievedAt"/>
            <rdf:Description rdf:about="http://www.w3.org/2006/time#intervalDuring"/>
        </owl:propertyChainAxiom>
        <owl:propertyChainAxiom rdf:parseType="Collection">
            <rdf:Description>
                <owl:inverseOf rdf:resource="https://w3id.org/citydata/part1/v1/preconditionOf"/>
            </rdf:Description>
            <rdf:Description rdf:about="https://w3id.org/citydata/part1/v1/beginOf"/>
        </owl:propertyChainAxiom>
    </owl:ObjectProperty>
    

    <!-- https://w3id.org/citydata/part1/v1/beginOf -->

    <owl:ObjectProperty rdf:about="https://w3id.org/citydata/part1/v1/beginOf">
        <skos:definition>Identifies the time Instant at which the Activity occurs.</skos:definition>
        <rdfs:subPropertyOf rdf:resource="https://w3id.org/citydata/part1/v1/ActivityObjectProperty"/>
        <rdfs:domain rdf:resource="https://w3id.org/citydata/part1/v1/Activity"/>
        <rdfs:range rdf:resource="http://www.w3.org/2006/time#Instant"/>
        <!-- Issue: Axioms not in ISO/IEC 5087-1 -->
        <owl:propertyChainAxiom rdf:parseType="Collection">
            <rdf:Description rdf:about="https://w3id.org/citydata/part1/v1/occursAt"/>
            <rdf:Description rdf:about="http://www.w3.org/2006/time#hasBeginning"/>
        </owl:propertyChainAxiom>
    </owl:ObjectProperty>
    

    <!-- Issue: Was causedBy; revised to causedByActivity to align with ISO 5087-1 -->
    <!-- https://w3id.org/citydata/part1/v1/causedByActivity -->

    <owl:ObjectProperty rdf:about="https://w3id.org/citydata/part1/v1/causedByActivity">
        <skos:definition>Identifies an Activity that in some (indirect) way caused the State to be realized. The causedByActivity property is the inverse of the causes property and is a generalization (super-property) of the effectOf property.</skos:definition>
        <rdfs:subPropertyOf rdf:resource="https://w3id.org/citydata/part1/v1/ActivityObjectProperty"/>
        <rdfs:domain rdf:resource="https://w3id.org/citydata/part1/v1/State"/>
        <rdfs:range rdf:resource="https://w3id.org/citydata/part1/v1/Activity"/>
        <owl:inverseOf rdf:resource="https://w3id.org/citydata/part1/v1/causesState"/>
    </owl:ObjectProperty>
    

    <!-- Issue: Was causes; revised to causesState to align with ISO 5087-1 -->
    <!-- https://w3id.org/citydata/part1/v1/causesState -->

    <owl:ObjectProperty rdf:about="https://w3id.org/citydata/part1/v1/causesState">
        <skos:definition>identifies a State that in some (indirect) way was caused by the occurrence of the Activity. An Activity is caused by a State if the State is an effect of the Activity or if the State is an effect of some subactivity of the Activity. The causes property is a generalization (super-property) of the hasEffect property.</skos:definition>
        <rdfs:subPropertyOf rdf:resource="https://w3id.org/citydata/part1/v1/ActivityObjectProperty"/>
        <rdfs:domain rdf:resource="https://w3id.org/citydata/part1/v1/Activity"/>
        <rdfs:range rdf:resource="https://w3id.org/citydata/part1/v1/State"/>
    </owl:ObjectProperty>
    

    <!-- Issue: Not defined in ISO/IEC 5087-1 and seems redundant (i.e., a subproperty to assign a new name without any additional semantics) -->
    <!-- https://w3id.org/citydata/part1/v1/conjunctiveAchievedAt -->

    <owl:ObjectProperty rdf:about="https://w3id.org/citydata/part1/v1/conjunctiveAchievedAt">
        <rdfs:subPropertyOf rdf:resource="https://w3id.org/citydata/part1/v1/achievedAt"/>
        <rdfs:domain rdf:resource="https://w3id.org/citydata/part1/v1/ConjunctiveState"/>
    </owl:ObjectProperty>
    

    <!-- Issue: Note defined in ISO/IEC 5087-1 and seems redundant (i.e., a subproperty to assign a new name without any additional semantics) -->
    <!-- https://w3id.org/citydata/part1/v1/disjunctiveAchievedAt -->

    <owl:ObjectProperty rdf:about="https://w3id.org/citydata/part1/v1/disjunctiveAchievedAt">
        <rdfs:subPropertyOf rdf:resource="https://w3id.org/citydata/part1/v1/achievedAt"/>
        <rdfs:domain rdf:resource="https://w3id.org/citydata/part1/v1/DisjunctiveState"/>
    </owl:ObjectProperty>
    

    <!-- https://w3id.org/citydata/part1/v1/effectOf -->

    <owl:ObjectProperty rdf:about="https://w3id.org/citydata/part1/v1/effectOf">
        <skos:definition>Identifies an Activity that the State was realized by.</skos:definition>
        <rdfs:subPropertyOf rdf:resource="https://w3id.org/citydata/part1/v1/ActivityObjectProperty"/>
        <rdfs:domain rdf:resource="https://w3id.org/citydata/part1/v1/State"/>
        <rdfs:range rdf:resource="https://w3id.org/citydata/part1/v1/Activity"/>
        <owl:inverseOf rdf:resource="https://w3id.org/citydata/part1/v1/hasEffect"/>
    </owl:ObjectProperty>
    

    <!-- Issue: Was enabledBy; revised to enabledByState to align with ISO 5087-1-->
    <!-- https://w3id.org/citydata/part1/v1/enabledByState -->

    <owl:ObjectProperty rdf:about="https://w3id.org/citydata/part1/v1/enabledByState">
        <skos:definition>Identifies a State that in some (indirect) way enabled the Activity to occur. An Activity is enabled by a State if the State is a precondition for the Activity or if the State is a precondition of some subactivity of the Activity. The enabledByState property is a generalization (super-property) of the hasPrecondition property.</skos:definition>
        <rdfs:subPropertyOf rdf:resource="https://w3id.org/citydata/part1/v1/ActivityObjectProperty"/>
        <rdfs:domain rdf:resource="https://w3id.org/citydata/part1/v1/Activity"/>
        <rdfs:range rdf:resource="https://w3id.org/citydata/part1/v1/State"/>
        <owl:inverseOf rdf:resource="https://w3id.org/citydata/part1/v1/enablesActivity"/>
    </owl:ObjectProperty>
    

    <!-- Issue: Was enables; revised to enablesActivity to align with ISO 5087-1. -->
    <!-- https://w3id.org/citydata/part1/v1/enablesActivity -->

    <owl:ObjectProperty rdf:about="https://w3id.org/citydata/part1/v1/enablesActivity">
        <skos:definition>Identifies an Activity that in some (indirect) way was enabled by the State. The enables property is the inverse of the enabledByState property and is a generalization (super-property) of the preconditionOf property.</skos:definition>
        <rdfs:subPropertyOf rdf:resource="https://w3id.org/citydata/part1/v1/ActivityObjectProperty"/>
        <rdfs:domain rdf:resource="https://w3id.org/citydata/part1/v1/State"/>
        <rdfs:range rdf:resource="https://w3id.org/citydata/part1/v1/Activity"/>
    </owl:ObjectProperty>
    

    <!-- https://w3id.org/citydata/part1/v1/endOf -->

    <owl:ObjectProperty rdf:about="https://w3id.org/citydata/part1/v1/endOf">
        <skos:definition>Identifies the time Instant at which the Activity ends.</skos:definition>
        <rdfs:subPropertyOf rdf:resource="https://w3id.org/citydata/part1/v1/ActivityObjectProperty"/>
        <rdfs:domain rdf:resource="https://w3id.org/citydata/part1/v1/Activity"/>
        <rdfs:range rdf:resource="http://www.w3.org/2006/time#Instant"/>
        <!-- Issue: Axioms not in ISO/IEC 5087-1 -->
        <owl:propertyChainAxiom rdf:parseType="Collection">
            <rdf:Description rdf:about="https://w3id.org/citydata/part1/v1/occursAt"/>
            <rdf:Description rdf:about="http://www.w3.org/2006/time#hasEnd"/>
        </owl:propertyChainAxiom>
    </owl:ObjectProperty>
    

    <!-- https://w3id.org/citydata/part1/v1/hasDecomp -->

    <owl:ObjectProperty rdf:about="https://w3id.org/citydata/part1/v1/hasDecomp">
        <skos:definition>Identifies two or more States into which the State may be immediately decomposed, i.e. its direct children.</skos:definition>
        <rdfs:subPropertyOf rdf:resource="https://w3id.org/citydata/part1/v1/hasSubstate"/>
    </owl:ObjectProperty>
    

    <!-- https://w3id.org/citydata/part1/v1/hasEffect -->

    <owl:ObjectProperty rdf:about="https://w3id.org/citydata/part1/v1/hasEffect">
        <skos:definition>Identifies a State that is realized once the Activity has occurred.</skos:definition>
        <!-- Issue: changed the subProperty to be of causesState rather than causedByActivity to align with ISO/IEC 5087-1 and other rules -->
        <rdfs:subPropertyOf rdf:resource="https://w3id.org/citydata/part1/v1/causesState"/>
    </owl:ObjectProperty>
    

    <!-- https://w3id.org/citydata/part1/v1/hasPrecondition -->

    <owl:ObjectProperty rdf:about="https://w3id.org/citydata/part1/v1/hasPrecondition">
        <skos:definition>Identifies a State that must be realized in order for the Activity to occur.</skos:definition>
        <rdfs:subPropertyOf rdf:resource="https://w3id.org/citydata/part1/v1/enabledByState"/>
        <owl:inverseOf rdf:resource="https://w3id.org/citydata/part1/v1/preconditionOf"/>
    </owl:ObjectProperty>
    

    <!-- https://w3id.org/citydata/part1/v1/hasStatus -->

    <owl:ObjectProperty rdf:about="https://w3id.org/citydata/part1/v1/hasStatus">
        <skos:definition>Identifies the status of the parent Thing at some point or interval in time.</skos:definition>
        <rdfs:subPropertyOf rdf:resource="https://w3id.org/citydata/part1/v1/ActivityObjectProperty"/>
    </owl:ObjectProperty>
    

    <!-- https://w3id.org/citydata/part1/v1/hasSubactivity -->

    <owl:ObjectProperty rdf:about="https://w3id.org/citydata/part1/v1/hasSubactivity">
        <skos:definition>Identifies a more granular Activity into which the Activity may be decomposed.</skos:definition>
        <rdfs:subPropertyOf rdf:resource="https://w3id.org/citydata/part1/v1/ActivityObjectProperty"/>
        <rdfs:domain rdf:resource="https://w3id.org/citydata/part1/v1/Activity"/>
        <rdfs:range rdf:resource="https://w3id.org/citydata/part1/v1/Activity"/>
    </owl:ObjectProperty>
    

    <!-- https://w3id.org/citydata/part1/v1/hasSubstate -->

    <owl:ObjectProperty rdf:about="https://w3id.org/citydata/part1/v1/hasSubstate">
        <skos:definition>Identifies a State into which the complex state decomposes, at any level (i.e. its child state, grandchild state, etc.). The hasSubState property is transitive and a super-property of the hasDecomp property.</skos:definition>
        <rdfs:subPropertyOf rdf:resource="https://w3id.org/citydata/part1/v1/ActivityObjectProperty"/>
        <rdfs:domain rdf:resource="https://w3id.org/citydata/part1/v1/NonTerminalState"/>
        <rdfs:range rdf:resource="https://w3id.org/citydata/part1/v1/State"/>
        <rdf:type rdf:resource="http://www.w3.org/2002/07/owl#TransitiveProperty"/>
    </owl:ObjectProperty>
    

    <!-- Issue: v1.2.0 addition: ISO/IEC 5087-1 only defines occursBefore -->
    <!-- https://w3id.org/citydata/part1/v1/occursAfter -->

    <owl:ObjectProperty rdf:about="https://w3id.org/citydata/part1/v1/occursAfter">
        <rdfs:subPropertyOf rdf:resource="https://w3id.org/citydata/part1/v1/ActivityObjectProperty"/>
        <owl:inverseOf rdf:resource="https://w3id.org/citydata/part1/v1/occursBefore"/>
    </owl:ObjectProperty>
    

    <!-- Issue: changed from time:TemporalEntity to time:Interval to align with ISO/IEC 5087-1 -->
    <!-- https://w3id.org/citydata/part1/v1/occursAt -->

    <owl:ObjectProperty rdf:about="https://w3id.org/citydata/part1/v1/occursAt">
        <skos:definition>Identifies a time Interval over which the Activity occurs.</skos:definition>
        <rdfs:subPropertyOf rdf:resource="https://w3id.org/citydata/part1/v1/ActivityObjectProperty"/>
        <rdfs:domain rdf:resource="https://w3id.org/citydata/part1/v1/Activity"/>
        <rdfs:range rdf:resource="http://www.w3.org/2006/time#Interval"/>
    </owl:ObjectProperty>
    

    <!-- https://w3id.org/citydata/part1/v1/occursBefore -->

    <owl:ObjectProperty rdf:about="https://w3id.org/citydata/part1/v1/occursBefore">
        <skos:definition>Identifies an Activity that the Activity occurred before.</skos:definition>
        <rdfs:subPropertyOf rdf:resource="https://w3id.org/citydata/part1/v1/ActivityObjectProperty"/>
        <rdfs:domain rdf:resource="https://w3id.org/citydata/part1/v1/Activity"/>
        <rdfs:range rdf:resource="https://w3id.org/citydata/part1/v1/Activity"/>
        <rdf:type rdf:resource="http://www.w3.org/2002/07/owl#TransitiveProperty"/>
        <rdfs:comment>An activity occursBefore another if its endOf instant is before the beginOf instant of the other activity; the occursBefore relation is transitive. We cannot define this semantics in OWL, though it could be captured in future work by an extension with rules.</rdfs:comment>
    </owl:ObjectProperty>
    

    <!-- Issue: v1.2.0 addition: ISO/IEC 5087-1 only defines occursDirectlyBefore -->
    <!-- https://w3id.org/citydata/part1/v1/occursDirectlyAfter -->

    <owl:ObjectProperty rdf:about="https://w3id.org/citydata/part1/v1/occursDirectlyAfter">
        <rdfs:subPropertyOf rdf:resource="https://w3id.org/citydata/part1/v1/occursAfter"/>
        <owl:inverseOf rdf:resource="https://w3id.org/citydata/part1/v1/occursDirectlyBefore"/>
    </owl:ObjectProperty>
    

    <!-- https://w3id.org/citydata/part1/v1/occursDirectlyBefore -->

    <owl:ObjectProperty rdf:about="https://w3id.org/citydata/part1/v1/occursDirectlyBefore">
        <skos:definition>Identifies an Activity that occurred immediately prior to the Activity. The occursDirectlyBefore property is a sub-property of the occursBefore property.</skos:definition>
        <rdfs:subPropertyOf rdf:resource="https://w3id.org/citydata/part1/v1/occursBefore"/>
        <rdfs:domain rdf:resource="https://w3id.org/citydata/part1/v1/Activity"/>
        <rdfs:range rdf:resource="https://w3id.org/citydata/part1/v1/Activity"/>
        <rdfs:comment>An activity occursDirectlyBefore another if it occursAt an interval that meets the interval of the other activity. We cannot define this semantics in OWL, though it could be captured by an extension with rules.</rdfs:comment>
    </owl:ObjectProperty>
    

    <!-- Issue: Made subPropertyOf enablesActivity to align with ISO/IEC 5087-1 -->
    <!-- https://w3id.org/citydata/part1/v1/preconditionOf -->

    <owl:ObjectProperty rdf:about="https://w3id.org/citydata/part1/v1/preconditionOf">
        <skos:definition>Identifies an Activity that requires the State to be realized in order to occur.</skos:definition>
        <rdfs:subPropertyOf rdf:resource="https://w3id.org/citydata/part1/v1/enablesActivity"/>
        <rdfs:domain rdf:resource="https://w3id.org/citydata/part1/v1/State"/>
        <rdfs:range rdf:resource="https://w3id.org/citydata/part1/v1/Activity"/>
    </owl:ObjectProperty>
    

    <!-- https://w3id.org/citydata/part1/v1/satisfiedBy -->

    <owl:ObjectProperty rdf:about="https://w3id.org/citydata/part1/v1/satisfiedBy">
        <skos:definition>Specifies the Manifestation that is to be satisfied (i.e., realized).</skos:definition>
        <rdfs:subPropertyOf rdf:resource="https://w3id.org/citydata/part1/v1/ActivityObjectProperty"/>
        <rdfs:domain rdf:resource="https://w3id.org/citydata/part1/v1/ManifestationState"/>
        <rdfs:range rdf:resource="https://w3id.org/citydata/part1/v1/Manifestation"/>
    </owl:ObjectProperty>
    

    <!-- https://w3id.org/citydata/part1/v1/scheduledFor -->

    <owl:ObjectProperty rdf:about="https://w3id.org/citydata/part1/v1/scheduledFor">
        <skos:definition>Identifies a time Interval during which a Thing occurs.</skos:definition>
        <rdfs:subPropertyOf rdf:resource="https://w3id.org/citydata/part1/v1/ActivityObjectProperty"/>
        <rdfs:range rdf:resource="http://www.w3.org/2006/time#Interval"/>
    </owl:ObjectProperty>
    

    <!-- Issue: v1.2.0 addition -->
    <!-- https://w3id.org/citydata/part1/v1/terminalAchievedAt -->

    <owl:ObjectProperty rdf:about="https://w3id.org/citydata/part1/v1/terminalAchievedAt">
        <rdfs:subPropertyOf rdf:resource="https://w3id.org/citydata/part1/v1/achievedAt"/>
        <rdfs:domain rdf:resource="https://w3id.org/citydata/part1/v1/TerminalState"/>
    </owl:ObjectProperty>


    <!-- 
    ///////////////////////////////////////////////////////////////////////////////////////
    //
    // Classes
    //
    ///////////////////////////////////////////////////////////////////////////////////////
     -->

    <!-- https://w3id.org/citydata/part1/v1/ActivityThing -->

    <owl:Class rdf:about="https://w3id.org/citydata/part1/v1/ActivityThing">
        <skos:definition>Added for organizational purposes, to identify all classes defined in the Activity pattern.</skos:definition>
        <rdfs:subClassOf rdf:resource="https://w3id.org/citydata/part1/v1/FoundationalCdmThing"/>
    </owl:Class>
    

    <!-- https://w3id.org/citydata/part1/v1/Activity -->

    <owl:Class rdf:about="https://w3id.org/citydata/part1/v1/Activity">
        <skos:definition>An Activity describes something that occurs in the domain.
An Activity may be further defined by (decomposed into) Subactivities.
An Activity may have precondition and/or effect State.
An Activity may be enabled by or cause some State. An enabling of causing state is a generalization of a precondition/effect; an Activity is enabled by or causes some State if it has a subactivity with a precondition or effect (respectively) of that State. 
In other words, the state may not be required directly before, or cause directly after the activity, but by some more specialized sub-activity.
An Activity occurs at some point in time and space.
An Activity takes place during some interval, and so has some duration.
An Activity may have some Manifestations that participate in it.</skos:definition>
        <rdfs:subClassOf rdf:resource="https://w3id.org/citydata/part1/v1/ActivityThing"/>
        <rdfs:subClassOf rdf:resource="http://www.w3.org/ns/prov#Activity"/>
        <rdfs:subClassOf>
            <owl:Restriction>
                <owl:onProperty rdf:resource="https://w3id.org/citydata/part1/v1/hasSubactivity"/>
                <owl:allValuesFrom rdf:resource="https://w3id.org/citydata/part1/v1/Activity"/>
            </owl:Restriction>
        </rdfs:subClassOf>
        <rdfs:subClassOf>
            <owl:Restriction>
                <owl:onProperty rdf:resource="https://w3id.org/citydata/part1/v1/hasStatus"/>
                <owl:qualifiedCardinality rdf:datatype="http://www.w3.org/2001/XMLSchema#nonNegativeInteger">1</owl:qualifiedCardinality>
                <owl:onClass rdf:resource="https://w3id.org/citydata/part1/v1/ActivityStatus"/>
            </owl:Restriction>
        </rdfs:subClassOf>
        <rdfs:subClassOf>
            <owl:Restriction>
                <owl:onProperty rdf:resource="https://w3id.org/citydata/part1/v1/hasPrecondition"/>
                <owl:allValuesFrom rdf:resource="https://w3id.org/citydata/part1/v1/State"/>
            </owl:Restriction>
        </rdfs:subClassOf>
        <rdfs:subClassOf>
            <owl:Restriction>
                <owl:onProperty rdf:resource="https://w3id.org/citydata/part1/v1/enabledByState"/>
                <owl:allValuesFrom rdf:resource="https://w3id.org/citydata/part1/v1/State"/>
            </owl:Restriction>
        </rdfs:subClassOf>
        <rdfs:subClassOf>
            <owl:Restriction>
                <owl:onProperty rdf:resource="https://w3id.org/citydata/part1/v1/hasEffect"/>
                <owl:allValuesFrom rdf:resource="https://w3id.org/citydata/part1/v1/State"/>
            </owl:Restriction>
        </rdfs:subClassOf>
        <rdfs:subClassOf>
            <owl:Restriction>
                <owl:onProperty rdf:resource="https://w3id.org/citydata/part1/v1/causesState"/>
                <owl:allValuesFrom rdf:resource="https://w3id.org/citydata/part1/v1/State"/>
            </owl:Restriction>
        </rdfs:subClassOf>
        <rdfs:subClassOf>
            <owl:Restriction>
                <owl:onProperty rdf:resource="https://w3id.org/citydata/part1/v1/scheduledFor"/>
                <owl:qualifiedCardinality rdf:datatype="http://www.w3.org/2001/XMLSchema#nonNegativeInteger">1</owl:qualifiedCardinality>
                <owl:onClass rdf:resource="http://www.w3.org/2006/time#Interval"/>
            </owl:Restriction>
        </rdfs:subClassOf>
        <rdfs:subClassOf>
            <owl:Restriction>
                <owl:onProperty rdf:resource="https://w3id.org/citydata/part1/v1/occursAt"/>
                <owl:someValuesFrom rdf:resource="http://www.w3.org/2006/time#Interval"/>
            </owl:Restriction>
        </rdfs:subClassOf>
        <rdfs:subClassOf>
            <owl:Restriction>
                <owl:onProperty rdf:resource="https://w3id.org/citydata/part1/v1/beginOf"/>
                <owl:someValuesFrom rdf:resource="http://www.w3.org/2006/time#Instant"/>
            </owl:Restriction>
        </rdfs:subClassOf>
        <rdfs:subClassOf>
            <owl:Restriction>
                <owl:onProperty rdf:resource="https://w3id.org/citydata/part1/v1/endOf"/>
                <owl:someValuesFrom rdf:resource="http://www.w3.org/2006/time#Instant"/>
            </owl:Restriction>
        </rdfs:subClassOf>
        <rdfs:subClassOf>
            <owl:Restriction>
                <owl:onProperty rdf:resource="https://w3id.org/citydata/part1/v1/associatedLocation"/>
                <owl:allValuesFrom rdf:resource="https://w3id.org/citydata/part1/v1/Location"/>
            </owl:Restriction>
        </rdfs:subClassOf>
        <rdfs:subClassOf>
            <owl:Restriction>
                <owl:onProperty rdf:resource="https://w3id.org/citydata/part1/v1/occursBefore"/>
                <owl:allValuesFrom rdf:resource="https://w3id.org/citydata/part1/v1/Activity"/>
            </owl:Restriction>
        </rdfs:subClassOf>
        <rdfs:subClassOf>
            <owl:Restriction>
                <owl:onProperty rdf:resource="https://w3id.org/citydata/part1/v1/occursDirectlyBefore"/>
                <owl:allValuesFrom rdf:resource="https://w3id.org/citydata/part1/v1/Activity"/>
            </owl:Restriction>
        </rdfs:subClassOf>
    </owl:Class>
    

    <!-- Issue: It seems like this should be a Code rather than a Thing. -->
    <!-- https://w3id.org/citydata/part1/v1/ActivityStatus -->

    <owl:Class rdf:about="https://w3id.org/citydata/part1/v1/ActivityStatus">
        <skos:definition>The status of the Activity.</skos:definition>
        <rdfs:subClassOf rdf:resource="https://w3id.org/citydata/part1/v1/ActivityThing"/>
    </owl:Class>
    

    <!-- https://w3id.org/citydata/part1/v1/ConjunctiveState -->

    <owl:Class rdf:about="https://w3id.org/citydata/part1/v1/ConjunctiveState">
        <skos:definition>A type of NonTerminalState that is defined by the conjunction of its child States.</skos:definition>
        <rdfs:subClassOf rdf:resource="https://w3id.org/citydata/part1/v1/NonTerminalState"/>
        <owl:disjointWith rdf:resource="https://w3id.org/citydata/part1/v1/DisjunctiveState"/>
    </owl:Class>
    

    <!-- https://w3id.org/citydata/part1/v1/DisjunctiveState -->

    <owl:Class rdf:about="https://w3id.org/citydata/part1/v1/DisjunctiveState">
        <skos:definition>A type of NonTerminalState that is defined by the disjunction of its child States. A State cannot be both conjunctive and disjunctive. </skos:definition>
        <rdfs:subClassOf rdf:resource="https://w3id.org/citydata/part1/v1/NonTerminalState"/>
    </owl:Class>
    

    <!-- https://w3id.org/citydata/part1/v1/ManifestationState -->

    <owl:Class rdf:about="https://w3id.org/citydata/part1/v1/ManifestationState">
        <skos:definition>A specialization of TerminalState, the ManifestationState specifies a Manifestation class that an individual must satisfy in order for the ManifestationState to be true.</skos:definition>
        <rdfs:subClassOf rdf:resource="https://w3id.org/citydata/part1/v1/TerminalState"/>
        <rdfs:subClassOf>
            <owl:Restriction>
                <owl:onProperty rdf:resource="https://w3id.org/citydata/part1/v1/satisfiedBy"/>
                <owl:allValuesFrom rdf:resource="https://w3id.org/citydata/part1/v1/Manifestation"/>
            </owl:Restriction>
        </rdfs:subClassOf>
    </owl:Class>
    

    <!-- By definition, it seems as if hasSubstate should also be min 2 (i.e., the 2 hasDecomp would apply ) -->
    <!-- https://w3id.org/citydata/part1/v1/NonTerminalState -->

    <owl:Class rdf:about="https://w3id.org/citydata/part1/v1/NonTerminalState">
        <skos:definition>A NonTerminalState has child States (a.k.a., sub-states) that are either conjuctive or disjunctive. Each child may be a TerminalState or NonTerminalState; eventually a TerminalState is reached. A State cannot be both non-terminal and terminal.</skos:definition>
        <rdfs:subClassOf rdf:resource="https://w3id.org/citydata/part1/v1/State"/>
        <owl:disjointWith rdf:resource="https://w3id.org/citydata/part1/v1/TerminalState"/>
        <rdfs:subClassOf>
            <owl:Restriction>
                <owl:onProperty rdf:resource="https://w3id.org/citydata/part1/v1/hasDecomp"/>
                <owl:minQualifiedCardinality rdf:datatype="http://www.w3.org/2001/XMLSchema#nonNegativeInteger">2</owl:minQualifiedCardinality>
                <owl:onClass rdf:resource="https://w3id.org/citydata/part1/v1/State"/>
            </owl:Restriction>
        </rdfs:subClassOf>
        <rdfs:subClassOf>
            <owl:Restriction>
                <owl:onProperty rdf:resource="https://w3id.org/citydata/part1/v1/hasSubstate"/>
                <owl:allValuesFrom rdf:resource="https://w3id.org/citydata/part1/v1/State"/>
            </owl:Restriction>
        </rdfs:subClassOf>
        <rdfs:comment>hasDecomp is not a transitive relation, it only refers to the direct children of a non-terminal state type. A more general relation that is transitive is the substate relation.</rdfs:comment>
    </owl:Class>
    

    <!-- https://w3id.org/citydata/part1/v1/State -->

    <owl:Class rdf:about="https://w3id.org/citydata/part1/v1/State">
        <skos:definition>A State describes some situation in the world which may or may not be satisfied (true) at a given point in time. A State refers to a class of manifestations. It may be a precondition or effect of some Activity, or more generally it may be enabled or be caused by some Activity. If a state is complex, it may refer to some combination of classes of manifestations.
        Example: A shopping activity, Activity-Shop, can require both the VehicleW30LGas state, but also some state wherein the mall is open, OpenMall. Each state is defined separately. The combined state is then defined as the conjunction of the two states. Thus, we could say that the preconditions for Activity-Shop are: precondition(VehicleW30LGas,Activity-Shop) AND  precondition(OpenMall,Activity-Shop). Alternatively, if the preconditions were required disjunctively, we could state: precondition(VehicleW30LGas,Activity-Shop) OR precondition(OpenMall,Activity-Shop).
        In large and complex domains, there can be cases in which the above approach is undesirable. In particular, due to the complexity of the description that results as the state being described becomes more detailed. In many cases it will be more natural and convenient to be able to refer to a single, aggregate state. We therefore extend the representation of States to capture aggregation, as approached in the concept of state trees introduced by TOVE as a construct for the activity cluster.
        A State may be either non-terminal or terminal. A terminal state has no child states, and therefore refers directly to a class of manifestations, whereas a non-terminal state has child states, which may define some classes of manifestations, or further define some other complex states.
            NonTerminalState(x) v TerminalState(x) = State(x)
        A state  cannot be both non-terminal and terminal.
            TerminalState disjointWith NonTerminalState</skos:definition>
        <rdfs:subClassOf rdf:resource="https://w3id.org/citydata/part1/v1/ActivityThing"/>
        <rdfs:subClassOf>
            <owl:Restriction>
                <owl:onProperty rdf:resource="https://w3id.org/citydata/part1/v1/preconditionOf"/>
                <owl:allValuesFrom rdf:resource="https://w3id.org/citydata/part1/v1/Activity"/>
            </owl:Restriction>
        </rdfs:subClassOf>
        <rdfs:subClassOf>
            <owl:Restriction>
                <owl:onProperty rdf:resource="https://w3id.org/citydata/part1/v1/enablesActivity"/>
                <owl:allValuesFrom rdf:resource="https://w3id.org/citydata/part1/v1/Activity"/>
            </owl:Restriction>
        </rdfs:subClassOf>
        <rdfs:subClassOf>
            <owl:Restriction>
                <owl:onProperty rdf:resource="https://w3id.org/citydata/part1/v1/effectOf"/>
                <owl:allValuesFrom rdf:resource="https://w3id.org/citydata/part1/v1/Activity"/>
            </owl:Restriction>
        </rdfs:subClassOf>
        <rdfs:subClassOf>
            <owl:Restriction>
                <owl:onProperty rdf:resource="https://w3id.org/citydata/part1/v1/causedByActivity"/>
                <owl:allValuesFrom rdf:resource="https://w3id.org/citydata/part1/v1/Activity"/>
            </owl:Restriction>
        </rdfs:subClassOf>
        <rdfs:subClassOf>
            <owl:Restriction>
                <owl:onProperty rdf:resource="https://w3id.org/citydata/part1/v1/scheduledFor"/>
                <owl:maxQualifiedCardinality rdf:datatype="http://www.w3.org/2001/XMLSchema#nonNegativeInteger">1</owl:maxQualifiedCardinality>
                <owl:onClass rdf:resource="http://www.w3.org/2006/time#Interval"/>
            </owl:Restriction>
        </rdfs:subClassOf>
        <rdfs:subClassOf>
            <owl:Restriction>
                <owl:onProperty rdf:resource="https://w3id.org/citydata/part1/v1/achievedAt"/>
                <owl:allValuesFrom rdf:resource="http://www.w3.org/2006/time#TemporalEntity"/>
            </owl:Restriction>
        </rdfs:subClassOf>
        <rdfs:subClassOf>
            <owl:Restriction>
                <owl:onProperty rdf:resource="https://w3id.org/citydata/part1/v1/hasStatus"/>
                <owl:qualifiedCardinality rdf:datatype="http://www.w3.org/2001/XMLSchema#nonNegativeInteger">1</owl:qualifiedCardinality>
                <owl:onClass rdf:resource="https://w3id.org/citydata/part1/v1/StateStatus"/>
            </owl:Restriction>
        </rdfs:subClassOf>
    </owl:Class>
    

    <!-- https://w3id.org/citydata/part1/v1/StateStatus -->

    <owl:Class rdf:about="https://w3id.org/citydata/part1/v1/StateStatus">
        <rdfs:subClassOf rdf:resource="https://w3id.org/citydata/part1/v1/ActivityThing"/>
    </owl:Class>
    

    <!-- Issue: Resolved logical inconsistency; this had a restriction of exactly 0 States for hasDecomp, but the hasDecomp domain is restricted to NonTerminalState. Removed restriction as it does not apply -->
    <!-- https://w3id.org/citydata/part1/v1/TerminalState -->

    <owl:Class rdf:about="https://w3id.org/citydata/part1/v1/TerminalState">
        <skos:definition>A terminal state type has no substates (cannot be decomposed). It corresponds to a particular class of manifestations. A terminal state is achieved at some time if and only if there exists a manifestation within its defined classification, that exists at that time.</skos:definition>
        <rdfs:subClassOf rdf:resource="https://w3id.org/citydata/part1/v1/State"/>
    </owl:Class>

    
</rdf:RDF>
