<?xml version="1.0"?>
<rdf:RDF xmlns="https://w3id.org/citydata/part1/v1/"
     xml:base="https://w3id.org/citydata/part1/v1/"
     xmlns:cc="http://creativecommons.org/ns#"
     xmlns:dcterms="http://purl.org/dc/terms/"
     xmlns:owl="http://www.w3.org/2002/07/owl#"
     xmlns:rdf="http://www.w3.org/1999/02/22-rdf-syntax-ns#"
     xmlns:rdfs="http://www.w3.org/2000/01/rdf-schema#"
     xmlns:skos="http://www.w3.org/2004/02/skos/core#"
     xmlns:vann="http://purl.org/vocab/vann/"
     xmlns:xml="http://www.w3.org/XML/1998/namespace"
     xmlns:xsd="http://www.w3.org/2001/XMLSchema#"
     xmlns:time="http://www.w3.org/2006/time#">
    <owl:Ontology rdf:about="https://w3id.org/citydata/part1/v1/AgentPattern/">
    	<!-- Identity -->
    	<dcterms:title>Information technology - City data model - Part 1: Foundation level concepts - Agent Pattern</dcterms:title>
        <dcterms:alternative>CDM Agent Pattern</dcterms:alternative>
    	<skos:definition>This ontology specifies the foundation-level concepts related to the agent pattern of the city data model.</skos:definition>
    	<vann:preferredNamespaceUri>https://w3id.org/citydata/part1/v1/</vann:preferredNamespaceUri>
    	<vann:preferredNamespacePrefix>cdm1</vann:preferredNamespacePrefix>
    		
    	<!-- Provenance -->
        <dcterms:creator>Megan Katsumi</dcterms:creator>
        <dcterms:creator>Mark Fox</dcterms:creator>
    	<dcterms:creator>Kenneth Vaughn</dcterms:creator>
        <!-- Prior release -->
        <rdfs:comment>The prior version of this ontology used a different ontology IRI. This update remains semantically consistent with the version adopted as ISO 5087-1:2023.</rdfs:comment>
        <owl:priorVersion rdf:resource="https://standards.iso.org/iso-iec/5087/-1/ed-1/en/ontology/Agent/"/>
        <!-- This release -->
		<dcterms:modified rdf:datatype="http://www.w3.org/2001/XMLSchema#date">2026-02-12</dcterms:modified> 
        <owl:versionInfo>1.3.0</owl:versionInfo>
        <owl:versionIRI rdf:resource="https://w3id.org/citydata/part1/v1/AgentPattern/r3.0/"/>    
        
        <!-- License -->
        <cc:license>http://creativecommons.org/licenses/by/4.0/</cc:license>
        
        <!-- Imports -->
        <owl:imports rdf:resource="https://w3id.org/citydata/part1/v1/GenericPropertiesPattern/"/>
        <owl:imports rdf:resource="https://w3id.org/citydata/part1/v1/ResourcePattern/"/>
    </owl:Ontology>

    
    <!-- 
    ///////////////////////////////////////////////////////////////////////////////////////
    //
    // Object Properties
    //
    ///////////////////////////////////////////////////////////////////////////////////////
     -->

    <!-- https://w3id.org/citydata/part1/v1/AgentObjectProperty -->

    <owl:ObjectProperty rdf:about="https://w3id.org/citydata/part1/v1/AgentObjectProperty">
        <rdfs:subPropertyOf rdf:resource="https://w3id.org/citydata/part1/v1/FoundationalCdmObjectProperty"/>
        <skos:definition>Added for organizational purposes, to identify all agent object properties defined in the City Data Model.</skos:definition>
    </owl:ObjectProperty>


    <!-- https://w3id.org/citydata/part1/v1/performedBy -->

    <owl:ObjectProperty rdf:about="https://w3id.org/citydata/part1/v1/performedBy">
        <rdfs:subPropertyOf rdf:resource="https://w3id.org/citydata/part1/v1/AgentObjectProperty"/>
        <owl:inverseOf rdf:resource="https://w3id.org/citydata/part1/v1/performs"/>
    </owl:ObjectProperty>
    

    <!-- Issue: Removed ReflexiveProperty declaration as it was not defined in ISO/IEC 5087-1 and seemed inappropriate. -->
    <!-- https://w3id.org/citydata/part1/v1/performs -->

    <owl:ObjectProperty rdf:about="https://w3id.org/citydata/part1/v1/performs">
        <skos:definition>Identifies activities that the Agent performs.</skos:definition>
        <rdfs:subPropertyOf rdf:resource="https://w3id.org/citydata/part1/v1/AgentObjectProperty"/>
        <rdfs:domain rdf:resource="https://w3id.org/citydata/part1/v1/Agent"/>
        <rdfs:range rdf:resource="https://w3id.org/citydata/part1/v1/Activity"/>
    </owl:ObjectProperty>
    

    <!-- Issue: Addition in v1.2.0 -->
    <!-- https://w3id.org/citydata/part1/v1/performedBy -->

    <owl:ObjectProperty rdf:about="https://w3id.org/citydata/part1/v1/performedBy">
        <rdfs:subPropertyOf rdf:resource="https://w3id.org/citydata/part1/v1/AgentObjectProperty"/>
        <owl:inverseOf rdf:resource="https://w3id.org/citydata/part1/v1/performs"/>
    </owl:ObjectProperty>
    

    <!-- 
    ///////////////////////////////////////////////////////////////////////////////////////
    //
    // Classes
    //
    ///////////////////////////////////////////////////////////////////////////////////////
    -->

    <!-- https://w3id.org/citydata/part1/v1/AgentThing -->

    <owl:Class rdf:about="https://w3id.org/citydata/part1/v1/AgentThing">
        <skos:definition>Added for organizational purposes, to identify all classes defined in the Agent pattern.</skos:definition>
        <rdfs:subClassOf rdf:resource="https://w3id.org/citydata/part1/v1/FoundationalCdmThing"/>
    </owl:Class>


    <!-- https://w3id.org/citydata/part1/v1/Agent -->

    <owl:Class rdf:about="https://w3id.org/citydata/part1/v1/Agent">
        <skos:definition>An Agent affects, is affected by, or performs some Activity(s). An Agent may be a Person or Organization, but not Software or a Mechanical Device (at this time). An Agent can be a member of an organization and hold zero or more posts in an organization.</skos:definition>
        <rdfs:subClassOf rdf:resource="https://w3id.org/citydata/part1/v1/AgentThing"/>
        <rdfs:subClassOf rdf:resource="http://xmlns.com/foaf/0.1/Agent"/>
        <rdfs:subClassOf rdf:resource="http://www.w3.org/ns/prov#Agent"/>
        <rdfs:subClassOf>
            <owl:Restriction>
                <owl:onProperty rdf:resource="https://w3id.org/citydata/part1/v1/performs"/>
                <owl:allValuesFrom rdf:resource="https://w3id.org/citydata/part1/v1/Activity"/>
            </owl:Restriction>
        </rdfs:subClassOf>
        <rdfs:subClassOf>
            <owl:Restriction>
                <owl:onProperty rdf:resource="https://w3id.org/citydata/part1/v1/resourceOf"/>
                <owl:allValuesFrom rdf:resource="https://w3id.org/citydata/part1/v1/TerminalResourceState"/>
            </owl:Restriction>
        </rdfs:subClassOf>
        <rdfs:subClassOf>
            <owl:Restriction>
                <owl:onProperty rdf:resource="https://w3id.org/citydata/part1/v1/hasName"/>
                <owl:qualifiedCardinality rdf:datatype="http://www.w3.org/2001/XMLSchema#nonNegativeInteger">1</owl:qualifiedCardinality>
                <owl:onDataRange rdf:resource="http://www.w3.org/2001/XMLSchema#string"/>
            </owl:Restriction>
        </rdfs:subClassOf>
    </owl:Class>
    

</rdf:RDF>
