<?xml version="1.0"?>
<rdf:RDF xmlns="https://w3id.org/citydata/part1/v1/"
     xml:base="https://w3id.org/citydata/part1/v1/"
     xmlns:cc="http://creativecommons.org/ns#"
     xmlns:dcterms="http://purl.org/dc/terms/"
     xmlns:owl="http://www.w3.org/2002/07/owl#"
     xmlns:rdf="http://www.w3.org/1999/02/22-rdf-syntax-ns#"
     xmlns:rdfs="http://www.w3.org/2000/01/rdf-schema#"
     xmlns:skos="http://www.w3.org/2004/02/skos/core#"
     xmlns:vann="http://purl.org/vocab/vann/"
     xmlns:xml="http://www.w3.org/XML/1998/namespace"
     xmlns:xsd="http://www.w3.org/2001/XMLSchema#"
     xmlns:time="http://www.w3.org/2006/time#">
    <owl:Ontology rdf:about="https://w3id.org/citydata/part1/v1/AgreementPattern/">
    	<!-- Identity -->
    	<dcterms:title>Information technology - City data model - Part 1: Foundation level concepts - Agreement Pattern</dcterms:title>
        <dcterms:alternative>CDM Agreement Pattern</dcterms:alternative>
    	<skos:definition>This ontology specifies the foundation-level concepts related to the agreement pattern of the city data model.</skos:definition>
    	<vann:preferredNamespaceUri>https://w3id.org/citydata/part1/v1/</vann:preferredNamespaceUri>
    	<vann:preferredNamespacePrefix>cdm1</vann:preferredNamespacePrefix>
    		
    	<!-- Provenance -->
        <dcterms:creator>Megan Katsumi</dcterms:creator>
        <dcterms:creator>Mark Fox</dcterms:creator>
    	<dcterms:creator>Kenneth Vaughn</dcterms:creator>
        <!-- Prior release -->
        <rdfs:comment>The prior version of this ontology used a different ontology IRI. This update remains semantically consistent with the version adopted as ISO 5087-1:2023.</rdfs:comment>
        <owl:priorVersion rdf:resource="https://standards.iso.org/iso-iec/5087/-1/ed-1/en/ontology/Agreement/"/>
        <!-- This release -->
		<dcterms:modified rdf:datatype="http://www.w3.org/2001/XMLSchema#date">2026-02-12</dcterms:modified> 
        <owl:versionInfo>1.3.0</owl:versionInfo>
        <owl:versionIRI rdf:resource="https://w3id.org/citydata/part1/v1/AgreementPattern/r3.0/"/>    
        
        <!-- License -->
        <cc:license>http://creativecommons.org/licenses/by/4.0/</cc:license>
        
        <!-- Imports -->
        <owl:imports rdf:resource="https://w3id.org/citydata/part1/v1/AgentPattern/"/>
    </owl:Ontology>


    <!-- 
    ///////////////////////////////////////////////////////////////////////////////////////
    //
    // Object Properties
    //
    ///////////////////////////////////////////////////////////////////////////////////////
     -->


    <!-- https://w3id.org/citydata/part1/v1/AgreementObjectProperty -->

    <owl:ObjectProperty rdf:about="https://w3id.org/citydata/part1/v1/AgreementObjectProperty">
        <rdfs:subPropertyOf rdf:resource="https://w3id.org/citydata/part1/v1/FoundationalCdmObjectProperty"/>
        <skos:definition>Added for organizational purposes, to identify all agreement object properties defined in the City Data Model.</skos:definition>
    </owl:ObjectProperty>

    <!-- https://w3id.org/citydata/part1/v1/agentInvolvedIn -->

    <owl:ObjectProperty rdf:about="https://w3id.org/citydata/part1/v1/agentInvolvedIn">
        <rdfs:subPropertyOf rdf:resource="https://w3id.org/citydata/part1/v1/AgreementObjectProperty"/>
        <owl:inverseOf rdf:resource="https://w3id.org/citydata/part1/v1/involvesAgent"/>
    </owl:ObjectProperty>
    

    <!-- https://w3id.org/citydata/part1/v1/commitsToActivity -->

    <owl:ObjectProperty rdf:about="https://w3id.org/citydata/part1/v1/commitsToActivity">
        <skos:definition>A commitment to some activity</skos:definition>
        <rdfs:subPropertyOf rdf:resource="https://w3id.org/citydata/part1/v1/ActivityObjectProperty"/>
        <rdfs:domain rdf:resource="https://w3id.org/citydata/part1/v1/AtomicAgreement"/>
        <rdfs:range rdf:resource="https://w3id.org/citydata/part1/v1/Activity"/>
    </owl:ObjectProperty>
    

    <!-- https://w3id.org/citydata/part1/v1/establishedOn -->

    <owl:ObjectProperty rdf:about="https://w3id.org/citydata/part1/v1/establishedOn">
        <skos:definition>Specifies the Instant of time at which the Agreement was created.</skos:definition>
        <rdfs:subPropertyOf rdf:resource="https://w3id.org/citydata/part1/v1/AgreementObjectProperty"/>
        <rdfs:domain rdf:resource="https://w3id.org/citydata/part1/v1/Agreement"/>
        <rdfs:range rdf:resource="http://www.w3.org/2006/time#Instant"/>
    </owl:ObjectProperty>
    

    <!-- https://w3id.org/citydata/part1/v1/hasClaim -->

    <owl:ObjectProperty rdf:about="https://w3id.org/citydata/part1/v1/hasClaim">
        <skos:definition>Indicates that an Agent is the beneficiary of an Activity fulfilled by another Agent in the Agreement (i.e., the Agent with the duty to fulfil the Activity), e.g. payment of wages, provision of services.</skos:definition>
        <rdfs:subPropertyOf rdf:resource="https://w3id.org/citydata/part1/v1/agentInvolvedIn"/>
        <rdfs:range rdf:resource="https://w3id.org/citydata/part1/v1/AtomicAgreement"/>
    </owl:ObjectProperty>
    

    <!-- https://w3id.org/citydata/part1/v1/hasDuty -->

    <owl:ObjectProperty rdf:about="https://w3id.org/citydata/part1/v1/hasDuty">
        <skos:definition>Indicates that an Agent is required to fulfil the described Activity.</skos:definition>
        <rdfs:subPropertyOf rdf:resource="https://w3id.org/citydata/part1/v1/agentInvolvedIn"/>
        <rdfs:range rdf:resource="https://w3id.org/citydata/part1/v1/AtomicAgreement"/>
    </owl:ObjectProperty>
    

    <!-- https://w3id.org/citydata/part1/v1/hasNoClaim -->

    <owl:ObjectProperty rdf:about="https://w3id.org/citydata/part1/v1/hasNoClaim">
        <skos:definition>Indicates that an Agent has no claim on (i.e. has no right to the described Activity).</skos:definition>
        <rdfs:subPropertyOf rdf:resource="https://w3id.org/citydata/part1/v1/agentInvolvedIn"/>
        <rdfs:range rdf:resource="https://w3id.org/citydata/part1/v1/AtomicAgreement"/>
    </owl:ObjectProperty>
    

    <!-- https://w3id.org/citydata/part1/v1/hasPrivilege -->

    <owl:ObjectProperty rdf:about="https://w3id.org/citydata/part1/v1/hasPrivilege">
        <skos:definition>Indicates that an Agent may but is not required to fulfil the described Activity.</skos:definition>
        <rdfs:subPropertyOf rdf:resource="https://w3id.org/citydata/part1/v1/agentInvolvedIn"/>
        <rdfs:range rdf:resource="https://w3id.org/citydata/part1/v1/AtomicAgreement"/>
    </owl:ObjectProperty>
    

    <!-- https://w3id.org/citydata/part1/v1/hasSubAgreement -->

    <owl:ObjectProperty rdf:about="https://w3id.org/citydata/part1/v1/hasSubAgreement">
        <skos:definition>Identifies two or more Agreements that comprise the Agreement.</skos:definition>
        <rdfs:subPropertyOf rdf:resource="https://w3id.org/citydata/part1/v1/AgreementObjectProperty"/>
        <rdfs:domain rdf:resource="https://w3id.org/citydata/part1/v1/Agreement"/>
        <rdfs:range rdf:resource="https://w3id.org/citydata/part1/v1/Agreement"/>
    </owl:ObjectProperty>
    

    <!-- https://w3id.org/citydata/part1/v1/involvesAgent -->

    <owl:ObjectProperty rdf:about="https://w3id.org/citydata/part1/v1/involvesAgent">
        <skos:definition>Identifies the Agents that are party to the Agreement.</skos:definition>
        <rdfs:subPropertyOf rdf:resource="https://w3id.org/citydata/part1/v1/AgreementObjectProperty"/>
        <rdfs:domain rdf:resource="https://w3id.org/citydata/part1/v1/Agreement"/>
        <rdfs:range rdf:resource="https://w3id.org/citydata/part1/v1/Agent"/>
    </owl:ObjectProperty>
    

    <!-- https://w3id.org/citydata/part1/v1/validFor -->

    <owl:ObjectProperty rdf:about="https://w3id.org/citydata/part1/v1/validFor">
        <skos:definition>Specifies the time Interval during which the Thing is valid or in force.</skos:definition>
        <rdfs:subPropertyOf rdf:resource="https://w3id.org/citydata/part1/v1/AgreementObjectProperty"/>
        <rdfs:range rdf:resource="http://www.w3.org/2006/time#Interval"/>
    </owl:ObjectProperty>
    

    <!-- https://w3id.org/citydata/part1/v1/validIn -->

    <owl:ObjectProperty rdf:about="https://w3id.org/citydata/part1/v1/validIn">
        <skos:definition>Identifies the location where the Thing is valid.</skos:definition>
        <rdfs:subPropertyOf rdf:resource="https://w3id.org/citydata/part1/v1/AgreementObjectProperty"/>
        <rdfs:range rdf:resource="https://w3id.org/citydata/part1/v1/Location"/>
    </owl:ObjectProperty>
    

    <!-- 
    ///////////////////////////////////////////////////////////////////////////////////////
    //
    // Classes
    //
    ///////////////////////////////////////////////////////////////////////////////////////
     -->


    <!-- https://w3id.org/citydata/part1/v1/AgreementThing -->

    <owl:Class rdf:about="https://w3id.org/citydata/part1/v1/AgreementThing">
        <skos:definition>Added for organizational purposes, to identify all classes defined in the Agreement pattern.</skos:definition>
        <rdfs:subClassOf rdf:resource="https://w3id.org/citydata/part1/v1/FoundationalCdmThing"/>
    </owl:Class>
    

    <!-- https://w3id.org/citydata/part1/v1/Agent -->

    <owl:Class rdf:about="https://w3id.org/citydata/part1/v1/Agent">
        <rdfs:comment>The base concept of Agent is defined in https://w3id.org/citydata/part1/v1/Agent.</rdfs:comment>
        <rdfs:subClassOf rdf:resource="https://w3id.org/citydata/part1/v1/AgreementThing"/>
        <rdfs:subClassOf>
            <owl:Restriction>
                <owl:onProperty rdf:resource="https://w3id.org/citydata/part1/v1/hasClaim"/>
                <owl:allValuesFrom rdf:resource="https://w3id.org/citydata/part1/v1/AtomicAgreement"/>
            </owl:Restriction>
        </rdfs:subClassOf>
        <rdfs:subClassOf>
            <owl:Restriction>
                <owl:onProperty rdf:resource="https://w3id.org/citydata/part1/v1/hasDuty"/>
                <owl:allValuesFrom rdf:resource="https://w3id.org/citydata/part1/v1/AtomicAgreement"/>
            </owl:Restriction>
        </rdfs:subClassOf>
        <rdfs:subClassOf>
            <owl:Restriction>
                <owl:onProperty rdf:resource="https://w3id.org/citydata/part1/v1/hasNoClaim"/>
                <owl:allValuesFrom rdf:resource="https://w3id.org/citydata/part1/v1/AtomicAgreement"/>
            </owl:Restriction>
        </rdfs:subClassOf>
        <rdfs:subClassOf>
            <owl:Restriction>
                <owl:onProperty rdf:resource="https://w3id.org/citydata/part1/v1/hasPrivilege"/>
                <owl:allValuesFrom rdf:resource="https://w3id.org/citydata/part1/v1/AtomicAgreement"/>
            </owl:Restriction>
        </rdfs:subClassOf>
    </owl:Class>


    <!-- https://w3id.org/citydata/part1/v1/Agreement -->

    <owl:Class rdf:about="https://w3id.org/citydata/part1/v1/Agreement">
        <skos:definition>An agreement exists between two or more agents. It is established at some point in time and it may be considered valid only in some Location and/or for some interval in time. An agreement may be defined at varying levels of detail, this is supported with the introduction of the ComplexAgreement and AtomicAgreement class. Finally, agreements involve some specification of rights or commitments of the involved parties. This is represented as a relationship between the involved Agent and a particular activity. </skos:definition>
        <rdfs:subClassOf rdf:resource="https://w3id.org/citydata/part1/v1/AgreementThing"/>
        <rdfs:subClassOf>
            <owl:Restriction>
                <owl:onProperty rdf:resource="https://w3id.org/citydata/part1/v1/establishedOn"/>
                <owl:allValuesFrom rdf:resource="http://www.w3.org/2006/time#Instant"/>
            </owl:Restriction>
        </rdfs:subClassOf>
        <rdfs:subClassOf>
            <owl:Restriction>
                <owl:onProperty rdf:resource="https://w3id.org/citydata/part1/v1/validFor"/>
                <owl:allValuesFrom rdf:resource="http://www.w3.org/2006/time#Interval"/>
            </owl:Restriction>
        </rdfs:subClassOf>
        <rdfs:subClassOf>
            <owl:Restriction>
                <owl:onProperty rdf:resource="https://w3id.org/citydata/part1/v1/validIn"/>
                <owl:allValuesFrom rdf:resource="https://w3id.org/citydata/part1/v1/Location"/>
            </owl:Restriction>
        </rdfs:subClassOf>
        <rdfs:subClassOf>
            <owl:Restriction>
                <owl:onProperty rdf:resource="https://w3id.org/citydata/part1/v1/involvesAgent"/>
                <owl:minQualifiedCardinality rdf:datatype="http://www.w3.org/2001/XMLSchema#nonNegativeInteger">2</owl:minQualifiedCardinality>
                <owl:onClass rdf:resource="https://w3id.org/citydata/part1/v1/Agent"/>
            </owl:Restriction>
        </rdfs:subClassOf>
    </owl:Class>
    

    <!-- https://w3id.org/citydata/part1/v1/AtomicAgreement -->

    <owl:Class rdf:about="https://w3id.org/citydata/part1/v1/AtomicAgreement">
        <skos:definition>An atomic agreement is a simple agreement that cannot be further decomposed into sub-agreements. It is a subclass of Agreement and specifies the “essence” of an agreement.  In particular it identifies how agents participating in the agreement are involved: whether they have a claim, duty, no-claim or privilege with respect to some activity that is committed to in the agreement.</skos:definition>
        <rdfs:subClassOf rdf:resource="https://w3id.org/citydata/part1/v1/Agreement"/>
        <!-- Issue: ISO/IEC 5087-1 does not have commitsToActivity some Activity; instead it has forActivity min 1 Activity -->
        <rdfs:subClassOf>
            <owl:Restriction>
                <owl:onProperty rdf:resource="https://w3id.org/citydata/part1/v1/commitsToActivity"/>
                <owl:someValuesFrom rdf:resource="https://w3id.org/citydata/part1/v1/Activity"/>
            </owl:Restriction>
        </rdfs:subClassOf>
        <rdfs:subClassOf>
            <owl:Restriction>
                <owl:onProperty>
                    <rdf:Description>
                        <owl:inverseOf rdf:resource="https://w3id.org/citydata/part1/v1/hasClaim"/>
                    </rdf:Description>
                </owl:onProperty>
                <owl:allValuesFrom rdf:resource="https://w3id.org/citydata/part1/v1/Agent"/>
            </owl:Restriction>
        </rdfs:subClassOf>
        <rdfs:subClassOf>
            <owl:Restriction>
                <owl:onProperty>
                    <rdf:Description>
                        <owl:inverseOf rdf:resource="https://w3id.org/citydata/part1/v1/hasDuty"/>
                    </rdf:Description>
                </owl:onProperty>
                <owl:allValuesFrom rdf:resource="https://w3id.org/citydata/part1/v1/Agent"/>
            </owl:Restriction>
        </rdfs:subClassOf>
        <rdfs:subClassOf>
            <owl:Restriction>
                <owl:onProperty>
                    <rdf:Description>
                        <owl:inverseOf rdf:resource="https://w3id.org/citydata/part1/v1/hasNoClaim"/>
                    </rdf:Description>
                </owl:onProperty>
                <owl:allValuesFrom rdf:resource="https://w3id.org/citydata/part1/v1/Agent"/>
            </owl:Restriction>
        </rdfs:subClassOf>
        <rdfs:subClassOf>
            <owl:Restriction>
                <owl:onProperty>
                    <rdf:Description>
                        <owl:inverseOf rdf:resource="https://w3id.org/citydata/part1/v1/hasPrivilege"/>
                    </rdf:Description>
                </owl:onProperty>
                <owl:allValuesFrom rdf:resource="https://w3id.org/citydata/part1/v1/Agent"/>
            </owl:Restriction>
        </rdfs:subClassOf>
        <rdfs:subClassOf>
            <owl:Restriction>
                <owl:onProperty rdf:resource="https://w3id.org/citydata/part1/v1/hasSubAgreement"/>
                <owl:qualifiedCardinality rdf:datatype="http://www.w3.org/2001/XMLSchema#nonNegativeInteger">0</owl:qualifiedCardinality>
                <owl:onClass rdf:resource="https://w3id.org/citydata/part1/v1/Agreement"/>
            </owl:Restriction>
        </rdfs:subClassOf>
        <owl:disjointWith rdf:resource="https://w3id.org/citydata/part1/v1/ComplexAgreement"/>
        <rdfs:label xml:lang="en">Atomic Agreement</rdfs:label>
    </owl:Class>
    

    <!-- https://w3id.org/citydata/part1/v1/ComplexAgreement -->

    <owl:Class rdf:about="https://w3id.org/citydata/part1/v1/ComplexAgreement">
        <rdfs:label xml:lang="en">Complex Agreement</rdfs:label>
        <skos:definition>A complex agreement is an agreement that is composed of two or more atomic agreements. It is a subclass of Agreement and specifies the “essence” of a complex agreement.  In particular it identifies how atomic agreements are composed to form a complex agreement.</skos:definition>
        <rdfs:subClassOf rdf:resource="https://w3id.org/citydata/part1/v1/Agreement"/>
        <rdfs:subClassOf>
            <owl:Restriction>
                <owl:onProperty rdf:resource="https://w3id.org/citydata/part1/v1/hasSubAgreement"/>
                <owl:minQualifiedCardinality rdf:datatype="http://www.w3.org/2001/XMLSchema#nonNegativeInteger">2</owl:minQualifiedCardinality>
                <owl:onClass rdf:resource="https://w3id.org/citydata/part1/v1/Agreement"/>
            </owl:Restriction>
        </rdfs:subClassOf>
    </owl:Class>
    

    <!-- https://w3id.org/citydata/part1/v1/ConjunctiveAgreement -->

    <owl:Class rdf:about="https://w3id.org/citydata/part1/v1/ConjunctiveAgreement">
        <skos:definition>A conjunctive agreement is a complex agreement where all sub-agreements must be satisfied for the overall agreement to hold.</skos:definition>
        <rdfs:subClassOf rdf:resource="https://w3id.org/citydata/part1/v1/ComplexAgreement"/>
        <owl:disjointWith rdf:resource="https://w3id.org/citydata/part1/v1/DisjunctiveAgreement"/>
    </owl:Class>
    

    <!-- https://w3id.org/citydata/part1/v1/DisjunctiveAgreement -->

    <owl:Class rdf:about="https://w3id.org/citydata/part1/v1/DisjunctiveAgreement">
        <skos:definition>A disjunctive agreement is a complex agreement where at least one sub-agreement must be satisfied for the overall agreement to hold.</skos:definition>
        <rdfs:subClassOf rdf:resource="https://w3id.org/citydata/part1/v1/ComplexAgreement"/>
    </owl:Class>


</rdf:RDF>
