<?xml version="1.0"?>
<rdf:RDF xmlns="https://w3id.org/citydata/part1/v1/"
     xml:base="https://w3id.org/citydata/part1/v1/"
     xmlns:cc="http://creativecommons.org/ns#"
     xmlns:dcterms="http://purl.org/dc/terms/"
     xmlns:owl="http://www.w3.org/2002/07/owl#"
     xmlns:rdf="http://www.w3.org/1999/02/22-rdf-syntax-ns#"
     xmlns:rdfs="http://www.w3.org/2000/01/rdf-schema#"
     xmlns:skos="http://www.w3.org/2004/02/skos/core#"
     xmlns:vann="http://purl.org/vocab/vann/"
     xmlns:xml="http://www.w3.org/XML/1998/namespace"
     xmlns:xsd="http://www.w3.org/2001/XMLSchema#">
    <owl:Ontology rdf:about="https://w3id.org/citydata/part1/v1/Core">
    	<!-- Identity -->
    	<dcterms:title>Information technology - City data model - Part 1: Foundation level concepts - Core</dcterms:title>
        <dcterms:alternative>CDM Core</dcterms:alternative>
    	<skos:definition>This ontology specifies the foundation-level concepts that are used by all other patterns of the city data model.</skos:definition>
    	<vann:preferredNamespaceUri>https://w3id.org/citydata/part1/v1/</vann:preferredNamespaceUri>
    	<vann:preferredNamespacePrefix>cdm1</vann:preferredNamespacePrefix>
    		
    	<!-- Provenance -->
        <dcterms:creator>Megan Katsumi</dcterms:creator>
        <dcterms:creator>Mark Fox</dcterms:creator>
    	<dcterms:creator>Kenneth Vaughn</dcterms:creator>
        <!-- This release -->
		<dcterms:modified rdf:datatype="http://www.w3.org/2001/XMLSchema#date">2026-02-12</dcterms:modified> 
        <owl:versionInfo>1.3.0</owl:versionInfo>
        <owl:versionIRI rdf:resource="https://w3id.org/citydata/part1/v1/Core/r3.0"/>
   
        <!-- License -->
        <cc:license>http://creativecommons.org/licenses/by/4.0/</cc:license>
        
        <!-- Imports -->
        <owl:imports rdf:resource="http://www.w3.org/2006/time#"/> <!-- Used everywhere -->

    </owl:Ontology>

    <owl:AnnotationProperty rdf:about="https://w3id.org/citydata/part1/v1/mainModule">
        <skos:definition>Identifies whether an ontology file is the main ontology file within a directory.</skos:definition>
        <rdfs:range rdf:resource="http://www.w3.org/2001/XMLSchema#boolean"/>
    </owl:AnnotationProperty>

    <!-- 
    ///////////////////////////////////////////////////////////////////////////////////////
    //
    // Object Properties
    //
    ///////////////////////////////////////////////////////////////////////////////////////
     -->


    <!-- https://w3id.org/citydata/part1/v1/CdmObjectProperty -->

    <owl:ObjectProperty rdf:about="https://w3id.org/citydata/part1/v1/CdmObjectProperty">
        <skos:definition>Added for organizational purposes, to identify all object properties defined in the City Data Model.</skos:definition>
    </owl:ObjectProperty>


    <!-- https://w3id.org/citydata/part1/v1/FoundationalCdmObjectProperty -->

    <owl:ObjectProperty rdf:about="https://w3id.org/citydata/part1/v1/FoundationalCdmObjectProperty">
        <rdfs:subPropertyOf rdf:resource="https://w3id.org/citydata/part1/v1/CdmObjectProperty"/>
        <skos:definition>Added for organizational purposes, to identify all foundational object properties defined in the City Data Model.</skos:definition>
    </owl:ObjectProperty>


    <!-- 
    ///////////////////////////////////////////////////////////////////////////////////////
    //
    // Data properties
    //
    ///////////////////////////////////////////////////////////////////////////////////////
     -->


    <!-- https://w3id.org/citydata/part1/v1/CdmDataProperty -->

    <owl:DatatypeProperty rdf:about="https://w3id.org/citydata/part1/v1/CdmDataProperty">
        <skos:definition>Added for organizational purposes, to identify all data properties defined in the City Data Model.</skos:definition>
    </owl:DatatypeProperty>


    <!-- https://w3id.org/citydata/part1/v1/FoundationalCdmDataProperty -->

    <owl:DatatypeProperty rdf:about="https://w3id.org/citydata/part1/v1/FoundationalCdmDataProperty">
        <rdfs:subPropertyOf rdf:resource="https://w3id.org/citydata/part1/v1/CdmDataProperty"/>
        <skos:definition>Added for organizational purposes, to identify data properties defined in the Foundation-level CDM ontology.</skos:definition>
    </owl:DatatypeProperty>

     <!-- 
    ///////////////////////////////////////////////////////////////////////////////////////
    //
    // Classes
    //
    ///////////////////////////////////////////////////////////////////////////////////////
     -->

    <!-- https://w3id.org/citydata/part1/v1/CdmThing -->

    <owl:Class rdf:about="https://w3id.org/citydata/part1/v1/CdmThing">
        <skos:definition>Added for organizational purposes, to identify all classes defined in the City Data Model.</skos:definition>
    </owl:Class>


    <!-- https://w3id.org/citydata/part1/v1/FoundationalCdmThing -->

    <owl:Class rdf:about="https://w3id.org/citydata/part1/v1/FoundationalCdmThing">
        <skos:definition>Added for organizational purposes, to identify all classes defined in the Foundation-level CDM ontology.</skos:definition>
        <rdfs:subClassOf rdf:resource="https://w3id.org/citydata/part1/v1/CdmThing"/>
    </owl:Class>


</rdf:RDF>    