<?xml version="1.0"?>
<rdf:RDF xmlns="https://w3id.org/citydata/part1/v1/"
     xml:base="https://w3id.org/citydata/part1/v1/"
     xmlns:cc="http://creativecommons.org/ns#"
     xmlns:dcterms="http://purl.org/dc/terms/"
     xmlns:owl="http://www.w3.org/2002/07/owl#"
     xmlns:rdf="http://www.w3.org/1999/02/22-rdf-syntax-ns#"
     xmlns:rdfs="http://www.w3.org/2000/01/rdf-schema#"
     xmlns:skos="http://www.w3.org/2004/02/skos/core#"
     xmlns:vann="http://purl.org/vocab/vann/"
     xmlns:xml="http://www.w3.org/XML/1998/namespace"
     xmlns:xsd="http://www.w3.org/2001/XMLSchema#">
    <owl:Ontology rdf:about="https://w3id.org/citydata/part1/v1/GenericPropertiesPattern">
    	<!-- Identity -->
    	<dcterms:title>Information technology - City data model - Part 1: Foundation level concepts - Generic Properties Pattern</dcterms:title>
    	<skos:definition>This ontology specifies the foundation-level concepts related to the generic properties pattern of the city data model.</skos:definition>
    	<vann:preferredNamespaceUri>https://w3id.org/citydata/part1/v1/</vann:preferredNamespaceUri>
    	<vann:preferredNamespacePrefix>cdm1</vann:preferredNamespacePrefix>
    		
    	<!-- Provenance -->
        <dcterms:creator>Megan Katsumi</dcterms:creator>
        <dcterms:creator>Mark Fox</dcterms:creator>
    	<dcterms:creator>Kenneth Vaughn</dcterms:creator>
        <dcterms:issued rdf:datatype="http://www.w3.org/2001/XMLSchema#date">2023</dcterms:issued> <!-- Date of the source document, comment out if draft -->
        <owl:priorVersion rdf:datatype="http://www.w3.org/2001/XMLSchema#date">2017-11-05</owl:priorVersion> <!-- Date of prior ontology file, if any -->
		<dcterms:modified rdf:datatype="http://www.w3.org/2001/XMLSchema#date">2026-02-06</dcterms:modified> <!-- Date of this ontology file -->
        <owl:versionInfo>1.3.0</owl:versionInfo>
        <owl:versionIRI rdf:resource="https://w3id.org/citydata/part1/v1/r3.0"/>
        <rdfs:comment>The prior version of this ontology used a different ontology IRI. This update remains semantically consistent with the version adopted as ISO 5087-1:2023.</rdfs:comment>
        
        <!-- License -->
        <cc:license>http://creativecommons.org/licenses/by/4.0/</cc:license>
        
        <!-- Imports -->
        <owl:imports rdf:resource="https://w3id.org/citydata/part1/v1/Core"/>
    </owl:Ontology>

    
    <!-- 
    ///////////////////////////////////////////////////////////////////////////////////////
    //
    // Data properties
    //
    ///////////////////////////////////////////////////////////////////////////////////////
     -->

    <!-- https://w3id.org/citydata/part1/v1/GeneralDataProperty -->

    <owl:DatatypeProperty rdf:about="https://w3id.org/citydata/part1/v1/GeneralDataProperty">
        <skos:definition>Added for organizational purposes, to identify object properties defined in the General Properties Pattern of the CDM ontology.</skos:definition>
        <rdfs:subPropertyOf rdf:resource="https://w3id.org/citydata/part1/v1/FoundationalCdmDataProperty"/>
    </owl:DatatypeProperty>


    <!-- https://w3id.org/citydata/part1/v1/hasDescription -->

    <owl:DatatypeProperty rdf:about="https://w3id.org/citydata/part1/v1/hasDescription">
        <skos:definition>Descriptive information about an object.</skos:definition>
        <rdfs:subPropertyOf rdf:resource="https://w3id.org/citydata/part1/v1/GeneralDataProperty"/>
    </owl:DatatypeProperty>
    


    <!-- https://w3id.org/citydata/part1/v1/hasIdentifier -->

    <owl:DatatypeProperty rdf:about="https://w3id.org/citydata/part1/v1/hasIdentifier">
        <skos:definition>Unique identifier for an object.</skos:definition>
        <rdfs:subPropertyOf rdf:resource="https://w3id.org/citydata/part1/v1/GeneralDataProperty"/>
    </owl:DatatypeProperty>
    


    <!-- https://w3id.org/citydata/part1/v1/hasName -->

    <owl:DatatypeProperty rdf:about="https://w3id.org/citydata/part1/v1/hasName">
        <skos:definition>Name of an object.</skos:definition>
        <rdfs:subPropertyOf rdf:resource="https://w3id.org/citydata/part1/v1/GeneralDataProperty"/>
    </owl:DatatypeProperty>
    

</rdf:RDF>
