<?xml version="1.0"?>
<rdf:RDF xmlns="https://w3id.org/citydata/part1/v1/"
     xml:base="https://w3id.org/citydata/part1/v1/"
     xmlns:cc="http://creativecommons.org/ns#"
     xmlns:dcterms="http://purl.org/dc/terms/"
     xmlns:owl="http://www.w3.org/2002/07/owl#"
     xmlns:rdf="http://www.w3.org/1999/02/22-rdf-syntax-ns#"
     xmlns:rdfs="http://www.w3.org/2000/01/rdf-schema#"
     xmlns:skos="http://www.w3.org/2004/02/skos/core#"
     xmlns:vann="http://purl.org/vocab/vann/"
     xmlns:xml="http://www.w3.org/XML/1998/namespace"
     xmlns:xsd="http://www.w3.org/2001/XMLSchema#"
     xmlns:geo="http://www.opengis.net/ont/geosparql#">
    <owl:Ontology rdf:about="https://w3id.org/citydata/part1/v1/SpatialLocPattern">
    	<!-- Identity -->
    	<dcterms:title>Information technology - City data model - Part 1: Foundation level concepts - Spatial Location Pattern</dcterms:title>
    	<skos:definition>This ontology specifies the foundation-level concepts related to the spatial location pattern of the city data model.</skos:definition>
    	<vann:preferredNamespaceUri>https://w3id.org/citydata/part1/v1/</vann:preferredNamespaceUri>
    	<vann:preferredNamespacePrefix>cdm1</vann:preferredNamespacePrefix>
    		
    	<!-- Provenance -->
        <dcterms:creator>Megan Katsumi</dcterms:creator>
        <dcterms:creator>Mark Fox</dcterms:creator>
    	<dcterms:creator>Kenneth Vaughn</dcterms:creator>
        <dcterms:issued rdf:datatype="http://www.w3.org/2001/XMLSchema#date">2023</dcterms:issued> <!-- Date of the source document, comment out if draft -->
        <owl:priorVersion rdf:datatype="http://www.w3.org/2001/XMLSchema#date">2017-11-05</owl:priorVersion> <!-- Date of prior ontology file, if any -->
		<dcterms:modified rdf:datatype="http://www.w3.org/2001/XMLSchema#date">2026-02-06</dcterms:modified> <!-- Date of this ontology file -->
        <owl:versionInfo>1.3.0</owl:versionInfo>
        <owl:versionIRI rdf:resource="https://w3id.org/citydata/part1/v1/r3.0"/>
        <rdfs:comment>The prior version of this ontology used a different ontology IRI. This update remains semantically consistent with the version adopted as ISO 5087-1:2023.</rdfs:comment>
        
        <!-- License -->
        <cc:license>http://creativecommons.org/licenses/by/4.0/</cc:license>
        
        <!-- Imports -->
        <owl:imports rdf:resource="http://www.opengis.net/ont/geosparql"/>
        <owl:imports rdf:resource="https://w3id.org/citydata/part1/v1/MereologyPattern"/>
    </owl:Ontology>

    
    <!-- 
    ///////////////////////////////////////////////////////////////////////////////////////
    //
    // Datatypes
    //
    ///////////////////////////////////////////////////////////////////////////////////////
     -->

    <!-- Added in v1.2.0 but probably not appropriate. Deleted. -->
    <!-- http://franz.com/ns/allegrograph/5.0/geo/nd#_lat_la_-9.+1_+9.+1_+1.-4_+1.-1_lon_lo_-1.8+2_+1.8+2_+1.-4 -->

    <!-- <rdfs:Datatype rdf:about="http://franz.com/ns/allegrograph/5.0/geo/nd#_lat_la_-9.+1_+9.+1_+1.-4_+1.-1_lon_lo_-1.8+2_+1.8+2_+1.-4">
        <skos:prefLabel>nD Lat Lon</skos:prefLabel>
    </rdfs:Datatype>  -->
    

    <!-- 
    ///////////////////////////////////////////////////////////////////////////////////////
    //
    // Object Properties
    //
    ///////////////////////////////////////////////////////////////////////////////////////
     -->


    <!-- https://w3id.org/citydata/part1/v1/LocationObjectProperty -->

    <owl:ObjectProperty rdf:about="https://w3id.org/citydata/part1/v1/LocationObjectProperty">
        <rdfs:subPropertyOf rdf:resource="https://w3id.org/citydata/part1/v1/FoundationalCdmObjectProperty"/>
        <skos:definition>Added for organizational purposes, to identify all location object properties defined in the City Data Model.</skos:definition>
    </owl:ObjectProperty>


    <!-- https://w3id.org/citydata/part1/v1/associatedLocation -->

    <owl:ObjectProperty rdf:about="https://w3id.org/citydata/part1/v1/associatedLocation">
        <skos:definition>Captures the association of a non-spatial object with a Location. For example, an activity is not a spatial object but may be associated with some location in which it (mostly) takes place.</skos:definition>
        <rdfs:subPropertyOf rdf:resource="https://w3id.org/citydata/part1/v1/LocationObjectProperty"/>
        <rdfs:range rdf:resource="https://w3id.org/citydata/part1/v1/Location"/>
    </owl:ObjectProperty>
    

    <!-- https://w3id.org/citydata/part1/v1/hasLocation -->

    <owl:ObjectProperty rdf:about="https://w3id.org/citydata/part1/v1/hasLocation">
        <skos:definition>Specifies the Location of an object.</skos:definition>
        <rdfs:subPropertyOf rdf:resource="https://w3id.org/citydata/part1/v1/LocationObjectProperty"/>
        <rdfs:range rdf:resource="https://w3id.org/citydata/part1/v1/Location"/>
    </owl:ObjectProperty>
    

    <!-- Issue: No definition provided for nonTangentialProperPart -->
    <!-- https://w3id.org/citydata/part1/v1/nonTangentialProperPart -->

    <owl:ObjectProperty rdf:about="https://w3id.org/citydata/part1/v1/nonTangentialProperPart">
        <rdfs:subPropertyOf rdf:resource="http://www.opengis.net/ont/geosparql#rcc8ntpp"/>
        <rdfs:subPropertyOf rdf:resource="https://w3id.org/citydata/part1/v1/properPartOf"/>
    </owl:ObjectProperty>
    

    <!-- Issue: No definition provided for tangentialProperPart -->
    <!-- https://w3id.org/citydata/part1/v1/tangentialProperPart -->

    <owl:ObjectProperty rdf:about="https://w3id.org/citydata/part1/v1/tangentialProperPart">
        <rdfs:subPropertyOf rdf:resource="http://www.opengis.net/ont/geosparql#rcc8tpp"/>
        <rdfs:subPropertyOf rdf:resource="https://w3id.org/citydata/part1/v1/properPartOf"/>
    </owl:ObjectProperty>
    
    <!-- 
    ///////////////////////////////////////////////////////////////////////////////////////
    //
    // Data properties
    //
    ///////////////////////////////////////////////////////////////////////////////////////
     -->

    
    <!-- https://w3id.org/citydata/part1/v1/SpatialLocOntologyDataProperty -->

    <owl:DatatypeProperty rdf:about="https://w3id.org/citydata/part1/v1/LocationDataProperty">
        <rdfs:comment>Created for organizational purposes, to identify location data properties.</rdfs:comment>
        <rdfs:subPropertyOf rdf:resource="https://w3id.org/citydata/part1/v1/FoundationalCdmDataProperty"/>
    </owl:DatatypeProperty>
    

    <!-- Added in v1.2.0, but not in standard and probably not the right element. Deleted. -->
    <!-- https://w3id.org/citydata/part1/v1/as_nDLatLon -->

<!--    <owl:DatatypeProperty rdf:about="https://w3id.org/citydata/part1/v1/as_nDLatLon">
        <rdfs:subPropertyOf rdf:resource="https://w3id.org/citydata/part1/v1/hasSerialization"/>
        <rdfs:domain rdf:resource="http://www.opengis.net/ont/geosparql#Geometry"/>
        <rdfs:range rdf:resource="http://franz.com/ns/allegrograph/5.0/geo/nd#_lat_la_-9.+1_+9.+1_+1.-4_+1.-1_lon_lo_-1.8+2_+1.8+2_+1.-4"/>
    </owl:DatatypeProperty>   -->
    


    <!-- Issue: hasSerialization added in v1.2.0 -->
    <!-- https://w3id.org/citydata/part1/v1/hasSerialization -->

    <owl:DatatypeProperty rdf:about="https://w3id.org/citydata/part1/v1/hasSerialization">
        <rdfs:subPropertyOf rdf:resource="https://w3id.org/citydata/part1/v1/LocationDataProperty"/>
    </owl:DatatypeProperty>
    

    <!-- 
    ///////////////////////////////////////////////////////////////////////////////////////
    //
    // Classes
    //
    ///////////////////////////////////////////////////////////////////////////////////////
     -->

    
    <!-- https://w3id.org/citydata/part1/v1/LocationThing -->

    <owl:Class rdf:about="https://w3id.org/citydata/part1/v1/SpatialLocThing">
        <skos:definition>Added for organizational purposes, to identify all classes defined in the Location pattern of the CDM ontology.</skos:definition>
        <rdfs:subClassOf rdf:resource="https://w3id.org/citydata/part1/v1/FoundationalCdmThing"/>
    </owl:Class>
    

    <owl:Class rdf:about="https://w3id.org/citydata/part1/v1/Location">
        <skos:definition>A location.</skos:definition>
        <rdfs:subClassOf rdf:resource="http://www.opengis.net/ont/geosparql#Geometry"/>
        <rdfs:subClassOf rdf:resource="https://w3id.org/citydata/part1/v1/SpatialLocThing"/>
    </owl:Class>
    

</rdf:RDF>



<!-- Generated by the OWL API (version 4.5.25.2023-02-15T19:15:49Z) https://github.com/owlcs/owlapi -->
